format-version: 1.2
date: 25:07:2017 17:10
saved-by: AAfolabi
auto-generated-by: OBO-Edit 2.3.1
default-namespace: CassavaTraitOntology
namespace-id-rule: * CO_334:$sequence(7,0100000,0999999)$
ontology: co_334
owl-axioms: Prefix(owl:=<http://www.w3.org/2002/07/owl#>)\nPrefix(rdf:=<http://www.w3.org/1999/02/22-rdf-syntax-ns#>)\nPrefix(xml:=<http://www.w3.org/XML/1998/namespace>)\nPrefix(xsd:=<http://www.w3.org/2001/XMLSchema#>)\nPrefix(rdfs:=<http://www.w3.org/2000/01/rdf-schema#>)\n\n\nOntology(\nDeclaration(AnnotationProperty(<http://www.geneontology.org/formats/oboInOwl#id>))\n\n\nAnnotationAssertion(<http://www.geneontology.org/formats/oboInOwl#id> <http://purl.obolibrary.org/obo/co_334.owl#CO_334:0004030> \"CO_334:0001064\"^^xsd:string)\nAnnotationAssertion(<http://www.geneontology.org/formats/oboInOwl#id> <http://purl.obolibrary.org/obo/co_334.owl#CO_334:0004031> \"CO_334:0001065\"^^xsd:string)\nAnnotationAssertion(<http://www.geneontology.org/formats/oboInOwl#id> <http://purl.obolibrary.org/obo/co_334.owl#CO_334:0004032> \"CO_334:0004016\"^^xsd:string)\nAnnotationAssertion(<http://www.geneontology.org/formats/oboInOwl#id> <http://purl.obolibrary.org/obo/co_334.owl#CO_334:0004033> \"CO_334:0004017\"^^xsd:string)\nAnnotationAssertion(<http://www.geneontology.org/formats/oboInOwl#id> <http://purl.obolibrary.org/obo/co_334.owl#CO_334:0004034> \"CO_334:0001065\"^^xsd:string)\nAnnotationAssertion(<http://www.geneontology.org/formats/oboInOwl#id> <http://purl.obolibrary.org/obo/co_334.owl#CO_334:0004035> \"CO_334:0001065\"^^xsd:string)\nAnnotationAssertion(<http://www.geneontology.org/formats/oboInOwl#id> <http://purl.obolibrary.org/obo/co_334.owl#CO_334:0004036> \"CO_334:0001065\"^^xsd:string)\nAnnotationAssertion(<http://www.geneontology.org/formats/oboInOwl#id> <http://purl.obolibrary.org/obo/co_334.owl#CO_334:0004037> \"CO_334:0001065\"^^xsd:string)\nAnnotationAssertion(<http://www.geneontology.org/formats/oboInOwl#id> <http://purl.obolibrary.org/obo/co_334.owl#CO_334:0004038> \"CO_334:0001065\"^^xsd:string)\nAnnotationAssertion(<http://www.geneontology.org/formats/oboInOwl#id> <http://purl.obolibrary.org/obo/co_334.owl#CO_334:0004039> \"CO_334:0001065\"^^xsd:string)\n)

[Term]
id: CO_334:0000000
name: CGIAR cassava trait ontology
namespace: cassava_trait
def: "controlled vocabulary to describe each trait as a distinguishable, characteristic, quality or phenotypic feature of a developing or mature cassava plant." [CO:curators]

[Term]
id: CO_334:0000001
name: Agronomic trait
namespace: cassava_trait
def: "A characteristic in a cassava plant that will add economic value to agricultural production." [CO:curators]
is_a: CO_334:0000000 ! CGIAR cassava trait ontology

[Term]
id: CO_334:0000002
name: Morphological trait
namespace: cassava_trait
def: "Physical attributes that describe the shape or form of cassava plant." [CO:curators]
is_a: CO_334:0000000 ! CGIAR cassava trait ontology

[Term]
id: CO_334:0000003
name: Physiological trait
namespace: cassava_trait
def: "Characteristics related to the functioning of living cassava." [CO:curators]
is_a: CO_334:0000000 ! CGIAR cassava trait ontology

[Term]
id: CO_334:0000004
name: Quality trait
namespace: cassava_trait
def: "A characteristic or distinguishing feature of cassava related to its utilization after harvest." [CO:curators]
synonym: "post-harvest trait" EXACT []
is_a: CO_334:0000000 ! CGIAR cassava trait ontology

[Term]
id: CO_334:0000005
name: Stress trait
namespace: cassava_trait
def: "A characteristic related to plant functioning in the presence of a biotic or abiotic challenge to normal or optimal growing conditions." [CO:curators]
is_a: CO_334:0000000 ! CGIAR cassava trait ontology

[Term]
id: CO_334:0000006
name: abiotic stress trait
namespace: cassava_trait
def: "Response in terms of resistance or sensitivity to abiotic stress." [CO:curators]
is_a: CO_334:0000005 ! Stress trait

[Term]
id: CO_334:0000007
name: biotic stress trait
namespace: cassava_trait
def: "Response in terms of resistance, susceptibility or tolerance to biotic stress." [CO:curators]
is_a: CO_334:0000005 ! Stress trait

[Term]
id: CO_334:0000008
name: sprouting proportion
namespace: cassava_trait
def: "Proportion of stakes germinated scored three month after planting." [CO:curators]
synonym: "sprout" EXACT []
synonym: "sprout_comp_r" EXACT []
is_a: CO_334:0001000 ! Variables
relationship: variable_of CO_334:0000472 ! Sprouting
relationship: variable_of CO_334:0010220 ! Counting: Sprouting_method
relationship: variable_of CO_334:0100582 ! ratio

[Term]
id: CO_334:0000009
name: initial vigor assessment 1-7
namespace: cassava_trait
def: "Visual assessment of plant vigor during establishment scored one month after planting. 3 = Not vigorous, 5 = Medium vigor, 7 = highly vigorous." [CO:curators]
synonym: "Can't fall when there is strong wind" EXACT []
synonym: "IVig_IITAVisScg_1to7" EXACT []
synonym: "vigor" EXACT []
xref: TO:0000250
is_a: CO_334:0001000 ! Variables
is_a: CO_334:0002010 ! Farmer trait
relationship: variable_of CO_334:0000386 ! Initial vigor
relationship: variable_of CO_334:0010228 ! Visual Rating: Initial vigor_method
relationship: variable_of CO_334:0100434 ! 7pt scale

[Term]
id: CO_334:0000010
name: plant stands harvested counting
namespace: cassava_trait
def: "A count of the number of plant stands at harvest." [CO:curators]
synonym: "nohav" EXACT []
synonym: "NoHvstPlnt_Count_Plnt" EXACT []
is_a: CO_334:0001000 ! Variables
relationship: variable_of CO_334:0000434 ! Plant stands harvested
relationship: variable_of CO_334:0010284 ! Counting: Plant stands harvested_method
relationship: variable_of CO_334:0100490 ! plant

[Term]
id: CO_334:0000011
name: root number per plot counting
namespace: cassava_trait
def: "A count of the total number of storage roots (marketable and non-marketable) harvested per plot." [CO:curators]
synonym: "NoHvstRt_Count_Rt" EXACT []
synonym: "plotrtno" RELATED []
synonym: "rtno" EXACT []
is_a: CO_334:0001000 ! Variables
relationship: variable_of CO_334:0000452 ! Root number
relationship: variable_of CO_334:0010285 ! Counting: Root number_method
relationship: variable_of CO_334:0100491 ! root

[Term]
id: CO_334:0000012
name: fresh storage root weight per plot
namespace: cassava_trait
def: "Total fresh weight of storage roots harvested per plot measured in kilogram (kg)." [CO:curators]
synonym: "rtwt" EXACT []
synonym: "RtWt_Wgh_kg" EXACT []
is_a: CO_334:0001000 ! Variables
relationship: variable_of CO_334:0000302 ! Storage root weight by plot
relationship: variable_of CO_334:0010286 ! Measurement: Fresh weight of storage root_method
relationship: variable_of CO_334:0100493 ! kg

[Term]
id: CO_334:0000013
name: fresh root yield
namespace: cassava_trait
def: "Fresh weight of harvested roots expressed in tons per hectares (t/ha) per plant." [CO:curators]
synonym: "Can easily fill a sack or the truck" EXACT []
synonym: "Can provide at least ten cassava tubers per plant stand" EXACT []
synonym: "fyld" EXACT []
synonym: "RtYld_Fresh_tha" EXACT []
is_a: CO_334:0001000 ! Variables
is_a: CO_334:0001027 ! farmer preference trait at harvest
is_a: CO_334:0002010 ! Farmer trait
relationship: variable_of CO_334:0000456 ! Root yield
relationship: variable_of CO_334:0010329 ! Calculation: Fresh root yield_method
relationship: variable_of CO_334:0100535 ! t/ha

[Term]
id: CO_334:0000014
name: dry yield
namespace: cassava_trait
def: "Dry weight of harvested roots derived by multiplying fresh storage root yield by dry matter content expressed in tons per hectares (t/ha)." [CO:curators]
synonym: "dyld" EXACT []
synonym: "RtYld_Dry_tha" EXACT []
is_a: CO_334:0001000 ! Variables
relationship: variable_of CO_334:0000456 ! Root yield
relationship: variable_of CO_334:0010330 ! Calculation: Dry yield_method
relationship: variable_of CO_334:0100535 ! t/ha

[Term]
id: CO_334:0000015
name: harvest index variable
namespace: cassava_trait
def: "Proportion of fresh root weight in total biomass." [CO:curators]
synonym: "HI" EXACT []
xref: TO:0000128
is_a: CO_334:0001000 ! Variables
relationship: derives_from CO_334:0000013 ! fresh root yield
relationship: derives_from CO_334:0000017 ! top yield
relationship: variable_of CO_334:0000267 ! Harvest index
relationship: variable_of CO_334:0010512 ! Calculation: Harvest index_method
relationship: variable_of CO_334:0100582 ! ratio

[Term]
id: CO_334:0000016
name: fresh shoot weight measurement in kg per plot
namespace: cassava_trait
def: "Total fresh weight of harvested foliage and stems in kilograms per plot." [CO:curators]
synonym: "shtwt" EXACT []
synonym: "ShWt_Meas_kg" EXACT []
is_a: CO_334:0001000 ! Variables
relationship: variable_of CO_334:0000305 ! Fresh shoot weight by plot
relationship: variable_of CO_334:0010287 ! Measurement: Fresh shoot weight_method
relationship: variable_of CO_334:0100493 ! kg

[Term]
id: CO_334:0000017
name: top yield
namespace: cassava_trait
def: "Total fresh weight of harvested foliage and stems expressed in tons per hectare (t/ha)." [CO:curators]
synonym: "RtYld_FreshAerial_tha" EXACT []
synonym: "tyld" EXACT []
is_a: CO_334:0001000 ! Variables
relationship: variable_of CO_334:0000456 ! Root yield
relationship: variable_of CO_334:0010332 ! Calculation: Top yield_method
relationship: variable_of CO_334:0100535 ! t/ha

[Term]
id: CO_334:0000018
name: plant height measurement in cm
namespace: cassava_trait
def: "Vertical height of plants from the ground to top of the canopy measured in centimeter (cm)." [CO:curators]
synonym: "PlntH_Meas_cm" EXACT []
synonym: "pltht" EXACT []
xref: TO:0000207
is_a: CO_334:0001000 ! Variables
relationship: variable_of CO_334:0000432 ! Plant height
relationship: variable_of CO_334:0010303 ! Measurement: Plant height_method
relationship: variable_of CO_334:0100558 ! cm

[Term]
id: CO_334:0000019
name: storage root size visual rating 1-7
namespace: cassava_trait
def: "Visual rating of storage root size with 3 = short, 5 = medium, and 7 = long." [CO:curators]
synonym: "Ease of digging out root form the soil" EXACT []
synonym: "RtLng_VisScg_1to7" EXACT []
synonym: "rtsz" EXACT []
is_a: CO_334:0001000 ! Variables
is_a: CO_334:0002010 ! Farmer trait
relationship: variable_of CO_334:0000492 ! Storage Root Size
relationship: variable_of CO_334:0010288 ! Visual Rating: Storage root size_method
relationship: variable_of CO_334:0100494 ! 7pt scale

[Term]
id: CO_334:0000020
name: storage root shape visual rating 1-6
namespace: cassava_trait
def: "Visual rating of storage root shape with 1 = conical, 2 = conical-cylindrical, 3 = cylindrical, 4 = fusiform, 5 = Irrregular, and 6 = Combination of shapes." [CO:curators]
synonym: "rtshp" EXACT []
synonym: "RtShp_VisClsn_1to6" EXACT []
is_a: CO_334:0001000 ! Variables
relationship: variable_of CO_334:0000491 ! Storage Root Shape
relationship: variable_of CO_334:0010289 ! Visual Rating: Storage root shape_method
relationship: variable_of CO_334:0100495 ! 6pt scale

[Term]
id: CO_334:0000021
name: storage root pulp color visual rating 1-3
namespace: cassava_trait
def: "Visual rating of most frequent pulp color with 1 = white or cream, 2 = yellow, and 3 = pink." [CO:curators]
synonym: "plpcol" EXACT []
synonym: "PlpCol_VisClsn_1to3" EXACT []
is_a: CO_334:0001000 ! Variables
relationship: variable_of CO_334:0000490 ! Storage Root Pulp Color
relationship: variable_of CO_334:0010292 ! Visual Rating: Storage root pulp color _method
relationship: variable_of CO_334:0100498 ! 3pt scale

[Term]
id: CO_334:0000022
name: root neck length visual rating 0-7
namespace: cassava_trait
def: "Visual rating of root neck length with 0 = absent or sessile, 3 = short, 5 = intermediate, and 7 = long." [CO:curators]
synonym: "nklgt" EXACT []
synonym: "NkLng_VisClsn_0to7" EXACT []
is_a: CO_334:0001000 ! Variables
relationship: variable_of CO_334:0000451 ! Storage root neck length
relationship: variable_of CO_334:0010293 ! Visual Rating: Root neck length_method
relationship: variable_of CO_334:0100499 ! 8pt scale

[Term]
id: CO_334:0000023
name: petiole color visual rating 1-9
namespace: cassava_trait
def: "Visual rating of the petiole color with 3 = light green, 5 = dark green, 7 = green-purple, 8 = red, and 9 = purple." [CO:curators]
synonym: "petcol" EXACT []
synonym: "PtlCol_VisClsn_1to9" EXACT []
is_a: CO_334:0001000 ! Variables
relationship: variable_of CO_334:0000427 ! Petiole Color
relationship: variable_of CO_334:0010345 ! Visual Rating: Petiole color_method
relationship: variable_of CO_334:0100551 ! 7pt scale

[Term]
id: CO_334:0000024
name: petiole length visual rating 0-7
namespace: cassava_trait
def: "Visual rating of petiole length with 0 = petiole absent, 3 = short (5-10cm), 5 = medium (15-20cm), and 7 = long (25-30cm)." [CO:curators]
synonym: "petlgt" EXACT []
synonym: "PtlLng_VisScg_0to7" EXACT []
is_a: CO_334:0001000 ! Variables
relationship: variable_of CO_334:0000429 ! Petiole length
relationship: variable_of CO_334:0010344 ! Visual Rating: Petiole Length_method
relationship: variable_of CO_334:0100550 ! 4pt scale

[Term]
id: CO_334:0000025
name: young stem pubescence visual rating 0-7
namespace: cassava_trait
def: "Visual rating of young stem pubescence with 0 = absent or glabrous, 3 = little pubescence, 5 = moderate pubescence, and 7 = high pubescence." [CO:curators]
synonym: "stmpub" EXACT []
synonym: "StPub_VisScg_1to7" EXACT []
is_a: CO_334:0001000 ! Variables
relationship: variable_of CO_334:0000506 ! Young Stem Pubescence
relationship: variable_of CO_334:0010348 ! Visual Rating: Young stem pubescence_method
relationship: variable_of CO_334:0100554 ! 8pt scale

[Term]
id: CO_334:0000026
name: apical pubescence visual rating 0-7
namespace: cassava_trait
def: "Visual rating of young leaf pubescence with 0 = absent or glabrous, 3 = little pubescence, 5 = moderate pubescence, and 7 = high pubescence." [CO:curators]
synonym: "apubes" EXACT []
synonym: "LfPub_VisClsn_0to7" EXACT []
is_a: CO_334:0001000 ! Variables
relationship: variable_of CO_334:0000283 ! Apical pubescence
relationship: variable_of CO_334:0010338 ! Visual Rating: Apical pubescence_method
relationship: variable_of CO_334:0100544 ! 8pt scale

[Term]
id: CO_334:0000027
name: bacterial disease
namespace: cassava_trait
def: "Traits related to incidence and severity of cassava response to bacterial pathogens." [CO:curators]
is_a: CO_334:0000007 ! biotic stress trait
created_by: BAKARE
creation_date: 2010-11-08T06:42:36Z

[Term]
id: CO_334:0000028
name: viral disease
namespace: cassava_trait
def: "Traits related to incidence and severity of cassava response to viral pathogens." [CO:curators]
is_a: CO_334:0000007 ! biotic stress trait
created_by: BAKARE
creation_date: 2010-11-08T06:43:31Z

[Term]
id: CO_334:0000029
name: fungal disease
namespace: cassava_trait
def: "Traits related to incidence and severity of cassava response to fungal pathogens." [CO:curators]
is_a: CO_334:0000007 ! biotic stress trait
created_by: BAKARE
creation_date: 2010-11-08T06:44:26Z

[Term]
id: CO_334:0000030
name: insect damage
namespace: cassava_trait
def: "Traits related to damage caused by insects." [CO:curators]
is_a: CO_334:0000007 ! biotic stress trait
created_by: BAKARE
creation_date: 2010-11-08T06:45:42Z

[Term]
id: CO_334:0000031
name: Cassava bacterial blight severity
namespace: cassava_trait
def: "Severity of bacterial blight disease caused by Xanthomonas axonopodis pv. Manihotis" [CO:curators]
synonym: "Cassava bacterial blight severity - Cassavabase" EXACT []
synonym: "CBBSev" EXACT []
xref: TO:0000770
is_a: CO_334:0000027 ! bacterial disease

[Term]
id: CO_334:0000032
name: Cassava anthracnose disease severity
namespace: cassava_trait
def: "Severity of the Cassava anthracnose disease caused by Colletotrichum gloeosporioides f. sp." [CO:curators]
synonym: "CADSev" EXACT []
synonym: "Cassava anthracnose disease severity - Cassavabase" EXACT []
xref: TO:0000439
is_a: CO_334:0000029 ! fungal disease

[Term]
id: CO_334:0000033
name: Cassava green mite severity
namespace: cassava_trait
def: "Severity of the damage caused by cassava green mite" [CO:curators]
synonym: "Cassava green mite severity - Cassavabase" EXACT []
synonym: "CGMSev" EXACT []
xref: TO:0000261
is_a: CO_334:0000030 ! insect damage

[Term]
id: CO_334:0000034
name: cassava mealy bug severity by visual rating 1-5
namespace: cassava_trait
def: "Visual rating of damage caused by cassava mealy-bug, Phenacoccus Manihoti. Symptoms rated from 1 = (clean, no infection) to 5 = (extremely severe, severely diseased)." [CO:curators]
synonym: "cmbs" EXACT []
synonym: "CMBSev_Est_1to5" EXACT []
is_a: CO_334:0001000 ! Variables
relationship: variable_of CO_334:0000340 ! Cassava mealy bug severity
relationship: variable_of CO_334:0010267 ! Visual Observation: Cassava mealy bug severity_method
relationship: variable_of CO_334:0100473 ! 5 pt scale

[Term]
id: CO_334:0000035
name: Cassava mosaic disease severity
namespace: cassava_trait
def: "Severity of the symptoms caused by the cassava mosaic virus, in the family Geminiviridae and genus Begomovirus" [CO:curators]
synonym: "Cassava mosaic disease severity - Cassavabase" EXACT []
synonym: "CMDSev" EXACT []
xref: TO:0000148
is_a: CO_334:0000028 ! viral disease

[Term]
id: CO_334:0000036
name: Cassava brown streak disease leaf severity
namespace: cassava_trait
def: "Severity of the symptoms on leaf caused by cassava brown streak virus in the family of Potyviridae and genus Ipomovirus" [CO:curators]
synonym: "Cassava brown streak disease leaf severity - Cassavabase" EXACT []
synonym: "CBSDRtSev" EXACT []
xref: TO:0000148
is_a: CO_334:0000028 ! viral disease

[Term]
id: CO_334:0000037
name: Cassava bacterial blight incidence
namespace: cassava_trait
def: "Incidence of the cassava bacterial blight" [CO:curators]
synonym: "CBBInc" EXACT []
xref: TO:0000770
is_a: CO_334:0000027 ! bacterial disease

[Term]
id: CO_334:0000038
name: Cassava anthracnose disease incidence
namespace: cassava_trait
def: "Proportion of plants within a plot showing symptoms of cassava anthracnose disease" [CO:curators]
synonym: "cadi" EXACT []
xref: TO:0000439
is_a: CO_334:0000029 ! fungal disease

[Term]
id: CO_334:0000039
name: Cassava mosaic disease incidence
namespace: cassava_trait
def: "Proportion of plants within a plot showing  symptoms of cassava mosaic disease" [CO:curators]
synonym: "cmdi" EXACT []
xref: TO:0000148
is_a: CO_334:0000028 ! viral disease

[Term]
id: CO_334:0000040
name: Cassava brown streak disease leaf incidence
namespace: cassava_trait
def: "Proportion of plants within a plot showing  symptoms of cassava brown streak disease" [CO:curators]
synonym: "cbsdli" EXACT []
xref: TO:0000148
is_a: CO_334:0000028 ! viral disease

[Term]
id: CO_334:0000041
name: cassava mealy bug incidence by ratio
namespace: cassava_trait
def: "Proportion of plants within a plot showing symptoms of cassava mealy-bug damage." [CO:curators]
synonym: "cmbi" EXACT []
synonym: "CMBInc_Est_1to5" EXACT []
is_a: CO_334:0001000 ! Variables
relationship: variable_of CO_334:0000339 ! Cassava mealy bug incidence
relationship: variable_of CO_334:0010268 ! Counting: Cassava mealy bug incidence_method
relationship: variable_of CO_334:0100582 ! ratio

[Term]
id: CO_334:0000042
name: spiraling whitefly severity : visual 1-5
namespace: cassava_trait
def: "Visual rating of damage caused by spiraling white fly, Aleurodicus dispersus. Symptoms rated from 1 = (clean, no damage) to 5 = (extremely severe, severely damaged)." [CO:curators]
synonym: "Swfs" EXACT []
synonym: "SWfSev_VisScg_1to5" EXACT []
is_a: CO_334:0001000 ! Variables
relationship: variable_of CO_334:0000465 ! Spiraling whitefly severity
relationship: variable_of CO_334:0010325 ! Visual Observation: Spiraling whitefly severity_method
relationship: variable_of CO_334:0100531 ! 5 pt scale

[Term]
id: CO_334:0000043
name: spiraling whitefly incidence by proportion
namespace: cassava_trait
def: "Proportion of plants within a plot showing evidence of colonization by spiraling whitefly." [CO:curators]
synonym: "Swfi" EXACT []
synonym: "SWfInc_Comp_r" EXACT []
is_a: CO_334:0001000 ! Variables
relationship: variable_of CO_334:0000464 ! Spiraling whitefly incidence
relationship: variable_of CO_334:0010326 ! Counting: Spiraling whitefly incidence_method
relationship: variable_of CO_334:0100582 ! ratio

[Term]
id: CO_334:0000044
name: red spider mite severity : visual 1-5
namespace: cassava_trait
def: "Visual rating of damage caused by red spider mite, Oligonychus gossypii and Tetranychus spp. Symptoms rated from 1 = (clean, no infection) to 5 = (extremely severe, severely damaged)." [CO:curators]
synonym: "rsms" EXACT []
synonym: "RSMSev_VisScg_1to5" EXACT []
is_a: CO_334:0001000 ! Variables
relationship: variable_of CO_334:0000444 ! Red spider mite severity
relationship: variable_of CO_334:0010323 ! Visual Observation: Red spider mite severity_method
relationship: variable_of CO_334:0100529 ! 5 pt scale

[Term]
id: CO_334:0000045
name: red spider mite incidence by proportion
namespace: cassava_trait
def: "Proportion of plants within a plot showing evidence of colonization by red spider mite." [CO:curators]
synonym: "rsmi" EXACT []
synonym: "RSMInc_Comp_r" EXACT []
is_a: CO_334:0001000 ! Variables
relationship: variable_of CO_334:0000443 ! Red spider mite incidence
relationship: variable_of CO_334:0010324 ! Counting: Red spider mite incidence_method
relationship: variable_of CO_334:0100582 ! ratio

[Term]
id: CO_334:0000046
name: petiole insertion angle visual rating 0-7
namespace: cassava_trait
def: "Visual rating of orientation or angle between the branch and petiole with 0 = no petiole, 3 = 15-30 degrees, 5 = 45-70 degrees, and 7 = 75-90 degrees." [CO:curators]
synonym: "petang" EXACT []
synonym: "PtlAng_VisScg_0to7" EXACT []
is_a: CO_334:0001000 ! Variables
relationship: variable_of CO_334:0000428 ! Petiole Insertion Angle
relationship: variable_of CO_334:0010343 ! Visual Rating: Petiole Insertion Angle_method
relationship: variable_of CO_334:0100549 ! 7pt scale

[Term]
id: CO_334:0000047
name: abscisic acid content of leaf ug/g
namespace: cassava_trait
def: "Abscisic acid content of leaf sample." [CO:curators]
synonym: "abscon" EXACT []
synonym: "AbsCt_Meas_ugg" EXACT []
is_a: CO_334:0001000 ! Variables
relationship: variable_of CO_334:0000276 ! Abscisic acid content
relationship: variable_of CO_334:0010366 ! Estimation: Abscisic acid content_method
relationship: variable_of CO_334:0100572 ! ug/g

[Term]
id: CO_334:0000048
name: leaf retention visual rating 1-5
namespace: cassava_trait
def: "Visual rating of leaf longevity using a scale of 1 =(very poor retention) to 5 = (outstanding leaf retention)." [CO:curators]
synonym: "lfret" EXACT []
synonym: "LfRet_VisSc_1to5" EXACT []
is_a: CO_334:0001000 ! Variables
relationship: variable_of CO_334:0000396 ! Leaf retention
relationship: variable_of CO_334:0010305 ! Visual Rating: Leaf retention_method
relationship: variable_of CO_334:0100511 ! 5pt scale

[Term]
id: CO_334:0000049
name: leaf life span in days
namespace: cassava_trait
def: "Measures leaf life span estimated as number of days." [CO:curators]
synonym: "lflife" EXACT []
synonym: "LfLife_Count_days" EXACT []
is_a: CO_334:0001000 ! Variables
relationship: variable_of CO_334:0000390 ! Leaf life span
relationship: variable_of CO_334:0010367 ! Calculation: Leaf life _method
relationship: variable_of CO_334:0100611 ! days

[Term]
id: CO_334:0000050
name: storage root peduncle visual rating 0-5
namespace: cassava_trait
def: "Visual rating of root peduncle length using a scale of 0 = sessile, 3 = pedunculate, and 5 = mixed." [CO:curators]
synonym: "RtPed_VisClsn_0to7" EXACT []
synonym: "rtpedu" EXACT []
is_a: CO_334:0001000 ! Variables
relationship: variable_of CO_334:0000488 ! Storage Root Peduncle
relationship: variable_of CO_334:0010309 ! Visual Rating: Storage root peduncle_method
relationship: variable_of CO_334:0100515 ! 8pt scale

[Term]
id: CO_334:0000051
name: storage root constriction visual scoring 0&1
namespace: cassava_trait
def: "Visual scoring of mature root constrictions recorded as 0= absent and 1=present." [CO:curators]
synonym: "rtcons" EXACT []
synonym: "RtConsPrsnc_VisClsn_0or1" EXACT []
is_a: CO_334:0001000 ! Variables
relationship: variable_of CO_334:0000485 ! Storage Root Constrictions
relationship: variable_of CO_334:0010310 ! Visual Rating: Storage root constrictions_method
relationship: variable_of CO_334:0100516 ! 2pt scale

[Term]
id: CO_334:0000052
name: root position visual rating 1-3
namespace: cassava_trait
def: "Visual rating root position in the soil with 1 = tending toward vertical, 2 = tending toward horizontal, and 3 = irregular." [CO:curators]
synonym: "RtPos_VisClsn_1to3" EXACT []
synonym: "rtpost" EXACT []
is_a: CO_334:0001000 ! Variables
relationship: variable_of CO_334:0000453 ! Root Position
relationship: variable_of CO_334:0010364 ! Visual Rating: Root position_method
relationship: variable_of CO_334:0100570 ! 3pt scale

[Term]
id: CO_334:0000053
name: root surface color visual rating 1-3
namespace: cassava_trait
def: "Visual rating of storage root surface color with 1 = white or cream, 2 =light brown, and 3 = dark brown." [CO:curators]
synonym: "rtscol" EXACT []
synonym: "RtSurfCol_VisClsn_1to3" EXACT []
is_a: CO_334:0001000 ! Variables
relationship: variable_of CO_334:0000454 ! Storage root surface color
relationship: variable_of CO_334:0010311 ! Visual Rating: Root surface color_method
relationship: variable_of CO_334:0100517 ! 3pt scale

[Term]
id: CO_334:0000054
name: root surface texture visual rating 1-7
namespace: cassava_trait
def: "Visual rating of storage root texture with 3 = smooth, 5 = intermediate, and 7 = rough." [CO:curators]
synonym: "RtSurfTex_VisClsn_1to7" EXACT []
synonym: "rttext" EXACT []
is_a: CO_334:0001000 ! Variables
relationship: variable_of CO_334:0000455 ! Storage root surface texture
relationship: variable_of CO_334:0010312 ! Visual Rating: Root surface texture_method
relationship: variable_of CO_334:0100518 ! 3pt scale

[Term]
id: CO_334:0000055
name: storage root diameter visual rating 1-7
namespace: cassava_trait
def: "Visual rating of storage root diameter with 3 = short, 5 = medium and 7 = long." [CO:curators]
synonym: "RtDia_VisScg_1to7" EXACT []
synonym: "rtdiam" EXACT []
is_a: CO_334:0001000 ! Variables
relationship: variable_of CO_334:0000487 ! Storage Root Diameter
relationship: variable_of CO_334:0010365 ! Visual Rating: Storage root diameter_method
relationship: variable_of CO_334:0100571 ! 7pt scale

[Term]
id: CO_334:0000056
name: caruncle color visual scoring 1-3
namespace: cassava_trait
def: "Visual scoring of caruncle color with 1 = white or cream, 2 = pink or red, and 3 = purple." [CO:curators]
synonym: "carcol" EXACT []
synonym: "CarunCol_VisClsn_1to3" EXACT []
is_a: CO_334:0001000 ! Variables
relationship: variable_of CO_334:0000298 ! Caruncle Color
relationship: variable_of CO_334:0010363 ! Visual Rating: Caruncle color_method
relationship: variable_of CO_334:0100569 ! 4pt scale

[Term]
id: CO_334:0000057
name: stigma color visual scoring 1-5
namespace: cassava_trait
def: "Visual scoring of stigma color with 1 = white, 2 = orange, 3 = green, 4 = red, and 5 = purple." [CO:curators]
synonym: "stgmco" EXACT []
synonym: "StgmCol_VisClsn_1to5" EXACT []
is_a: CO_334:0001000 ! Variables
relationship: variable_of CO_334:0000481 ! Stigma Color
relationship: variable_of CO_334:0010355 ! Visual Rating: Stigma color_method
relationship: variable_of CO_334:0100561 ! 5pt scale

[Term]
id: CO_334:0000058
name: ovary color visual rating 1-5
namespace: cassava_trait
def: "Visual scoring of ovary color with 1 = white, 2 = orange, 3 = green, 4 = red, and 5 = purple." [CO:curators]
synonym: "OvrCol_VisClsn_1to5" EXACT []
synonym: "ovryco" EXACT []
is_a: CO_334:0001000 ! Variables
relationship: variable_of CO_334:0000421 ! Ovary Color
relationship: variable_of CO_334:0010356 ! Visual Rating: Ovary color_method
relationship: variable_of CO_334:0100562 ! 5pt scale

[Term]
id: CO_334:0000059
name: disc color visual scoring 1-5
namespace: cassava_trait
def: "Visual scoring of floral disc color with 1 = white, 2 = orange, 3 = green, 4 = red, and 5 = purple." [CO:curators]
synonym: "DiscCol_VisClsn_1to5" EXACT []
synonym: "discol" EXACT []
is_a: CO_334:0001000 ! Variables
relationship: variable_of CO_334:0000360 ! Disc color
relationship: variable_of CO_334:0010354 ! Visual Rating: Disc color_method
relationship: variable_of CO_334:0100560 ! 5pt scale

[Term]
id: CO_334:0000060
name: sepal color visual rating 1-5
namespace: cassava_trait
def: "Visual scoring of sepal color with 1 = white, 2 = orange, 3 = green, 4 = red, and 5 = purple." [CO:curators]
synonym: "SepCol_VisClsn_1to5" EXACT []
synonym: "splcol" EXACT []
is_a: CO_334:0001000 ! Variables
relationship: variable_of CO_334:0000462 ! Sepal Color
relationship: variable_of CO_334:0010353 ! Visual Rating: Sepal color_method
relationship: variable_of CO_334:0100559 ! 5pt scale

[Term]
id: CO_334:0000061
name: anther color visual rating 1-3
namespace: cassava_trait
def: "Visual scoring of anther color with 1 = cream, 2 = yellow, and 3 = other." [CO:curators]
synonym: "AnthCol_VisClsn_1to5" EXACT []
synonym: "anther" EXACT []
is_a: CO_334:0001000 ! Variables
relationship: variable_of CO_334:0000280 ! Anther Color
relationship: variable_of CO_334:0010357 ! Visual Rating: Anther color_method
relationship: variable_of CO_334:0100563 ! 3pt scale

[Term]
id: CO_334:0000062
name: stem color visual scoring 1-4
namespace: cassava_trait
def: "Visual scoring of stem color with 1 = silver green, 2 = light brown or orange, 3 = dark brown, 4 = dark green, and 5 = golden." [CO:curators]
synonym: "stmcol" EXACT []
synonym: "StmCol_VisClsn_1to4" EXACT []
is_a: CO_334:0001000 ! Variables
relationship: variable_of CO_334:0000475 ! Stem Color
relationship: variable_of CO_334:0010301 ! Visual Scoring: Stem color_method
relationship: variable_of CO_334:0100507 ! 4pt scale

[Term]
id: CO_334:0000063
name: seed color visual rating 1-5
namespace: cassava_trait
def: "Visual scoring of seed color with 1 = brown, 2 = grey, 3 = mottled, 4 = black, and 5 = dark brown." [CO:curators]
synonym: "SdCol_VisClsn_1to5" EXACT []
synonym: "seedco" EXACT []
is_a: CO_334:0001000 ! Variables
relationship: variable_of CO_334:0000459 ! Seed color
relationship: variable_of CO_334:0010362 ! Visual Rating: Seed color_method
relationship: variable_of CO_334:0100568 ! 5pt scale

[Term]
id: CO_334:0000064
name: storage root periderm color visual rating 1-4
namespace: cassava_trait
def: "Visual rating of the color of outer surface of storage root periderm (outer skin color) with 1 = white or cream, 2 = yellow, 3 = light brown, 4 = dark brown." [CO:curators]
synonym: "outcol" EXACT []
synonym: "RtPeridCol_VisClsn_1to4" EXACT []
is_a: CO_334:0001000 ! Variables
relationship: variable_of CO_334:0000489 ! Storage Root Periderm Color
relationship: variable_of CO_334:0010291 ! Visual Rating: Storage root periderm color_method
relationship: variable_of CO_334:0100497 ! 4pt scale

[Term]
id: CO_334:0000065
name: ascorbic acid in root percentage
namespace: cassava_trait
def: "Antioxidant and water soluble vitamin of cassava storage root." [CO:curators]
synonym: "AscACt_Meas_pct" EXACT []
is_a: CO_334:0001000 ! Variables
relationship: variable_of CO_334:0000284 ! Ascorbic acid
relationship: variable_of CO_334:0010377 ! Estimation: Ascorbic acid_method
relationship: variable_of CO_334:0100583 ! pct (%)

[Term]
id: CO_334:0000066
name: ash content in percentage
namespace: cassava_trait
def: "Residue left behind after all organic matter has been burnt off, a measure of total mineral salts in a food estimated in percentage (%)." [CO:curators]
synonym: "ash" EXACT []
synonym: "MinCt_Burng_pct" EXACT []
is_a: CO_334:0001000 ! Variables
relationship: variable_of CO_334:0000285 ! Ash content
relationship: variable_of CO_334:0010378 ! Estimation: Ash content_method
relationship: variable_of CO_334:0100583 ! pct (%)

[Term]
id: CO_334:0000067
name: fibre content estimation in percentage
namespace: cassava_trait
def: "Part of tuber root that cannot be digested by humans estimated in percentage (%)." [CO:curators]
synonym: "FibCt_Meas_pct" EXACT []
synonym: "fibre" EXACT []
synonym: "Longer varieties has less fibre in them" EXACT []
is_a: CO_334:0001000 ! Variables
is_a: CO_334:0002010 ! Farmer trait
relationship: variable_of CO_334:0000366 ! Fibre content
relationship: variable_of CO_334:0010373 ! Estimation: Fibre content_method
relationship: variable_of CO_334:0100583 ! pct (%)

[Term]
id: CO_334:0000068
name: iron content in roots by ppm (mg/kg)
namespace: cassava_trait
def: "Estimation of total iron content in cassava storage roots expressed in part per million or milligram per kilogram." [CO:curators]
synonym: "fe" EXACT []
synonym: "FeCt_Meas_ugg" EXACT []
is_a: CO_334:0001000 ! Variables
relationship: variable_of CO_334:0000387 ! Iron content
relationship: variable_of CO_334:0010370 ! Estimation: Iron content_method
relationship: variable_of CO_334:0100572 ! ug/g

[Term]
id: CO_334:0000069
name: moisture content in percentage
namespace: cassava_trait
def: "Percentage (%) of water contained in cassava storage root." [CO:curators]
synonym: "mc" EXACT []
synonym: "RtMoistCt_Comp_pct" EXACT []
is_a: CO_334:0001000 ! Variables
relationship: variable_of CO_334:0000407 ! Moisture content of fresh root
relationship: variable_of CO_334:0010314 ! Estimation: Moisture content_method
relationship: variable_of CO_334:0100583 ! pct (%)

[Term]
id: CO_334:0000070
name: protein content in percentage
namespace: cassava_trait
def: "Percentage (%) of protein content in cassava storage root." [CO:curators]
synonym: "ProtCt_Meas_pct" EXACT []
synonym: "protei" EXACT []
is_a: CO_334:0001000 ! Variables
relationship: variable_of CO_334:0000442 ! Protein content
relationship: variable_of CO_334:0010372 ! Estimation: Protein content_method
relationship: variable_of CO_334:0100583 ! pct (%)

[Term]
id: CO_334:0000071
name: starch content percentage
namespace: cassava_trait
def: "Percentage (%) of complex carbohydrate found in cassava storage root." [CO:curators]
synonym: "starch" EXACT []
synonym: "StrchCt_Est_pct" EXACT []
is_a: CO_334:0001000 ! Variables
relationship: variable_of CO_334:0000474 ! Starch Content
relationship: variable_of CO_334:0010313 ! Estimation: Starch content _method
relationship: variable_of CO_334:0100583 ! pct (%)

[Term]
id: CO_334:0000072
name: sugar content in percentage
namespace: cassava_trait
def: "Estimation of sugar content in cassava storage root expressed in percentage (%)." [CO:curators]
synonym: "sugar" EXACT []
synonym: "SugPCt_Meas_pct" EXACT []
is_a: CO_334:0001000 ! Variables
relationship: variable_of CO_334:0000495 ! Sugar content
relationship: variable_of CO_334:0010379 ! Estimation: Sugar content_method
relationship: variable_of CO_334:0100583 ! pct (%)

[Term]
id: CO_334:0000073
name: total carotenoid content in ug/g
namespace: cassava_trait
def: "Total extracted carotenoids in cassava storage root as estimated by spectrophotometer and expressed in ug per gram fresh weight." [CO:curators]
synonym: "CarotCt_spectro_ugg" EXACT []
synonym: "tc" EXACT []
is_a: CO_334:0001000 ! Variables
relationship: variable_of CO_334:0000297 ! Carotenoid content
relationship: variable_of CO_334:0010368 ! Estimation: Total carotenoid content_method
relationship: variable_of CO_334:0100574 ! ug beta caroten / g fresh weight

[Term]
id: CO_334:0000074
name: poundability assessment 0-4
namespace: cassava_trait
def: "Mealiness of boiled cassava storage root rating as 0 = Non poundable, 1 = slightly poundable, 2 = poundable, 3 = very poundable." [CO:curators]
synonym: "pd" EXACT []
synonym: "Pd_SensScg_1to4" EXACT []
synonym: "Soft and easy to eat for a toothless or weak tooth person" EXACT []
is_a: CO_334:0001000 ! Variables
is_a: CO_334:0001025 ! farmer preference trait post-harvest
is_a: CO_334:0002010 ! Farmer trait
relationship: variable_of CO_334:0000437 ! Poundability
relationship: variable_of CO_334:0010296 ! Sensory Assesment: Poundability_method
relationship: variable_of CO_334:0100502 ! 4pt scale

[Term]
id: CO_334:0000075
name: amylose content in ug/g percentage
namespace: cassava_trait
def: "Estimation of amylose content of cassava roots in percentage (%)." [CO:curators]
synonym: "amyl" EXACT []
synonym: "AmylCt_Meas_pct" EXACT []
is_a: CO_334:0001000 ! Variables
relationship: variable_of CO_334:0000279 ! Amylose content
relationship: variable_of CO_334:0010374 ! Estimation: Amylose  content_method
relationship: variable_of CO_334:0100572 ! ug/g

[Term]
id: CO_334:0000076
name: hydrogen cyanide potential enzymatic method
namespace: cassava_trait
def: "Cyanogenic potential is an indicator of the potential production of hydrogen cyanide in cassava storage roots with less than 5mg/100g fresh weight of root = low, 5-10mg/100g fresh weight of root = medium, and 10mg/100g fresh weight of root = high." [CO:curators]
synonym: "hcn_enz" EXACT []
synonym: "RtCyanCt_Enz_1to3" EXACT []
is_a: CO_334:0001000 ! Variables
relationship: variable_of CO_334:0000502 ! Storage root cyanide content
relationship: variable_of CO_334:0010334 ! Estimation: Hydrogen cyanide potential enzymatic method
relationship: variable_of CO_334:0100540 ! 3pt scale

[Term]
id: CO_334:0000077
name: post-harvest physiological deterioration variable 0-10 scale measured 12 months after planting.
namespace: cassava_trait
def: "Internal root discoloration or vascular streaking that renders cassava roots unfit for human or animal consumption.\nA number of root samples are cut into 7 slices  and each slice is scored on a 0-10 scale. 0 = No symptom of root discoloration, 1 = 10% of the root surface has root discoloration, 2 = 30% of the root surface has root discoloration, 3 = 30% of the root surface has root discoloration, 4 = 40% of the root surface has root discoloration, 5 = 50% of the root surface has root discoloration, 6 = 60% of the root surface has root discoloration, 7 = 70% of the root surface has root discoloration, 8 = 80% of the root surface has root discoloration, 9 = 90% of the root surface has root discoloration, 100 = 100% of the root surface has root discoloration" [CO:curators]
is_a: CO_334:0001000 ! Variables
is_a: CO_334:0001025 ! farmer preference trait post-harvest
relationship: variable_of CO_334:0000266 ! Post-harvest physiological deterioration
relationship: variable_of CO_334:0010001 ! Estimation: Post-harvest physiological deterioration method
relationship: variable_of CO_334:0100680 ! 11pt scale

[Term]
id: CO_334:0000078
name: zinc content in storage root ug/g
namespace: cassava_trait
def: "Total zinc content in cassava storage root." [CO:curators]
synonym: "zn" EXACT []
synonym: "ZnCt_Meas_ugg" EXACT []
is_a: CO_334:0001000 ! Variables
relationship: variable_of CO_334:0000507 ! Zinc content
relationship: variable_of CO_334:0010371 ! Estimation: Zinc content_method
relationship: variable_of CO_334:0100572 ! ug/g

[Term]
id: CO_334:0000079
name: branching level counting
namespace: cassava_trait
def: "Count of the actual number of levels of branching at or before harvest." [CO:curators]
synonym: "BrnchLvl_Count_Lvl" EXACT []
synonym: "brnlev" EXACT []
is_a: CO_334:0001000 ! Variables
relationship: variable_of CO_334:0000296 ! Branching Levels
relationship: variable_of CO_334:0010351 ! Counting: Branching levels_method
relationship: variable_of CO_334:0100557 ! number of levels

[Term]
id: CO_334:0000080
name: branching angle visual rating 0-7
namespace: cassava_trait
def: "Visual rating of a measured angle between vertical plane and first primary branching with 0 = non branching, 3 = 15-30 degrees, 5 = 45-60 degrees, and 7 = 75-90 degrees." [CO:curators]
synonym: "brnang" EXACT []
synonym: "BrnchAng_VisScg_0to7" EXACT []
is_a: CO_334:0001000 ! Variables
relationship: variable_of CO_334:0000294 ! Branching Angle
relationship: variable_of CO_334:0010302 ! Visual Scoring: Branching angle_method
relationship: variable_of CO_334:0100508 ! 8pt scale

[Term]
id: CO_334:0000081
name: leaf vein color visual rating 1-9
namespace: cassava_trait
def: "Visual scoring of leaf vein color with 3 = light green, 5 = dark green, 7 = green-purple, and 9 = purple." [CO:curators]
synonym: "LfVeinCol_VisClsn_1to9" EXACT []
synonym: "lfvnco" EXACT []
is_a: CO_334:0001000 ! Variables
relationship: variable_of CO_334:0000401 ! Leaf Vein Color
relationship: variable_of CO_334:0010337 ! Visual Rating: Leaf vein color_method
relationship: variable_of CO_334:0100543 ! 9pt scale

[Term]
id: CO_334:0000082
name: leaf lobe number counting
namespace: cassava_trait
def: "Most common number of leaf lobes assessed on five leaves from the middle of the plant at six months after planting." [CO:curators]
synonym: "lflbno" EXACT []
synonym: "LfLbNo_Count_Lb" EXACT []
is_a: CO_334:0001000 ! Variables
relationship: variable_of CO_334:0000395 ! Leaf Lobes Number
relationship: variable_of CO_334:0010340 ! Visual Rating: Leaf lobes number_method
relationship: variable_of CO_334:0100546 ! number

[Term]
id: CO_334:0000083
name: leaf lobe position visual rating 1-4
namespace: cassava_trait
def: "Visual rating of the position leaf lobes are held with 1 = erect, 2 = horizontal, 3 = deflexed, and 4 = retorse." [CO:curators]
synonym: "LfLbPo_VisClsn_1to4" EXACT []
synonym: "lflobp" EXACT []
is_a: CO_334:0001000 ! Variables
relationship: variable_of CO_334:0000393 ! Leaf Lobe Position
relationship: variable_of CO_334:0010341 ! Visual Rating: Leaf lobe position_method
relationship: variable_of CO_334:0100547 ! 4pt scale

[Term]
id: CO_334:0000084
name: rotted storage root counting
namespace: cassava_trait
def: "A count of the number of rotted storage roots per plot at the time of harvest." [CO:curators]
synonym: "NoRotRt_Count_Rt" EXACT []
synonym: "rtrot" EXACT []
is_a: CO_334:0001000 ! Variables
relationship: variable_of CO_334:0000457 ! Rotted storage roots
relationship: variable_of CO_334:0010295 ! Counting: Rotted storage roots _method
relationship: variable_of CO_334:0100491 ! root

[Term]
id: CO_334:0000085
name: taste of boiled root rating 1-3
namespace: cassava_trait
def: "Taste of boiled root rating as 1 = sweet, 2 = bland, and 3 = bitter." [CO:curators]
synonym: "Has a taste that cannot even be refused by the pigs. When it is bitter, the pigs rejects it." EXACT []
synonym: "pdtas" EXACT []
synonym: "RtTast_SensClsn_1to3" EXACT []
is_a: CO_334:0001000 ! Variables
is_a: CO_334:0001025 ! farmer preference trait post-harvest
is_a: CO_334:0002010 ! Farmer trait
relationship: variable_of CO_334:0000498 ! Taste of boiled roots
relationship: variable_of CO_334:0010297 ! Gustation: Taste of boiled roots_method
relationship: variable_of CO_334:0100503 ! 3pt scale

[Term]
id: CO_334:0000086
name: apical branching counting of number of weeks
namespace: cassava_trait
def: "Number of weeks from planting to first apical branching associated with the formation of inflorescence." [CO:curators]
synonym: "brntim" EXACT []
synonym: "FstBrnchTim_Count_wk" EXACT []
is_a: CO_334:0001000 ! Variables
relationship: variable_of CO_334:0000282 ! Apical branching
relationship: variable_of CO_334:0010350 ! Visual Rating: Apical branching_method
relationship: variable_of CO_334:0100556 ! weeks

[Term]
id: CO_334:0000087
name: bemisia tabaci adult by counting
namespace: cassava_trait
def: "Number of Bemisia tabaci adult white flies on the top five leaves." [CO:curators]
synonym: "BTAdNo_Count_BTad" EXACT []
synonym: "btadt" EXACT []
is_a: CO_334:0001000 ! Variables
relationship: variable_of CO_334:0000410 ! Number of bemisia tabaci adult
relationship: variable_of CO_334:0010327 ! Counting: Bemisia tabaci adult_method
relationship: variable_of CO_334:0100546 ! number

[Term]
id: CO_334:0000088
name: bemisia tabaci nymphs by counting
namespace: cassava_trait
def: "Number of Bemisia tabaci nymphs white flies on the14th leaf." [CO:curators]
synonym: "btnym" EXACT []
synonym: "BTNymNo_Count_BTNym" EXACT []
is_a: CO_334:0001000 ! Variables
relationship: variable_of CO_334:0000411 ! Number of bemisia tabaci nymphs
relationship: variable_of CO_334:0010328 ! Counting: Bemisia tabaci nymphs_method
relationship: variable_of CO_334:0100546 ! number

[Term]
id: CO_334:0000089
name: Cassava brown streak disease root incidence
namespace: cassava_trait
def: "Proportion of plants within a plot showing root symptoms of cassava brown streak disease" [CO:curators]
synonym: "cbsdr12i" EXACT []
xref: TO:0000148
is_a: CO_334:0000028 ! viral disease

[Term]
id: CO_334:0000090
name: Cassava brown streak disease root severity
namespace: cassava_trait
def: "Cassava brown streak disease root symptoms severity" [CO:curators]
synonym: "Cassava brown streak disease root severity - Cassavabase" EXACT []
synonym: "CBSDLfSev" EXACT []
xref: TO:0000148
is_a: CO_334:0000028 ! viral disease

[Term]
id: CO_334:0000091
name: hydrogen cyanide potential picrate method 1-9
namespace: cassava_trait
def: "Estimate of storage root cyanide content by picrate test with 1 = not detectable and 9 = very high." [CO:curators]
synonym: "hcnpic" EXACT []
synonym: "RtCyanCt_Picrate_1to9" EXACT []
xref: TO:0000955
is_a: CO_334:0001000 ! Variables
relationship: variable_of CO_334:0000502 ! Storage root cyanide content
relationship: variable_of CO_334:0010299 ! Estimation: Hydrogen cyanide potential picrate method
relationship: variable_of CO_334:0100505 ! 9pt scale

[Term]
id: CO_334:0000092
name: dry matter content percentage
namespace: cassava_trait
def: "Percentage dry matter storage root." [CO:curators]
synonym: "dm" EXACT []
synonym: "DMCt_Comp_r" EXACT []
synonym: "Water content" EXACT []
is_a: CO_334:0001000 ! Variables
is_a: CO_334:0001025 ! farmer preference trait post-harvest
is_a: CO_334:0002010 ! Farmer trait
relationship: variable_of CO_334:0000424 ! Root dry matter content
relationship: variable_of CO_334:0010300 ! Estimation: Root dry matter content_method
relationship: variable_of CO_334:0100582 ! ratio
relationship: variable_of CO_334:0100583 ! pct (%)

[Term]
id: CO_334:0000093
name: frog skin disease : visual 1-5
namespace: cassava_trait
def: "Visual rating of symptoms caused by unknown causal agent. Symptoms rated from 1 = (clean, no infection) to 5 = (extremely severe, severely diseased)." [CO:curators]
synonym: "fsd" EXACT []
synonym: "FSDisSev_VisScg_1to5" EXACT []
is_a: CO_334:0001000 ! Variables
relationship: variable_of CO_334:0000370 ! Frog skin disease
relationship: variable_of CO_334:0010283 ! Visual Observation: Frog skin disease_method
relationship: variable_of CO_334:0100489 ! 5 pt scale

[Term]
id: CO_334:0000094
name: proportion lodged plants in percentage
namespace: cassava_trait
def: "Proportion of lodged plants (>45 degrees) in a plot." [CO:curators]
synonym: "LodgPlntProp_Comp_r" EXACT []
synonym: "lodplt" EXACT []
is_a: CO_334:0001000 ! Variables
relationship: variable_of CO_334:0000440 ! Lodged plants
relationship: variable_of CO_334:0010304 ! Counting: Proportion of lodged plants_method
relationship: variable_of CO_334:0100582 ! ratio

[Term]
id: CO_334:0000095
name: beta carotene content ug/g
namespace: cassava_trait
def: "Concentration of beta carotene extracted from root samples and estimated by HPLC expressed in ug per gram fresh weight. \n\nFresh cassava roots are ground into a mash and carotenoids are extracted with acetone and petroleum ether. The extracts are analyzed by HPLC with mobile phases (methanol + ammonium acetate) followed by methy-ter-butyl-ether. The resulting peaks are identified and quantified using calibration standards and calibration curve. Concentrations are expressed in ug/g wet basis." [CO:curators]
synonym: "bcret" EXACT []
synonym: "BetaCarotCt_HPLC_ugg" EXACT []
is_a: CO_334:0001000 ! Variables
relationship: variable_of CO_334:0000291 ! Beta carotene
relationship: variable_of CO_334:0010369 ! Estimation: Beta carotene_method
relationship: variable_of CO_334:0100572 ! ug/g

[Term]
id: CO_334:0000096
name: gari content g/kg
namespace: cassava_trait
def: "Percentage (%) gari processed from fresh storage roots." [CO:curators]
synonym: "garcon" EXACT []
synonym: "GariCt_Comp_gkg" EXACT []
is_a: CO_334:0001000 ! Variables
is_a: CO_334:0001025 ! farmer preference trait post-harvest
relationship: variable_of CO_334:0000374 ! Gari content
relationship: variable_of CO_334:0010315 ! Measurement: Gari content_method
relationship: variable_of CO_334:0100586 ! g/kg

[Term]
id: CO_334:0000097
name: fufu content in g/kg
namespace: cassava_trait
def: "Percentage (%) fufu processed from fresh storage roots." [CO:curators]
synonym: "FfCt_Meas_gkg" EXACT []
synonym: "fufucnt" EXACT []
is_a: CO_334:0001000 ! Variables
is_a: CO_334:0001025 ! farmer preference trait post-harvest
relationship: variable_of CO_334:0000373 ! Fufu content
relationship: variable_of CO_334:0010380 ! Estimation: Fufu content_method
relationship: variable_of CO_334:0100586 ! g/kg

[Term]
id: CO_334:0000098
name: lafun content g/kg
namespace: cassava_trait
def: "Percentage (%) lafun processed from fresh storage roots." [CO:curators]
synonym: "LafuCt_Comp_gkg" EXACT []
synonym: "lafun" EXACT []
is_a: CO_334:0001000 ! Variables
relationship: variable_of CO_334:0000388 ! Lafun content
relationship: variable_of CO_334:0010381 ! Estimation: Lafun content_method
relationship: variable_of CO_334:0100586 ! g/kg

[Term]
id: CO_334:0000099
name: plant architecture visual rating 1-5
namespace: cassava_trait
def: "Plant architecture on a 1-5 scale with 1 = excellent, 2 good, 3 = fair, 4 = bad, and 5 = very bad." [CO:curators]
synonym: "plarch" EXACT []
synonym: "PlntArch_VisScg_1to5" EXACT []
is_a: CO_334:0001000 ! Variables
relationship: variable_of CO_334:0000431 ! Plant architecture
relationship: variable_of CO_334:0010306 ! Visual Rating: Plant architecture_method
relationship: variable_of CO_334:0100512 ! 5pt scale

[Term]
id: CO_334:0000100
name: stipule length visual rating 1-7
namespace: cassava_trait
def: "A qualitative scoring of the length of the leaflike appendage at the base of the leaf with 3= short, 5 = medium, and 7 = long." [CO:curators]
synonym: "stipgt" EXACT []
synonym: "StplLng_VisScg_1to7" EXACT []
is_a: CO_334:0001000 ! Variables
relationship: variable_of CO_334:0000483 ! Stipules length
relationship: variable_of CO_334:0010339 ! Visual Rating: Stipules length_method
relationship: variable_of CO_334:0100545 ! 7pt scale

[Term]
id: CO_334:0000101
name: unexpanded apical leaf color visual rating 1-9
namespace: cassava_trait
def: "Visual rating of unexpanded apical leaf color with 3 = light green, 5 = dark green, 7 = green-purple, and 9 = purple." [CO:curators]
synonym: "LfCol_ApVisClsn_1to9" EXACT []
synonym: "lfcola" EXACT []
is_a: CO_334:0001000 ! Variables
relationship: variable_of CO_334:0000389 ! Leaf color
relationship: variable_of CO_334:0010335 ! Visual Rating: Unexpanded apical leaves colors_method
relationship: variable_of CO_334:0100541 ! 9pt scale

[Term]
id: CO_334:0000102
name: first fully expanded leaf color visual rating 1-9
namespace: cassava_trait
def: "Visual rating of first fully expanded leaf color with 3 = light green, 5 = dark green, 7 = green-purple, and 9 = purple." [CO:curators]
synonym: "LfCol_VisClsn_1to9" EXACT []
synonym: "lfcolf" EXACT []
is_a: CO_334:0001000 ! Variables
relationship: variable_of CO_334:0000389 ! Leaf color
relationship: variable_of CO_334:0010336 ! Visual Rating: First fully expanded leaf color_method
relationship: variable_of CO_334:0100542 ! 9pt scale

[Term]
id: CO_334:0000103
name: anthocyanin pigmentation visual rating 0-3
namespace: cassava_trait
def: "Visual rating of distribution of anthocyanin pigmentation with 0 = absent, 1 = top part, 2 = central part, 3 = totally pigmented." [CO:curators]
synonym: "ACyanPig_VisScg_0to3" EXACT []
synonym: "anthop" EXACT []
is_a: CO_334:0001000 ! Variables
relationship: variable_of CO_334:0000281 ! Anthocyanin pigmentation
relationship: variable_of CO_334:0010346 ! Visual Rating: Anthocyanin pigmentation_method
relationship: variable_of CO_334:0100552 ! 4pt scale

[Term]
id: CO_334:0000104
name: young stem growth habit visual rating 1&2
namespace: cassava_trait
def: "Visual rating of growth habit of young stem with 1= straight and 2 = zig-zag." [CO:curators]
synonym: "stemgh" EXACT []
synonym: "StGrwHab_VisScg_1to2" EXACT []
is_a: CO_334:0001000 ! Variables
relationship: variable_of CO_334:0000505 ! Young Stem Growth Habit
relationship: variable_of CO_334:0010347 ! Visual Rating: Young stem growth habit_method
relationship: variable_of CO_334:0100553 ! 2pt scale

[Term]
id: CO_334:0000105
name: leaf scar prominence visual rating 1-7
namespace: cassava_trait
def: "Visual rating of prominence leaf scars (measured on fresh scars) with 3 = little prominence, 5 = moderately prominent, and 7 = prominent." [CO:curators]
synonym: "lfscar" EXACT []
synonym: "LfScProm_VisScg_1to7" EXACT []
is_a: CO_334:0001000 ! Variables
relationship: variable_of CO_334:0000400 ! Leaf Scar Prominence
relationship: variable_of CO_334:0010349 ! Visual Rating: Leaf scar prominence_method
relationship: variable_of CO_334:0100555 ! 7pt scale

[Term]
id: CO_334:0000106
name: first apical branch height measurement in cm
namespace: cassava_trait
def: "Height of first apical branch (ground level to point of first Apical branch, 9 months after planting) in cm." [CO:curators]
synonym: "BrnchHt_Meas_cm" EXACT []
synonym: "brnht" EXACT []
is_a: CO_334:0001000 ! Variables
relationship: variable_of CO_334:0000293 ! Branch height
relationship: variable_of CO_334:0010352 ! Measurement: First apical branch height_method
relationship: variable_of CO_334:0100558 ! cm

[Term]
id: CO_334:0000107
name: male sterile visual rating 0&1
namespace: cassava_trait
def: "Cassava plants that do no produce viable pollen." [CO:curators]
synonym: "ms" EXACT []
synonym: "PolPrsnc_VisClsn_0or1" EXACT []
is_a: CO_334:0001000 ! Variables
relationship: variable_of CO_334:0000404 ! Male sterile
relationship: variable_of CO_334:0010359 ! Visual Rating: Male sterile_method
relationship: variable_of CO_334:0100565 ! 2pt scale

[Term]
id: CO_334:0000108
name: female staminoids assessment 0&1
namespace: cassava_trait
def: "Visual observation of female cassava flowers without rudimentary stamen scored as 0 = absent and 1 = present." [CO:curators]
synonym: "femsta" EXACT []
synonym: "StamPrsnc_VisClsn_0or1" EXACT []
is_a: CO_334:0001000 ! Variables
relationship: variable_of CO_334:0000365 ! Female stamenoids
relationship: variable_of CO_334:0010358 ! Visual Rating: Female stamenoids_method
relationship: variable_of CO_334:0100564 ! 2pt scale

[Term]
id: CO_334:0000109
name: root constriction visual rating 1-3
namespace: cassava_trait
def: "Visual ratings of root constrcitions (1 = few, 2 = intermediate, 3 = many) as being evaluated by CIAT." [CO:curators]
synonym: "rtcon" EXACT []
synonym: "RtConsNo_Est_1to3" EXACT []
is_a: CO_334:0001000 ! Variables
relationship: variable_of CO_334:0000446 ! Root constrictions number
relationship: variable_of CO_334:0010428 ! Visual rating: Root constriction_method
relationship: variable_of CO_334:0100634 ! 3pt scale

[Term]
id: CO_334:0000110
name: fruit set visual rating 0&1
namespace: cassava_trait
def: "Visual rating of cassava fruit set with 0 = absent and 1 = present." [CO:curators]
synonym: "frtset" EXACT []
synonym: "FrtSetPrsnc_VisClsn_0or1" EXACT []
is_a: CO_334:0001000 ! Variables
relationship: variable_of CO_334:0000372 ! Fruit set presence
relationship: variable_of CO_334:0010308 ! Visual Rating: Fruit set _method
relationship: variable_of CO_334:0100514 ! 2pt scale

[Term]
id: CO_334:0000111
name: flower visual rating 0&1
namespace: cassava_trait
def: "Visual rating of flowers (50%) in plant with 0 = absent and 1 = present." [CO:curators]
synonym: "flower" EXACT []
synonym: "FlwAb_Est_0or1" EXACT []
is_a: CO_334:0001000 ! Variables
relationship: variable_of CO_334:0000367 ! Flowering
relationship: variable_of CO_334:0010434 ! Visual Observation: Flowering_method
relationship: variable_of CO_334:0100513 ! 2pt scale

[Term]
id: CO_334:0000112
name: fruit exocarp texture assessment 1-7
namespace: cassava_trait
def: "Sensory assessment of the texture of outer most layer of the cassava fruit scored as 3 = smooth and 7 = rough." [CO:curators]
synonym: "ExocTex_VisClsn_1to7" EXACT []
synonym: "fruexo" EXACT []
is_a: CO_334:0001000 ! Variables
relationship: variable_of CO_334:0000371 ! Fruit exocarp texture
relationship: variable_of CO_334:0010360 ! Visual Rating: Fruit exocarp Texture_method
relationship: variable_of CO_334:0100566 ! 7pt scale

[Term]
id: CO_334:0000113
name: ploidy level visual rating 1-4
namespace: cassava_trait
def: "Ploidy level (n = 1,2,3,4 ) (by morphological characteristics)." [CO:curators]
synonym: "PldLvl_VisScg_1to4" EXACT []
synonym: "ploidy" EXACT []
is_a: CO_334:0001000 ! Variables
relationship: variable_of CO_334:0000436 ! Ploidy
relationship: variable_of CO_334:0010361 ! Visual Rating: Ploidy_method
relationship: variable_of CO_334:0100567 ! 4pt scale

[Term]
id: CO_334:0000114
name: boiled storage root color visual 1-3
namespace: cassava_trait
def: "Colour of boiled storage roots with  1 = white , 2 = cream , 3 = yellow." [CO:curators]
synonym: "BoilRtCol_VisClsn_1to3" EXACT []
synonym: "pdcol" EXACT []
is_a: CO_334:0001000 ! Variables
relationship: variable_of CO_334:0000355 ! Color of boiled storage roots
relationship: variable_of CO_334:0010298 ! Visual Rating: Color of boiled storage roots_method
relationship: variable_of CO_334:0100504 ! 3pt scale

[Term]
id: CO_334:0000115
name: storage root cortex color visual rating 1-4
namespace: cassava_trait
def: "Visual rating of the color of outer surface of storage root cortex (inner skin color) with 1 = white or cream, 2 = yellow, 3 = pink, 4 = purple." [CO:curators]
synonym: "inncol" EXACT []
synonym: "RtCtxCol_VisClsn_1to4" EXACT []
is_a: CO_334:0001000 ! Variables
relationship: variable_of CO_334:0000486 ! Storage Root Cortex Color
relationship: variable_of CO_334:0010290 ! Visual Rating: Storage root cortex color_method
relationship: variable_of CO_334:0100496 ! 4pt scale

[Term]
id: CO_334:0000116
name: ease of peeling root cortex visual rating 1-7
namespace: cassava_trait
def: "Visual rating of ease of peeling root cortex with 3 = easy and 7 = difficult." [CO:curators]
synonym: "easepl" EXACT []
synonym: "PeelEase_Clsn_1to7" EXACT []
is_a: CO_334:0001000 ! Variables
relationship: variable_of CO_334:0000362 ! Ease of peeling storage root cortex
relationship: variable_of CO_334:0010294 ! Visual Scoring: Ease of peeling root cortex_method
relationship: variable_of CO_334:0100500 ! 7pt scale

[Term]
id: CO_334:0000117
name: beta carotene retention percentage
namespace: cassava_trait
def: "The percentage (%) of beta carotene content in a prepared food product compared to the nutrient content in the raw food." [CO:curators]
synonym: "BCarotRet_Meas_pct" EXACT []
synonym: "bcret" EXACT []
is_a: CO_334:0001000 ! Variables
relationship: variable_of CO_334:0000292 ! Beta carotenoid retention
relationship: variable_of CO_334:0010382 ! Estimation: Beta carotenoid retention_method
relationship: variable_of CO_334:0100583 ! pct (%)

[Term]
id: CO_334:0000118
name: total carotenoid retention percentage
namespace: cassava_trait
def: "The percentage (%) of total carotene content in a prepared food product compared to the nutrient content in the raw food." [CO:curators]
synonym: "CarotRet_Meas_pct" EXACT []
synonym: "tcret" EXACT []
is_a: CO_334:0001000 ! Variables
relationship: variable_of CO_334:0000500 ! Total carotenoid retention
relationship: variable_of CO_334:0010383 ! Estimation: Total carotenoid retention_method
relationship: variable_of CO_334:0100583 ! pct (%)

[Term]
id: CO_334:0000119
name: central leaf shape visual rating 1-10
namespace: cassava_trait
def: "Shape of central leaf taken from a mid-height position rated from 1 = ovoid, 2 = elliptic-lanceolate, 3 = obovate-lanceolate, 4 = oblong-lanceolate, 5 = lanceolate, 6 = straight or linear, 7 = pandurate, 8 = linear-piramidal, 9 = linear-pandurate, and 10 = linear-hostatilobalate." [CO:curators]
synonym: "lfshp" EXACT []
synonym: "LfShp_VisClsn_1to6" EXACT []
is_a: CO_334:0001000 ! Variables
relationship: variable_of CO_334:0000353 ! Central Leaf Shape
relationship: variable_of CO_334:0010342 ! Visual Rating: Central leaf shape_method
relationship: variable_of CO_334:0100548 ! 10pt scale

[Term]
id: CO_334:0000120
name: suitability for intercropping visual rating 0&1
namespace: cassava_trait
def: "Qualitative rating of compatibility for use in intercropping with 0 = unsuitable and 1 = suitable." [CO:curators]
synonym: "intcrp" EXACT []
synonym: "InterCrpSuit_VisClsn_0or1" EXACT []
is_a: CO_334:0001000 ! Variables
relationship: variable_of CO_334:0000496 ! Suitability for intercropping
relationship: variable_of CO_334:0010333 ! Visual Rating: Suitability for intercropping_method
relationship: variable_of CO_334:0100539 ! 2pt scale

[Term]
id: CO_334:0000121
name: amylopectin content ug/g in percentage
namespace: cassava_trait
def: "Estimation of amylopectin content of cassava roots in percentage(%)." [CO:curators]
synonym: "amylp" EXACT []
synonym: "AmylPCt_Meas_pct" EXACT []
is_a: CO_334:0001000 ! Variables
relationship: variable_of CO_334:0000277 ! Amylopectin content
relationship: variable_of CO_334:0010375 ! Estimation: Amylopectin content_method
relationship: variable_of CO_334:0100572 ! ug/g

[Term]
id: CO_334:0000122
name: Cassava green mite incidence
namespace: cassava_trait
def: "Proportion of plants affected by cassava green mite" [CO:curators]
synonym: "cgmi" EXACT []
xref: TO:0000261
is_a: CO_334:0000030 ! insect damage

[Term]
id: CO_334:0000123
name: plant height with leaf in cm
namespace: cassava_trait
def: "Portion of the stem with leaves measured as the distance in centimeter from the point of attachment of the oldest leaf to the youngest leaf (apical leaf portion)." [CO:curators]
synonym: "PLHTLF" EXACT []
is_a: CO_334:0001000 ! Variables
relationship: variable_of CO_334:0000478 ! Stem height
relationship: variable_of CO_334:0010000 ! Measurement: Plant height with leaf_method
relationship: variable_of CO_334:0100558 ! cm

[Term]
id: CO_334:0000124
name: amylose amylopectin root content ratio
namespace: cassava_trait
def: "The amylose content of a cassava root sample divided by the amylopectin content of the same sample." [CO:curators]
synonym: "AmylR_Comp_r" EXACT []
synonym: "amylrt" EXACT []
is_a: CO_334:0001000 ! Variables
relationship: variable_of CO_334:0000278 ! Amylose amylopectin ratio
relationship: variable_of CO_334:0010376 ! Calculation: Amylose amylopectin ratio_method
relationship: variable_of CO_334:0100582 ! ratio

[Term]
id: CO_334:0000125
name: plant height without leaf
namespace: cassava_trait
def: "Portion of stem with no leaf measured in centimeter (cm) by deducting plant height with leaf from plant height." [CO:curators]
synonym: "phtwlf" EXACT []
synonym: "StHt_Meas_cm" EXACT []
is_a: CO_334:0001000 ! Variables
relationship: variable_of CO_334:0000478 ! Stem height
relationship: variable_of CO_334:0010384 ! Measurement: Plant height without leaf_method
relationship: variable_of CO_334:0100558 ! cm

[Term]
id: CO_334:0000126
name: plantable stem assessment
namespace: cassava_trait
def: "Portion of stems (matured and disease free) from few centimeter (cm) above the stump comprising the hardwood, semi hardwood upper shoot portion but excluding the immature greenish shoot portion." [CO:curators]
synonym: "plbstm" EXACT []
synonym: "PltbStLng_Meas_cm" EXACT []
is_a: CO_334:0001000 ! Variables
relationship: variable_of CO_334:0000435 ! Plantable stem length
relationship: variable_of CO_334:0010385 ! Measurement: Plantable stem_method
relationship: variable_of CO_334:0100558 ! cm

[Term]
id: CO_334:0000127
name: stem weight measurement in kg
namespace: cassava_trait
def: "Fresh weight of plantable portion of the plant excluding the leaves, and stump." [CO:curators]
synonym: "stemwt" EXACT []
synonym: "StWt_Meas_kg" EXACT []
is_a: CO_334:0001000 ! Variables
relationship: variable_of CO_334:0000480 ! Stem weight
relationship: variable_of CO_334:0010386 ! Measurement: Stem weight_method
relationship: variable_of CO_334:0100493 ! kg

[Term]
id: CO_334:0000128
name: average stem length
namespace: cassava_trait
def: "Total stem length per plot or per number of plant stands, measure in centimeter (cm)." [CO:curators]
synonym: "astmlt" EXACT []
synonym: "StHt_AvgPlot_cm" EXACT []
is_a: CO_334:0001000 ! Variables
relationship: variable_of CO_334:0000478 ! Stem height
relationship: variable_of CO_334:0010387 ! Measurement: Average stem length_method
relationship: variable_of CO_334:0100558 ! cm

[Term]
id: CO_334:0000129
name: stem number counting
namespace: cassava_trait
def: "A count of the number of stems per plot." [CO:curators]
synonym: "stemno" EXACT []
synonym: "StNo_Count_St" EXACT []
is_a: CO_334:0001000 ! Variables
relationship: variable_of CO_334:0000479 ! Stem number
relationship: variable_of CO_334:0010388 ! Counting: Stem number_method
relationship: variable_of CO_334:0100594 ! stem

[Term]
id: CO_334:0000130
name: tip shoot weight measurement in kg
namespace: cassava_trait
def: "Weight of the tip shoot portion of the stem measured in kilogram (kg)." [CO:curators]
synonym: "TipShWt_Wgh_kg" EXACT []
synonym: "tpshwt" EXACT []
is_a: CO_334:0001000 ! Variables
relationship: variable_of CO_334:0000499 ! Tip shoot weight
relationship: variable_of CO_334:0010389 ! Measurement: Tip shoot weight_method
relationship: variable_of CO_334:0100493 ! kg

[Term]
id: CO_334:0000131
name: marketable root weight measurement in kg
namespace: cassava_trait
def: "Weight of harvested cassava roots in kilogram (kg), visually classified as large sized and medium sized roots excluding the small sized roots." [CO:curators]
synonym: "mkrtwt" EXACT []
synonym: "MkRtWt_Wgh_kg" EXACT []
is_a: CO_334:0001000 ! Variables
relationship: variable_of CO_334:0000406 ! Marketable root weight
relationship: variable_of CO_334:0010390 ! Measurement: Marketable root weight_method
relationship: variable_of CO_334:0100493 ! kg

[Term]
id: CO_334:0000132
name: non marketable root weight measurement in kg
namespace: cassava_trait
def: "Weight of small sized roots that do not attract any market value, measured in kilogram (kg)." [CO:curators]
synonym: "NMkRtWt_Wgh_kg" EXACT []
synonym: "nmrtwt" EXACT []
is_a: CO_334:0001000 ! Variables
relationship: variable_of CO_334:0000409 ! Non marketable root weight
relationship: variable_of CO_334:0010391 ! Measurement: Non marketable root weight_method
relationship: variable_of CO_334:0100493 ! kg

[Term]
id: CO_334:0000133
name: stem rot counting per plot
namespace: cassava_trait
def: "A count of the number of rotted stems per plot at the time of harvest." [CO:curators]
synonym: "RotStmNo_Count_Stm" EXACT []
synonym: "stmrot" EXACT []
is_a: CO_334:0001000 ! Variables
relationship: variable_of CO_334:0000417 ! Number of rotten stem
relationship: variable_of CO_334:0010392 ! Counting: Stem rot_method
relationship: variable_of CO_334:0100546 ! number

[Term]
id: CO_334:0000134
name: leaf weight measurement in kg
namespace: cassava_trait
def: "Weight of fresh foliage leaf (the above ground biomass excluding the stem), measured in kilogram" [CO:curators]
synonym: "lfwt" EXACT []
synonym: "LfWt_Wgh_kg" EXACT []
is_a: CO_334:0001000 ! Variables
relationship: variable_of CO_334:0000402 ! Leaf weight
relationship: variable_of CO_334:0010393 ! Measurement: Leaf weight_method
relationship: variable_of CO_334:0100493 ! kg

[Term]
id: CO_334:0000135
name: stump weight measurement in kg
namespace: cassava_trait
def: "Fresh weight (measured in kilogram) of plant parts at the soil level from the neck of the root to the beginning of the plantable stems." [CO:curators]
synonym: "stmpwt" EXACT []
synonym: "StmpWt_Wgh_kg" EXACT []
is_a: CO_334:0001000 ! Variables
relationship: variable_of CO_334:0000494 ! Stump weight
relationship: variable_of CO_334:0010394 ! Measurement: Stump weight_method
relationship: variable_of CO_334:0100493 ! kg

[Term]
id: CO_334:0000136
name: leaf scar number counting
namespace: cassava_trait
def: "A count of the number of leaf scars on the main stem, where a leaf scar is a node without a leaf." [CO:curators]
synonym: "lfscno" EXACT []
synonym: "LfScNo_Count_Scars" EXACT []
is_a: CO_334:0001000 ! Variables
relationship: variable_of CO_334:0000399 ! Leaf scar number
relationship: variable_of CO_334:0010395 ! Counting: Leaf scar number_method
relationship: variable_of CO_334:0100601 ! scars

[Term]
id: CO_334:0000137
name: leaf scar level measurement in cm
namespace: cassava_trait
def: "The height of the plant  measured in centimeter (cm), from the ground level to the lowest retained leaf on the main stem." [CO:curators]
synonym: "LfScHt_Meas_cm" EXACT []
synonym: "scrlvl" EXACT []
is_a: CO_334:0001000 ! Variables
relationship: variable_of CO_334:0000398 ! Leaf scar height
relationship: variable_of CO_334:0010396 ! Measurement: Leaf scar level_method
relationship: variable_of CO_334:0100558 ! cm

[Term]
id: CO_334:0000138
name: sprout count discrete counting
namespace: cassava_trait
def: "A count of the number of stakes germinated, after planting." [CO:curators]
synonym: "NGermStk_Count_Stk" EXACT []
synonym: "sprtct" EXACT []
is_a: CO_334:0001000 ! Variables
relationship: variable_of CO_334:0000466 ! Sprout count
relationship: variable_of CO_334:0010222 ! Counting: Sprout count _method
relationship: variable_of CO_334:0100546 ! number

[Term]
id: CO_334:0000139
name: branching visual rating 0-3
namespace: cassava_trait
def: "Visual rating of branch height on a scale of 0 = no branching, 1 = low branching (<0.5m), 2 = medium branching (>0.5m <= 1m), 3 = high branching (>= 1)." [CO:curators]
synonym: "branching" EXACT []
synonym: "BrnchHt_VisClsn_0to3" EXACT []
is_a: CO_334:0001000 ! Variables
relationship: variable_of CO_334:0000293 ! Branch height
relationship: variable_of CO_334:0010322 ! Visual Rating: Branching_method
relationship: variable_of CO_334:0100528 ! 4pt scale

[Term]
id: CO_334:0000140
name: branching habit visual observation 1-4
namespace: cassava_trait
def: "Visual observation of the lowest or first branching on a scale of 1 = erect, 2 = dichotomous, 3 = trichotomous, 4 = tetrachotomous. The most frequent occurence on the plot is recorded." [CO:curators]
synonym: "BrnchHab_VisClsn_1to4" EXACT []
synonym: "brnhbt" EXACT []
is_a: CO_334:0001000 ! Variables
relationship: variable_of CO_334:0000295 ! Branching habit
relationship: variable_of CO_334:0010397 ! Visual Rating: Branching habit_method
relationship: variable_of CO_334:0100603 ! 4pt scale

[Term]
id: CO_334:0000141
name: days to 50% branching visual observation
namespace: cassava_trait
def: "Visual observation of when (actual date in the format of dd/mm/yyyy from the date of planting) fifty percent of the plant stand per plot branches. 2 forks/branches (dichotomous), 3 forks/branches (trichotomous), or 4 forks/branches (tetrachotomous)." [CO:curators]
synonym: "flw50b" EXACT []
synonym: "Tim50Brnch_Count_days" EXACT []
is_a: CO_334:0001000 ! Variables
relationship: variable_of CO_334:0000357 ! Days to 50% branching
relationship: variable_of CO_334:0010398 ! Visual Observation: Days to 50% branching_method
relationship: variable_of CO_334:0100611 ! days

[Term]
id: CO_334:0000142
name: days to first inflorescence visual observation
namespace: cassava_trait
def: "Visual observation (actual date in the format of dd/mm/yyyy from the date of planting) of the appearance of a developing inflorescence on a plant or plot." [CO:curators]
synonym: "flwdfi" EXACT []
synonym: "Tim1Flwr_Count_days" EXACT []
is_a: CO_334:0001000 ! Variables
relationship: variable_of CO_334:0000359 ! Days to first inflorescence
relationship: variable_of CO_334:0010399 ! Visual Observation: Days to first inflorescence_method
relationship: variable_of CO_334:0100611 ! days

[Term]
id: CO_334:0000143
name: female flower number at the first 3 branching levels counting
namespace: cassava_trait
def: "A count of the Number female flowers after the buds appear, mature, and grow in size to become distinctive at the first, second, and third branch levels." [CO:curators]
synonym: "FFlwNo_Count_Flw" EXACT []
synonym: "flwfno" EXACT []
is_a: CO_334:0001000 ! Variables
relationship: variable_of CO_334:0000364 ! Female flower number
relationship: variable_of CO_334:0010400 ! Counting: Female flower number_method
relationship: variable_of CO_334:0100606 ! flowers

[Term]
id: CO_334:0000144
name: male flower number counting
namespace: cassava_trait
def: "A count of the number male flowers after the buds appears, matures, and grows in size to become distinctive at the first, second, and third branch levels." [CO:curators]
synonym: "flwmno" EXACT []
synonym: "MFlwNo_Count_Flw" EXACT []
is_a: CO_334:0001000 ! Variables
relationship: variable_of CO_334:0000403 ! Male flower number
relationship: variable_of CO_334:0010401 ! Counting: Male flower number_method
relationship: variable_of CO_334:0100606 ! flowers

[Term]
id: CO_334:0000145
name: number of flowering stalks per branch level counting
namespace: cassava_trait
def: "A count of the number of stalks carrying the buds at every point of branching, where inflorescence starts." [CO:curators]
synonym: "flwstk" EXACT []
synonym: "FlwStlkNo_Count_Stlk" EXACT []
is_a: CO_334:0001000 ! Variables
relationship: variable_of CO_334:0000412 ! Number of flowering stalks
relationship: variable_of CO_334:0010402 ! Counting: Number of flowering stalks per branch level _method
relationship: variable_of CO_334:0100608 ! stalks

[Term]
id: CO_334:0000146
name: number of forks counting
namespace: cassava_trait
def: "Number of branches (2 forks/branches (dichotomous), 3 forks/branches (trichotomous), or 4 forks/branches (tetrachotomous)) at every branching level." [CO:curators]
synonym: "BrnchNo_Count_Brnch" EXACT []
synonym: "flwfrk" EXACT []
is_a: CO_334:0001000 ! Variables
relationship: variable_of CO_334:0000413 ! Number of  forks
relationship: variable_of CO_334:0010403 ! Counting: Number of forks_method
relationship: variable_of CO_334:0100609 ! forks

[Term]
id: CO_334:0000147
name: days to first anthesis visual observation
namespace: cassava_trait
def: "Visual observation of when (actual date in the format of dd/mm/yyyy from the date of planting) any female flower opens up to expose the pistil per plot." [CO:curators]
synonym: "flwdfa" EXACT []
synonym: "TimFstAnth_Comp_days" EXACT []
is_a: CO_334:0001000 ! Variables
relationship: variable_of CO_334:0000358 ! Days to first anthesis
relationship: variable_of CO_334:0010404 ! Visual Observation: Days to first anthesis_method
relationship: variable_of CO_334:0100611 ! days

[Term]
id: CO_334:0000148
name: days to 50% anthesis visual observation
namespace: cassava_trait
def: "Visual observation of when (actual date in the format of dd/mm/yyyy from the date of planting) fifty percent of the female flower opens up to expose the pistil per plot." [CO:curators]
synonym: "flw50a" EXACT []
synonym: "Tim50Anth_Comp_days" EXACT []
is_a: CO_334:0001000 ! Variables
relationship: variable_of CO_334:0000356 ! Days to 50% anthesis
relationship: variable_of CO_334:0010405 ! Visual Observation: Days to 50% anthesis_method
relationship: variable_of CO_334:0100611 ! days

[Term]
id: CO_334:0000149
name: number of fruitset counting
namespace: cassava_trait
def: "A count of the number of fruits formed from the seeds after pollination." [CO:curators]
synonym: "flwfrt" EXACT []
synonym: "FrtSetNo_Count_Frt" EXACT []
is_a: CO_334:0001000 ! Variables
relationship: variable_of CO_334:0000415 ! Number of fruitset
relationship: variable_of CO_334:0010406 ! Counting: Number of fruitset_method
relationship: variable_of CO_334:0100612 ! fruits

[Term]
id: CO_334:0000150
name: bemisia tabaci nymphs yellow : counting
namespace: cassava_trait
def: "Number of yellow Bemisia tabaci whitefly nymphs on fourteenth leaf of the same tallest shoot." [CO:curators]
synonym: "btwfy" EXACT []
synonym: "BTYlwN_Count_Nymph" EXACT []
is_a: CO_334:0001000 ! Variables
relationship: variable_of CO_334:0000290 ! Bemisia tabaci nymphs yellow
relationship: variable_of CO_334:0010407 ! Counting: Bemisia tabaci nymphs yellow_method
relationship: variable_of CO_334:0100614 ! nymphs

[Term]
id: CO_334:0000151
name: bemisia tabaci nymphs black : counting
namespace: cassava_trait
def: "Number of black Bemisia tabaci whitefly nymphs on fourteenth leaf of the same tallest shoot." [CO:curators]
synonym: "BTNBlkY_Count_Nymph" EXACT []
synonym: "btwfb" EXACT []
is_a: CO_334:0001000 ! Variables
relationship: variable_of CO_334:0000288 ! Bemisia tabaci nymphs black
relationship: variable_of CO_334:0010408 ! Counting: Bemisia tabaci nymphs black_method
relationship: variable_of CO_334:0100614 ! nymphs

[Term]
id: CO_334:0000152
name: bemisia tabaci nymphs severity : visual 1-5
namespace: cassava_trait
def: "Visual rating of chlorotic blotches infestation on leaves, caused by whitefly on a rating of 1 = none, 2 = mild chlorotic blotches on <10% of leaves, 3 = damage moderate chlorotic blotches on 10-30% of leaves, 4 = chlorosis on 30-50% of leaves, 5 = chlorosis on >50% of leaves." [CO:curators]
synonym: "BTNSev_Est_1to5" EXACT []
synonym: "btwfs" EXACT []
is_a: CO_334:0001000 ! Variables
relationship: variable_of CO_334:0000289 ! Bemisia tabaci nymphs severity
relationship: variable_of CO_334:0010409 ! Visual Observation: Bemisia tabaci nymphs severity_method
relationship: variable_of CO_334:0100615 ! 5pt scale

[Term]
id: CO_334:0000153
name: Typhlodromalus aripo : visual 1/0
namespace: cassava_trait
def: "Visual observation of the presence of T. aripo with 1 = present, 0 = absence." [CO:curators]
synonym: "taripo" EXACT []
synonym: "TAripoPrns_Est_0or1" EXACT []
is_a: CO_334:0001000 ! Variables
relationship: variable_of CO_334:0000503 ! Typhlodromalus aripo
relationship: variable_of CO_334:0010410 ! Visual Observation: Typhlodromalus aripo_method
relationship: variable_of CO_334:0100616 ! 2pt scale

[Term]
id: CO_334:0000154
name: plant number with inflorescence in proportion
namespace: cassava_trait
def: "Proportion of plants per plot that have an inflorescence at varying growth stages. Plant with pollinated and unpollinated flowers are all counted together." [CO:curators]
synonym: "InflPlntProp_Comp_r" EXACT []
synonym: "pnoinf" EXACT []
is_a: CO_334:0001000 ! Variables
relationship: variable_of CO_334:0000441 ! Proportion of plant with inflorescence
relationship: variable_of CO_334:0010411 ! Counting: Plant number with inflorescence_method
relationship: variable_of CO_334:0100617 ! proportion

[Term]
id: CO_334:0000155
name: number of terminal branches with inflorescence counting
namespace: cassava_trait
def: "The maximum number of  terminal branches with inflorescence observed at all levels of branching in a plot." [CO:curators]
synonym: "InflBrnchNo_Count_Brnch" EXACT []
synonym: "tmbrno" EXACT []
is_a: CO_334:0001000 ! Variables
relationship: variable_of CO_334:0000420 ! Number of terminal branches with inflorescence
relationship: variable_of CO_334:0010412 ! Counting: Number of terminal branches with inflorescence_method
relationship: variable_of CO_334:0100609 ! forks

[Term]
id: CO_334:0000156
name: number of fruits counting
namespace: cassava_trait
def: "Number of fruit observed at all levels of branching per plot." [CO:curators]
synonym: "FrtNo_Count_Frt" EXACT []
synonym: "fruitno" EXACT []
is_a: CO_334:0001000 ! Variables
relationship: variable_of CO_334:0000414 ! Number of fruits
relationship: variable_of CO_334:0010413 ! Counting: Number of fruits _method
relationship: variable_of CO_334:0100546 ! number

[Term]
id: CO_334:0000157
name: root weight in air
namespace: cassava_trait
def: "Weight of cassava root samples usually between 4-5kg of each of the harvested plots in a trial for the purpose of determining the dry matter by specific gravity." [CO:curators]
synonym: "RtWt_DryWgh_kg" EXACT []
synonym: "rwtair" EXACT []
is_a: CO_334:0001000 ! Variables
relationship: variable_of CO_334:0000302 ! Storage root weight by plot
relationship: variable_of CO_334:0010415 ! Measurement: Root weight in air_method
relationship: variable_of CO_334:0100493 ! kg

[Term]
id: CO_334:0000158
name: root weight in water
namespace: cassava_trait
def: "Weight obtained by suspending same root sample initially weighed in air, in water for the purpose of determining the sample dry matter by specific gravity method." [CO:curators]
synonym: "RtWt_WtrWgh_kg" EXACT []
synonym: "rwtwat" EXACT []
is_a: CO_334:0001000 ! Variables
relationship: variable_of CO_334:0000302 ! Storage root weight by plot
relationship: variable_of CO_334:0010416 ! Measurement: Root weight in water_method
relationship: variable_of CO_334:0100493 ! kg

[Term]
id: CO_334:0000159
name: number of planted stakes per plot counting
namespace: cassava_trait
def: "The total number of stakes planted per plot." [CO:curators]
synonym: "NStk_Count_Stk" EXACT []
synonym: "stkplt" EXACT []
is_a: CO_334:0001000 ! Variables
relationship: variable_of CO_334:0000416 ! Number of planted stakes
relationship: variable_of CO_334:0010221 ! Counting: Number of planted stakes_method
relationship: variable_of CO_334:0100546 ! number

[Term]
id: CO_334:0000160
name: dry matter content by specific gravity method
namespace: cassava_trait
def: "Percentage dry matter content derived from the specific gravity (CO_334:0000163) value of weighted cassava (4-5kg). It is calculated as 158.3 * specific gravity  - 142.0" [CO:curators]
synonym: "DMCt_Est_kg" EXACT []
synonym: "dmspg" EXACT []
synonym: "Water content" EXACT []
is_a: CO_334:0001000 ! Variables
is_a: CO_334:0001025 ! farmer preference trait post-harvest
is_a: CO_334:0002010 ! Farmer trait
relationship: variable_of CO_334:0000424 ! Root dry matter content
relationship: variable_of CO_334:0010318 ! Estimation: Dry matter content by specific gravity method
relationship: variable_of CO_334:0100493 ! kg

[Term]
id: CO_334:0000161
name: total carotenoid by chart 1-8
namespace: cassava_trait
def: "Assessment of the level of yellowness in cassava storage root pulp using the tc chart on a scale of : 1 = white, 2 = light cream, 3 = cream, 4 = light yellow, 5 = yellow, 6 = deep yellow, 7 = orange, 8 = pink." [CO:curators]
synonym: "CarotCt_VisClsn_1to8" EXACT []
synonym: "tchart" EXACT []
is_a: CO_334:0001000 ! Variables
relationship: variable_of CO_334:0000297 ! Carotenoid content
relationship: variable_of CO_334:0010319 ! Visual Rating: Total carotenoid by chart_method
relationship: variable_of CO_334:0100525 ! 8pt scale

[Term]
id: CO_334:0000162
name: total carotenoid by iCheck method
namespace: cassava_trait
def: "Measurement of total carotenoid content in a given cassava storage root sample using iCheck kit or device." [CO:curators]
synonym: "CarotCt_icheck_ugg" EXACT []
synonym: "tcichk" EXACT []
is_a: CO_334:0001000 ! Variables
relationship: variable_of CO_334:0000297 ! Carotenoid content
relationship: variable_of CO_334:0010414 ! Estimation: Total carotenoid by icheck method
relationship: variable_of CO_334:0100572 ! ug/g

[Term]
id: CO_334:0000163
name: specific gravity
namespace: cassava_trait
def: "Estimated value obtained by weighing 4-5 kilogram of cassava root in air, and in water.It is calculated as root weight in air divided by the sum of root weight in air and root weight in water. Once calculated, it is used to empirically derive percentage dry matter and starch content of cassava." [CO:curators]
synonym: "spgrv" EXACT []
is_a: CO_334:0001000 ! Variables
relationship: variable_of CO_334:0000447 ! Dry matter content
relationship: variable_of CO_334:0010417 ! Measurement: Specific gravity_method
relationship: variable_of CO_334:0100623 ! g

[Term]
id: CO_334:0000164
name: leaf lobe length measurement in cm
namespace: cassava_trait
def: "Measurement of the length of the middle finger or lobe of a matured leaf in centimeter (cm)." [CO:curators]
synonym: "lflblt" EXACT []
synonym: "LfLobLng_Meas_cm" EXACT []
is_a: CO_334:0001000 ! Variables
relationship: variable_of CO_334:0000391 ! Leaf lobe length
relationship: variable_of CO_334:0010418 ! Measurement: Leaf lobe length_method
relationship: variable_of CO_334:0100558 ! cm

[Term]
id: CO_334:0000165
name: leaf lobe width measurement in cm
namespace: cassava_trait
def: "Measurement of the width of middle finger or lobe of a matured leaf in centimeter (cm)." [CO:curators]
synonym: "lflbwh" EXACT []
synonym: "LfLobWdt_Meas_cm" EXACT []
is_a: CO_334:0001000 ! Variables
relationship: variable_of CO_334:0000394 ! Leaf lobe width
relationship: variable_of CO_334:0010419 ! Measurement: Leaf lobe width_method
relationship: variable_of CO_334:0100558 ! cm

[Term]
id: CO_334:0000166
name: germination count
namespace: cassava_trait
def: "Count of the number of emerging seedlings from each family in the pre-nursery done on a daily basis until its ready for transplanting." [CO:curators]
synonym: "germcnt" EXACT []
synonym: "SdlngNo_Count_Sdlng" EXACT []
is_a: CO_334:0001000 ! Variables
relationship: variable_of CO_334:0000460 ! Seedling number
relationship: variable_of CO_334:0010420 ! Counting: Germination count_method
relationship: variable_of CO_334:0100626 ! seedling

[Term]
id: CO_334:0000167
name: number of seed sown counting
namespace: cassava_trait
def: "Count of the number of seeds sown per family in the pre-nursery or directly in the nursery bed." [CO:curators]
synonym: "seedno" EXACT []
synonym: "SownSdNo_Count_Sd" EXACT []
is_a: CO_334:0001000 ! Variables
relationship: variable_of CO_334:0000418 ! Number of seeds sown
relationship: variable_of CO_334:0010421 ! Counting: Number of seeds sown_method
relationship: variable_of CO_334:0100627 ! seed

[Term]
id: CO_334:0000168
name: non marketable root number counting
namespace: cassava_trait
def: "Count of the number of storage root sizes visually adjudged to be small and less than one (1) kilogram." [CO:curators]
synonym: "nmkrtno" EXACT []
synonym: "NMkRtNo_Count_Rt" EXACT []
is_a: CO_334:0001000 ! Variables
relationship: variable_of CO_334:0000408 ! Non marketable root number
relationship: variable_of CO_334:0010320 ! Counting: Non marketable root number_method
relationship: variable_of CO_334:0100546 ! number

[Term]
id: CO_334:0000169
name: marketable root number counting
namespace: cassava_trait
def: "Count of the number of storage root sizes visually adjudged to be big and weigh above one (1) kilogram." [CO:curators]
synonym: "MkRtNo_Count_Rt" EXACT []
synonym: "mktrtno" EXACT []
is_a: CO_334:0001000 ! Variables
relationship: variable_of CO_334:0000405 ! Marketable root number
relationship: variable_of CO_334:0010321 ! Counting: Marketable root number_method
relationship: variable_of CO_334:0100546 ! number

[Term]
id: CO_334:0000170
name: stock weight measurement in kg
namespace: cassava_trait
def: "Measurement of fresh weight of the planted part anchoring the storage roots, and measured in kilogram (kg)" [CO:curators]
synonym: "stkwt" EXACT []
synonym: "StkWt_Meas_kg" EXACT []
is_a: CO_334:0001000 ! Variables
relationship: variable_of CO_334:0000484 ! Stock weight
relationship: variable_of CO_334:0010316 ! Measurement: Stock weight_method
relationship: variable_of CO_334:0100493 ! kg

[Term]
id: CO_334:0000171
name: stem yield estimation
namespace: cassava_trait
def: "Fresh weight in kilogram (kg) of above ground harvested plant biomass excluding the leaves." [CO:curators]
synonym: "StmWt_Wgh_kg" EXACT []
synonym: "stmyld" EXACT []
is_a: CO_334:0001000 ! Variables
relationship: variable_of CO_334:0000480 ! Stem weight
relationship: variable_of CO_334:0010317 ! Counting: Stem yield_method
relationship: variable_of CO_334:0100493 ! kg

[Term]
id: CO_334:0000172
name: trans 9 beta carotene activity in percentage
namespace: cassava_trait
def: "Estimation of  beta carotenoid components with 100% proVitamin A activity." [CO:curators]
synonym: "trans-9" EXACT []
synonym: "Trans9Act_Est_pct" EXACT []
is_a: CO_334:0001000 ! Variables
relationship: variable_of CO_334:0000501 ! Trans-9 activity
relationship: variable_of CO_334:0010422 ! Estimation: Trans 9_method
relationship: variable_of CO_334:0100583 ! pct (%)

[Term]
id: CO_334:0000173
name: cis 9 isomer activity in percentage
namespace: cassava_trait
def: "Estimation of  isomer activity with 50% proVitamin A in percentage (%)." [CO:curators]
synonym: "cis-9" EXACT []
synonym: "Cis9Act_Est_pct" EXACT []
is_a: CO_334:0001000 ! Variables
relationship: variable_of CO_334:0000354 ! Cis 9 activity
relationship: variable_of CO_334:0010423 ! Estimation: Cis 9_method
relationship: variable_of CO_334:0100583 ! pct (%)

[Term]
id: CO_334:0000174
name: B Cryptoxanthin estimation in percentage
namespace: cassava_trait
def: "Estimation of B-cryptoxanthin (carotenoid that has hydroxyl group with 50% activity)." [CO:curators]
synonym: "b-crypto" EXACT []
synonym: "BCryptoAct_Est_pct" EXACT []
is_a: CO_334:0001000 ! Variables
relationship: variable_of CO_334:0000287 ! B crypto activity
relationship: variable_of CO_334:0010424 ! Estimation: B crypto_method
relationship: variable_of CO_334:0100583 ! pct (%)

[Term]
id: CO_334:0000175
name: cassava bacterial blight severity 3-month evaluation
namespace: cassava_trait
def: "Visual rating of symptoms in response to the bacterial blight disease caused by Xanthonomas axonopodis pv. Manihotis, evaluated between two and three months after planting. Symptoms rated from 1 = (clean, no infection), 2 = Small lesions around points of infections on the leaves, 3 = Extension and appearance of new lesions on leaves and stems. Some leaves wilt, 4 = Extensive leaf wilting and defoliation,  5 = extremely severe with leaf wilting, defoliation and dieback." [CO:curators]
synonym: "cbb3s" EXACT []
synonym: "CBBSev_VisScg_1to5_T3m" EXACT []
is_a: CO_334:0001000 ! Variables
relationship: variable_of CO_334:0000031 ! Cassava bacterial blight severity
relationship: variable_of CO_334:0010242 ! Visual Observation: Cassava bacterial blight severity 3-month evalution_method
relationship: variable_of CO_334:0100448 ! 5 pt scale

[Term]
id: CO_334:0000176
name: cassava bacterial blight severity 6-month evaluation
namespace: cassava_trait
def: "Visual rating of symptoms in response to the bacterial blight disease caused by Xanthonomas axonopodis pv. Manihotis,evaluated four and six months after planting. Symptoms rated from 1 = (clean, no infection), 2 = Small lesions around points of infections on the leaves, 3 = Extension and appearance of new lesions on leaves and stems. Some leaves wilt, 4 = Extensive leaf wilting and defoliation,  5 = extremely severe with leaf wilting, defoliation and dieback." [CO:curators]
synonym: "cbb6s" EXACT []
synonym: "CBBSev_VisScg_1to5_T6m" EXACT []
is_a: CO_334:0001000 ! Variables
relationship: variable_of CO_334:0000031 ! Cassava bacterial blight severity
relationship: variable_of CO_334:0010243 ! Visual Observation: Cassava bacterial blight severity 6-month evalution_method
relationship: variable_of CO_334:0100449 ! 5 pt scale

[Term]
id: CO_334:0000177
name: cassava bacterial blight severity 9-month evaluation
namespace: cassava_trait
def: "Visual rating of symptoms in response to the bacterial blight disease caused by Xanthonomas axonopodis pv. Manihotis,evaluated between seven and nine months after planting. Symptoms rated from 1 = (clean, no infection), 2 = Small lesions around points of infections on the leaves, 3 = Extension and appearance of new lesions on leaves and stems. Some leaves wilt, 4 = Extensive leaf wilting and defoliation,  5 = extremely severe with leaf wilting, defoliation and dieback." [CO:curators]
synonym: "cbb9s" EXACT []
synonym: "CBBSev_VisScg_1to5_T9m" EXACT []
is_a: CO_334:0001000 ! Variables
is_a: CO_334:0001027 ! farmer preference trait at harvest
relationship: variable_of CO_334:0000031 ! Cassava bacterial blight severity
relationship: variable_of CO_334:0010244 ! Visual Observation: Cassava bacterial blight severity 9-month evalution_method
relationship: variable_of CO_334:0100450 ! 5 pt scale

[Term]
id: CO_334:0000178
name: cassava bacterial blight incidence 3-month evaluation
namespace: cassava_trait
def: "Proportion of plants within a plot showing symptoms of cassava bacterial blight, evaluated between two and three months after planting." [CO:curators]
synonym: "cbb3i" EXACT []
synonym: "CBBInc_Comp_r_T3m" EXACT []
is_a: CO_334:0001000 ! Variables
relationship: variable_of CO_334:0000037 ! Cassava bacterial blight incidence
relationship: variable_of CO_334:0010247 ! Counting: Cassava bacterial blight incidence 3-month evalution_method
relationship: variable_of CO_334:0100582 ! ratio

[Term]
id: CO_334:0000179
name: cassava bacterial blight incidence 6-month evaluation
namespace: cassava_trait
def: "Proportion of plants within a plot showing symptoms of cassava bacterial blight, evaluated between four and six months after planting." [CO:curators]
synonym: "cbb6i" EXACT []
synonym: "CBBInc_Comp_r_T6m" EXACT []
is_a: CO_334:0001000 ! Variables
relationship: variable_of CO_334:0000037 ! Cassava bacterial blight incidence
relationship: variable_of CO_334:0010248 ! Counting: Cassava bacterial blight incidence 6-month evalution_method
relationship: variable_of CO_334:0100582 ! ratio

[Term]
id: CO_334:0000180
name: cassava bacterial blight incidence 9-month evaluation
namespace: cassava_trait
def: "Proportion of plants within a plot showing symptoms of cassava bacterial blight, evaluated between seven and nine months after planting." [CO:curators]
synonym: "cbb9i" EXACT []
synonym: "CBBInc_Comp_r_T9m" EXACT []
is_a: CO_334:0001000 ! Variables
relationship: variable_of CO_334:0000037 ! Cassava bacterial blight incidence
relationship: variable_of CO_334:0010249 ! Counting: Cassava bacterial blight incidence 9-month evalution_method
relationship: variable_of CO_334:0100582 ! ratio

[Term]
id: CO_334:0000181
name: cassava anthractnose disease incidence in 6-month
namespace: cassava_trait
def: "Proportion of plants within a plot showing symptoms of cassava anthracnose disease evaluated between four and six months after planting (6MAP)." [CO:curators]
synonym: "cad6i" EXACT []
synonym: "CADisInc_Comp_r_T6m" EXACT []
is_a: CO_334:0001000 ! Variables
relationship: variable_of CO_334:0000038 ! Cassava anthracnose disease incidence
relationship: variable_of CO_334:0010258 ! Counting: Cassava anthractnose disease incidence in 6-months_method
relationship: variable_of CO_334:0100582 ! ratio

[Term]
id: CO_334:0000182
name: cassava anthractnose disease incidence in 9-month
namespace: cassava_trait
def: "Proportion of plants within a plot showing symptoms of cassava anthracnose disease evaluated between seven and nine months after planting (9MAP)." [CO:curators]
synonym: "cad9i" EXACT []
synonym: "CADisInc_Comp_r_T9m" EXACT []
is_a: CO_334:0001000 ! Variables
relationship: variable_of CO_334:0000038 ! Cassava anthracnose disease incidence
relationship: variable_of CO_334:0010259 ! Counting: Cassava anthractnose disease incidence in 9-months_method
relationship: variable_of CO_334:0100582 ! ratio

[Term]
id: CO_334:0000183
name: cassava anthractnose disease incidence in12-month
namespace: cassava_trait
def: "Proportion of plants within a plot showing symptoms of cassava anthracnose disease evaluated between ten and twelve months after planting (12MAP)." [CO:curators]
synonym: "cad12i" EXACT []
synonym: "CADisInc_Comp_r_T12m" EXACT []
is_a: CO_334:0001000 ! Variables
relationship: variable_of CO_334:0000038 ! Cassava anthracnose disease incidence
relationship: variable_of CO_334:0010260 ! Counting: Cassava anthractnose disease incidence in 12-months_method
relationship: variable_of CO_334:0100582 ! ratio

[Term]
id: CO_334:0000184
name: cassava anthractnose disease severity in 6-month
namespace: cassava_trait
def: "Visual rating of symptoms in response to the anthracnose disease caused by Colletotrichum gloeosporioides f. sp., evaluated between four and six months after planting (6MAP). Symptoms rated from 1 = (clean, no infection) 2 = Few shallow cankers on stem late in the growing season, 3 = Many deep cankers on stems followed by distortion, 4 = Many oval lesions on hard and woody stems, 5 = Highly severe with many lesions on hard and woody stems and severe necrosis at leaf axils followed by wilting and severe defoliation." [CO:curators]
synonym: "cad6s" EXACT []
synonym: "CADisSev_VisScg_1to5_T6m" EXACT []
is_a: CO_334:0001000 ! Variables
relationship: variable_of CO_334:0000032 ! Cassava anthracnose disease severity
relationship: variable_of CO_334:0010253 ! Visual Observation: Cassava anthractnose disease severity in 6-months_method
relationship: variable_of CO_334:0100459 ! 5 pt scale

[Term]
id: CO_334:0000185
name: cassava anthractnose disease severity in 9-month
namespace: cassava_trait
def: "Visual rating of symptoms in response to the anthracnose disease caused by Colletotrichum gloeosporioides f. sp., evaluated between seven and nine months after planting (9MAP). Symptoms rated from 1 = (clean, no infection) 2 = Few shallow cankers on stem late in the growing season, 3 = Many deep cankers on stems followed by distortion, 4 = Many oval lesions on hard and woody stems, 5 = Highly severe with many lesions on hard and woody stems and severe necrosis at leaf axils followed by wilting and severe defoliation." [CO:curators]
synonym: "cad9s" EXACT []
synonym: "CADisSev_VisScg_1to5_T9m" EXACT []
is_a: CO_334:0001000 ! Variables
relationship: variable_of CO_334:0000032 ! Cassava anthracnose disease severity
relationship: variable_of CO_334:0010254 ! Visual Observation: Cassava anthractnose disease severity in 9-months_method
relationship: variable_of CO_334:0100460 ! 5 pt scale

[Term]
id: CO_334:0000186
name: cassava anthractnose disease severity in12-month
namespace: cassava_trait
def: "Visual rating of symptoms in response to the anthracnose disease caused by Colletotrichum gloeosporioides f. sp., evaluated between ten and twelve months after planting (12MAP). Symptoms rated from 1 = (clean, no infection) 2 = Few shallow cankers on stem late in the growing season, 3 = Many deep cankers on stems followed by distortion, 4 = Many oval lesions on hard and woody stems, 5 = Highly severe with many lesions on hard and woody stems and severe necrosis at leaf axils followed by wilting and severe defoliation." [CO:curators]
synonym: "cad12s" EXACT []
synonym: "CADisSev_VisScg_1to5_T12m" EXACT []
is_a: CO_334:0001000 ! Variables
is_a: CO_334:0001027 ! farmer preference trait at harvest
relationship: variable_of CO_334:0000032 ! Cassava anthracnose disease severity
relationship: variable_of CO_334:0010255 ! Visual Observation: Cassava anthractnose disease severity in 12-months_method
relationship: variable_of CO_334:0100461 ! 5 pt scale

[Term]
id: CO_334:0000187
name: cassava green mite incidence first evaluation
namespace: cassava_trait
def: "Proportion of plants within a plot affected by cassava green mite, Mononychellus tanajoa evaluated at the peak of dry season." [CO:curators]
synonym: "cgm1i" EXACT []
synonym: "CGMInc_Comp_r" EXACT []
is_a: CO_334:0001000 ! Variables
relationship: variable_of CO_334:0000122 ! Cassava green mite incidence
relationship: variable_of CO_334:0010262 ! Counting: Cassava green mite incidence first evaluation_method
relationship: variable_of CO_334:0100582 ! ratio

[Term]
id: CO_334:0000188
name: cassava green mite incidence second evaluation
namespace: cassava_trait
def: "Proportion of plants within a plot affected by cassava green mite, Mononychellus tanajoa evaluated at the peak of dry season." [CO:curators]
synonym: "cgm2i" EXACT []
synonym: "CGMInc_Comp_r" EXACT []
is_a: CO_334:0001000 ! Variables
relationship: variable_of CO_334:0000122 ! Cassava green mite incidence
relationship: variable_of CO_334:0010263 ! Counting: Cassava green mite incidence second evaluation_method
relationship: variable_of CO_334:0100582 ! ratio

[Term]
id: CO_334:0000189
name: cassava green mite severity first evaluation
namespace: cassava_trait
def: "Visual rating of damage caused by cassava green mite (Mononychellus tanajoa), evaluated at the early period of the peak of dry season. Symptoms rated from 1 = (clean, no infection) 2 = Slight spackling and reduction in leaf size, 3 = Serious spackling and reduction in leaf size, 4 = Bunchy top symptoms , obvious reduction of internode length, severe reduction in lead size and leaf area,  to 5 = Candlestick appearance, internode length reduction, young portion of shoot curved and completely defoliated." [CO:curators]
synonym: "cgm1" EXACT []
synonym: "CGMsev_VisScg_1to5" EXACT []
is_a: CO_334:0001000 ! Variables
is_a: CO_334:0001027 ! farmer preference trait at harvest
relationship: variable_of CO_334:0000033 ! Cassava green mite severity
relationship: variable_of CO_334:0010265 ! Visual Observation: Cassava green mite severity first evaluation_method
relationship: variable_of CO_334:0100471 ! 5 pt scale

[Term]
id: CO_334:0000190
name: cassava green mite severity second evaluation
namespace: cassava_trait
def: "Visual rating of damage caused by cassava green mite (Mononychellus tanajoa), evaluated late into the peak of dry season. Symptoms rated from 1 = (clean, no infection) 2 = Slight spackling and reduction in leaf size, 3 = Serious spackling and reduction in leaf size, 4 = Bunchy top symptoms , obvious reduction of internode length, severe reduction in lead size and leaf area,  to 5 = Candlestick appearance, internode length reduction, young portion of shoot curved and completely defoliated." [CO:curators]
synonym: "cgm2" EXACT []
synonym: "CGMsev_VisScg_1to5" EXACT []
is_a: CO_334:0001000 ! Variables
is_a: CO_334:0001027 ! farmer preference trait at harvest
relationship: variable_of CO_334:0000033 ! Cassava green mite severity
relationship: variable_of CO_334:0010266 ! Visual Observation: Cassava green mite severity second evaluation_method
relationship: variable_of CO_334:0100472 ! 5 pt scale

[Term]
id: CO_334:0000191
name: cassava mosaic disease severity 1-month evaluation
namespace: cassava_trait
def: "Visual rating of symptoms caused by cassava mosaic virus,in the family Geminiviridae and genus Begomovirus , evalutaed between one to six weeks after planting. Symptoms rated from 1 = (clean, no infection), 2= Up to 25% leaf area chlorotic, mild leaf distortion, no stunting, 3 = 25-50% leaf area chlorotic, moderate leaf distortion, no stunting, 4 = 50-75% leaf area chlorotic, severe leaf distortion, moderate stunting, 5 = 75 - 100% leaf area chlorotic, severe leaf distortion, small leaflets (almost no lamina), severe stunting." [CO:curators]
synonym: "cmd1s" EXACT []
synonym: "CMDisSev_VisScg_1to5_T1m" EXACT []
is_a: CO_334:0001000 ! Variables
relationship: variable_of CO_334:0000035 ! Cassava mosaic disease severity
relationship: variable_of CO_334:0010230 ! Visual Observation: Cassava mosaic disease severity 1-month evaluation_method
relationship: variable_of CO_334:0100436 ! 5 point scales

[Term]
id: CO_334:0000192
name: cassava mosaic disease severity 3-month evaluation
namespace: cassava_trait
def: "Visual rating of symptoms caused by cassava mosaic virus,in the family Geminiviridae and genus Begomovirus , evalutaed between two and three months after planting.  Symptoms rated from 1 = (clean, no infection), 2= Up to 25% leaf area chlorotic, mild leaf distortion, no stunting, 3 = 25-50% leaf area chlorotic, moderate leaf distortion, no stunting, 4 = 50-75% leaf area chlorotic, severe leaf distortion, moderate stunting, 5 = 75 - 100% leaf area chlorotic, severe leaf distortion, small leaflets (almost no lamina), severe stunting." [CO:curators]
synonym: "cmd3s" EXACT []
synonym: "CMDisSev_VisScg_1to5_T3m" EXACT []
is_a: CO_334:0001000 ! Variables
relationship: variable_of CO_334:0000035 ! Cassava mosaic disease severity
relationship: variable_of CO_334:0010231 ! Visual Observation: Cassava mosaic disease severity 3-month evaluation_method
relationship: variable_of CO_334:0100437 ! 5pt scale

[Term]
id: CO_334:0000193
name: cassava mosaic disease severity 9-month evaluation
namespace: cassava_trait
def: "Visual rating of symptoms caused by cassava mosaic virus,in the family Geminiviridae and genus Begomovirus , evaluated between seven and nine months after planting.  Symptoms rated from 1 = (clean, no infection), 2= Up to 25% leaf area chlorotic, mild leaf distortion, no stunting, 3 = 25-50% leaf area chlorotic, moderate leaf distortion, no stunting, 4 = 50-75% leaf area chlorotic, severe leaf distortion, moderate stunting, 5 = 75 - 100% leaf area chlorotic, severe leaf distortion, small leaflets (almost no lamina), severe stunting." [CO:curators]
synonym: "cmd9s" EXACT []
synonym: "CMDisSev_VisScg_1to5_T9m" EXACT []
is_a: CO_334:0001000 ! Variables
relationship: variable_of CO_334:0000035 ! Cassava mosaic disease severity
relationship: variable_of CO_334:0010233 ! Visual Observation: Cassava mosaic disease severity 9-month evaluation_method
relationship: variable_of CO_334:0100439 ! 5 pt scale

[Term]
id: CO_334:0000194
name: cassava mosaic disease severity 6-month evaluation
namespace: cassava_trait
def: "Visual rating of symptoms caused by cassava mosaic virus,in the family Geminiviridae and genus Begomovirus , evalutaed between four and six months after planting.  Symptoms rated from 1 = (clean, no infection), 2= Up to 25% leaf area chlorotic, mild leaf distortion, no stunting, 3 = 25-50% leaf area chlorotic, moderate leaf distortion, no stunting, 4 = 50-75% leaf area chlorotic, severe leaf distortion, moderate stunting, 5 = 75 - 100% leaf area chlorotic, severe leaf distortion, small leaflets (almost no lamina), severe stunting." [CO:curators]
synonym: "cmd6s" EXACT []
synonym: "CMDisSev_VisScg_1to5_T6m" EXACT []
is_a: CO_334:0001000 ! Variables
relationship: variable_of CO_334:0000035 ! Cassava mosaic disease severity
relationship: variable_of CO_334:0010232 ! Visual Observation: Cassava mosaic disease severity 6-month evaluation_method
relationship: variable_of CO_334:0100438 ! 5 pt scale

[Term]
id: CO_334:0000195
name: cassava mosaic disease incidence 1-month evaluation
namespace: cassava_trait
def: "Proportion of plants within a plot showing symptoms of cassava mosaic disease, evaluated between one and  six weeks after planting." [CO:curators]
synonym: "cmd1i" EXACT []
synonym: "CMDisInc_Comp_r_T1m" EXACT []
is_a: CO_334:0001000 ! Variables
relationship: variable_of CO_334:0000039 ! Cassava mosaic disease incidence
relationship: variable_of CO_334:0010236 ! Counting: Cassava mosaic disease incidence 1-month evaluation_method
relationship: variable_of CO_334:0100582 ! ratio

[Term]
id: CO_334:0000196
name: cassava mosaic disease incidence 3-month evaluation
namespace: cassava_trait
def: "Proportion of plants within a plot showing symptoms of cassava mosaic disease, evaluated two and three months after planting." [CO:curators]
synonym: "cmd3i" EXACT []
synonym: "CMDisInc_Comp_r_T3m" EXACT []
is_a: CO_334:0001000 ! Variables
relationship: variable_of CO_334:0000039 ! Cassava mosaic disease incidence
relationship: variable_of CO_334:0010237 ! Counting: Cassava mosaic disease incidence 3-month evaluation_method
relationship: variable_of CO_334:0100582 ! ratio

[Term]
id: CO_334:0000197
name: cassava mosaic disease incidence 9-month evaluation
namespace: cassava_trait
def: "Proportion of plants within a plot showing symptoms of cassava mosaic disease, evaluated between seven and nine months after planting." [CO:curators]
synonym: "cmd9i" EXACT []
synonym: "CMDisInc_Comp_r_T9m" EXACT []
is_a: CO_334:0001000 ! Variables
relationship: variable_of CO_334:0000039 ! Cassava mosaic disease incidence
relationship: variable_of CO_334:0010239 ! Counting: Cassava mosaic disease incidence 9-month evaluation_method
relationship: variable_of CO_334:0100582 ! ratio

[Term]
id: CO_334:0000198
name: cassava mosaic disease incidence 6-month evaluation
namespace: cassava_trait
def: "Proportion of plants within a plot showing symptoms of cassava mosaic disease, evaluated between four and six months after planting." [CO:curators]
synonym: "cmd6i" EXACT []
synonym: "CMDisInc_Comp_r_T6m" EXACT []
is_a: CO_334:0001000 ! Variables
relationship: variable_of CO_334:0000039 ! Cassava mosaic disease incidence
relationship: variable_of CO_334:0010238 ! Counting: Cassava mosaic disease incidence 6-month evaluation_method
relationship: variable_of CO_334:0100582 ! ratio

[Term]
id: CO_334:0000199
name: cassava mosaic disease severity 12-month evaluation
namespace: cassava_trait
def: "Visual rating of symptoms caused by cassava mosaic virus,in the family Geminiviridae and genus Begomovirus , evalutaed between ten and  twelve months after planting. Symptoms rated from 1 = (clean, no infection), 2= Up to 25% leaf area chlorotic, mild leaf distortion, no stunting, 3 = 25-50% leaf area chlorotic, moderate leaf distortion, no stunting, 4 = 50-75% leaf area chlorotic, severe leaf distortion, moderate stunting, 5 = 75 - 100% leaf area chlorotic, severe leaf distortion, small leaflets (almost no lamina), severe stunting." [CO:curators]
synonym: "cmd12s" EXACT []
synonym: "CMDisSev_VisScg_1to5_T12m" EXACT []
is_a: CO_334:0001000 ! Variables
is_a: CO_334:0001027 ! farmer preference trait at harvest
relationship: variable_of CO_334:0000035 ! Cassava mosaic disease severity
relationship: variable_of CO_334:0010234 ! Visual Observation: Cassava mosaic disease severity 12-month evaluation_method
relationship: variable_of CO_334:0100440 ! 5 pt scale

[Term]
id: CO_334:0000200
name: cassava mosaic disease incidence 12-month evaluation
namespace: cassava_trait
def: "Proportion of plants within a plot showing symptoms of cassava mosaic disease, evaluated between ten and twelve months after planting." [CO:curators]
synonym: "cmd12i" EXACT []
synonym: "CMDisInc_Comp_r_T12m" EXACT []
is_a: CO_334:0001000 ! Variables
relationship: variable_of CO_334:0000039 ! Cassava mosaic disease incidence
relationship: variable_of CO_334:0010240 ! Counting: Cassava mosaic disease incidence 12-month evaluation_method
relationship: variable_of CO_334:0100582 ! ratio

[Term]
id: CO_334:0000201
name: cassava brown streak disease root severity 12-month evaluation
namespace: cassava_trait
def: "Visual rating of root symptoms caused by cassava brown streak virus at twelve months after planting, in the family Potyviridae and genus Ipomovirus. Symptoms rated from 1 = (clean, no infection), 2 = less than 5% of storage root tissue is necrotic, 3 = 5-10% of storage root tissue is necrotic 4 = 10-50% of storage root tissue is necrotic,   5 = More than 50% of storage root tissue is necrotic." [CO:curators]
synonym: "CBSDisRtSev_Scg_1to5" EXACT []
synonym: "cbsdr12s" EXACT []
is_a: CO_334:0001000 ! Variables
is_a: CO_334:0001027 ! farmer preference trait at harvest
relationship: variable_of CO_334:0000090 ! Cassava brown streak disease root severity
relationship: variable_of CO_334:0010280 ! Visual Observation: Cassava brown streak disease root severity 12-month evaluation_method
relationship: variable_of CO_334:0100486 ! 5 pt scale

[Term]
id: CO_334:0000202
name: cassava brown streak disease root incidence 12-month evaluation
namespace: cassava_trait
def: "Proportion of plants within a plot showing root symptoms of cassava brown streak disease at twelve months after planting." [CO:curators]
synonym: "CBSDisRtInc_Comp_r" EXACT []
synonym: "cbsdr12i" EXACT []
is_a: CO_334:0001000 ! Variables
relationship: variable_of CO_334:0000089 ! Cassava brown streak disease root incidence
relationship: variable_of CO_334:0010282 ! Counting: Cassava brown streak disease root incidence 12-month evaluation_method
relationship: variable_of CO_334:0100582 ! ratio

[Term]
id: CO_334:0000203
name: cassava brown streak disease leaf severity 1-month evaluation
namespace: cassava_trait
def: "Visual rating of leaf symptoms caused by cassava brown streak virus evaluated between one and six weeks after planting, in the family Potyviridae and genus Ipomovirus. Symptoms rated from 1 = (clean, no infection), 2 = mild/slight vein yellowing or chlorotic blotches on leaves, no brown streaks/lesions on green stem portions\n, 3 = mild/slight vein yellowing or chlorotic blotches on leaves mild brown streaks/lesions on green stem portions, 4 = severe/extensive vein yellowing or chlorotic blotches on leaves severe brown streaks/lesions on green stem portions no defoliation, stem dieback or stunting, 4 =  to 5 = severe/extensive vein yellowing or chlorotic blotches on leaves severe brown streaks/lesions on green stem portions defoliation, stem dieback or stunting." [CO:curators]
synonym: "CBSDisLfSev_Scg_1to5_T1m" EXACT []
synonym: "cbsdl1s" EXACT []
is_a: CO_334:0001000 ! Variables
relationship: variable_of CO_334:0000036 ! Cassava brown streak disease leaf severity
relationship: variable_of CO_334:0010270 ! Visual Observation: Cassava brown streak disease leaf severity 1-month evaluation_method
relationship: variable_of CO_334:0100476 ! 5 pt scale

[Term]
id: CO_334:0000204
name: cassava brown streak disease leaf severity 3-month evaluation
namespace: cassava_trait
def: "Visual rating of leaf symptoms caused by cassava brown streak virus evaluated between two and three months after planting, in the family Potyviridae and genus Ipomovirus. Symptoms rated from 1 = (clean, no infection), 2 = mild/slight vein yellowing or chlorotic blotches on leaves, no brown streaks/lesions on green stem portions\n, 3 = mild/slight vein yellowing or chlorotic blotches on leaves mild brown streaks/lesions on green stem portions, 4 = severe/extensive vein yellowing or chlorotic blotches on leaves severe brown streaks/lesions on green stem portions no defoliation, stem dieback or stunting, 4 =  to 5 = severe/extensive vein yellowing or chlorotic blotches on leaves severe brown streaks/lesions on green stem portions defoliation, stem dieback or stunting." [CO:curators]
synonym: "CBSDisLfSev_Scg_1to5_T3m" EXACT []
synonym: "cbsdl3s" EXACT []
is_a: CO_334:0001000 ! Variables
relationship: variable_of CO_334:0000036 ! Cassava brown streak disease leaf severity
relationship: variable_of CO_334:0010271 ! Visual Observation: Cassava brown streak disease leaf severity 3-month evaluation_method
relationship: variable_of CO_334:0100477 ! 5 pt scale

[Term]
id: CO_334:0000205
name: cassava brown streak disease leaf severity 6-month evaluation
namespace: cassava_trait
def: "Visual rating of leaf symptoms caused by cassava brown streak virus between four and months after planting, in the family Potyviridae and genus Ipomovirus.Symptoms rated from 1 = (clean, no infection), 2 = mild/slight vein yellowing or chlorotic blotches on leaves, no brown streaks/lesions on green stem portions\n, 3 = mild/slight vein yellowing or chlorotic blotches on leaves mild brown streaks/lesions on green stem portions, 4 = severe/extensive vein yellowing or chlorotic blotches on leaves severe brown streaks/lesions on green stem portions no defoliation, stem dieback or stunting, 4 =  to 5 = severe/extensive vein yellowing or chlorotic blotches on leaves severe brown streaks/lesions on green stem portions defoliation, stem dieback or stunting." [CO:curators]
synonym: "CBSDisLfSev_Scg_1to5_6m" EXACT []
synonym: "cbsdl6s" EXACT []
is_a: CO_334:0001000 ! Variables
relationship: variable_of CO_334:0000036 ! Cassava brown streak disease leaf severity
relationship: variable_of CO_334:0010272 ! Visual Observation: Cassava brown streak disease leaf severity 6-month evaluation_method
relationship: variable_of CO_334:0100478 ! 5 pt scale

[Term]
id: CO_334:0000206
name: cassava brown streak disease leaf severity 9-month evaluation
namespace: cassava_trait
def: "Visual rating of leaf symptoms caused by cassava brown streak virus between seven and nine months after planting, in the family Potyviridae and genus Ipomovirus.Symptoms rated from 1 = (clean, no infection), 2 = mild/slight vein yellowing or chlorotic blotches on leaves, no brown streaks/lesions on green stem portions\n, 3 = mild/slight vein yellowing or chlorotic blotches on leaves mild brown streaks/lesions on green stem portions, 4 = severe/extensive vein yellowing or chlorotic blotches on leaves severe brown streaks/lesions on green stem portions no defoliation, stem dieback or stunting, 4 =  to 5 = severe/extensive vein yellowing or chlorotic blotches on leaves severe brown streaks/lesions on green stem portions defoliation, stem dieback or stunting." [CO:curators]
synonym: "CBSDisLfSev_Scg_1to5_9m" EXACT []
synonym: "cbsdl9s" EXACT []
is_a: CO_334:0001000 ! Variables
is_a: CO_334:0001027 ! farmer preference trait at harvest
relationship: variable_of CO_334:0000036 ! Cassava brown streak disease leaf severity
relationship: variable_of CO_334:0010273 ! Visual Observation: Cassava brown streak disease leaf severity 9-month evaluation_method
relationship: variable_of CO_334:0100479 ! 5 pt scale

[Term]
id: CO_334:0000207
name: cassava brown streak disease leaf incidence 1-month evaluation
namespace: cassava_trait
def: "Proportion of plants within a plot showing leaf symptoms of cassava brown streak disease, evaluated between one and six weeks after planting." [CO:curators]
synonym: "CBSDisLfInc_Comp_r_T1m" EXACT []
synonym: "cbsdl1i" EXACT []
is_a: CO_334:0001000 ! Variables
relationship: variable_of CO_334:0000040 ! Cassava brown streak disease leaf incidence
relationship: variable_of CO_334:0010275 ! Counting: Cassava brown streak disease leaf incidence 1-month evaluation_method
relationship: variable_of CO_334:0100582 ! ratio

[Term]
id: CO_334:0000208
name: cassava brown streak disease leaf incidence 3-month evaluation
namespace: cassava_trait
def: "Proportion of plants within a plot showing leaf symptoms of cassava brown streak disease, evaluated between two and three months after planting." [CO:curators]
synonym: "CBSDisLfInc_Comp_r_T3m" EXACT []
synonym: "cbsdl3i" EXACT []
is_a: CO_334:0001000 ! Variables
relationship: variable_of CO_334:0000040 ! Cassava brown streak disease leaf incidence
relationship: variable_of CO_334:0010276 ! Counting: Cassava brown streak disease leaf incidence 3-month evaluation_method
relationship: variable_of CO_334:0100582 ! ratio

[Term]
id: CO_334:0000209
name: cassava brown streak disease leaf incidence 6-month evaluation
namespace: cassava_trait
def: "Proportion of plants within a plot showing leaf symptoms of cassava brown streak disease, evaluated between four and six months after planting." [CO:curators]
synonym: "CBSDisLfInc_Comp_r_T6m" EXACT []
synonym: "cbsdl6i" EXACT []
is_a: CO_334:0001000 ! Variables
relationship: variable_of CO_334:0000040 ! Cassava brown streak disease leaf incidence
relationship: variable_of CO_334:0010277 ! Counting: Cassava brown streak disease leaf incidence 6-month evaluation_method
relationship: variable_of CO_334:0100582 ! ratio

[Term]
id: CO_334:0000210
name: cassava brown streak disease leaf incidence 9-month evaluation
namespace: cassava_trait
def: "Proportion of plants within a plot showing leaf symptoms of cassava brown streak disease, evaluated between seven and nine months after planting." [CO:curators]
synonym: "CBSDisLfInc_Comp_r_T9m" EXACT []
synonym: "cbsdl9i" EXACT []
is_a: CO_334:0001000 ! Variables
relationship: variable_of CO_334:0000040 ! Cassava brown streak disease leaf incidence
relationship: variable_of CO_334:0010278 ! Counting: Cassava brown streak disease leaf incidence 9-month evaluation_method
relationship: variable_of CO_334:0100582 ! ratio

[Term]
id: CO_334:0000211
name: cassava bacterial blight incidence 12-month evaluation
namespace: cassava_trait
def: "Proportion of plants within a plot showing symptoms of cassava bacterial blight, evaluated between ten and twelve months after planting." [CO:curators]
synonym: "cbb12i" EXACT []
synonym: "CBBInc_Comp_rT_12m" EXACT []
is_a: CO_334:0001000 ! Variables
relationship: variable_of CO_334:0000037 ! Cassava bacterial blight incidence
relationship: variable_of CO_334:0010250 ! Counting: Cassava bacterial blight incidence 12-month evaluation_method
relationship: variable_of CO_334:0100582 ! ratio

[Term]
id: CO_334:0000212
name: cassava bacterial blight severity 12-month evaluation
namespace: cassava_trait
def: "Visual rating of symptoms in response to the bacterial blight disease caused by Xanthonomas axonopodis pv. Manihotis ,evaluated bewteen ten and twelve months after planting. Symptoms rated from 1 = (clean, no infection), 2 = Small lesions around points of infections on the leaves, 3 = Extension and appearance of new lesions on leaves and stems. Some leaves wilt, 4 = Extensive leaf wilting and defoliation,  5 = extremely severe with leaf wilting, defoliation and dieback." [CO:curators]
synonym: "cbb12s" EXACT []
synonym: "CBBSev_VisScg_1to5_T12m" EXACT []
is_a: CO_334:0001000 ! Variables
relationship: variable_of CO_334:0000031 ! Cassava bacterial blight severity
relationship: variable_of CO_334:0010245 ! Visual Observation: Cassava bacterial blight severity 12-month evaluation_method
relationship: variable_of CO_334:0100451 ! 5 pt scale

[Term]
id: CO_334:0000213
name: sprout count at one-month
namespace: cassava_trait
def: "A count of the number of stakes germinated, one month after planting." [CO:curators]
synonym: "NoGermStk_Count_Stk_T1m" EXACT []
synonym: "sprtct1" EXACT []
is_a: CO_334:0001000 ! Variables
relationship: variable_of CO_334:0000466 ! Sprout count
relationship: variable_of CO_334:0010223 ! Counting: Sprout count at one-month_method
relationship: variable_of CO_334:0100546 ! number

[Term]
id: CO_334:0000214
name: sprout count at three-month
namespace: cassava_trait
def: "A count of the number of stakes germinated, three months after planting." [CO:curators]
synonym: "NoGermStk_Count_Stk_T3m" EXACT []
synonym: "sprtct3" EXACT []
is_a: CO_334:0001000 ! Variables
relationship: variable_of CO_334:0000466 ! Sprout count
relationship: variable_of CO_334:0010224 ! Counting: Sprout count at three-month_method
relationship: variable_of CO_334:0100546 ! number

[Term]
id: CO_334:0000215
name: sprout count at six-month
namespace: cassava_trait
def: "A count of the number of stakes germinated, six months after planting." [CO:curators]
synonym: "NoGermStk_Count_Stk_T6m" EXACT []
synonym: "sprtct6" EXACT []
is_a: CO_334:0001000 ! Variables
relationship: variable_of CO_334:0000466 ! Sprout count
relationship: variable_of CO_334:0010225 ! Counting: Sprout count at six-month_method
relationship: variable_of CO_334:0100546 ! number

[Term]
id: CO_334:0000216
name: sprout count at nine-month
namespace: cassava_trait
def: "A count of the number of stakes germinated, nine months after planting." [CO:curators]
synonym: "NoGermStk_Count_Stk_T9m" EXACT []
synonym: "sprtct9" EXACT []
is_a: CO_334:0001000 ! Variables
relationship: variable_of CO_334:0000466 ! Sprout count
relationship: variable_of CO_334:0010226 ! Counting: Sprout count at nine-month_method
relationship: variable_of CO_334:0100546 ! number

[Term]
id: CO_334:0000217
name: sprout count at twelve-month
namespace: cassava_trait
def: "A count of the number of stakes germinated, twelve months after planting." [CO:curators]
synonym: "NoGermStk_Count_Stk_T12m" EXACT []
synonym: "sprtct12" EXACT []
is_a: CO_334:0001000 ! Variables
relationship: variable_of CO_334:0000466 ! Sprout count
relationship: variable_of CO_334:0010227 ! Counting: Sprout count at twelve-month_method
relationship: variable_of CO_334:0100546 ! number

[Term]
id: CO_334:0000218
name: cassava anthractnose disease severity in 3-month
namespace: cassava_trait
def: "Visual rating of symptoms in response to the anthracnose disease caused by Colletotrichum gloeosporioides f. sp., evaluated between two and three months after planting. Symptoms rated from 1 = (clean, no infection) 2 = Few shallow cankers on stem late in the growing season, 3 = Many deep cankers on stems followed by distortion, 4 = Many oval lesions on hard and woody stems, 5 = Highly severe with many lesions on hard and woody stems and severe necrosis at leaf axils followed by wilting and severe defoliation." [CO:curators]
synonym: "cad3s" EXACT []
synonym: "CADisSev_VisScg_1to5_T3m" EXACT []
is_a: CO_334:0001000 ! Variables
relationship: variable_of CO_334:0000032 ! Cassava anthracnose disease severity
relationship: variable_of CO_334:0010252 ! Visual Observation: Cassava anthractnose disease severity in 3-months_method
relationship: variable_of CO_334:0100458 ! 5 pt scale

[Term]
id: CO_334:0000219
name: cassava anthractnose disease incidence in 3-month
namespace: cassava_trait
def: "Proportion of plants within a plot showing symptoms of cassava anthracnose disease evaluated between two and three months after planting." [CO:curators]
synonym: "cad3i" EXACT []
synonym: "CADisInc_Comp_r_T3m" EXACT []
is_a: CO_334:0001000 ! Variables
relationship: variable_of CO_334:0000038 ! Cassava anthracnose disease incidence
relationship: variable_of CO_334:0010257 ! Counting: Cassava anthractnose disease incidence in 3-months_method
relationship: variable_of CO_334:0100582 ! ratio

[Term]
id: CO_334:0000220
name: initial plant vigor assessment 1-5
namespace: cassava_trait
def: "Visual assessment of plant vigor during establishment (1=very little vigor, and 5 = very vigorous). as being evaluated by CIAT." [CO:curators]
synonym: "Can't fall when there is strong wind" EXACT []
synonym: "IVig_CIATVisScg_1to5" EXACT []
synonym: "vigour" EXACT []
is_a: CO_334:0001000 ! Variables
is_a: CO_334:0002010 ! Farmer trait
relationship: variable_of CO_334:0000386 ! Initial vigor
relationship: variable_of CO_334:0010435 ! Visual Rating: Initial plant vigor_method
relationship: variable_of CO_334:0100641 ! 2pt scale

[Term]
id: CO_334:0000221
name: root color visual rating 1-3
namespace: cassava_trait
def: "Visual rating of storage root surface color with 1 = white , 2 = intermediate, and 3 = dark brown, as being evaluated by CIAT." [CO:curators]
synonym: "rtcol" EXACT []
synonym: "RtSurfCol_ClsnCIAT_1to3" EXACT []
is_a: CO_334:0001000 ! Variables
relationship: variable_of CO_334:0000454 ! Storage root surface color
relationship: variable_of CO_334:0010436 ! Visual Rating: Root color_method
relationship: variable_of CO_334:0100642 ! 3pt scale

[Term]
id: CO_334:0000222
name: root flesh color visual rating 1-3
namespace: cassava_trait
def: "Visual rating of root pulp color with 1 = white, 2 = cream, 3 = yellow, as being evaluated by CIAT." [CO:curators]
synonym: "PlpCol_ClsnCIAT_1to3" EXACT []
synonym: "rtfcol" EXACT []
xref: TO:1000007
is_a: CO_334:0001000 ! Variables
relationship: variable_of CO_334:0000490 ! Storage Root Pulp Color
relationship: variable_of CO_334:0010437 ! Visual Rating: Root flesh color_method
relationship: variable_of CO_334:0100643 ! 3pt scale

[Term]
id: CO_334:0000223
name: storage root neck length visual rating 1-3
namespace: cassava_trait
def: "Visual rating of root neck length with 1 = short, 2 = intermediate, 3 = long, as being evaluated by CIAT." [CO:curators]
synonym: "RtNeckLng_ClsnCIAT_1to3" EXACT []
synonym: "rtnklgt" EXACT []
is_a: CO_334:0001000 ! Variables
relationship: variable_of CO_334:0000451 ! Storage root neck length
relationship: variable_of CO_334:0010438 ! Visual Rating: Root neck length_method
relationship: variable_of CO_334:0100644 ! 3pt scale

[Term]
id: CO_334:0000224
name: staygreen visual scale 1-9
namespace: cassava_trait
def: "Visual rating of leaf longevity using a scale of 1 = Normal plant with full canopy, retaining most formed leaves which are green, turgid and photosynthetically active. 3 = 30% of the leaves have dropped , less than 50% of the remaining leaves are droppy, partially wilted and practically dry, most of the young leaves have reduced greenness or are yellowing. 5 = 50% reduction of the leaf number compared to full canopy; most of the older leaves are droppy, wilted and practically dry; most of the young leaves have reduced greeness or are yellowing. 7 = 80% reduction of the leaf number compareed to full canopy; more than 75% of the remaining old leaves are wilted or brown; young leaves have reduced greeness or are yellowing\". 9 = Complete defoliation of the stem with candlestick appearance; dieback is also evident on the stem." [CO:curators]
synonym: "SG" EXACT []
xref: CO:334\:0000048
is_a: CO_334:0001000 ! Variables
relationship: variable_of CO_334:0000396 ! Leaf retention
relationship: variable_of CO_334:0010440 ! Visual Rating: Staygreen_method
relationship: variable_of CO_334:0100646 ! 9pt scale

[Term]
id: CO_334:0000225
name: ease of harvest assessment 1-3
namespace: cassava_trait
def: "An assessment of the difficulty in pulling the plants from the ground during harvesting with 1 = easy, 2= intermediate, 3 = difficult." [CO:curators]
synonym: "easehav" EXACT []
synonym: "EasHvst_Est_1to3" EXACT []
xref: TO:0001042
is_a: CO_334:0001000 ! Variables
relationship: variable_of CO_334:0000361 ! Ease of harvest
relationship: variable_of CO_334:0010425 ! Sensory Assesment: Ease of harvest_method
relationship: variable_of CO_334:0100631 ! 3pt scale

[Term]
id: CO_334:0000226
name: root length evaluation scaled 1-3
namespace: cassava_trait
def: "Visual assessment of the root length on a scale of 1, 2, 3 (1=short;  2= intermediate; 3=long)" [CO:curators]
synonym: "rtlgt" EXACT []
synonym: "RtLng_Est_1to3" EXACT []
xref: TO:0000227
is_a: CO_334:0001000 ! Variables
relationship: variable_of CO_334:0000450 ! Root length
relationship: variable_of CO_334:0010426 ! Visual Rating: Root length evaluation_method
relationship: variable_of CO_334:0100632 ! 3pt scale

[Term]
id: CO_334:0000227
name: stalk length evaluation
namespace: cassava_trait
def: "Visual assessment of the average length of the stalks (1=short; 2=intermediate; 3=long)" [CO:curators]
synonym: "stklgt" EXACT []
synonym: "StkLng_Est_1to3" EXACT []
is_a: CO_334:0001000 ! Variables
relationship: variable_of CO_334:0000473 ! Stalk length
relationship: variable_of CO_334:0010427 ! Visual Rating: Stalk average length evaluation_method
relationship: variable_of CO_334:0100633 ! 3pt scale

[Term]
id: CO_334:0000228
name: root evaluation scaled 1-5
namespace: cassava_trait
def: "An evaluation of the integration of  root shape, size, diameter, constriction, neck length on a scale of 1-5 with 1=very good; 5=very bad. Before scoring the roots, the field technician walks the harvested plot to get an idea of the average root type of the trial which will then be used as a score of 3. Genotypes better than average will be scored 2 and 1 in that order. Similiar genotype that are certainly worse compared to the average score are rated 4 and 5 in that order. Trait description is provided by Hernan Ceballos of CIAT." [CO:curators]
synonym: "rteval" EXACT []
synonym: "RtEval_Est_1to5" EXACT []
is_a: CO_334:0001000 ! Variables
relationship: variable_of CO_334:0000448 ! Root evaluation
relationship: variable_of CO_334:0010429 ! Visual Rating: Root evaluation_method
relationship: variable_of CO_334:0100635 ! 5pt scale

[Term]
id: CO_334:0000229
name: rotten root percentage
namespace: cassava_trait
def: "Number of rotten storage root relative to the storage root harvested in a plot estimated in percentage (%)." [CO:curators]
synonym: "rotpct" EXACT []
synonym: "RotRtProp_Est_pct" EXACT []
xref: TO:0001042
is_a: CO_334:0001000 ! Variables
relationship: variable_of CO_334:0000458 ! Rotten root proportion
relationship: variable_of CO_334:0010430 ! Calculation: Percent of rotten roots_method
relationship: variable_of CO_334:0100583 ! pct (%)

[Term]
id: CO_334:0000230
name: plant yield
namespace: cassava_trait
def: "Average yield per plant in a plot measured in kilogram (kg). It is estimated by dividing the total weight of roots by the number of plants harvested." [CO:curators]
synonym: "pltyld" EXACT []
synonym: "RtYld_PerPlnt_kgPlnt" EXACT []
is_a: CO_334:0001000 ! Variables
relationship: variable_of CO_334:0000456 ! Root yield
relationship: variable_of CO_334:0010431 ! Estimation: Plant yield_method
relationship: variable_of CO_334:0100637 ! kg/plant

[Term]
id: CO_334:0000231
name: yield per year
namespace: cassava_trait
def: "Annual root yield estimated in tonnes per hectare (t/ha) using yield per hectare as a function of the crop duration. Trait description provided by Hernan Ceballos in CIAT" [CO:curators]
synonym: "RtYld_PerYr_thayr" EXACT []
synonym: "yldyr" EXACT []
xref: TO:0001041
is_a: CO_334:0001000 ! Variables
relationship: variable_of CO_334:0000456 ! Root yield
relationship: variable_of CO_334:0010432 ! Estimation: Yield per year_method
relationship: variable_of CO_334:0100638 ! t/ha/year

[Term]
id: CO_334:0000232
name: selected variety boolean 0&1
namespace: cassava_trait
def: "Selected variety (1=yes; 0=no)" [CO:curators]
synonym: "select" EXACT []
synonym: "SelVar_Est_0or1" EXACT []
is_a: CO_334:0001000 ! Variables
relationship: variable_of CO_334:0000461 ! Selected variety
relationship: variable_of CO_334:0010433 ! Selection: Selected variety_method
relationship: variable_of CO_334:0100639 ! yes/no scale

[Term]
id: CO_334:0000233
name: flowering ability visual assessment 0-3
namespace: cassava_trait
def: "Presence of flowers (0=none; 1=little; 2=intermediate; 3=many)." [CO:curators]
synonym: "flowerab" EXACT []
synonym: "FlwAb_Est_0to3" EXACT []
is_a: CO_334:0001000 ! Variables
relationship: variable_of CO_334:0000367 ! Flowering
relationship: variable_of CO_334:0010434 ! Visual Observation: Flowering_method
relationship: variable_of CO_334:0100640 ! 4pt scale

[Term]
id: CO_334:0000234
name: female flower evaluation visual rating
namespace: cassava_trait
def: "Visual rating of the count of the number of female flowers present at all branching levels on a plant stand on per plot basis; with 0 = absence of flower, 1 = low number of female flowers [below 5], 2 =  [Medium] 5 to 15 female flowers present, 3 =  [High] above 15 female flowers present)." [CO:curators]
synonym: "FFlwNo_Est_0to5" EXACT []
synonym: "flwfeval" EXACT []
is_a: CO_334:0001000 ! Variables
relationship: variable_of CO_334:0000364 ! Female flower number
relationship: variable_of CO_334:0010439 ! Visual Rating: Female flower evaluation_method
relationship: variable_of CO_334:0100645 ! 4pt scale

[Term]
id: CO_334:0000235
name: female flower incidence in proportion
namespace: cassava_trait
def: "Proportion of the number of female flowers in a plot to the number of plant stand in the plot." [CO:curators]
synonym: "FFlwProp_Comp_ratio" EXACT []
synonym: "flowinc" EXACT []
is_a: CO_334:0001000 ! Variables
relationship: variable_of CO_334:0000439 ! Proportion of female flower
relationship: variable_of CO_334:0010441 ! Counting: Flowering incidence_method
relationship: variable_of CO_334:0100582 ! ratio

[Term]
id: CO_334:0000236
name: sooty mould : visual 1-5
namespace: cassava_trait
def: "Percentage of black mould on the lower leave caused by green mite, aphid, whitefly on cassava leaves with 1 = none, 2 = mild sooty mould on <5% of leaves, 3 = mild sooty mould on 5-20% of leaves,  4 = moderate sooty mould on >20% of leaves; mild leaf curling, 5 = heavy sooty mould on 20-50% of leaves; strong leaf curling of lower leaves; stunted growth of bottom half of plant." [CO:curators]
synonym: "SootMould_Est_1to5" EXACT []
synonym: "sooty" EXACT []
is_a: CO_334:0001000 ! Variables
relationship: variable_of CO_334:0000463 ! Sooty mould
relationship: variable_of CO_334:0010443 ! Visual Observation: Sooty mould_method
relationship: variable_of CO_334:0100649 ! 5pt scale

[Term]
id: CO_334:0000237
name: hairiness visual observation 1-5
namespace: cassava_trait
def: "The level of pubescence on the growing part. It is a proportion of tissue covered by hair on the tip leaves. 1 = Glaborous (No hair) 2 = scatter hair on the edges of tip leaves and bracts, 3 = moderate hair on the edges of tip leaves and bract, 4 = about 50% - 70% hair cover the tip leaves, 5 = 75% - 100% of hair cover the tip leaves." [CO:curators]
synonym: "hairiness" EXACT []
synonym: "PlntHair_Est_1to5" EXACT []
is_a: CO_334:0001000 ! Variables
relationship: variable_of CO_334:0000382 ! Hairiness
relationship: variable_of CO_334:0010442 ! Visual Observation: Hairiness_method
relationship: variable_of CO_334:0100648 ! 5pt scale

[Term]
id: CO_334:0000238
name: gari starch percentage
namespace: cassava_trait
def: "Percentage of starch compostion of gari. This is done locally by using hydraulic jerk to press the gari while it is fresh after grating." [CO:curators]
synonym: "GariStrchCt_Meas_pct" EXACT []
synonym: "gstarch" EXACT []
is_a: CO_334:0001000 ! Variables
relationship: variable_of CO_334:0000380 ! Gari starch
relationship: variable_of CO_334:0010452 ! Estimation: Gari starch_method
relationship: variable_of CO_334:0100583 ! pct (%)

[Term]
id: CO_334:0000239
name: gari fibre by sensory assessment 0-3
namespace: cassava_trait
def: "Sensory assessment of the fibre content. This is done locally by sieving the fried gari, milled locally, and prepared as eba (A popular food in Nigeria). 0 = none, 1 = moderately fibrous, 2 = fibrous, 3 = highly fibrous." [CO:curators]
synonym: "GariFbrCt_Est_0to3" EXACT []
synonym: "gfibre" EXACT []
is_a: CO_334:0001000 ! Variables
relationship: variable_of CO_334:0000378 ! Gari fibre
relationship: variable_of CO_334:0010453 ! Sensory Assesment: Gari fibre_method
relationship: variable_of CO_334:0100659 ! 4pt scale

[Term]
id: CO_334:0000240
name: gari taste : culinary assessment 1-3
namespace: cassava_trait
def: "Taste of gari. 1 = normal, 2 = sweet, and 3 = sour" [CO:curators]
synonym: "GariTaste_Est_1to3" EXACT []
synonym: "gtaste" EXACT []
is_a: CO_334:0001000 ! Variables
relationship: variable_of CO_334:0000381 ! Gari taste
relationship: variable_of CO_334:0010454 ! Gustation: Gari taste_method
relationship: variable_of CO_334:0100660 ! 3pt scale

[Term]
id: CO_334:0000241
name: gari swelling capacity by visual rating 1-3
namespace: cassava_trait
def: "Visual assessment of the increment in quantity when water is added to the gari. 1 = Less than its original volume, 2 = twice the original volume and 3 =thrice the original volume" [CO:curators]
synonym: "GariSwel_Est_1to3" EXACT []
synonym: "swelling" EXACT []
is_a: CO_334:0001000 ! Variables
relationship: variable_of CO_334:0000497 ! Gari swelling capacity
relationship: variable_of CO_334:0010455 ! Visual Rating: Swelling capacity_method
relationship: variable_of CO_334:0100661 ! 3pt scale

[Term]
id: CO_334:0000242
name: gari weight after grinding in kilograms
namespace: cassava_trait
def: "The weight of grated cassava in kilogram (kg) before fermentation in jute bags ." [CO:curators]
synonym: "GdGariWt_Meas_kg" EXACT []
synonym: "wtagrind" EXACT []
is_a: CO_334:0001000 ! Variables
relationship: variable_of CO_334:0000377 ! Gari weight after grinding
relationship: variable_of CO_334:0010447 ! Measurement: Gari weight after grinding_method
relationship: variable_of CO_334:0100493 ! kg

[Term]
id: CO_334:0000243
name: weight of mashed cassava cake in kg
namespace: cassava_trait
def: "Weight of cassava cake after pressing and dehydrating using hydraulic press. Measured in kilogram (kg)" [CO:curators]
synonym: "CakeWt_Meas_kg" EXACT []
synonym: "wtamash" EXACT []
is_a: CO_334:0001000 ! Variables
relationship: variable_of CO_334:0000504 ! Weight of mashed cassava cake
relationship: variable_of CO_334:0010448 ! Measurement: Weight of mashed cassava cake_method
relationship: variable_of CO_334:0100493 ! kg

[Term]
id: CO_334:0000244
name: gari chaff weight in kg
namespace: cassava_trait
def: "Weight of residue in kilogram (kg) after sieving the roasted gari." [CO:curators]
synonym: "GariShftWt_Meas_kg" EXACT []
synonym: "shaftwt" EXACT []
is_a: CO_334:0001000 ! Variables
relationship: variable_of CO_334:0000375 ! Gari chaff weight
relationship: variable_of CO_334:0010449 ! Measurement: Gari shaft weight_method
relationship: variable_of CO_334:0100493 ! kg

[Term]
id: CO_334:0000245
name: gari sample weight g/kg
namespace: cassava_trait
def: "Sample of gari measured in kilogram per gram (kg/g) before and after frying usually for experimental purposes" [CO:curators]
synonym: "gariwt" EXACT []
synonym: "GariWt_Meas_kgg" EXACT []
is_a: CO_334:0001000 ! Variables
relationship: variable_of CO_334:0000379 ! Gari sampled weight
relationship: variable_of CO_334:0010450 ! Measurement: Gari sampled weight_method
relationship: variable_of CO_334:0100657 ! kg/g

[Term]
id: CO_334:0000246
name: gari weight after drying in kg/g
namespace: cassava_trait
def: "weight of cassava in kilogram per gram (kg/g) after drying using the frying pan." [CO:curators]
synonym: "GariDryWt_Meas_kgg" EXACT []
synonym: "gdrywt" EXACT []
is_a: CO_334:0001000 ! Variables
relationship: variable_of CO_334:0000376 ! Gari weight after drying
relationship: variable_of CO_334:0010451 ! Measurement: Gari weight after drying_method
relationship: variable_of CO_334:0100657 ! kg/g

[Term]
id: CO_334:0000247
name: root weight after washing
namespace: cassava_trait
def: "This is the weight of fresh roots cassava washed  in water.It is measured in kilogram (kg) using weighing pan and suspended salter scale; usually for gari preparation." [CO:curators]
synonym: "RtWt_WashWgh_kg" EXACT []
synonym: "wtwash" EXACT []
is_a: CO_334:0001000 ! Variables
relationship: variable_of CO_334:0000302 ! Storage root weight by plot
relationship: variable_of CO_334:0010444 ! Measurement: Root weight after washing_method
relationship: variable_of CO_334:0100493 ! kg

[Term]
id: CO_334:0000248
name: root weight after peel
namespace: cassava_trait
def: "This is weight of the peeled washed  cassava roots in kilogram (kg) using salter scale and weighing pan." [CO:curators]
synonym: "RtWt_PeelWgh_kg" EXACT []
synonym: "rwtapl" EXACT []
is_a: CO_334:0001000 ! Variables
relationship: variable_of CO_334:0000302 ! Storage root weight by plot
relationship: variable_of CO_334:0010445 ! Measurement: Root weight after peel_method
relationship: variable_of CO_334:0100493 ! kg

[Term]
id: CO_334:0000249
name: peel weight measurement in kg
namespace: cassava_trait
def: "The weight of the peels (outer and inner skin) removed from the fresh root cassava; using salter scale. It is measured in Kilogram (kg)." [CO:curators]
synonym: "peelwt" EXACT []
synonym: "PeelWt_Wgh_kg" EXACT []
is_a: CO_334:0001000 ! Variables
relationship: variable_of CO_334:0000422 ! Peel weight
relationship: variable_of CO_334:0010446 ! Measurement: Peel weight_method
relationship: variable_of CO_334:0100493 ! kg

[Term]
id: CO_334:0000250
name: number of stakes counting
namespace: cassava_trait
def: "An estimated number of plantable stakes (about 20cm long, with approximately six nodes) that can be made out of the total number of stems in a plot." [CO:curators]
synonym: "PlntableStkNo_Est_stk" EXACT []
synonym: "stkno" EXACT []
is_a: CO_334:0001000 ! Variables
relationship: variable_of CO_334:0000419 ! Number of stakes
relationship: variable_of CO_334:0010456 ! Counting: Number of stakes_method
relationship: variable_of CO_334:0100662 ! stakes

[Term]
id: CO_334:0000251
name: percentage leaf retention
namespace: cassava_trait
def: "An estimation of the percentage stem length with retained leaf measured in percentage (%) using a representative plant stand in a plot." [CO:curators]
synonym: "LfRet_Est_Pct" EXACT []
synonym: "lrcent" EXACT []
is_a: CO_334:0001000 ! Variables
relationship: variable_of CO_334:0000396 ! Leaf retention
relationship: variable_of CO_334:0010457 ! Estimation: Percentage leaf retention_method
relationship: variable_of CO_334:0100583 ! pct (%)

[Term]
id: CO_334:0000252
name: percentage leaf retention at 5 months after planting
namespace: cassava_trait
def: "An estimation of the percentage stem length with retained leaf measured in percentage (%) using a representative plant stand in a plot, between 5 to 6 months after planting." [CO:curators]
synonym: "lrcent5" EXACT []
is_a: CO_334:0001000 ! Variables
relationship: variable_of CO_334:0000396 ! Leaf retention
relationship: variable_of CO_334:0010458 ! Estimation: Percentage leaf retention at 5 months after planting_method
relationship: variable_of CO_334:0100583 ! pct (%)

[Term]
id: CO_334:0000253
name: percentage leaf retention at 6 months after planting
namespace: cassava_trait
def: "An estimation of the percentage stem length with retained leaf measured in percentage (%) using a representative plant stand in a plot, between 6 to 7 months after planting." [CO:curators]
synonym: "lrcent6" EXACT []
is_a: CO_334:0001000 ! Variables
relationship: variable_of CO_334:0000396 ! Leaf retention
relationship: variable_of CO_334:0010459 ! Estimation: Percentage leaf retention at 6 months after planting_method
relationship: variable_of CO_334:0100583 ! pct (%)

[Term]
id: CO_334:0000254
name: percentage leaf retention at 7 months after planting
namespace: cassava_trait
def: "An estimation of the percentage stem length with retained leaf measured in percentage (%) using a representative plant stand in a plot, between 7 to 8 months after planting." [CO:curators]
synonym: "lrcent7" EXACT []
is_a: CO_334:0001000 ! Variables
relationship: variable_of CO_334:0000396 ! Leaf retention
relationship: variable_of CO_334:0010460 ! Estimation: Percentage leaf retention at 7 months after planting_method
relationship: variable_of CO_334:0100583 ! pct (%)

[Term]
id: CO_334:0000255
name: leaf retention at harvest
namespace: cassava_trait
def: "An estimation of the percentage stem length with retained leaf measured in percentage (%) using a representative plant stand in a plot, at harvest." [CO:curators]
synonym: "LfRet_HvstEst_Pct" EXACT []
synonym: "lrcenth" EXACT []
is_a: CO_334:0001000 ! Variables
relationship: variable_of CO_334:0000396 ! Leaf retention
relationship: variable_of CO_334:0010461 ! Estimation: Leaf retention at harvest_method
relationship: variable_of CO_334:0100583 ! pct (%)

[Term]
id: CO_334:0000256
name: assessment of apical pubescence boolean 0&1
namespace: cassava_trait
def: "Assessment of the young leaf pubescence . Record the most frequent occurrence scored as 0 = Absent, 1 = Present." [CO:curators]
synonym: "APUBESA" RELATED []
is_a: CO_334:0001000 ! Variables
relationship: variable_of CO_334:0000283 ! Apical pubescence
relationship: variable_of CO_334:0010513 ! Visual Rating: Apical pubescence_method
created_by: AAfolabi
creation_date: 2015-09-28T17:48:12Z

[Term]
id: CO_334:0000257
name: stem diameter measurement in cm
namespace: cassava_trait
def: "Measurement of stem diameter taken on the middle of the plant in centimeter (cm) using the vernier caliper." [CO:curators]
synonym: "STE" RELATED []
synonym: "STMDIAM" RELATED []
is_a: CO_334:0001000 ! Variables
relationship: variable_of CO_334:0000480 ! Stem weight
relationship: variable_of CO_334:0010005 ! Measurement: Stem diameter_method
relationship: variable_of CO_334:0100558 ! cm
created_by: AAfolabi
creation_date: 2015-09-28T17:55:20Z

[Term]
id: CO_334:0000258
name: petiole length measurement in cm
namespace: cassava_trait
def: "Observe from the middle third of the plant. Measure two leaves per plant. Expressed in centimeter (cm)" [CO:curators]
synonym: "petlgth" EXACT []
is_a: CO_334:0001000 ! Variables
relationship: variable_of CO_334:0000429 ! Petiole length
relationship: variable_of CO_334:0010464 ! Measurement: Petiole length_method
relationship: variable_of CO_334:0100558 ! cm

[Term]
id: CO_334:0000259
name: petiole orientation visual observation 1-7
namespace: cassava_trait
def: "Visual observation of petiole orientation. Observe from the middle of the plant, take a general picture across the row. No intermediates allowed. Scored as 1 = Inclined upwards, 3 = Horizontal, 5 = Inclined downwards, 7 = Irregular." [CO:curators]
synonym: "petort" EXACT []
is_a: CO_334:0001000 ! Variables
relationship: variable_of CO_334:0000430 ! Petiole orientation
relationship: variable_of CO_334:0010465 ! Visual Observation: Petiole orientation_method
relationship: variable_of CO_334:0100671 ! 4pt scale

[Term]
id: CO_334:0000260
name: presence of pollen visual observation 0&1
namespace: cassava_trait
def: "Visual observation of the presence of pollen. Scored as the same time as flowering. 0 = Absent, 1 = Present." [CO:curators]
synonym: "pollen" EXACT []
is_a: CO_334:0001000 ! Variables
relationship: variable_of CO_334:0000438 ! Presence of pollen
relationship: variable_of CO_334:0010466 ! Visual Observation: Presence of pollen_method
relationship: variable_of CO_334:0100672 ! 2pt scale

[Term]
id: CO_334:0000261
name: stem cortex color visual rating 1-3
namespace: cassava_trait
def: "Visual scoring of stem color. Observe from the middle third of the plant. Make a small shallow cut and peel back the epidermis, score as 1  = Orange, 2  = Light green, 3 = Dark green." [CO:curators]
synonym: "stmctcol" EXACT []
is_a: CO_334:0001000 ! Variables
relationship: variable_of CO_334:0000476 ! Stem cortex color
relationship: variable_of CO_334:0010467 ! Visual Scoring: Stem cortex color_method
relationship: variable_of CO_334:0100673 ! 3pt scale

[Term]
id: CO_334:0000262
name: stem epidermis color visual scoring 1-4
namespace: cassava_trait
def: "Visual scoring of stem color. Peel epidermis back and look at underside of epidermis(skin). Scored as 1 = Cream, 2 = Light brown, 3 = Dark brown, 4 = Orange." [CO:curators]
synonym: "stmepcol" EXACT []
is_a: CO_334:0001000 ! Variables
relationship: variable_of CO_334:0000477 ! Stem epidermis color
relationship: variable_of CO_334:0010468 ! Visual Scoring: Stem epidermis color_method
relationship: variable_of CO_334:0100674 ! 4pt scale

[Term]
id: CO_334:0000263
name: leaf scar distance visual rating 1-7
namespace: cassava_trait
def: "Measurement of the distance between leaf scars. Measured from the middle of stem on the middle third of the plant, where the scars are not flat. Make a measurement along the stem then divide the distance by the number of nodes in the measured part. Avoid taking measurement on mealy bug infected plants. For conservation to qualitative data score 3 as Short (<=8cm), 5 as Medium (8-15cm), 7 as Long(>=15cm)." [CO:curators]
synonym: "lfscdist" EXACT []
is_a: CO_334:0001000 ! Variables
relationship: variable_of CO_334:0000397 ! Leaf scar distance
relationship: variable_of CO_334:0010469 ! Visual Rating: Leaf scar distance_method
relationship: variable_of CO_334:0100675 ! 7pt scale

[Term]
id: CO_334:0000264
name: plant shape visual assessment 1-4
namespace: cassava_trait
def: "Visual assessment of the shape of plant. Record the frequent occurrence on the plot.. Scored as 1= Compact, 2 = Open, 3 = Umbrella, 4 = Cylindrical." [CO:curators]
synonym: "Ability to form a forest" EXACT []
synonym: "pltshp" EXACT []
is_a: CO_334:0001000 ! Variables
is_a: CO_334:0002010 ! Farmer trait
relationship: variable_of CO_334:0000433 ! Plant shape
relationship: variable_of CO_334:0010470 ! Visual Observation: Plant shape_method
relationship: variable_of CO_334:0100676 ! 4pt scale

[Term]
id: CO_334:0000265
name: stipule margin visual observation 1&2
namespace: cassava_trait
def: "Observe from the upper third of plant and record the most frequent occurence. No intermediates is allowed. Scored as 1 = entire, 2 = split or forked." [CO:curators]
synonym: "stpmrg" EXACT []
is_a: CO_334:0001000 ! Variables
relationship: variable_of CO_334:0000482 ! Stipule margin
relationship: variable_of CO_334:0010471 ! Visual Observation: Stipule margin_method
relationship: variable_of CO_334:0100677 ! 2pt scale

[Term]
id: CO_334:0000266
name: Post-harvest physiological deterioration
namespace: cassava_trait
def: "Internal root discoloration or vascular streaking that renders cassava roots unfit for human or animal consumption." [CO:curators]
is_a: CO_334:0000004 ! Quality trait
created_by: naama
creation_date: 2015-09-25T11:44:40Z

[Term]
id: CO_334:0000267
name: Harvest index
namespace: cassava_trait
is_a: CO_334:0000001 ! Agronomic trait
created_by: naama
creation_date: 2015-09-24T16:40:07Z

[Term]
id: CO_334:0000268
name: Shoot apices
namespace: cassava_trait
def: "Structure/arrangement of  shoot apices." [CO:curators]
synonym: "STS" RELATED []
is_a: CO_334:0000001 ! Agronomic trait
created_by: AAfolabi
creation_date: 2015-09-28T18:02:43Z

[Term]
id: CO_334:0000269
name: size of shoot apices assessment 1-3
namespace: cassava_trait
def: "Visual assessment of shoot apices based on how large or small the shoot apices are and categorised on a scale of 1-3 where 1 = small 2= medium and 3 = large." [CO:curators]
is_a: CO_334:0001000 ! Variables
relationship: variable_of CO_334:0000268 ! Shoot apices
relationship: variable_of CO_334:0010003 ! Visual Rating: Size of shoot apices_method
relationship: variable_of CO_334:0100001 ! 3pt scale
created_by: AAfolabi
creation_date: 2015-09-28T18:04:39Z

[Term]
id: CO_334:0000270
name: compactness of shoot apices visual 1-3
namespace: cassava_trait
def: "Visual assessment of the compactness of shoot apices based on how closely the shoot apices are; with 1 = loose, 2 = moderately compact, 3 = compact." [CO:curators]
synonym: "STC" RELATED []
is_a: CO_334:0001000 ! Variables
relationship: variable_of CO_334:0000268 ! Shoot apices
relationship: variable_of CO_334:0010004 ! Visual Rating: Compactness of shoot apices_method
relationship: variable_of CO_334:0100002 ! 3pt scale
created_by: AAfolabi
creation_date: 2015-09-28T18:09:28Z

[Term]
id: CO_334:0000271
name: staygreen visual scale 1-3
namespace: cassava_trait
def: "Visual rating of leaf longevity using a scale of 1 = poor (50% of the leaves are live and green); 2 = moderately good (50-74% of the leaves are live and green); 3 = very good (>75% of the leaves are live and green)." [CO:curators]
is_a: CO_334:0001000 ! Variables
relationship: variable_of CO_334:0000396 ! Leaf retention
relationship: variable_of CO_334:0010002 ! Visual Rating: Staygreen_method
relationship: variable_of CO_334:0100000 ! 3pt scale
created_by: AAfolabi
creation_date: 2015-09-29T12:26:06Z

[Term]
id: CO_334:0000272
name: female flower number counting on all levels
namespace: cassava_trait
def: "Count the number of female flowers after the buds appear, mature, and grow in size to become distinctive at all branch levels." []
is_a: CO_334:0001000 ! Variables
relationship: variable_of CO_334:0000364 ! Female flower number
relationship: variable_of CO_334:0010006 ! Counting: Female flower number all levels_method
relationship: variable_of CO_334:0100606 ! flowers
created_by: aafolabi
creation_date: 2016-05-12T12:45:13Z

[Term]
id: CO_334:0000273
name: LfRet_VisSc_1to9
synonym: "sg" EXACT []
is_obsolete: true

[Term]
id: CO_334:0000274
name: male flower number counting on all levels
namespace: cassava_trait
def: "A count of the number male flowers after the buds appears, matures, and grows in size to become distinctive at all branching levels." []
synonym: "aflwmno" EXACT []
is_a: CO_334:0001000 ! Variables
relationship: variable_of CO_334:0000403 ! Male flower number
relationship: variable_of CO_334:0010007 ! Counting: Male flower number on all levels_method
relationship: variable_of CO_334:0100606 ! flowers
created_by: aafolabi
creation_date: 2016-05-12T14:43:50Z

[Term]
id: CO_334:0000275
name: LfPub_VisClsn_0or1
synonym: "apubes" EXACT []
is_obsolete: true

[Term]
id: CO_334:0000276
name: Abscisic acid content
namespace: cassava_trait
def: "Abscisic acid content of leaf sample" [CO:curators]
synonym: "abscon" EXACT []
xref: TO:0002667
is_a: CO_334:0000003 ! Physiological trait

[Term]
id: CO_334:0000277
name: Amylopectin content
namespace: cassava_trait
def: "Amylopectin content" [CO:curators]
synonym: "amylp" EXACT []
xref: TO:0000097
is_a: CO_334:0000004 ! Quality trait

[Term]
id: CO_334:0000278
name: Amylose amylopectin ratio
namespace: cassava_trait
def: "Amylopectin:amylose ratio" [CO:curators]
synonym: "RtAmylProp" EXACT []
xref: TO:0000372
is_a: CO_334:0000004 ! Quality trait

[Term]
id: CO_334:0000279
name: Amylose content
namespace: cassava_trait
def: "Amylose content" [CO:curators]
synonym: "amyl" EXACT []
xref: TO:0000196
is_a: CO_334:0000004 ! Quality trait

[Term]
id: CO_334:0000280
name: Anther Color
namespace: cassava_trait
def: "Color of anthers" [CO:curators]
synonym: "anther" EXACT []
xref: TO:0000187
is_a: CO_334:0000336 ! Flower and flowering morphological trait

[Term]
id: CO_334:0000281
name: Anthocyanin pigmentation
namespace: cassava_trait
def: "Distribution of anthocyanin pigmentation" [CO:curators]
synonym: "AnthrCPig" EXACT []
xref: TO:0000071
is_a: CO_334:0000001 ! Agronomic trait

[Term]
id: CO_334:0000282
name: Apical branching
namespace: cassava_trait
def: "Time to first apical branching (associated with formation of inflorescence)" [CO:curators]
synonym: "BrnchTim" EXACT []
xref: TO:0000933
is_a: CO_334:0000002 ! Morphological trait

[Term]
id: CO_334:0000283
name: Apical pubescence
namespace: cassava_trait
def: "Pubescence of young leaves" [CO:curators]
synonym: "LfPub" EXACT []
xref: TO:0002722
is_a: CO_334:0000002 ! Morphological trait

[Term]
id: CO_334:0000284
name: Ascorbic acid
namespace: cassava_trait
def: "Ascorbic acid content" [CO:curators]
synonym: "Vitamin C" EXACT []
xref: TO:0000281
is_a: CO_334:0000004 ! Quality trait

[Term]
id: CO_334:0000285
name: Ash content
namespace: cassava_trait
def: "Ash content" [CO:curators]
synonym: "ash" EXACT []
synonym: "Storage root mineral salt content" EXACT []
xref: TO:0000607
is_a: CO_334:0000004 ! Quality trait

[Term]
id: CO_334:0000286
name: Days to first male flower opens
namespace: cassava_trait
def: "First male flower (pistillate) mature and opens." []
synonym: "flwdmo" EXACT []
is_a: CO_334:0000336 ! Flower and flowering morphological trait
created_by: aafolabi
creation_date: 2016-05-12T17:24:01Z

[Term]
id: CO_334:0000287
name: B crypto activity
namespace: cassava_trait
def: "b-cryptoxanthin (carotenoid that has hydroxyl group with 50% activity) content" [CO:curators]
synonym: "BCryptoCt" EXACT []
xref: TO:0020079
is_a: CO_334:0000004 ! Quality trait

[Term]
id: CO_334:0000288
name: Bemisia tabaci nymphs black
namespace: cassava_trait
def: "Number of black bemisia tabaci nymphs on 14th leaf" [CO:curators]
synonym: "btwfb" EXACT []
xref: TO:0000261
is_a: CO_334:0000030 ! insect damage

[Term]
id: CO_334:0000289
name: Bemisia tabaci nymphs severity
namespace: cassava_trait
def: "Severity of the chlorotic blotches on leaf caused by the nymphs of Bemisia tabaci" [CO:curators]
synonym: "BTNSev" EXACT []
xref: TO:0000261
is_a: CO_334:0000030 ! insect damage

[Term]
id: CO_334:0000290
name: Bemisia tabaci nymphs yellow
namespace: cassava_trait
def: "Number of yellow bemisia tabaci nymphs on 14th leaf" [CO:curators]
synonym: "btwfy" EXACT []
xref: TO:0000261
is_a: CO_334:0000030 ! insect damage

[Term]
id: CO_334:0000291
name: Beta carotene
namespace: cassava_trait
def: "beta-carotene (ug/g fresh wt)" [CO:curators]
synonym: "bc" EXACT []
xref: TO:0002695
is_a: CO_334:0001042 ! carotene content

[Term]
id: CO_334:0000292
name: Beta carotenoid retention
namespace: cassava_trait
def: "Beta carotene content after cooking" [CO:curators]
synonym: "BCaroRet" EXACT []
xref: TO:0002695
is_a: CO_334:0000291 ! Beta carotene

[Term]
id: CO_334:0000293
name: Branch height
namespace: cassava_trait
def: "Branch height" [CO:curators]
synonym: "branching" EXACT []
synonym: "BrnchHt" EXACT []
xref: TO:1000008
is_a: CO_334:0000329 ! Plant branch morphological trait

[Term]
id: CO_334:0000294
name: Branching Angle
namespace: cassava_trait
def: "Angle of branching (Angle between vertical plane and first branches)" [CO:curators]
synonym: "brnang" EXACT []
xref: TO:1000009
is_a: CO_334:0000329 ! Plant branch morphological trait

[Term]
id: CO_334:0000295
name: Branching habit
namespace: cassava_trait
def: "Branching habit" [CO:curators]
synonym: "brnhbt" EXACT []
xref: TO:0000740
is_a: CO_334:0000329 ! Plant branch morphological trait

[Term]
id: CO_334:0000296
name: Branching Levels
namespace: cassava_trait
def: "Number of levels of branching (Actual number of levels (at or before harvest))." [CO:curators]
synonym: "brnlev" EXACT []
xref: TO:0000740
is_a: CO_334:0000329 ! Plant branch morphological trait

[Term]
id: CO_334:0000297
name: Carotenoid content
namespace: cassava_trait
def: "Cassava storage root pulp carotenoid content" [CO:curators]
synonym: "CarotCt" EXACT []
xref: TO:0000496
is_a: CO_334:0001042 ! carotene content

[Term]
id: CO_334:0000298
name: Caruncle Color
namespace: cassava_trait
def: "Color of caruncle" [CO:curators]
synonym: "carcol" EXACT []
xref: TO:1000010
is_a: CO_334:0000336 ! Flower and flowering morphological trait

[Term]
id: CO_334:0000299
name: days to first flower opens visual observation
namespace: cassava_trait
def: "Visual observation (actual date in the format of dd/mm/yyyy from the date of planting) of the opening of the first male flower." []
synonym: "flwdmo" EXACT []
is_a: CO_334:0001000 ! Variables
relationship: variable_of CO_334:0000286 ! Days to first male flower opens
relationship: variable_of CO_334:0010008 ! Visual Observation: Days to first male flower opens
relationship: variable_of CO_334:0100611 ! days
created_by: aafolabi
creation_date: 2016-05-12T17:33:16Z

[Term]
id: CO_334:0000300
name: number of planted stakes per plant counting
namespace: cassava_trait
is_a: CO_334:0001000 ! Variables
relationship: variable_of CO_334:0000416 ! Number of planted stakes
relationship: variable_of CO_334:0010456 ! Counting: Number of stakes_method
relationship: variable_of CO_334:0100662 ! stakes
created_by: naama
creation_date: 2016-10-27T15:44:39Z

[Term]
id: CO_334:0000301
name: lodged plants estimation 1-3
namespace: cassava_trait
def: "Visual scoring of plant lodging using 1 to 3 score. 1= very little lodging; 2= intermediate lodging which can be in relation the proportion of lodged plants (e.g. 50%), or the degree of lodging (e.g.  most plants are inclined 45degrees from the vertical axis); and 3= serious lodging regarding proportion and degree of inclination (most plants are truly lodged)." []
synonym: "Rollov" EXACT []
is_a: CO_334:0001000 ! Variables
relationship: variable_of CO_334:0000440 ! Lodged plants
created_by: naama
creation_date: 2016-10-27T15:47:21Z

[Term]
id: CO_334:0000302
name: Storage root weight by plot
namespace: cassava_trait
is_a: CO_334:0000493 ! Storage root weight
created_by: naama
creation_date: 2016-12-22T16:13:27Z

[Term]
id: CO_334:0000303
name: Storage root weight by plant
namespace: cassava_trait
is_a: CO_334:0000493 ! Storage root weight
created_by: naama
creation_date: 2016-12-22T16:15:30Z

[Term]
id: CO_334:0000304
name: fresh storage root weight per plant
namespace: cassava_trait
def: "Total fresh weight of storage roots harvested per plant measured in kilogram (kg)." [CO:Curators]
is_a: CO_334:0001000 ! Variables
relationship: variable_of CO_334:0000303 ! Storage root weight by plant
relationship: variable_of CO_334:0010514 ! Measurement: Storage root weight per plant_method
relationship: variable_of CO_334:0100493 ! kg
created_by: naama
creation_date: 2016-12-22T16:17:12Z

[Term]
id: CO_334:0000305
name: Fresh shoot weight by plot
namespace: cassava_trait
is_a: CO_334:0000369 ! Fresh shoot weight
created_by: naama
creation_date: 2016-12-22T16:23:13Z

[Term]
id: CO_334:0000306
name: Fresh shoot weight by plant
namespace: cassava_trait
is_a: CO_334:0000369 ! Fresh shoot weight
created_by: naama
creation_date: 2016-12-22T16:23:29Z

[Term]
id: CO_334:0000307
name: fresh shoot weight measurement in kg per plant
namespace: cassava_trait
def: "Total fresh weight of harvested foliage and stems in kilograms per plant" [CO:Curators]
is_a: CO_334:0001000 ! Variables
relationship: variable_of CO_334:0000306 ! Fresh shoot weight by plant
relationship: variable_of CO_334:0010515 ! Measurement: Fresh shoot weight per plant_method
relationship: variable_of CO_334:0100493 ! kg
created_by: naama
creation_date: 2016-12-22T16:24:39Z

[Term]
id: CO_334:0000308
name: ease of peeling root cortex visual rating 1-3
namespace: cassava_trait
def: "Visual rating of ease of peeling root cortex with 1 = easy, 2 = intermediate and 3 = difficult." []
synonym: "easepl" RELATED []
is_a: CO_334:0001000 ! Variables
relationship: variable_of CO_334:0000362 ! Ease of peeling storage root cortex
relationship: variable_of CO_334:0010518 ! Visual Rating: Ease of peel_method
relationship: variable_of CO_334:0100000 ! 3pt scale
created_by: AAfolabi
creation_date: 2017-02-10T10:54:15Z

[Term]
id: CO_334:0000309
name: apical pubescence visual rating 0-2
namespace: cassava_trait
def: "Visual rating of young leaf pubescence with 0 = absent, 1 = Moderate pubescence, 2 = high pubescence." []
synonym: "apubes" RELATED []
is_a: CO_334:0001000 ! Variables
relationship: variable_of CO_334:0000283 ! Apical pubescence
relationship: variable_of CO_334:0010513 ! Visual Rating: Apical pubescence_method
relationship: variable_of CO_334:0100000 ! 3pt scale
created_by: AAfolabi
creation_date: 2017-02-10T11:02:13Z

[Term]
id: CO_334:0000310
name: Plantable stem
namespace: cassava_trait
def: "A plantable stem (stick), has an estimated length of about 20cm." [CO:AA]
synonym: "plantable stem" EXACT []
is_a: CO_334:0000001 ! Agronomic trait
created_by: naama
creation_date: 2017-04-07T13:20:56Z

[Term]
id: CO_334:0000311
name: stick length
namespace: cassava_trait
def: "Length of the planting stick at the sampling time point in centimeters." []
synonym: "stem length" EXACT []
is_a: CO_334:0000310 ! Plantable stem
created_by: naama
creation_date: 2017-04-07T13:24:49Z

[Term]
id: CO_334:0000312
name: planting stick internode number
namespace: cassava_trait
def: "Number of the internodes of the planting stick." []
is_a: CO_334:0000310 ! Plantable stem
created_by: naama
creation_date: 2017-04-07T13:26:23Z

[Term]
id: CO_334:0000313
name: Number of planting stick internodes with roots
namespace: cassava_trait
def: "Number of the internodes which developed fibrous or storage roots." []
is_a: CO_334:0000310 ! Plantable stem
created_by: naama
creation_date: 2017-04-07T13:27:09Z

[Term]
id: CO_334:0000314
name: Number of fibrous roots on planting stick
namespace: cassava_trait
def: "Total number of fibrous roots emerging from the planting stick." []
is_a: CO_334:0000310 ! Plantable stem
created_by: naama
creation_date: 2017-04-07T13:39:34Z

[Term]
id: CO_334:0000315
name: Number storage roots on planting stick
namespace: cassava_trait
def: "Total number of storage roots emerging from the planting stick." []
is_a: CO_334:0000310 ! Plantable stem
created_by: naama
creation_date: 2017-04-07T13:40:26Z

[Term]
id: CO_334:0000316
name: Number roots at end of the planting stick
namespace: cassava_trait
def: "Total number of roots (fibrous and storage) which emerged from the cutting side at the end of the planting stick." []
is_a: CO_334:0000310 ! Plantable stem
created_by: naama
creation_date: 2017-04-07T13:40:56Z

[Term]
id: CO_334:0000317
name: Starch properties
namespace: cassava_trait
def: "Measurements related to starch traits." []
is_a: CO_334:0000004 ! Quality trait
created_by: naama
creation_date: 2017-04-07T14:03:18Z

[Term]
id: CO_334:0000318
name: Starch granule morphology
namespace: cassava_trait
is_a: CO_334:0000317 ! Starch properties
created_by: naama
creation_date: 2017-04-07T14:04:47Z

[Term]
id: CO_334:0000319
name: starch granule morphology (pictures)
namespace: cassava_trait
is_a: CO_334:0001000 ! Variables
relationship: variable_of CO_334:0000318 ! Starch granule morphology
relationship: variable_of CO_334:0010519 ! Measurement: Starch granule_method
relationship: variable_of CO_334:0100000 ! 3pt scale
created_by: naama
creation_date: 2017-04-07T14:05:27Z

[Term]
id: CO_334:0000320
name: Starch granule size
namespace: cassava_trait
is_a: CO_334:0000317 ! Starch properties
created_by: naama
creation_date: 2017-04-07T14:06:43Z

[Term]
id: CO_334:0000321
name: starch granule average diameter
namespace: cassava_trait
def: "Starch granule average diameter (µm)" []
is_a: CO_334:0001000 ! Variables
relationship: variable_of CO_334:0000320 ! Starch granule size
relationship: variable_of CO_334:0010519 ! Measurement: Starch granule_method
relationship: variable_of CO_334:0100692 ! um
created_by: naama
creation_date: 2017-04-07T14:06:56Z

[Term]
id: CO_334:0000322
name: starch granule size distribution
namespace: cassava_trait
def: "Starch granule size distribution with three categories. 1: between 0-7µm ; 2: 8-14 µm ; 3: 15 - 22 µm." []
is_a: CO_334:0001000 ! Variables
relationship: variable_of CO_334:0000320 ! Starch granule size
relationship: variable_of CO_334:0010519 ! Measurement: Starch granule_method
relationship: variable_of CO_334:0100000 ! 3pt scale
created_by: naama
creation_date: 2017-04-07T14:07:28Z

[Term]
id: CO_334:0000323
name: starch chain length distribution
namespace: cassava_trait
def: "Starch chain length distribution, values range from dp3 to dp82." []
is_a: CO_334:0001000 ! Variables
relationship: variable_of CO_334:0000320 ! Starch granule size
relationship: variable_of CO_334:0010519 ! Measurement: Starch granule_method
relationship: variable_of CO_334:0100693 ! dp
created_by: naama
creation_date: 2017-04-07T14:08:52Z

[Term]
id: CO_334:0000324
name: Total fresh weight
namespace: cassava_trait
is_a: CO_334:0000001 ! Agronomic trait
created_by: naama
creation_date: 2017-04-10T12:26:09Z

[Term]
id: CO_334:0000325
name: total fresh weight by plot
namespace: cassava_trait
def: "The sum of fresh root weight + fresh root weight by plot." [CO:curators]
is_a: CO_334:0001000 ! Variables
relationship: variable_of CO_334:0000324 ! Total fresh weight
relationship: variable_of CO_334:0010286 ! Measurement: Fresh weight of storage root_method
relationship: variable_of CO_334:0100493 ! kg
created_by: naama
creation_date: 2017-04-10T12:26:56Z

[Term]
id: CO_334:0000326
name: total fresh weight by plant
namespace: cassava_trait
def: "The sum of fresh root weight + fresh root weight by plant." [CO:curators]
is_a: CO_334:0001000 ! Variables
relationship: variable_of CO_334:0000324 ! Total fresh weight
relationship: variable_of CO_334:0010514 ! Measurement: Storage root weight per plant_method
relationship: variable_of CO_334:0100493 ! kg
created_by: naama
creation_date: 2017-04-10T12:41:21Z

[Term]
id: CO_334:0000327
name: fresh fibrous root weight per plant
namespace: cassava_trait
def: "Total fresh weight of fibrous roots harvested per plot measured in kilogram (kg)." [CO:Curators]
is_a: CO_334:0001000 ! Variables
relationship: variable_of CO_334:0002060 ! Fibrous root weight
relationship: variable_of CO_334:0010521 ! Measurement: Fresh fibrous root_method
relationship: variable_of CO_334:0100493 ! kg
created_by: naama
creation_date: 2017-05-04T15:44:25Z

[Term]
id: CO_334:0000328
name: fresh fibrous root weight per plot
namespace: cassava_trait
def: "Total fresh weight of fibrous roots harvested per plot measured in kilogram (kg)." [CO:curators]
synonym: "rtwt" EXACT []
synonym: "RtWt_Wgh_kg" EXACT []
is_a: CO_334:0001000 ! Variables
relationship: variable_of CO_334:0002060 ! Fibrous root weight
relationship: variable_of CO_334:0010521 ! Measurement: Fresh fibrous root_method
relationship: variable_of CO_334:0100493 ! kg
created_by: naama
creation_date: 2017-05-04T15:47:58Z

[Term]
id: CO_334:0000329
name: Plant branch morphological trait
namespace: cassava_trait
def: "Traits associated with branch and branching morphology." [CO:curators]
is_a: CO_334:0000002 ! Morphological trait
created_by: naama
creation_date: 2017-06-22T10:52:49Z

[Term]
id: CO_334:0000330
name: Leaf morphological trait
namespace: cassava_trait
def: "Traits associated with leaf morphology." [CO:curators]
is_a: CO_334:0000002 ! Morphological trait
created_by: naama
creation_date: 2017-06-22T10:58:52Z

[Term]
id: CO_334:0000331
name: Leaf lobe
namespace: cassava_trait
is_a: CO_334:0000330 ! Leaf morphological trait
created_by: naama
creation_date: 2017-06-22T10:59:47Z

[Term]
id: CO_334:0000332
name: Leaf scar
namespace: cassava_trait
is_a: CO_334:0000330 ! Leaf morphological trait
created_by: naama
creation_date: 2017-06-22T11:00:17Z

[Term]
id: CO_334:0000333
name: Root morphological trait
namespace: cassava_trait
def: "Traits associated with root morphology" []
is_a: CO_334:0000002 ! Morphological trait
created_by: naama
creation_date: 2017-06-22T11:06:53Z

[Term]
id: CO_334:0000334
name: Storage root morphological trait
namespace: cassava_trait
is_a: CO_334:0000333 ! Root morphological trait
created_by: naama
creation_date: 2017-06-22T11:07:39Z

[Term]
id: CO_334:0000335
name: Fibrous root morphological trait
namespace: cassava_trait
is_a: CO_334:0000333 ! Root morphological trait
created_by: naama
creation_date: 2017-06-22T11:08:25Z

[Term]
id: CO_334:0000336
name: Flower and flowering morphological trait
namespace: cassava_trait
is_a: CO_334:0000002 ! Morphological trait
created_by: naama
creation_date: 2017-06-22T11:16:26Z

[Term]
id: CO_334:0000337
name: Fruit morphological trait
namespace: cassava_trait
is_a: CO_334:0000002 ! Morphological trait
created_by: naama
creation_date: 2017-06-22T11:27:39Z

[Term]
id: CO_334:0000338
name: Stem morphological trait
namespace: cassava_trait
is_a: CO_334:0000002 ! Morphological trait
created_by: naama
creation_date: 2017-06-22T11:31:39Z

[Term]
id: CO_334:0000339
name: Cassava mealy bug incidence
namespace: cassava_trait
def: "Proportion of plants within a plot showing symptoms of cassava mealy-bug damage (Phenacoccus Manihoti)" [CO:curators]
synonym: "cmbi" EXACT []
xref: TO:0000261
is_a: CO_334:0000030 ! insect damage

[Term]
id: CO_334:0000340
name: Cassava mealy bug severity
namespace: cassava_trait
def: "Severity of the damage caused by Cassava mealy bug (Phenacoccus Manihoti)" [CO:curators]
synonym: "Cassava Mealy Bug Severity - Cassavabase" EXACT []
synonym: "CMBSev" EXACT []
xref: TO:0000261
is_a: CO_334:0000030 ! insect damage

[Term]
id: CO_334:0000341
name: Leaf petiole
namespace: cassava_trait
def: "Traits associated with the leaf petiole morphology." []
is_a: CO_334:0000330 ! Leaf morphological trait
created_by: naama
creation_date: 2017-06-22T11:33:00Z

[Term]
id: CO_334:0000342
name: Node number
namespace: cassava_trait
def: "Number of nodes on a stem." [CO:curators]
is_a: CO_334:0000338 ! Stem morphological trait
created_by: naama
creation_date: 2017-06-22T11:44:36Z

[Term]
id: CO_334:0000343
name: average number of nodes per plot counting
namespace: cassava_trait
def: "Average number of nodes per branch level.\nCounting all nodes per branch at each level. If more than one branch, select one branch and count nodes up to the apical shoot. Value averaged per plot." [CO:curators]
is_a: CO_334:0001000 ! Variables
relationship: variable_of CO_334:0000342 ! Node number
relationship: variable_of CO_334:0010520 ! Counting: Number of node_method
relationship: variable_of CO_334:0100546 ! number
created_by: naama
creation_date: 2017-06-22T11:46:27Z

[Term]
id: CO_334:0000344
name: female flower number at specific branching level
namespace: cassava_trait
def: "Count of number of female flowers at a predefined branching level." []
is_a: CO_334:0000364 ! Female flower number
created_by: naama
creation_date: 2017-06-26T12:02:41Z

[Term]
id: CO_334:0000345
name: female flower number at branching level 1 counting
namespace: cassava_trait
def: "Count of number of female flowers at the first branching level." []
is_a: CO_334:0001000 ! Variables
relationship: variable_of CO_334:0000344 ! female flower number at specific branching level
relationship: variable_of CO_334:0010400 ! Counting: Female flower number_method
relationship: variable_of CO_334:0100606 ! flowers
created_by: naama
creation_date: 2017-06-26T12:05:00Z

[Term]
id: CO_334:0000346
name: female flower number at branching level 2 counting
namespace: cassava_trait
def: "Count of number of female flowers at the second branching level." []
is_a: CO_334:0001000 ! Variables
relationship: variable_of CO_334:0000344 ! female flower number at specific branching level
relationship: variable_of CO_334:0010400 ! Counting: Female flower number_method
relationship: variable_of CO_334:0100606 ! flowers
created_by: naama
creation_date: 2017-06-26T12:05:00Z

[Term]
id: CO_334:0000347
name: female flower number at branching level 3 counting
namespace: cassava_trait
def: "Count of number of female flowers at the third branching level." []
is_a: CO_334:0001000 ! Variables
relationship: variable_of CO_334:0000344 ! female flower number at specific branching level
relationship: variable_of CO_334:0010400 ! Counting: Female flower number_method
relationship: variable_of CO_334:0100606 ! flowers
created_by: naama
creation_date: 2017-06-26T12:05:00Z

[Term]
id: CO_334:0000348
name: female flower number at branching level 4 counting
namespace: cassava_trait
def: "Count of number of female flowers at the forth branching level." []
is_a: CO_334:0001000 ! Variables
relationship: variable_of CO_334:0000344 ! female flower number at specific branching level
relationship: variable_of CO_334:0010400 ! Counting: Female flower number_method
relationship: variable_of CO_334:0100606 ! flowers
created_by: naama
creation_date: 2017-06-26T12:05:00Z

[Term]
id: CO_334:0000349
name: female flower number at branching level 5 counting
namespace: cassava_trait
def: "Count of number of female flowers at the fifth branching level." []
is_a: CO_334:0001000 ! Variables
relationship: variable_of CO_334:0000344 ! female flower number at specific branching level
relationship: variable_of CO_334:0010400 ! Counting: Female flower number_method
relationship: variable_of CO_334:0100606 ! flowers
created_by: naama
creation_date: 2017-06-26T12:05:00Z

[Term]
id: CO_334:0000350
name: female flower number at branching level 6 counting
namespace: cassava_trait
def: "Count of number of female flowers at the sixth branching level." []
is_a: CO_334:0001000 ! Variables
relationship: variable_of CO_334:0000344 ! female flower number at specific branching level
relationship: variable_of CO_334:0010400 ! Counting: Female flower number_method
relationship: variable_of CO_334:0100606 ! flowers
created_by: naama
creation_date: 2017-06-26T12:05:00Z

[Term]
id: CO_334:0000351
name: Node number per branch
namespace: cassava_trait
def: "Number of nodes at each branching level." []
is_a: CO_334:0000342 ! Node number
created_by: naama
creation_date: 2017-07-11T10:55:33Z

[Term]
id: CO_334:0000352
name: number of nodes at branching level 1 counting
namespace: cassava_trait
def: "Number of nodes at the first branching level." []
is_a: CO_334:0001000 ! Variables
relationship: variable_of CO_334:0000351 ! Node number per branch
relationship: variable_of CO_334:0010520 ! Counting: Number of node_method
relationship: variable_of CO_334:0100691 ! nodes
created_by: naama
creation_date: 2017-07-11T10:57:20Z

[Term]
id: CO_334:0000353
name: Central Leaf Shape
namespace: cassava_trait
def: "Shape of central leaf taken from a mid-height position." [CO:curators]
synonym: "lfshp" EXACT []
xref: TO:0000492
is_a: CO_334:0000330 ! Leaf morphological trait

[Term]
id: CO_334:0000354
name: Cis 9 activity
namespace: cassava_trait
def: "Cis 9 isomer activity" [CO:curators]
synonym: "cis-9" EXACT []
xref: TO:0000282
is_a: CO_334:0000004 ! Quality trait

[Term]
id: CO_334:0000355
name: Color of boiled storage roots
namespace: cassava_trait
def: "Color of boiled storage roots" [CO:curators]
synonym: "pdcol" EXACT []
xref: TO:1000007
is_a: CO_334:0000004 ! Quality trait

[Term]
id: CO_334:0000356
name: Days to 50% anthesis
namespace: cassava_trait
def: "50% of the female flower opened to expose the pistils per plot" [CO:curators]
synonym: "dyfl" EXACT []
synonym: "flw50a" EXACT []
xref: TO:0002616
is_a: CO_334:0000336 ! Flower and flowering morphological trait

[Term]
id: CO_334:0000357
name: Days to 50% branching
namespace: cassava_trait
def: "Time to reach 50% of the plants at the branching stage" [CO:curators]
synonym: "flw50b" EXACT []
xref: TO:0000933
is_a: CO_334:0000329 ! Plant branch morphological trait

[Term]
id: CO_334:0000358
name: Days to first anthesis
namespace: cassava_trait
def: "Exposing of the pistil per plot of any female flower" [CO:curators]
synonym: "flwdfa" EXACT []
xref: TO:0002616
is_a: CO_334:0000336 ! Flower and flowering morphological trait

[Term]
id: CO_334:0000359
name: Days to first inflorescence
namespace: cassava_trait
def: "Time to reach the first inflorescence." [CO:curators]
synonym: "flwdfi" EXACT []
xref: TO:0002616
is_a: CO_334:0000336 ! Flower and flowering morphological trait

[Term]
id: CO_334:0000360
name: Disc color
namespace: cassava_trait
def: "Color of disc" [CO:curators]
synonym: "discol" EXACT []
xref: TO:1000019
is_a: CO_334:0000002 ! Morphological trait

[Term]
id: CO_334:0000361
name: Ease of harvest
namespace: cassava_trait
def: "Ease of plant harvest" [CO:curators]
synonym: "easehav" EXACT []
xref: TO:0001042
is_a: CO_334:0000001 ! Agronomic trait

[Term]
id: CO_334:0000362
name: Ease of peeling storage root cortex
namespace: cassava_trait
def: "Ease of storage root cortex removal." [CO:curators]
synonym: "easepl" EXACT []
xref: TO:0001042
is_a: CO_334:0000333 ! Root morphological trait

[Term]
id: CO_334:0000363
name: number of nodes at branching level 2 counting
namespace: cassava_trait
def: "Number of nodes at the second branching level." []
is_a: CO_334:0001000 ! Variables
relationship: variable_of CO_334:0000351 ! Node number per branch
relationship: variable_of CO_334:0010520 ! Counting: Number of node_method
relationship: variable_of CO_334:0100691 ! nodes
created_by: naama
creation_date: 2017-07-11T10:57:20Z

[Term]
id: CO_334:0000364
name: Female flower number
namespace: cassava_trait
def: "Number of female flowers after the buds appear" [CO:curators]
synonym: "FFlwNo" EXACT []
xref: TO:0002736
is_a: CO_334:0000336 ! Flower and flowering morphological trait

[Term]
id: CO_334:0000365
name: Female stamenoids
namespace: cassava_trait
def: "Presence of stamen in female cassava flowers" [CO:curators]
synonym: "femsta" EXACT []
xref: TO:0000215
is_a: CO_334:0000001 ! Agronomic trait

[Term]
id: CO_334:0000366
name: Fibre content
namespace: cassava_trait
def: "Fibre content" [CO:curators]
synonym: "fibre" EXACT []
xref: TO:0002642
is_a: CO_334:0000004 ! Quality trait

[Term]
id: CO_334:0000367
name: Flowering
namespace: cassava_trait
def: "Abundance of flower" [CO:curators]
synonym: "flowerab" EXACT []
xref: TO:0002736
is_a: CO_334:0000336 ! Flower and flowering morphological trait

[Term]
id: CO_334:0000368
name: number of nodes at branching level 3 counting
namespace: cassava_trait
def: "Number of nodes at the third branching level." []
is_a: CO_334:0001000 ! Variables
relationship: variable_of CO_334:0000351 ! Node number per branch
relationship: variable_of CO_334:0010520 ! Counting: Number of node_method
relationship: variable_of CO_334:0100691 ! nodes
created_by: naama
creation_date: 2017-07-11T10:57:20Z

[Term]
id: CO_334:0000369
name: Fresh shoot weight
namespace: cassava_trait
def: "Total fresh weight of harvested foliage and stems" [CO:curators]
synonym: "ShFrWe" EXACT []
xref: TO:0000571
is_a: CO_334:0000001 ! Agronomic trait

[Term]
id: CO_334:0000370
name: Frog skin disease
namespace: cassava_trait
def: "Severity of the Frog skin disease caused by unknown causal agent" [CO:curators]
synonym: "fsd" EXACT []
xref: TO:0000439
is_a: CO_334:0000028 ! viral disease

[Term]
id: CO_334:0000371
name: Fruit exocarp texture
namespace: cassava_trait
def: "Texture of the outer most layer of the cassava fruit" [CO:curators]
synonym: "fruexo" EXACT []
xref: TO:0002624
is_a: CO_334:0000001 ! Agronomic trait

[Term]
id: CO_334:0000372
name: Fruit set presence
namespace: cassava_trait
def: "Fruit set" [CO:curators]
synonym: "frtset" EXACT []
xref: TO:0002640
is_a: CO_334:0000001 ! Agronomic trait

[Term]
id: CO_334:0000373
name: Fufu content
namespace: cassava_trait
def: "Fufu weight" [CO:curators]
synonym: "fufucnt" EXACT []
xref: TO:0001042
is_a: CO_334:0000004 ! Quality trait

[Term]
id: CO_334:0000374
name: Gari content
namespace: cassava_trait
def: "Gari content" [CO:curators]
synonym: "GarCt" EXACT []
synonym: "Gari Content - Cassavabase" EXACT []
xref: TO:0001042
is_a: CO_334:0000004 ! Quality trait

[Term]
id: CO_334:0000375
name: Gari chaff weight
namespace: cassava_trait
def: "Chaff weight" [CO:curators]
synonym: "chaffwt" EXACT []
xref: TO:0001042
is_a: CO_334:0000004 ! Quality trait

[Term]
id: CO_334:0000376
name: Gari weight after drying
namespace: cassava_trait
def: "Weight after drying cassava flakes" [CO:curators]
synonym: "gdrywt" EXACT []
xref: TO:0001042
is_a: CO_334:0000004 ! Quality trait

[Term]
id: CO_334:0000377
name: Gari weight after grinding
namespace: cassava_trait
def: "Weight after grinding" [CO:curators]
synonym: "wtagrind" EXACT []
xref: TO:0001042
is_a: CO_334:0000004 ! Quality trait

[Term]
id: CO_334:0000378
name: Gari fibre
namespace: cassava_trait
def: "gari fibre" [CO:curators]
synonym: "gfibre" EXACT []
xref: TO:0001042
is_a: CO_334:0000004 ! Quality trait

[Term]
id: CO_334:0000379
name: Gari sampled weight
namespace: cassava_trait
def: "gari sampled weight" [CO:curators]
synonym: "gariwt" EXACT []
xref: TO:0001042
is_a: CO_334:0000004 ! Quality trait

[Term]
id: CO_334:0000380
name: Gari starch
namespace: cassava_trait
def: "Assessment of the starch content of gari" [CO:curators]
synonym: "gstarch" EXACT []
xref: TO:0001042
is_a: CO_334:0000004 ! Quality trait

[Term]
id: CO_334:0000381
name: Gari taste
namespace: cassava_trait
def: "Taste of gari" [CO:curators]
synonym: "gtaste" EXACT []
xref: TO:0001042
is_a: CO_334:0000004 ! Quality trait

[Term]
id: CO_334:0000382
name: Hairiness
namespace: cassava_trait
def: "Hairiness" [CO:curators]
synonym: "hairiness" EXACT []
xref: TO:0000398
is_a: CO_334:0000002 ! Morphological trait

[Term]
id: CO_334:0000383
name: number of nodes at branching level 4 counting
namespace: cassava_trait
def: "Number of nodes at the fourth branching level." []
is_a: CO_334:0001000 ! Variables
relationship: variable_of CO_334:0000351 ! Node number per branch
relationship: variable_of CO_334:0010520 ! Counting: Number of node_method
relationship: variable_of CO_334:0100691 ! nodes
created_by: naama
creation_date: 2017-07-11T10:57:20Z

[Term]
id: CO_334:0000384
name: dry matter content of fibrous root percentage
namespace: cassava_trait
def: "Ratio of measured fibrous root dry weight and fibrous root fresh weight multiplied by 100." [CO:curator]
is_a: CO_334:0001000 ! Variables
relationship: variable_of CO_334:0000424 ! Root dry matter content
relationship: variable_of CO_334:0010011 ! Estimation: Dry matter content of fibrous root percentage
relationship: variable_of CO_334:0100583 ! pct (%)
created_by: AAfolabi
creation_date: 2017-07-18T14:45:13Z

[Term]
id: CO_334:0000385
name: dry matter content of lower stem percentage
namespace: cassava_trait
def: "Ratio of measured lower stem dry weight and lower stem fresh weight multiplied by 100." [CO:curator]
is_a: CO_334:0001000 ! Variables
relationship: variable_of CO_334:0002040 ! Leaf dry matter content
relationship: variable_of CO_334:0010010 ! Estimation: Dry matter content of lower stem percentage
relationship: variable_of CO_334:0100583 ! pct (%)
created_by: AAfolabi
creation_date: 2017-07-18T14:49:00Z

[Term]
id: CO_334:0000386
name: Initial vigor
namespace: cassava_trait
def: "Initial plant vigor at one month after planting" [CO:curators]
synonym: "vigor" EXACT []
xref: TO:0000250
is_a: CO_334:0000001 ! Agronomic trait

[Term]
id: CO_334:0000387
name: Iron content
namespace: cassava_trait
def: "Iron content." [CO:curators]
synonym: "fe" EXACT []
xref: TO:0020089
is_a: CO_334:0000004 ! Quality trait

[Term]
id: CO_334:0000388
name: Lafun content
namespace: cassava_trait
def: "Lafu weight" [CO:curators]
synonym: "lafun" EXACT []
xref: TO:0001042
is_a: CO_334:0000004 ! Quality trait

[Term]
id: CO_334:0000389
name: Leaf color
namespace: cassava_trait
def: "Leaf color" [CO:curators]
synonym: "LfCol" EXACT []
xref: TO:0000326
is_a: CO_334:0000330 ! Leaf morphological trait

[Term]
id: CO_334:0000390
name: Leaf life span
namespace: cassava_trait
def: "Leaf life span" [CO:curators]
synonym: "LfLiife" EXACT []
xref: TO:0000748
is_a: CO_334:0000003 ! Physiological trait

[Term]
id: CO_334:0000391
name: Leaf lobe length
namespace: cassava_trait
def: "Length of middle finger or lobe of matured leaf" [CO:curators]
synonym: "LfLbLng" EXACT []
xref: TO:1000014
is_a: CO_334:0000331 ! Leaf lobe

[Term]
id: CO_334:0000392
name: Leaf lobe margin
namespace: cassava_trait
def: "leaf lobe margin." [CO:curators]
synonym: "LobMgnShp" EXACT []
xref: TO:1000013
is_a: CO_334:0000331 ! Leaf lobe

[Term]
id: CO_334:0000393
name: Leaf Lobe Position
namespace: cassava_trait
def: "Position in which leaf lobes are held" [CO:curators]
synonym: "lflobp" EXACT []
xref: TO:1000013
is_a: CO_334:0000331 ! Leaf lobe

[Term]
id: CO_334:0000394
name: Leaf lobe width
namespace: cassava_trait
def: "Width of middle finger or lobe of matured leaf" [CO:curators]
synonym: "LfLbWdth" EXACT []
xref: TO:1000015
is_a: CO_334:0000331 ! Leaf lobe

[Term]
id: CO_334:0000395
name: Leaf Lobes Number
namespace: cassava_trait
def: "Number of leaf lobes" [CO:curators]
synonym: "lflbno" EXACT []
xref: TO:1000013
is_a: CO_334:0000331 ! Leaf lobe

[Term]
id: CO_334:0000396
name: Leaf retention
namespace: cassava_trait
def: "Leaf retention (stay green)" [CO:curators]
synonym: "LfRet" EXACT []
synonym: "Stay green, Leaf Retention - Cassavabase" EXACT []
xref: TO:0000748
is_a: CO_334:0000003 ! Physiological trait

[Term]
id: CO_334:0000397
name: Leaf scar distance
namespace: cassava_trait
def: "Distance between leaf scar" [CO:curators]
synonym: "lfscdist" EXACT []
xref: TO:0000361
is_a: CO_334:0000332 ! Leaf scar

[Term]
id: CO_334:0000398
name: Leaf scar height
namespace: cassava_trait
def: "Height from ground to leaf scar." [CO:curators]
synonym: "ScarHt" EXACT []
xref: TO:0000362
is_a: CO_334:0000332 ! Leaf scar

[Term]
id: CO_334:0000399
name: Leaf scar number
namespace: cassava_trait
def: "Number of leaf scars" [CO:curators]
synonym: "lfscno" EXACT []
xref: TO:0000363
is_a: CO_334:0000332 ! Leaf scar

[Term]
id: CO_334:0000400
name: Leaf Scar Prominence
namespace: cassava_trait
def: "Prominence of fresh leaf scars" [CO:curators]
synonym: "lfscar" EXACT []
xref: TO:0000364
is_a: CO_334:0000332 ! Leaf scar

[Term]
id: CO_334:0000401
name: Leaf Vein Color
namespace: cassava_trait
def: "Color of leaf vein" [CO:curators]
synonym: "lfvnco" EXACT []
xref: TO:0000719
is_a: CO_334:0000330 ! Leaf morphological trait

[Term]
id: CO_334:0000402
name: Leaf weight
namespace: cassava_trait
def: "Weight of leaf" [CO:curators]
synonym: "LfWt" EXACT []
xref: TO:0000505
is_a: CO_334:0000001 ! Agronomic trait

[Term]
id: CO_334:0000403
name: Male flower number
namespace: cassava_trait
def: "Number of male flowers after the buds appear" [CO:curators]
synonym: "flwmno" EXACT []
xref: TO:0002736
is_a: CO_334:0000336 ! Flower and flowering morphological trait

[Term]
id: CO_334:0000404
name: Male sterile
namespace: cassava_trait
def: "Cassava plants that do no produce viable pollen." [CO:curators]
synonym: "ms" EXACT []
xref: TO:0000437
is_a: CO_334:0000001 ! Agronomic trait

[Term]
id: CO_334:0000405
name: Marketable root number
namespace: cassava_trait
def: "Number of big or more than 1kg root size" [CO:curators]
synonym: "mktrtno" EXACT []
xref: TO:0001041
is_a: CO_334:0000001 ! Agronomic trait

[Term]
id: CO_334:0000406
name: Marketable root weight
namespace: cassava_trait
def: "Marketable root weight" [CO:curators]
synonym: "MkRtWt" EXACT []
xref: TO:0001041
is_a: CO_334:0000001 ! Agronomic trait

[Term]
id: CO_334:0000407
name: Moisture content of fresh root
namespace: cassava_trait
def: "Storage root moisture content" [CO:curators]
synonym: "mc" EXACT []
xref: TO:0000228
is_a: CO_334:0000004 ! Quality trait

[Term]
id: CO_334:0000408
name: Non marketable root number
namespace: cassava_trait
def: "Number of small or less than 1kg root size" [CO:curators]
synonym: "nmkrtno" EXACT []
xref: TO:0001042
is_a: CO_334:0000001 ! Agronomic trait

[Term]
id: CO_334:0000409
name: Non marketable root weight
namespace: cassava_trait
def: "Weight of non-marketable root- i.e., small sized root" [CO:curators]
synonym: "NMkRtWt" EXACT []
xref: TO:0001042
is_a: CO_334:0000001 ! Agronomic trait

[Term]
id: CO_334:0000410
name: Number of bemisia tabaci adult
namespace: cassava_trait
def: "Number of Bemisia tabaci adult white flies" [CO:curators]
synonym: "BTAdtNo" EXACT []
xref: TO:0000261
is_a: CO_334:0000030 ! insect damage

[Term]
id: CO_334:0000411
name: Number of bemisia tabaci nymphs
namespace: cassava_trait
def: "Number of Bemisia tabaci nymphs white flies" [CO:curators]
synonym: "BTNyNo" EXACT []
xref: TO:0000261
is_a: CO_334:0000030 ! insect damage

[Term]
id: CO_334:0000412
name: Number of flowering stalks
namespace: cassava_trait
def: "Number of stalks carrying buds" [CO:curators]
synonym: "FlwStlkNo" EXACT []
xref: TO:0000894
is_a: CO_334:0000336 ! Flower and flowering morphological trait

[Term]
id: CO_334:0000413
name: Number of  forks
namespace: cassava_trait
def: "Number of branches" [CO:curators]
synonym: "flwfrk" EXACT []
xref: TO:0000740
is_a: CO_334:0000329 ! Plant branch morphological trait

[Term]
id: CO_334:0000414
name: Number of fruits
namespace: cassava_trait
def: "Number of fruits" [CO:curators]
synonym: "fruitno" EXACT []
xref: TO:0000894
is_a: CO_334:0000337 ! Fruit morphological trait

[Term]
id: CO_334:0000415
name: Number of fruitset
namespace: cassava_trait
def: "Number of fruits formed after pollination" [CO:curators]
synonym: "flwfrt" EXACT []
xref: TO:0002640
is_a: CO_334:0000337 ! Fruit morphological trait

[Term]
id: CO_334:0000416
name: Number of planted stakes
namespace: cassava_trait
def: "Total number of stakes planted" [CO:curators]
synonym: "stkplt" EXACT []
is_a: CO_334:0000001 ! Agronomic trait

[Term]
id: CO_334:0000417
name: Number of rotten stem
namespace: cassava_trait
def: "Number of rotten stem" [CO:curators]
synonym: "RotStmNo" EXACT []
xref: TO:0000597
is_a: CO_334:0000001 ! Agronomic trait

[Term]
id: CO_334:0000418
name: Number of seeds sown
namespace: cassava_trait
def: "Number of seeds sown per family" [CO:curators]
synonym: "seedno" EXACT []
is_a: CO_334:0000001 ! Agronomic trait

[Term]
id: CO_334:0000419
name: Number of stakes
namespace: cassava_trait
def: "Number of plantable stakes" [CO:curators]
synonym: "Plantable stem number" EXACT []
synonym: "stkno" EXACT []
xref: TO:0000597
is_a: CO_334:0000001 ! Agronomic trait

[Term]
id: CO_334:0000420
name: Number of terminal branches with inflorescence
namespace: cassava_trait
def: "Number of terminal branches with inflorescence" [CO:curators]
synonym: "TermBrnchNo" EXACT []
xref: TO:0000582
is_a: CO_334:0000336 ! Flower and flowering morphological trait

[Term]
id: CO_334:0000421
name: Ovary Color
namespace: cassava_trait
def: "Color of ovary" [CO:curators]
synonym: "ovryco" EXACT []
xref: TO:1000016
is_a: CO_334:0000336 ! Flower and flowering morphological trait

[Term]
id: CO_334:0000422
name: Peel weight
namespace: cassava_trait
def: "Peel weight" [CO:curators]
synonym: "peelwt" EXACT []
xref: TO:0001042
is_a: CO_334:0000001 ! Agronomic trait

[Term]
id: CO_334:0000423
name: dry matter content of leaf percentage
namespace: cassava_trait
def: "Ratio of measured leaf dry weight and leaf fresh weight multiplied by 100." [CO:curator]
is_a: CO_334:0001000 ! Variables
relationship: variable_of CO_334:0002040 ! Leaf dry matter content
relationship: variable_of CO_334:0010009 ! Estimation: Dry matter content of leaf percentage
relationship: variable_of CO_334:0100583 ! pct (%)
created_by: AAfolabi
creation_date: 2017-07-18T14:52:38Z

[Term]
id: CO_334:0000424
name: Root dry matter content
namespace: cassava_trait
def: "Dry matter content of root related terms." [CO:curator]
is_a: CO_334:0000447 ! Dry matter content
created_by: AAfolabi
creation_date: 2017-07-18T14:58:31Z

[Term]
id: CO_334:0000425
name: Total leaf area
namespace: cassava_trait
def: "Measurement of leaf area." [CO:curator]
is_a: CO_334:0000330 ! Leaf morphological trait
created_by: AAfolabi
creation_date: 2017-07-18T15:29:42Z

[Term]
id: CO_334:0000426
name: total leaf area estimation
namespace: cassava_trait
def: "Estimation of leaf area by scanning all leaves of a plant on centimeter square using a handheld device." [CO:curator]
is_a: CO_334:0001000 ! Variables
relationship: variable_of CO_334:0000425 ! Total leaf area
relationship: variable_of CO_334:0010012 ! Estimation: Total leaf area_method
relationship: variable_of CO_334:0100007 ! cm square
created_by: AAfolabi
creation_date: 2017-07-18T15:30:58Z

[Term]
id: CO_334:0000427
name: Petiole Color
namespace: cassava_trait
def: "Petiole color" [CO:curators]
synonym: "petcol" EXACT []
xref: TO:0002707
is_a: CO_334:0000341 ! Leaf petiole

[Term]
id: CO_334:0000428
name: Petiole Insertion Angle
namespace: cassava_trait
def: "Angle between branch and petiole" [CO:curators]
synonym: "petang" EXACT []
xref: TO:0000765
is_a: CO_334:0000341 ! Leaf petiole

[Term]
id: CO_334:0000429
name: Petiole length
namespace: cassava_trait
def: "petiole length" [CO:curators]
synonym: "PetLng" EXACT []
xref: TO:0000766
is_a: CO_334:0000341 ! Leaf petiole

[Term]
id: CO_334:0000430
name: Petiole orientation
namespace: cassava_trait
def: "petiole orientation" [CO:curators]
synonym: "PetOrt" EXACT []
xref: TO:0000765
is_a: CO_334:0000341 ! Leaf petiole

[Term]
id: CO_334:0000431
name: Plant architecture
namespace: cassava_trait
def: "Plant architecture" [CO:curators]
synonym: "Plant Architecture - Cassavabase" EXACT []
synonym: "PlntArch" EXACT []
xref: TO:0000398
is_a: CO_334:0000002 ! Morphological trait

[Term]
id: CO_334:0000432
name: Plant height
namespace: cassava_trait
def: "Height of plant at harvest from ground level to top of canopy" [CO:curators]
synonym: "pltht" EXACT []
xref: TO:0000207
is_a: CO_334:0000001 ! Agronomic trait

[Term]
id: CO_334:0000433
name: Plant shape
namespace: cassava_trait
def: "Shape of plant" [CO:curators]
synonym: "pltshp" EXACT []
xref: TO:0000398
is_a: CO_334:0000002 ! Morphological trait

[Term]
id: CO_334:0000434
name: Plant stands harvested
namespace: cassava_trait
def: "Number of plant stands harvested" [CO:curators]
synonym: "nohav" EXACT []
is_a: CO_334:0000001 ! Agronomic trait

[Term]
id: CO_334:0000435
name: Plantable stem length
namespace: cassava_trait
def: "Plantable stem length" [CO:curators]
synonym: "PlStmHt" EXACT []
is_a: CO_334:0000001 ! Agronomic trait

[Term]
id: CO_334:0000436
name: Ploidy
namespace: cassava_trait
def: "Ploidy level (n = 1,2,3,4 ) (by morphological characteristics)" [CO:curators]
synonym: "ploidy" EXACT []
xref: TO:0000392
is_a: CO_334:0000002 ! Morphological trait

[Term]
id: CO_334:0000437
name: Poundability
namespace: cassava_trait
def: "Poundability (mealiness of boiled roots)" [CO:curators]
synonym: "mealiness" EXACT []
synonym: "pd" EXACT []
xref: TO:0001042
is_a: CO_334:0000004 ! Quality trait

[Term]
id: CO_334:0000438
name: Presence of pollen
namespace: cassava_trait
def: "Presence of pollen" [CO:curators]
synonym: "pollen" EXACT []
xref: TO:0000420
is_a: CO_334:0000336 ! Flower and flowering morphological trait

[Term]
id: CO_334:0000439
name: Proportion of female flower
namespace: cassava_trait
def: "Proportion of female flower" [CO:curators]
synonym: "FFlwProp" EXACT []
xref: TO:0000987
is_a: CO_334:0000336 ! Flower and flowering morphological trait

[Term]
id: CO_334:0000440
name: Lodged plants
namespace: cassava_trait
def: "Degree of plant inclination  from the vertical axis." [CO:curators]
synonym: "lodplt" EXACT []
is_a: CO_334:0000001 ! Agronomic trait

[Term]
id: CO_334:0000441
name: Proportion of plant with inflorescence
namespace: cassava_trait
def: "Proportion of plants per plot that have an inflorescence at varying growth stages. Plant with pollinated and unpollinated flowers are all counted together" [CO:curators]
synonym: "pnoinf" EXACT []
xref: TO:0000582
is_a: CO_334:0000336 ! Flower and flowering morphological trait

[Term]
id: CO_334:0000442
name: Protein content
namespace: cassava_trait
def: "Protein content" [CO:curators]
synonym: "protei" EXACT []
xref: TO:0000598
is_a: CO_334:0000004 ! Quality trait

[Term]
id: CO_334:0000443
name: Red spider mite incidence
namespace: cassava_trait
def: "Proportion of plants within a plot showing evidence of colonization by red spider mite." [CO:curators]
synonym: "rsmi" EXACT []
xref: TO:0000261
is_a: CO_334:0000030 ! insect damage

[Term]
id: CO_334:0000444
name: Red spider mite severity
namespace: cassava_trait
def: "Red spider mite severity" [CO:curators]
synonym: "RSMSev" EXACT []
xref: TO:0000261
is_a: CO_334:0000030 ! insect damage

[Term]
id: CO_334:0000445
name: Days to branching
namespace: cassava_trait
def: "Days to forking event." [CO:curator]
is_a: CO_334:0000329 ! Plant branch morphological trait
created_by: AAfolabi
creation_date: 2017-07-25T09:29:55Z

[Term]
id: CO_334:0000446
name: Root constrictions number
namespace: cassava_trait
def: "Number of constrictions on the storage root" [CO:curators]
synonym: "RtConsNo" EXACT []
synonym: "Storage root constriction presence" EXACT []
xref: TO:1000007
is_a: CO_334:0000333 ! Root morphological trait

[Term]
id: CO_334:0000447
name: Dry matter content
namespace: cassava_trait
def: "Dry matter content of storage roots." [CO:curators]
synonym: "dm" EXACT []
xref: TO:1000007
is_a: CO_334:0000004 ! Quality trait

[Term]
id: CO_334:0000448
name: Root evaluation
namespace: cassava_trait
def: "Evaluation of various root properties" [CO:curators]
synonym: "rteval" EXACT []
xref: TO:0001042
is_a: CO_334:0000001 ! Agronomic trait

[Term]
id: CO_334:0000449
name: Days to branching event
namespace: cassava_trait
def: "Days when forking event occured." [CO:curator]
is_a: CO_334:0000445 ! Days to branching
created_by: AAfolabi
creation_date: 2017-07-25T09:39:03Z

[Term]
id: CO_334:0000450
name: Root length
namespace: cassava_trait
def: "Root length" [CO:curators]
synonym: "RtLng" EXACT []
xref: TO:0000227
is_a: CO_334:0000001 ! Agronomic trait

[Term]
id: CO_334:0000451
name: Storage root neck length
namespace: cassava_trait
def: "Root neck length" [CO:curators]
synonym: "nklgt" EXACT []
xref: TO:1000007
is_a: CO_334:0000334 ! Storage root morphological trait

[Term]
id: CO_334:0000452
name: Root number
namespace: cassava_trait
def: "Number of storage roots (marketable and non-marketable)" [CO:curators]
synonym: "Root Number" EXACT []
synonym: "RtNo" EXACT []
xref: TO:1000007
is_a: CO_334:0000001 ! Agronomic trait

[Term]
id: CO_334:0000453
name: Root Position
namespace: cassava_trait
def: "Position of roots" [CO:curators]
synonym: "rtpost" EXACT []
xref: TO:1000007
is_a: CO_334:0000333 ! Root morphological trait

[Term]
id: CO_334:0000454
name: Storage root surface color
namespace: cassava_trait
def: "Storage root surface color" [CO:curators]
synonym: "rtscol" EXACT []
xref: TO:1000007
is_a: CO_334:0000334 ! Storage root morphological trait

[Term]
id: CO_334:0000455
name: Storage root surface texture
namespace: cassava_trait
def: "Storage root surface texture." [CO:curators]
synonym: "rttext" EXACT []
xref: TO:1000007
is_a: CO_334:0000334 ! Storage root morphological trait

[Term]
id: CO_334:0000456
name: Root yield
namespace: cassava_trait
def: "Storage root yield" [CO:curators]
synonym: "RtYld" EXACT []
xref: TO:0001041
is_a: CO_334:0000001 ! Agronomic trait

[Term]
id: CO_334:0000457
name: Rotted storage roots
namespace: cassava_trait
def: "Number of rotted storage roots." [CO:curators]
synonym: "RotRtNo" EXACT []
synonym: "Unmarketable roots, Rotted Storage Roots - Cassavabase" EXACT []
xref: TO:0001042
is_a: CO_334:0000334 ! Storage root morphological trait

[Term]
id: CO_334:0000458
name: Rotten root proportion
namespace: cassava_trait
def: "Proportion of rotten root" [CO:curators]
synonym: "RotRtPrp" EXACT []
xref: TO:0001042
is_a: CO_334:0000001 ! Agronomic trait

[Term]
id: CO_334:0000459
name: Seed color
namespace: cassava_trait
def: "Main color of seed" [CO:curators]
synonym: "seedco" EXACT []
xref: TO:0000486
is_a: CO_334:0000002 ! Morphological trait

[Term]
id: CO_334:0000460
name: Seedling number
namespace: cassava_trait
def: "Number of emerging seedlings" [CO:curators]
synonym: "SdlngNo" EXACT []
xref: TO:0000751
is_a: CO_334:0000001 ! Agronomic trait

[Term]
id: CO_334:0000461
name: Selected variety
namespace: cassava_trait
def: "Selected variety" [CO:curators]
synonym: "select" EXACT []
is_a: CO_334:0000001 ! Agronomic trait

[Term]
id: CO_334:0000462
name: Sepal Color
namespace: cassava_trait
def: "Color of sepals" [CO:curators]
synonym: "splcol" EXACT []
xref: TO:0000573
is_a: CO_334:0000336 ! Flower and flowering morphological trait

[Term]
id: CO_334:0000463
name: Sooty mould
namespace: cassava_trait
def: "Balck mould" [CO:curators]
synonym: "sooty" EXACT []
xref: TO:0000439
is_a: CO_334:0000030 ! insect damage

[Term]
id: CO_334:0000464
name: Spiraling whitefly incidence
namespace: cassava_trait
def: "Proportion of plants within a plot showing evidence of colonization by spiraling whitefly." [CO:curators]
synonym: "Swfi" EXACT []
xref: TO:0000261
is_a: CO_334:0000030 ! insect damage

[Term]
id: CO_334:0000465
name: Spiraling whitefly severity
namespace: cassava_trait
def: "Spiraling whitefly severity" [CO:curators]
synonym: "SWFSev" EXACT []
xref: TO:0000261
is_a: CO_334:0000030 ! insect damage

[Term]
id: CO_334:0000466
name: Sprout count
namespace: cassava_trait
def: "Number of germinated stakes" [CO:curators]
synonym: "sprtct" EXACT []
xref: TO:1000007
is_a: CO_334:0000001 ! Agronomic trait

[Term]
id: CO_334:0000467
name: days to first forking event visual observation
namespace: cassava_trait
def: "Visual observation of when (actual date in the format of dd/mm/yyyy from the date of planting) first forking event occured." [CO:curator]
is_a: CO_334:0001000 ! Variables
relationship: variable_of CO_334:0000449 ! Days to branching event
relationship: variable_of CO_334:0010013 ! Visual Observation: Days to branching event
relationship: variable_of CO_334:0100611 ! days
created_by: AAfolabi
creation_date: 2017-07-25T10:00:07Z

[Term]
id: CO_334:0000468
name: days to second forking event visual observation
namespace: cassava_trait
def: "Visual observation of when (actual date in the format of dd/mm/yyyy from the date of planting) second forking event occured." [CO:curator]
is_a: CO_334:0001000 ! Variables
relationship: variable_of CO_334:0000449 ! Days to branching event
relationship: variable_of CO_334:0010013 ! Visual Observation: Days to branching event
relationship: variable_of CO_334:0100611 ! days
created_by: AAfolabi
creation_date: 2017-07-25T10:05:36Z

[Term]
id: CO_334:0000469
name: days to third forking event visual observation
namespace: cassava_trait
def: "Visual observation of when (actual date in the format of dd/mm/yyyy from the date of planting) third forking event occured." [CO:curator]
is_a: CO_334:0001000 ! Variables
relationship: variable_of CO_334:0000449 ! Days to branching event
relationship: variable_of CO_334:0010013 ! Visual Observation: Days to branching event
relationship: variable_of CO_334:0100611 ! days
created_by: AAfolabi
creation_date: 2017-07-25T10:06:51Z

[Term]
id: CO_334:0000470
name: Days to abortion
namespace: cassava_trait
is_a: CO_334:0000336 ! Flower and flowering morphological trait
created_by: AAfolabi
creation_date: 2017-07-25T11:13:40Z

[Term]
id: CO_334:0000471
name: Days to abortion by branching levels
namespace: cassava_trait
def: "Days to the death of immatured flower." [CO:curator]
is_a: CO_334:0000470 ! Days to abortion
created_by: AAfolabi
creation_date: 2017-07-25T11:14:47Z

[Term]
id: CO_334:0000472
name: Sprouting
namespace: cassava_trait
def: "Proportion of stakes germinated" [CO:curators]
synonym: "Proportion of germinated stakes" EXACT []
synonym: "sprout" EXACT []
xref: TO:0000250
is_a: CO_334:0000001 ! Agronomic trait

[Term]
id: CO_334:0000473
name: Stalk length
namespace: cassava_trait
def: "Stalk length" [CO:curators]
synonym: "StkLng" EXACT []
xref: TO:0000920
is_a: CO_334:0000001 ! Agronomic trait

[Term]
id: CO_334:0000474
name: Starch Content
namespace: cassava_trait
def: "Starch content" [CO:curators]
synonym: "starch" EXACT []
xref: TO:0000696
is_a: CO_334:0000317 ! Starch properties

[Term]
id: CO_334:0000475
name: Stem Color
namespace: cassava_trait
def: "Stem color" [CO:curators]
synonym: "stmcol" EXACT []
xref: TO:0000056
is_a: CO_334:0000338 ! Stem morphological trait

[Term]
id: CO_334:0000476
name: Stem cortex color
namespace: cassava_trait
def: "Color of stem cortex" [CO:curators]
synonym: "stmctcol" EXACT []
xref: TO:1000017
is_a: CO_334:0000338 ! Stem morphological trait

[Term]
id: CO_334:0000477
name: Stem epidermis color
namespace: cassava_trait
def: "Color of stem epidermis" [CO:curators]
synonym: "stmepcol" EXACT []
xref: TO:1000018
is_a: CO_334:0000338 ! Stem morphological trait

[Term]
id: CO_334:0000478
name: Stem height
namespace: cassava_trait
def: "Plant height without leaf corresponding to the stem portion without leaf" [CO:curators]
synonym: "Stem height" EXACT []
synonym: "StmHt" EXACT []
xref: TO:0000576
is_a: CO_334:0000001 ! Agronomic trait

[Term]
id: CO_334:0000479
name: Stem number
namespace: cassava_trait
def: "Number of stem" [CO:curators]
synonym: "StmNo" EXACT []
xref: TO:0000953
is_a: CO_334:0000001 ! Agronomic trait

[Term]
id: CO_334:0000480
name: Stem weight
namespace: cassava_trait
def: "Weight of harvested plant biomass excluding leaves" [CO:curators]
synonym: "Stem yield" EXACT []
synonym: "StmYld" EXACT []
xref: TO:0000952
is_a: CO_334:0000001 ! Agronomic trait

[Term]
id: CO_334:0000481
name: Stigma Color
namespace: cassava_trait
def: "Color of stigma" [CO:curators]
synonym: "stgmco" EXACT []
xref: TO:0000185
is_a: CO_334:0000336 ! Flower and flowering morphological trait

[Term]
id: CO_334:0000482
name: Stipule margin
namespace: cassava_trait
def: "Observation of stipule's margin" [CO:curators]
synonym: "StpMrgShp" EXACT []
xref: TO:0000754
is_a: CO_334:0000001 ! Agronomic trait

[Term]
id: CO_334:0000483
name: Stipules length
namespace: cassava_trait
def: "Length of stipules" [CO:curators]
synonym: "stipgt" EXACT []
xref: TO:1000020
is_a: CO_334:0000001 ! Agronomic trait

[Term]
id: CO_334:0000484
name: Stock weight
namespace: cassava_trait
def: "Fresh weight of the planted part anchoring the storage root" [CO:curators]
synonym: "stkwt" EXACT []
xref: TO:0001042
is_a: CO_334:0000001 ! Agronomic trait

[Term]
id: CO_334:0000485
name: Storage Root Constrictions
namespace: cassava_trait
def: "Presence of constrictions on the storage root" [CO:curators]
synonym: "rtcons" EXACT []
synonym: "Storage root constriction presence" EXACT []
xref: TO:1000007
is_a: CO_334:0000334 ! Storage root morphological trait

[Term]
id: CO_334:0000486
name: Storage Root Cortex Color
namespace: cassava_trait
def: "Color of outer surface of storage root cortex (inner skin)" [CO:curators]
synonym: "inncol" EXACT []
synonym: "Inner skin color" EXACT []
xref: TO:1000007
is_a: CO_334:0000334 ! Storage root morphological trait

[Term]
id: CO_334:0000487
name: Storage Root Diameter
namespace: cassava_trait
def: "Storage root diameter" [CO:curators]
synonym: "rtdiam" EXACT []
xref: TO:1000006
is_a: CO_334:0000334 ! Storage root morphological trait

[Term]
id: CO_334:0000488
name: Storage Root Peduncle
namespace: cassava_trait
def: "Storage Root Peduncle" [CO:curators]
synonym: "rtpedu" EXACT []
xref: TO:1000007
is_a: CO_334:0000334 ! Storage root morphological trait

[Term]
id: CO_334:0000489
name: Storage Root Periderm Color
namespace: cassava_trait
def: "Color of outer surface of storage root periderm (outer skin)" [CO:curators]
synonym: "outcol" EXACT []
synonym: "Outer skin color" EXACT []
xref: TO:1000007
is_a: CO_334:0000334 ! Storage root morphological trait

[Term]
id: CO_334:0000490
name: Storage Root Pulp Color
namespace: cassava_trait
def: "Storage root pulp color" [CO:curators]
synonym: "plpcol" EXACT []
xref: TO:1000007
is_a: CO_334:0000334 ! Storage root morphological trait

[Term]
id: CO_334:0000491
name: Storage Root Shape
namespace: cassava_trait
def: "Storage root shape" [CO:curators]
synonym: "rtshp" EXACT []
xref: TO:1000007
is_a: CO_334:0000334 ! Storage root morphological trait

[Term]
id: CO_334:0000492
name: Storage Root Size
namespace: cassava_trait
def: "Storage root length" [CO:curators]
synonym: "rtsz" EXACT []
synonym: "Storage root length" EXACT []
xref: TO:1000007
is_a: CO_334:0000334 ! Storage root morphological trait

[Term]
id: CO_334:0000493
name: Storage root weight
namespace: cassava_trait
def: "Weight of harvested storage root" [CO:curators]
synonym: "Fresh Weight of Storage Root - Cassavabase" EXACT []
synonym: "RtWt" EXACT []
xref: TO:1000007
is_a: CO_334:0000001 ! Agronomic trait

[Term]
id: CO_334:0000494
name: Stump weight
namespace: cassava_trait
def: "Weight of stump" [CO:curators]
synonym: "StumpWt" EXACT []
xref: TO:0001042
is_a: CO_334:0000001 ! Agronomic trait

[Term]
id: CO_334:0000495
name: Sugar content
namespace: cassava_trait
def: "Sugar content" [CO:curators]
synonym: "sugar" EXACT []
xref: TO:0000333
is_a: CO_334:0000004 ! Quality trait

[Term]
id: CO_334:0000496
name: Suitability for intercropping
namespace: cassava_trait
def: "Compatibility for use in intercroping." [CO:curators]
synonym: "intcrp" EXACT []
is_a: CO_334:0000001 ! Agronomic trait

[Term]
id: CO_334:0000497
name: Gari swelling capacity
namespace: cassava_trait
def: "Swelling capacity of gari sample" [CO:curators]
synonym: "swelling" EXACT []
xref: TO:0001042
is_a: CO_334:0000004 ! Quality trait

[Term]
id: CO_334:0000498
name: Taste of boiled roots
namespace: cassava_trait
def: "Taste of boiled roots" [CO:curators]
synonym: "pdtas" EXACT []
xref: TO:0001042
is_a: CO_334:0000004 ! Quality trait

[Term]
id: CO_334:0000499
name: Tip shoot weight
namespace: cassava_trait
def: "Tip shoot weight" [CO:curators]
synonym: "TipShWt" EXACT []
xref: TO:0000568
is_a: CO_334:0000001 ! Agronomic trait

[Term]
id: CO_334:0000500
name: Total carotenoid retention
namespace: cassava_trait
def: "Total caroteneoid content after cooking" [CO:curators]
synonym: "CaroRet" EXACT []
xref: TO:0001042
is_a: CO_334:0000297 ! Carotenoid content

[Term]
id: CO_334:0000501
name: Trans-9 activity
namespace: cassava_trait
def: "Activity of trans 9 beta carotene" [CO:curators]
synonym: "Trans9Ct" EXACT []
xref: TO:0000282
is_a: CO_334:0000004 ! Quality trait

[Term]
id: CO_334:0000502
name: Storage root cyanide content
namespace: cassava_trait
def: "Cyanide content in storage roots" [CO:curators]
synonym: "RtCyanC" EXACT []
xref: TO:0000465
is_a: CO_334:0000004 ! Quality trait

[Term]
id: CO_334:0000503
name: Typhlodromalus aripo
namespace: cassava_trait
def: "Presence of Typhlodromalus aripo" [CO:curators]
synonym: "taripo" EXACT []
xref: TO:0000261
is_a: CO_334:0000030 ! insect damage

[Term]
id: CO_334:0000504
name: Weight of mashed cassava cake
namespace: cassava_trait
def: "Weight of mashed cassava cake" [CO:curators]
synonym: "wtamash" EXACT []
xref: TO:0001042
is_a: CO_334:0000004 ! Quality trait

[Term]
id: CO_334:0000505
name: Young Stem Growth Habit
namespace: cassava_trait
def: "Growth habit of young stem" [CO:curators]
synonym: "stemgh" EXACT []
xref: TO:0000361
is_a: CO_334:0000338 ! Stem morphological trait

[Term]
id: CO_334:0000506
name: Young Stem Pubescence
namespace: cassava_trait
def: "Pubescence of young stem" [CO:curators]
synonym: "stmpub" EXACT []
xref: TO:0000361
is_a: CO_334:0000338 ! Stem morphological trait

[Term]
id: CO_334:0000507
name: Zinc content
namespace: cassava_trait
def: "Zinc content" [CO:curators]
synonym: "zn" EXACT []
is_a: CO_334:0000004 ! Quality trait

[Term]
id: CO_334:0000508
name: days to abortion on the first branch visual observation
namespace: cassava_trait
def: "Visual observation (actual date in the format of dd/mm/yyyy from the date of planting) of the death of immatured on the first branching level. Color of buds changes from green to brown." [CO:curator]
is_a: CO_334:0001000 ! Variables
relationship: variable_of CO_334:0000471 ! Days to abortion by branching levels
relationship: variable_of CO_334:0010014 ! Visual Observation: Days to abortion by branching level
relationship: variable_of CO_334:0100611 ! days
created_by: AAfolabi
creation_date: 2017-07-25T11:17:03Z

[Term]
id: CO_334:0000509
name: days to abortion on the second branch visual observation
namespace: cassava_trait
def: "Visual observation (actual date in the format of dd/mm/yyyy from the date of planting) of the death of immatured on the second branching level. Color of buds changes from green to brown." [CO:curator]
is_a: CO_334:0001000 ! Variables
relationship: variable_of CO_334:0000471 ! Days to abortion by branching levels
relationship: variable_of CO_334:0010014 ! Visual Observation: Days to abortion by branching level
relationship: variable_of CO_334:0100611 ! days
created_by: AAfolabi
creation_date: 2017-07-25T11:22:50Z

[Term]
id: CO_334:0000510
name: days to abortion on the third branch visual observation
namespace: cassava_trait
def: "Visual observation (actual date in the format of dd/mm/yyyy from the date of planting) of the death of immatured on the third branching level. Color of buds changes from green to brown." [CO:curator]
is_a: CO_334:0001000 ! Variables
relationship: variable_of CO_334:0000471 ! Days to abortion by branching levels
relationship: variable_of CO_334:0010014 ! Visual Observation: Days to abortion by branching level
relationship: variable_of CO_334:0100611 ! days
created_by: AAfolabi
creation_date: 2017-07-25T11:26:48Z

[Term]
id: CO_334:0000511
name: Days to first female flower opens
namespace: cassava_trait
def: "First female flower (pistillate) mature and opens." [CO:curator]
is_a: CO_334:0000336 ! Flower and flowering morphological trait
created_by: AAfolabi
creation_date: 2017-07-25T11:46:46Z

[Term]
id: CO_334:0000512
name: Days to first female flower opens by branch levels
namespace: cassava_trait
def: "First female flower (pistillate) mature and opens by branching levels." [CO:curator]
is_a: CO_334:0000511 ! Days to first female flower opens
created_by: AAfolabi
creation_date: 2017-07-25T11:49:20Z

[Term]
id: CO_334:0000513
name: days to first female flower open on the first branch visual observation
namespace: cassava_trait
def: "Visual observation (actual date in the format of dd/mm/yyyy from the date of planting) of the opening of the first female flower on the first branching level." [CO:curator]
is_a: CO_334:0001000 ! Variables
relationship: variable_of CO_334:0000512 ! Days to first female flower opens by branch levels
relationship: variable_of CO_334:0010015 ! Visual Observation: Days to first female flower opens by branch levels
relationship: variable_of CO_334:0100611 ! days
created_by: AAfolabi
creation_date: 2017-07-25T11:52:02Z

[Term]
id: CO_334:0000514
name: days to first female flower open on the second branch visual observation
namespace: cassava_trait
def: "Visual observation (actual date in the format of dd/mm/yyyy from the date of planting) of the opening of the first female flower on the second branching level." [CO:curator]
is_a: CO_334:0001000 ! Variables
relationship: variable_of CO_334:0000512 ! Days to first female flower opens by branch levels
relationship: variable_of CO_334:0010015 ! Visual Observation: Days to first female flower opens by branch levels
relationship: variable_of CO_334:0100611 ! days
created_by: AAfolabi
creation_date: 2017-07-25T11:53:47Z

[Term]
id: CO_334:0000515
name: days to first female flower open on the third branch visual observation
namespace: cassava_trait
def: "Visual observation (actual date in the format of dd/mm/yyyy from the date of planting) of the opening of the first female flower on the third branching level." [CO:curator]
is_a: CO_334:0001000 ! Variables
relationship: variable_of CO_334:0000512 ! Days to first female flower opens by branch levels
relationship: variable_of CO_334:0010015 ! Visual Observation: Days to first female flower opens by branch levels
relationship: variable_of CO_334:0100611 ! days
created_by: AAfolabi
creation_date: 2017-07-25T11:55:08Z

[Term]
id: CO_334:0000516
name: Days to senescence
namespace: cassava_trait
def: "Days to senescence." [CO:curator]
is_a: CO_334:0000336 ! Flower and flowering morphological trait
created_by: AAfolabi
creation_date: 2017-07-25T12:16:27Z

[Term]
id: CO_334:0000517
name: Days to senescence by branch level
namespace: cassava_trait
is_a: CO_334:0000516 ! Days to senescence
created_by: AAfolabi
creation_date: 2017-07-25T12:17:45Z

[Term]
id: CO_334:0000518
name: days to senescence on the first branch visual observation
namespace: cassava_trait
def: "Visual observation (actual date in the format of dd/mm/yyyy from the date of planting) of the death of matured flowers on the first branching level. Usually done by observing the change in color of petal from yellow to brown." [CO:curator]
is_a: CO_334:0001000 ! Variables
relationship: variable_of CO_334:0000517 ! Days to senescence by branch level
relationship: variable_of CO_334:0010016 ! Visual Observation: Days to senescence by branch level
relationship: variable_of CO_334:0100611 ! days
created_by: AAfolabi
creation_date: 2017-07-25T12:18:35Z

[Term]
id: CO_334:0000519
name: days to senescence on the second branch visual observation
namespace: cassava_trait
def: "Visual observation (actual date in the format of dd/mm/yyyy from the date of planting) of the death of matured flowers on the second branching level. Usually done by observing the change in color of petal from yellow to brown." [CO:curator]
is_a: CO_334:0001000 ! Variables
relationship: variable_of CO_334:0000517 ! Days to senescence by branch level
relationship: variable_of CO_334:0010016 ! Visual Observation: Days to senescence by branch level
relationship: variable_of CO_334:0100611 ! days
created_by: AAfolabi
creation_date: 2017-07-25T12:24:11Z

[Term]
id: CO_334:0000520
name: days to senescence on the third branch visual observation
namespace: cassava_trait
def: "Visual observation (actual date in the format of dd/mm/yyyy from the date of planting) of the death of matured flowers on the third branching level. Usually done by observing the change in color of petal from yellow to brown." [CO:curator]
is_a: CO_334:0001000 ! Variables
relationship: variable_of CO_334:0000517 ! Days to senescence by branch level
relationship: variable_of CO_334:0010016 ! Visual Observation: Days to senescence by branch level
relationship: variable_of CO_334:0100611 ! days
created_by: AAfolabi
creation_date: 2017-07-25T12:26:27Z

[Term]
id: CO_334:0000521
name: Number of forks by branch level
namespace: cassava_trait
def: "Number of forks or branches at specific branching levels." [CO:curator]
is_a: CO_334:0000413 ! Number of  forks
created_by: AAfolabi
creation_date: 2017-07-25T14:53:49Z

[Term]
id: CO_334:0000522
name: number of forks on branching level 1 counting
namespace: cassava_trait
def: "Number of forks (2 forks/branches (dichotomous), 3 forks/branches (trichotomous), or 4 forks/branches (tetrachotomous)) on the first branching level." [CO:curator]
is_a: CO_334:0001000 ! Variables
relationship: variable_of CO_334:0000521 ! Number of forks by branch level
relationship: variable_of CO_334:0010017 ! Counting: Number of forks by branch level
relationship: variable_of CO_334:0100012 ! branches
created_by: AAfolabi
creation_date: 2017-07-25T14:56:41Z

[Term]
id: CO_334:0000523
name: number of forks on branching level 2 counting
namespace: cassava_trait
def: "Number of forks (2 forks/branches (dichotomous), 3 forks/branches (trichotomous), or 4 forks/branches (tetrachotomous)) on the second branching level." [CO:curator]
is_a: CO_334:0001000 ! Variables
relationship: variable_of CO_334:0000521 ! Number of forks by branch level
relationship: variable_of CO_334:0010017 ! Counting: Number of forks by branch level
relationship: variable_of CO_334:0100012 ! branches
created_by: AAfolabi
creation_date: 2017-07-25T15:01:01Z

[Term]
id: CO_334:0000524
name: number of forks on branching level 3 counting
namespace: cassava_trait
def: "Number of forks (2 forks/branches (dichotomous), 3 forks/branches (trichotomous), or 4 forks/branches (tetrachotomous)) on the third branching level." [CO:curator]
is_a: CO_334:0001000 ! Variables
relationship: variable_of CO_334:0000521 ! Number of forks by branch level
relationship: variable_of CO_334:0010017 ! Counting: Number of forks by branch level
relationship: variable_of CO_334:0100012 ! branches
created_by: AAfolabi
creation_date: 2017-07-25T15:02:13Z

[Term]
id: CO_334:0000525
name: Number of inflorescence by branch level
namespace: cassava_trait
def: "Number of inflorescence at specific branching level." [CO:curator]
is_a: CO_334:0000336 ! Flower and flowering morphological trait
created_by: AAfolabi
creation_date: 2017-07-25T15:54:07Z

[Term]
id: CO_334:0000526
name: number of inflorescence on the first branch counting
namespace: cassava_trait
def: "Number of inflorescence on the first branching level." [CO:curator]
is_a: CO_334:0001000 ! Variables
relationship: variable_of CO_334:0000525 ! Number of inflorescence by branch level
relationship: variable_of CO_334:0010018 ! Counting: Number of inflorescence by branch level
relationship: variable_of CO_334:0100014 ! inflorescence
created_by: AAfolabi
creation_date: 2017-07-25T15:58:19Z

[Term]
id: CO_334:0000527
name: number of inflorescence on the second branch counting
namespace: cassava_trait
def: "Number of inflorescence on the second branching level." [CO:curator]
is_a: CO_334:0001000 ! Variables
relationship: variable_of CO_334:0000525 ! Number of inflorescence by branch level
relationship: variable_of CO_334:0010018 ! Counting: Number of inflorescence by branch level
relationship: variable_of CO_334:0100014 ! inflorescence
created_by: AAfolabi
creation_date: 2017-07-25T16:00:49Z

[Term]
id: CO_334:0000528
name: number of inflorescence on the third branch counting
namespace: cassava_trait
def: "Number of inflorescence on the third branching level." [CO:curator]
is_a: CO_334:0001000 ! Variables
relationship: variable_of CO_334:0000525 ! Number of inflorescence by branch level
relationship: variable_of CO_334:0010018 ! Counting: Number of inflorescence by branch level
relationship: variable_of CO_334:0100014 ! inflorescence
created_by: AAfolabi
creation_date: 2017-07-25T16:02:21Z

[Term]
id: CO_334:0000529
name: Number of buds
namespace: cassava_trait
def: "Number of buds." [CO:curator]
is_a: CO_334:0000336 ! Flower and flowering morphological trait
created_by: AAfolabi
creation_date: 2017-07-25T16:16:00Z

[Term]
id: CO_334:0000530
name: Number of buds by branch level
namespace: cassava_trait
def: "Count of the number of buds at different branching level." [CO:curator]
is_a: CO_334:0000529 ! Number of buds
created_by: AAfolabi
creation_date: 2017-07-25T16:16:30Z

[Term]
id: CO_334:0000531
name: number of buds on branch 1 counting
namespace: cassava_trait
def: "Count of the number of flower buds (inability to distinguish a flower bud as a male Or female) on the first branching level." [CO:curator]
is_a: CO_334:0001000 ! Variables
relationship: variable_of CO_334:0000530 ! Number of buds by branch level
relationship: variable_of CO_334:0010019 ! Counting: Number of buds by branch level
relationship: variable_of CO_334:0100013 ! buds
created_by: AAfolabi
creation_date: 2017-07-25T16:19:03Z

[Term]
id: CO_334:0000532
name: number of buds on branch 2 counting
namespace: cassava_trait
def: "Counnt of the number of flower buds (inability to distinguish a flower bud as a male Or female) on the second branching level." [CO:curator]
is_a: CO_334:0001000 ! Variables
relationship: variable_of CO_334:0000530 ! Number of buds by branch level
relationship: variable_of CO_334:0010019 ! Counting: Number of buds by branch level
relationship: variable_of CO_334:0100013 ! buds
created_by: AAfolabi
creation_date: 2017-07-25T16:21:57Z

[Term]
id: CO_334:0000533
name: number of buds on branch 3 counting
namespace: cassava_trait
def: "Counnt of the number of flower buds (inability to distinguish a flower bud as a male Or female) on the third branching level." [CO:curator]
is_a: CO_334:0001000 ! Variables
relationship: variable_of CO_334:0000530 ! Number of buds by branch level
relationship: variable_of CO_334:0010019 ! Counting: Number of buds by branch level
relationship: variable_of CO_334:0100013 ! buds
created_by: AAfolabi
creation_date: 2017-07-25T16:22:40Z

[Term]
id: CO_334:0000534
name: male flower number counting by branch level
namespace: cassava_trait
def: "Number male flowers after the buds appears, matures, and grows in size to become distinctive at specific branch levels." [CO:curator]
is_a: CO_334:0000403 ! Male flower number
created_by: AAfolabi
creation_date: 2017-07-25T16:30:45Z

[Term]
id: CO_334:0000535
name: male flower number counting on branch 1
namespace: cassava_trait
def: "A count of the number male flowers after the buds appears, matures, and grows in size to become distinctive on the first branch levels." [CO:curator]
is_a: CO_334:0001000 ! Variables
relationship: variable_of CO_334:0000534 ! male flower number counting by branch level
relationship: variable_of CO_334:0010020 ! Counting: Male flower number by branch level
relationship: variable_of CO_334:0100606 ! flowers
created_by: AAfolabi
creation_date: 2017-07-25T16:33:09Z

[Term]
id: CO_334:0000536
name: male flower number counting on branch 2
namespace: cassava_trait
def: "A count of the number male flowers after the buds appears, matures, and grows in size to become distinctive on the second branch levels." [CO:curator]
is_a: CO_334:0001000 ! Variables
relationship: variable_of CO_334:0000534 ! male flower number counting by branch level
relationship: variable_of CO_334:0010020 ! Counting: Male flower number by branch level
relationship: variable_of CO_334:0100606 ! flowers
created_by: AAfolabi
creation_date: 2017-07-25T16:34:25Z

[Term]
id: CO_334:0000537
name: male flower number counting on branch 3
namespace: cassava_trait
def: "A count of the number male flowers after the buds appears, matures, and grows in size to become distinctive on the third branch levels." [CO:curator]
is_a: CO_334:0001000 ! Variables
relationship: variable_of CO_334:0000534 ! male flower number counting by branch level
relationship: variable_of CO_334:0010020 ! Counting: Male flower number by branch level
relationship: variable_of CO_334:0100606 ! flowers
created_by: AAfolabi
creation_date: 2017-07-25T16:35:19Z

[Term]
id: CO_334:0000538
name: Days to fruitset by branch level
namespace: cassava_trait
def: "Days to fruitset in a plant." [CO:curator]
is_a: CO_334:0000337 ! Fruit morphological trait
created_by: AAfolabi
creation_date: 2017-07-25T16:49:04Z

[Term]
id: CO_334:0000539
name: days to fruitset on branch 1 visual observation
namespace: cassava_trait
def: "Visual observation (actual date in the format of dd/mm/yyyy from the date of planting) of the date when fruit is first seen on the first branching level." [CO:curator]
is_a: CO_334:0001000 ! Variables
relationship: variable_of CO_334:0000538 ! Days to fruitset by branch level
relationship: variable_of CO_334:0010021 ! Visual Observation: Days to fruitset by branch level
relationship: variable_of CO_334:0100611 ! days
created_by: AAfolabi
creation_date: 2017-07-25T16:50:17Z

[Term]
id: CO_334:0000540
name: days to fruitset on branch 2 visual observation
namespace: cassava_trait
def: "Visual observation (actual date in the format of dd/mm/yyyy from the date of planting) of the date when fruit is first seen on the second branching level." [CO:curator]
is_a: CO_334:0001000 ! Variables
relationship: variable_of CO_334:0000538 ! Days to fruitset by branch level
relationship: variable_of CO_334:0010021 ! Visual Observation: Days to fruitset by branch level
relationship: variable_of CO_334:0100611 ! days
created_by: AAfolabi
creation_date: 2017-07-25T16:52:43Z

[Term]
id: CO_334:0000541
name: days to fruitset on branch 3 visual observation
namespace: cassava_trait
def: "Visual observation (actual date in the format of dd/mm/yyyy from the date of planting) of the date when fruit is first seen on the third branching level." [CO:curator]
is_a: CO_334:0001000 ! Variables
relationship: variable_of CO_334:0000538 ! Days to fruitset by branch level
relationship: variable_of CO_334:0010021 ! Visual Observation: Days to fruitset by branch level
relationship: variable_of CO_334:0100611 ! days
created_by: AAfolabi
creation_date: 2017-07-25T16:53:21Z

[Term]
id: CO_334:0000542
name: number of fruitset by branch level
namespace: cassava_trait
def: "Number of fruits formed from the seeds after pollination at different branching level." [CO:curator]
is_a: CO_334:0000415 ! Number of fruitset
created_by: AAfolabi
creation_date: 2017-07-25T16:58:36Z

[Term]
id: CO_334:0000543
name: number of fruitset on branch 1 counting
namespace: cassava_trait
def: "A count of the number of fruits formed from the seeds after pollination on the first branching level." [CO:curator]
is_a: CO_334:0001000 ! Variables
relationship: variable_of CO_334:0000542 ! number of fruitset by branch level
relationship: variable_of CO_334:0010022 ! Counting: Number of fruitset by branch level
relationship: variable_of CO_334:0100017 ! fruitset
created_by: AAfolabi
creation_date: 2017-07-25T17:00:04Z

[Term]
id: CO_334:0000544
name: number of fruitset on branch 2 counting
namespace: cassava_trait
def: "A count of the number of fruits formed from the seeds after pollination on the second branching level." [CO:curator]
is_a: CO_334:0001000 ! Variables
relationship: variable_of CO_334:0000542 ! number of fruitset by branch level
relationship: variable_of CO_334:0010022 ! Counting: Number of fruitset by branch level
relationship: variable_of CO_334:0100017 ! fruitset
created_by: AAfolabi
creation_date: 2017-07-25T17:03:07Z

[Term]
id: CO_334:0000545
name: number of fruitset on branch 3 counting
namespace: cassava_trait
def: "A count of the number of fruits formed from the seeds after pollination on the third branching level." [CO:curator]
is_a: CO_334:0001000 ! Variables
relationship: variable_of CO_334:0000542 ! number of fruitset by branch level
relationship: variable_of CO_334:0010022 ! Counting: Number of fruitset by branch level
relationship: variable_of CO_334:0100017 ! fruitset
created_by: AAfolabi
creation_date: 2017-07-25T17:04:28Z

[Term]
id: CO_334:0001000
name: Variables
namespace: CassavaVariable

[Term]
id: CO_334:0001001
name: Scales
namespace: CassavaScale

[Term]
id: CO_334:0001002
name: Methods
namespace: CassavaMethod

[Term]
id: CO_334:0001012
name: Softness of boiled cassava roots
namespace: cassava_trait
def: "Mechanical attribute of boiled cassava roots relating to force required to make them compressed" []
is_a: CO_334:0000004 ! Quality trait

[Term]
id: CO_334:0001016
name: softness of boiled cassava roots in newtons
namespace: cassava_trait
def: "Use of a penetrometer to record the maximum force used to penetrate the boiled root, measured in newtons." []
is_a: CO_334:0001000 ! Variables
relationship: variable_of CO_334:0001012 ! Softness of boiled cassava roots
relationship: variable_of CO_334:0010517 ! Calculation: Softness of boiled root_method
relationship: variable_of CO_334:0100695 ! newton

[Term]
id: CO_334:0001025
name: farmer preference trait post-harvest
namespace: cassava_trait
is_a: CO_334:0001026 ! Farmer preference trait

[Term]
id: CO_334:0001026
name: Farmer preference trait
namespace: cassava_trait
is_a: CO_334:0002010 ! Farmer trait

[Term]
id: CO_334:0001027
name: farmer preference trait at harvest
namespace: cassava_trait
is_a: CO_334:0001026 ! Farmer preference trait

[Term]
id: CO_334:0001028
name: textural characteristic end force to max force ratio extrusion percentage
namespace: cassava_trait
def: "The ratio of the end force measured at 20mm divided by the maximum force recorded during the texture-extrusion profile of a piece of cassava root boiled for a set time, and pushed through a 5-blade grid. The shape of the piece is a half-cylinder, approx. 5.5 cm diameter and 6 cm long.\n\nDerived trait calculated as percentage \n(CO_334:0002075/CO_334:0002073) * 100" []
is_a: CO_334:0001000 ! Variables
relationship: variable_of CO_334:0002071 ! Textural characteristic
relationship: variable_of CO_334:0010525 ! Measurement: Textural characteristic
relationship: variable_of CO_334:0100583 ! pct (%)

[Term]
id: CO_334:0001029
name: farmer preference at harvest observation 1-5 scale
namespace: cassava_trait
def: "Farmers were given three(3) varieties each and they give their opinion on each, rank and as well score on an ordinal scale of 1-5.\nThe score represents the farmer perception of a good cassava root at harvest." []
is_a: CO_334:0001000 ! Variables
relationship: variable_of CO_334:0001027 ! farmer preference trait at harvest
relationship: variable_of CO_334:0012000 ! Observation: Farmer trait preference_method
relationship: variable_of CO_334:0100436 ! 5 point scales

[Term]
id: CO_334:0001030
name: farmer preference post harvest observation 1-5 scale
namespace: cassava_trait
def: "Farmers were given three(3) varieties each and they give their opinion on each, rank and as well score on an ordinal scale of 1-5.\nThe score represents the farmer perception of a good cassava root post harvest." []
is_a: CO_334:0001000 ! Variables
relationship: variable_of CO_334:0001025 ! farmer preference trait post-harvest
relationship: variable_of CO_334:0012000 ! Observation: Farmer trait preference_method
relationship: variable_of CO_334:0100436 ! 5 point scales

[Term]
id: CO_334:0001034
name: root length measurement in cm
namespace: cassava_trait
xref: CO:curators
is_a: CO_334:0001000 ! Variables
relationship: variable_of CO_334:0000450 ! Root length
relationship: variable_of CO_334:0012001 ! Measurement: total root length_method
relationship: variable_of CO_334:0100558 ! cm

[Term]
id: CO_334:0001035
name: storage root diameter in cm
namespace: cassava_trait
def: "Measured as the total root diameter with a pachymeter." [CO:curators]
is_a: CO_334:0001000 ! Variables
relationship: variable_of CO_334:0000487 ! Storage Root Diameter
relationship: variable_of CO_334:0012002 ! Measurement: total root diameter_method
relationship: variable_of CO_334:0100558 ! cm

[Term]
id: CO_334:0001037
name: post-harvest physiological deterioration variable 0-10 scale measured 8 months after planting.
namespace: cassava_trait
def: "Internal root discoloration or vascular streaking that renders cassava roots unfit for human or animal consumption.\nA number of root samples are cut into 7 slices  and each slice is scored on a 0-10 scale. 0 = No symptom of root discoloration, 1 = 10% of the root surface has root discoloration, 2 = 30% of the root surface has root discoloration, 3 = 30% of the root surface has root discoloration, 4 = 40% of the root surface has root discoloration, 5 = 50% of the root surface has root discoloration, 6 = 60% of the root surface has root discoloration, 7 = 70% of the root surface has root discoloration, 8 = 80% of the root surface has root discoloration, 9 = 90% of the root surface has root discoloration, 100 = 100% of the root surface has root discoloration. Measured 8 moths after planting." [CO:curators]
is_a: CO_334:0001000 ! Variables
is_a: CO_334:0001025 ! farmer preference trait post-harvest
relationship: variable_of CO_334:0000266 ! Post-harvest physiological deterioration
relationship: variable_of CO_334:0010001 ! Estimation: Post-harvest physiological deterioration method
relationship: variable_of CO_334:0100680 ! 11pt scale

[Term]
id: CO_334:0001038
name: 'post-harvest physiological deterioration variable 0-10 month 10'
namespace: cassava_trait
def: "Internal root discoloration or vascular streaking that renders cassava roots unfit for human or animal consumption.\nA number of root samples are cut into 7 slices  and each slice is scored on a 0-10 scale. 0 = No symptom of root discoloration, 1 = 10% of the root surface has root discoloration, 2 = 30% of the root surface has root discoloration, 3 = 30% of the root surface has root discoloration, 4 = 40% of the root surface has root discoloration, 5 = 50% of the root surface has root discoloration, 6 = 60% of the root surface has root discoloration, 7 = 70% of the root surface has root discoloration, 8 = 80% of the root surface has root discoloration, 9 = 90% of the root surface has root discoloration, 100 = 100% of the root surface has root discoloration. Measured 10 moths after planting." [CO:curators]
is_a: CO_334:0001000 ! Variables
is_a: CO_334:0001025 ! farmer preference trait post-harvest
relationship: variable_of CO_334:0000266 ! Post-harvest physiological deterioration
relationship: variable_of CO_334:0010001 ! Estimation: Post-harvest physiological deterioration method
relationship: variable_of CO_334:0100680 ! 11pt scale

[Term]
id: CO_334:0001039
name: post-harvest physiological deterioration variable 0-10 scale measured 11 months after planting.
namespace: cassava_trait
def: "Internal root discoloration or vascular streaking that renders cassava roots unfit for human or animal consumption.\nA number of root samples are cut into 7 slices  and each slice is scored on a 0-10 scale. 0 = No symptom of root discoloration, 1 = 10% of the root surface has root discoloration, 2 = 30% of the root surface has root discoloration, 3 = 30% of the root surface has root discoloration, 4 = 40% of the root surface has root discoloration, 5 = 50% of the root surface has root discoloration, 6 = 60% of the root surface has root discoloration, 7 = 70% of the root surface has root discoloration, 8 = 80% of the root surface has root discoloration, 9 = 90% of the root surface has root discoloration, 100 = 100% of the root surface has root discoloration. Measured 11 moths after planting." [CO:curators]
is_a: CO_334:0001000 ! Variables
is_a: CO_334:0001025 ! farmer preference trait post-harvest
relationship: variable_of CO_334:0000266 ! Post-harvest physiological deterioration
relationship: variable_of CO_334:0010001 ! Estimation: Post-harvest physiological deterioration method
relationship: variable_of CO_334:0100680 ! 11pt scale

[Term]
id: CO_334:0001041
name: Biochemical trait
namespace: cassava_trait
def: "traits for biochemical metabolites." [CO:curators]
is_a: CO_334:0000004 ! Quality trait

[Term]
id: CO_334:0001042
name: carotene content
namespace: cassava_trait
def: "carotene content." [CO:curators]
is_a: CO_334:0001041 ! Biochemical trait

[Term]
id: CO_334:0001043
name: Total carotenes HPLC ug/g
namespace: cassava_trait
def: "Total carotene content using HPLC. Fresh cassava roots are ground into a mash and carotenoids are extracted with acetone and petroleum ether. The extracts are analyzed by HPLC with mobile phases (methanol + ammonium acetate) followed by methy-ter-butyl-ether. The resulting peaks are identified and quantified using calibration standards and calibration curve. Total carotenes are evaluated by summing the peaks, and expressed in ug/g wet basis.." [CO:curators]
synonym: "CarTot HPLC" EXACT []
is_a: CO_334:0001000 ! Variables
relationship: variable_of CO_334:0001042 ! carotene content
relationship: variable_of CO_334:0001044 ! Estimation: total carotenes HPLC method
relationship: variable_of CO_334:0100572 ! ug/g

[Term]
id: CO_334:0001044
name: Estimation: total carotenes HPLC method
namespace: CassavaMethod
def: "Total carotene content using HPLC. Fresh cassava roots are ground into a mash and carotenoids are extracted with acetone and petroleum ether. The extracts are analyzed by HPLC with mobile phases (methanol + ammonium acetate) followed by methy-ter-butyl-ether. The resulting peaks are identified and quantified using calibration standards and calibration curve. Total carotenes are evaluated by summing the peaks, and expressed in ug/g wet basis." [CO:curators]
is_a: CO_334:0001002 ! Methods
relationship: method_of CO_334:0000291 ! Beta carotene

[Term]
id: CO_334:0001045
name: protein content percentage evaluated by NIRS 400-2500nm
namespace: cassava_trait
def: "The protein content of mashed fresh cassava roots evaluated by NIRS prediction (% wb). Measured using laboratory table-top Near InfraRed Spectrophotometry (NIRS). Output are spectrum with wavelength range of 400 to 2500, and are converted to concentration in percent (wet weight basis) using prediction model." [CO:curators]
synonym: "protei" EXACT []
synonym: "Protein NIRS (% wb)" EXACT []
is_a: CO_334:0001000 ! Variables
relationship: variable_of CO_334:0000442 ! Protein content
relationship: variable_of CO_334:0001046 ! Measurement: Protein content percentage NIRS 400-2500 nm
relationship: variable_of CO_334:0100583 ! pct (%)

[Term]
id: CO_334:0001046
name: Measurement: Protein content percentage NIRS 400-2500 nm
namespace: CassavaMethod
def: "measurement using laboratory table-top Near InfraRed Spectrophotometry (NIRS). Output are spectrum with wavelength range of 400 to 2500, and are converted to concentration in percent (wet weight basis) using prediction model." [CO:curators]
is_a: CO_334:0001002 ! Methods
relationship: method_of CO_334:0000442 ! Protein content

[Term]
id: CO_334:0001047
name: starch content percentage NIRS 400-2500nm
namespace: cassava_trait
def: "The starch content of mashed fresh cassava roots evaluated by NIRS prediction (% wb). Measured using laboratory table-top Near InfraRed Spectrophotometry (NIRS). Output are spectrum with wavelength range of 400 to 2500, and are converted to concentration in percent (wet weight basis) using prediction model." [CO:curators]
synonym: "Starch NIRS (% wb)" EXACT []
is_a: CO_334:0001000 ! Variables
relationship: variable_of CO_334:0000474 ! Starch Content
relationship: variable_of CO_334:0001048 ! Measurement: Starch content % NIRS 400-2500 nm
relationship: variable_of CO_334:0100583 ! pct (%)

[Term]
id: CO_334:0001048
name: Measurement: Starch content % NIRS 400-2500 nm
namespace: CassavaMethod
def: "The starch content of mashed fresh cassava roots evaluated by NIRS prediction (% wb) measured using laboratory table-top Near InfraRed Spectrophotometry (NIRS). Output are spectrum with wavelength range of 400 to 2500, and are converted to concentration in percent (wet weight basis) using prediction model." [CO:curators]
is_a: CO_334:0001002 ! Methods
relationship: method_of CO_334:0000474 ! Starch Content

[Term]
id: CO_334:0001049
name: The amylose content percetage NIRS 400-2500 nm
namespace: cassava_trait
def: "The amylose content of mashed fresh cassava roots evaluated by NIRS prediction (% wb). Measured using laboratory table-top Near InfraRed Spectrophotometry (NIRS). Output are spectrum with wavelength range of 400 to 2500, and are converted to concentration in percent (wet weight basis) using prediction model." [CO:curators]
synonym: "Amylose NIRS (% wb)" EXACT []
is_a: CO_334:0001000 ! Variables
relationship: variable_of CO_334:0000279 ! Amylose content
relationship: variable_of CO_334:0001050 ! Measurement: Amylose  content percetange NIRS 400-2500 nm
relationship: variable_of CO_334:0100572 ! ug/g

[Term]
id: CO_334:0001050
name: Measurement: Amylose  content percetange NIRS 400-2500 nm
namespace: CassavaMethod
def: "Measured amylose content of cassava roots using laboratory table-top Near InfraRed Spectrophotometry (NIRS). Output are spectrum with wavelength range of 400 to 2500, and are converted to concentration in percent (wet weight basis) using prediction model." [CO:curators]
is_a: CO_334:0001002 ! Methods
relationship: method_of CO_334:0000279 ! Amylose content

[Term]
id: CO_334:0001051
name: Total carotenes ug/g NIRS 400-2500 nm
namespace: cassava_trait
def: "The total carotene content of mashed fresh cassava roots evaluated by NIRS prediction (ug/g wb). Measured using laboratory table-top Near InfraRed Spectrophotometry (NIRS). Output are spectrum with wavelength range of 400 to 2500, and are converted to concentration in ppm (wet weight basis) using prediction model." [CO:curators]
synonym: "CarTot NIRS (ug/g wb)" EXACT []
is_a: CO_334:0001000 ! Variables
relationship: variable_of CO_334:0001042 ! carotene content
relationship: variable_of CO_334:0001052 ! Measurement: total carotenes NIRS 400-2500 nm method
relationship: variable_of CO_334:0100572 ! ug/g

[Term]
id: CO_334:0001052
name: Measurement: total carotenes NIRS 400-2500 nm method
namespace: CassavaMethod
def: "Total carotene content measured using laboratory table-top Near InfraRed Spectrophotometry (NIRS). Output are spectrum with wavelength range of 400 to 2500, and are converted to concentration in ppm (wet weight basis) using prediction model." [CO:curators]
is_a: CO_334:0001002 ! Methods
relationship: method_of CO_334:0000291 ! Beta carotene

[Term]
id: CO_334:0001053
name: beta carotene content ug/g NIRS 400-2500 nm
namespace: cassava_trait
def: "The beta-carotene content of mashed fresh cassava roots evaluated by NIRS prediction. Measured using laboratory table-top Near InfraRed Spectrophotometry (NIRS). Output are spectrum with wavelength range of 400-2500 nm." [CO:curators]
synonym: "bcret" EXACT []
synonym: "BetaCarotCt_HPLC_ugg" EXACT []
is_a: CO_334:0001000 ! Variables
relationship: variable_of CO_334:0000291 ! Beta carotene
relationship: variable_of CO_334:0001054 ! Measurement: Beta carotene NIRS method 400-2500 nm
relationship: variable_of CO_334:0100572 ! ug/g

[Term]
id: CO_334:0001054
name: Measurement: Beta carotene NIRS method 400-2500 nm
namespace: CassavaMethod
def: "Beta carotene content using laboratory table-top Near InfraRed Spectrophotometry (NIRS). Output are spectrum with wavelength range of 400-2500 nm." [CO:curators]
is_a: CO_334:0001002 ! Methods
relationship: method_of CO_334:0000291 ! Beta carotene

[Term]
id: CO_334:0001055
name: hydrogen cyanide ug/g wet basis
namespace: cassava_trait
def: "The cyanogenic potential of extracts from cassava roots (or other cassava-based products), evaluated by reaction with linamarase followed by colorimetric determination of cyanide concentration and expressed in ug/g of sample wet basis. \n\nSample is ground into a mash and cyanogenic compounds extracted using a buffer of orthophosphoric acid. The extracts are incubated with linamarase to release CN ions, which are quantified by spectrophotometry at 605 nm (in presence of chloramin T and isonicotinic/1,3 dimethyl-barbituric reagent)." [CO:curators]
synonym: "HCN linamarase (ug/g wb)" EXACT []
is_a: CO_334:0001000 ! Variables
relationship: variable_of CO_334:0000502 ! Storage root cyanide content
relationship: variable_of CO_334:0010334 ! Estimation: Hydrogen cyanide potential enzymatic method
relationship: variable_of CO_334:0100572 ! ug/g

[Term]
id: CO_334:0001064
name: Gari quality
namespace: cassava_trait
def: "The quality of gari depends on various factors ranging from the quality of cassava used to the processing techniques employed." []
synonym: "GarQt" EXACT []
is_a: CO_334:0000004 ! Quality trait

[Term]
id: CO_334:0001065
name: Bulk density of gari g cm−3
namespace: cassava_trait
def: "Bulk density refers to the mass of a substance divided by its volume when it is in a bulk or loose state is measured in grams per cubic meter." [CO:curators]
synonym: "BD(g/cm3)" EXACT []
is_a: CO_334:0001000 ! Variables
relationship: variable_of CO_334:0001064 ! Gari quality
relationship: variable_of CO_334:0001066 ! Calculation: Gari bulk density_method
relationship: variable_of CO_334:0001067 ! g/cm-3

[Term]
id: CO_334:0001066
name: Calculation: Gari bulk density_method
namespace: CassavaMethod
def: "Calculation of gari bulk density - mass divided by volume." [CO:curators]
is_a: CO_334:0001002 ! Methods
relationship: method_of CO_334:0001064 ! Gari quality

[Term]
id: CO_334:0001067
name: g/cm-3
namespace: CassavaScale
def: "grams per cubic centimeter" []
is_a: CO_334:0001001 ! Scales
relationship: scale_of CO_334:0001066 ! Calculation: Gari bulk density_method

[Term]
id: CO_334:0002001
name: number of plants with rotten roots counting
namespace: cassava_trait
def: "Number of plant stand harvested with rotten root" []
synonym: "pltrot" EXACT []
is_a: CO_334:0001000 ! Variables
relationship: variable_of CO_334:0000434 ! Plant stands harvested
relationship: variable_of CO_334:0010284 ! Counting: Plant stands harvested_method
relationship: variable_of CO_334:0100490 ! plant
created_by: aafolabi
creation_date: 2018-04-24T10:07:21Z

[Term]
id: CO_334:0002002
name: Peel thickness
namespace: cassava_trait
is_a: CO_334:0000001 ! Agronomic trait

[Term]
id: CO_334:0002003
name: In-ground storability
namespace: cassava_trait
is_a: CO_334:0000001 ! Agronomic trait

[Term]
id: CO_334:0002004
name: Early bulking
namespace: cassava_trait
is_a: CO_334:0000001 ! Agronomic trait

[Term]
id: CO_334:0002005
name: Weed tolerance
namespace: cassava_trait
is_a: CO_334:0000001 ! Agronomic trait

[Term]
id: CO_334:0002006
name: peel thickness measurement in cm
namespace: cassava_trait
def: "Thickness of cassava peel after peeling it off the cortex" []
synonym: "peeltk" EXACT []
is_a: CO_334:0001000 ! Variables
relationship: variable_of CO_334:0002002 ! Peel thickness
relationship: variable_of CO_334:0010472 ! Measurement: Peel thickness_method
relationship: variable_of CO_334:0100558 ! cm

[Term]
id: CO_334:0002007
name: in-ground storability visual rating 0-3
namespace: cassava_trait
def: "Duration of underground storage of cassava without signs of rot or deterioration" []
synonym: "Can stay in the farm for a long time" EXACT []
synonym: "Does not create urgent need for harvesting" EXACT []
synonym: "igstor" EXACT []
is_a: CO_334:0001000 ! Variables
is_a: CO_334:0001027 ! farmer preference trait at harvest
is_a: CO_334:0002010 ! Farmer trait
relationship: variable_of CO_334:0002003 ! In-ground storability
relationship: variable_of CO_334:0010473 ! Visual Rating: In-ground storability_method
relationship: variable_of CO_334:0100502 ! 4pt scale

[Term]
id: CO_334:0002008
name: early bulking visual rating 0-3
namespace: cassava_trait
def: "time taken for storage roots to begin to accumulate and store starch in the root" []
synonym: "bulkrt" EXACT []
synonym: "Matures quickly and rot if harvesting is delayed" EXACT []
is_a: CO_334:0001000 ! Variables
is_a: CO_334:0001027 ! farmer preference trait at harvest
is_a: CO_334:0002010 ! Farmer trait
relationship: variable_of CO_334:0002004 ! Early bulking
relationship: variable_of CO_334:0010474 ! Visual Rating: Early bulking_method
relationship: variable_of CO_334:0100502 ! 4pt scale

[Term]
id: CO_334:0002009
name: weed tolerance visual rating 0-3
namespace: cassava_trait
def: "Ability of cassava plant to withstand weed infestation without or with minimal negative effect on the growth performance and yield of the plant." []
synonym: "weedtl" EXACT []
is_a: CO_334:0001000 ! Variables
relationship: variable_of CO_334:0002005 ! Weed tolerance
relationship: variable_of CO_334:0010475 ! Visual Rating: Weed tolerance_method
relationship: variable_of CO_334:0100502 ! 4pt scale

[Term]
id: CO_334:0002010
name: Farmer trait
def: "Farmer's description of breeder's trait as used in Participatory Vaerietal Selection (PVS) study" []
is_a: CO_334:0000000 ! CGIAR cassava trait ontology

[Term]
id: CO_334:0002011
name: yield visual rating 1-3
namespace: cassava_trait
def: "Visual rating of how good the fresh root yield is. 1 = low 2= moderate 3 = high" []
synonym: "yldQ" EXACT []
xref: CO:curators
is_a: CO_334:0001000 ! Variables
relationship: variable_of CO_334:0000456 ! Root yield
relationship: variable_of CO_334:0010476 ! Visual Rating: Yield rating_method
relationship: variable_of CO_334:0100000 ! 3pt scale

[Term]
id: CO_334:0002012
name: dry matter visual rating 1-3
namespace: cassava_trait
def: "Visual rating of dry matter content of fresh cassava root. 1 = low, 2 = moderate, 3 = high." []
xref: CO:curators
is_a: CO_334:0001000 ! Variables
is_a: CO_334:0001027 ! farmer preference trait at harvest
relationship: variable_of CO_334:0000424 ! Root dry matter content
relationship: variable_of CO_334:0010477 ! Visual Rating: Dry matter rating_method
relationship: variable_of CO_334:0100000 ! 3pt scale

[Term]
id: CO_334:0002013
name: fufu initial weight in kg
namespace: cassava_trait
def: "Initial weight of cassava root in kilogram(kg), before processing into fufu." []
synonym: "fufuinwt" EXACT []
xref: CO:curators
is_a: CO_334:0001000 ! Variables
relationship: variable_of CO_334:0000373 ! Fufu content
relationship: variable_of CO_334:0010478 ! Measurement: Fufu initial weight_method
relationship: variable_of CO_334:0100493 ! kg

[Term]
id: CO_334:0002014
name: fufu peel weight in kg
namespace: cassava_trait
def: "Weight of root peels for processing fufu in kilogram (kg)." []
synonym: "fufuplwt" EXACT []
xref: CO:curators
is_a: CO_334:0001000 ! Variables
relationship: variable_of CO_334:0000373 ! Fufu content
relationship: variable_of CO_334:0010479 ! Measurement: Fufu peel weight_method
relationship: variable_of CO_334:0100493 ! kg

[Term]
id: CO_334:0002015
name: fufu peeled root weight in kg
namespace: cassava_trait
def: "Weight of peeled of cassava root in kilogram(kg) before processing into fufu." []
synonym: "fufuplrtwt" EXACT []
xref: CO:curator
is_a: CO_334:0001000 ! Variables
relationship: variable_of CO_334:0000373 ! Fufu content
relationship: variable_of CO_334:0010480 ! Measurement: Fufu peeled root weight_method
relationship: variable_of CO_334:0100493 ! kg

[Term]
id: CO_334:0002016
name: fufu fibre weight in g
namespace: cassava_trait
def: "Weight of oven dried fibre in kilogram(kg), after washing soaked root." []
synonym: "fufufibwt" EXACT []
xref: CO:curator
is_a: CO_334:0001000 ! Variables
relationship: variable_of CO_334:0000373 ! Fufu content
relationship: variable_of CO_334:0010481 ! Measurement: Fufu fibre weight_method
relationship: variable_of CO_334:0100623 ! g

[Term]
id: CO_334:0002017
name: fufu mash weight in kg
namespace: cassava_trait
def: "Weight of root in kilogram (kg) after grinding for processing fufu." []
synonym: "fufumshwt" EXACT []
xref: CO:curator
is_a: CO_334:0001000 ! Variables
relationship: variable_of CO_334:0000373 ! Fufu content
relationship: variable_of CO_334:0010482 ! Measurement: Fufu mash weight_method
relationship: variable_of CO_334:0100493 ! kg

[Term]
id: CO_334:0002018
name: fufu pressed weight in kg
namespace: cassava_trait
def: "Weight of pressed mash (grinded root) in kilogram (kg)." []
synonym: "fufuprwt" EXACT []
xref: CO:curator
is_a: CO_334:0001000 ! Variables
relationship: variable_of CO_334:0000373 ! Fufu content
relationship: variable_of CO_334:0010483 ! Measurement: Fufu pressed weight_method
relationship: variable_of CO_334:0100493 ! kg

[Term]
id: CO_334:0002019
name: fufu dry weight in kg
namespace: cassava_trait
def: "Weight of oven dried fufu in kilogram (kg)." []
synonym: "fufudrywt" EXACT []
xref: CO:curator
is_a: CO_334:0001000 ! Variables
relationship: variable_of CO_334:0000373 ! Fufu content
relationship: variable_of CO_334:0010484 ! Measurement: Fufu dry weight_method
relationship: variable_of CO_334:0100493 ! kg

[Term]
id: CO_334:0002020
name: gari initial weight in kg
namespace: cassava_trait
def: "Initial weight of root in kilogram (kg) before processing into gari." []
synonym: "garinwt" EXACT []
xref: CO:curator
is_a: CO_334:0001000 ! Variables
relationship: variable_of CO_334:0000374 ! Gari content
relationship: variable_of CO_334:0010485 ! Measurement: Gari initial weight_method
relationship: variable_of CO_334:0100493 ! kg

[Term]
id: CO_334:0002021
name: gari peel weight in kg
namespace: cassava_trait
def: "Weight of cassava peels in kilogram (kg) for before processing into gari" []
synonym: "gariplwt" EXACT []
xref: CO:curator
is_a: CO_334:0001000 ! Variables
relationship: variable_of CO_334:0000374 ! Gari content
relationship: variable_of CO_334:0010486 ! Measurement: Gari peel weight_method
relationship: variable_of CO_334:0100493 ! kg

[Term]
id: CO_334:0002022
name: gari peeled root weight in kg
namespace: cassava_trait
def: "Weight of peeled roots in kilogram for processing into gari." []
synonym: "gariplrtwt" EXACT []
xref: CO:curator
is_a: CO_334:0001000 ! Variables
relationship: variable_of CO_334:0000374 ! Gari content
relationship: variable_of CO_334:0010487 ! Measurement: Gari peeled root weight_method
relationship: variable_of CO_334:0100493 ! kg

[Term]
id: CO_334:0002023
name: gari mash weight in kg
namespace: cassava_trait
def: "Weight of root in kilogram (kg) after grinding for processing into gari" []
synonym: "dewatered_mash" RELATED []
synonym: "garimashwt" EXACT []
xref: CO:curator
is_a: CO_334:0001000 ! Variables
relationship: variable_of CO_334:0000374 ! Gari content
relationship: variable_of CO_334:0010488 ! Measurement: Gari mash weight_method
relationship: variable_of CO_334:0100493 ! kg

[Term]
id: CO_334:0002024
name: gari pressed weight in kg
namespace: cassava_trait
def: "Weight of pressed mash in kilogram (kg) for processing into gari." []
synonym: "gariprwt" EXACT []
xref: CO:curator
is_a: CO_334:0001000 ! Variables
relationship: variable_of CO_334:0000374 ! Gari content
relationship: variable_of CO_334:0010489 ! Measurement: Gari pressed weight_method
relationship: variable_of CO_334:0100493 ! kg

[Term]
id: CO_334:0002025
name: gari pulverised weight in kg
namespace: cassava_trait
def: "Weight of pulverized mash in kilogram (kg)" []
synonym: "gariplvwt" EXACT []
xref: CO:curator
is_a: CO_334:0001000 ! Variables
relationship: variable_of CO_334:0000374 ! Gari content
relationship: variable_of CO_334:0010490 ! Measurement: Gari pulverised weight_method
relationship: variable_of CO_334:0100493 ! kg

[Term]
id: CO_334:0002026
name: gari fried weight in kg
namespace: cassava_trait
def: "Weight of gari in kilogram (kg) after frying and sieving." []
synonym: "garifrwt" EXACT []
xref: CO:curator
is_a: CO_334:0001000 ! Variables
relationship: variable_of CO_334:0000374 ! Gari content
relationship: variable_of CO_334:0010491 ! Measurement: Gari fried weight_method
relationship: variable_of CO_334:0100493 ! kg

[Term]
id: CO_334:0002027
name: gari chaff coarse weight in g
namespace: cassava_trait
def: "Weight of shaft in gram using coarse sieve for gari." []
synonym: "garicoshfwt" EXACT []
xref: CO:curator
is_a: CO_334:0001000 ! Variables
relationship: variable_of CO_334:0000375 ! Gari chaff weight
relationship: variable_of CO_334:0010492 ! Measurement: Gari shaft weight coarse_method
relationship: variable_of CO_334:0100623 ! g

[Term]
id: CO_334:0002028
name: gari chaff medium weight in g
namespace: cassava_trait
def: "Weight of shaft in gram using medium sieve for gari." []
synonym: "garimdshfwt" EXACT []
xref: CO:curator
is_a: CO_334:0001000 ! Variables
relationship: variable_of CO_334:0000375 ! Gari chaff weight
relationship: variable_of CO_334:0010493 ! Measurement: Gari shaft weight medium_method
relationship: variable_of CO_334:0100623 ! g

[Term]
id: CO_334:0002029
name: Remote sensing trait
def: "Remote sensing related traits." []
xref: CO:curator
is_a: CO_334:0000000 ! CGIAR cassava trait ontology

[Term]
id: CO_334:0002030
name: Plot volume
namespace: cassava_trait
def: "Volume derived from probability distribution (Weibull)." []
xref: CO:curator
is_a: CO_334:0002029 ! Remote sensing trait

[Term]
id: CO_334:0002031
name: Plant height per plot
namespace: cassava_trait
def: "Plant height calculated from result of drone image analysis." []
xref: CO:curator
is_a: CO_334:0002029 ! Remote sensing trait

[Term]
id: CO_334:0002032
name: plot volume in m3
namespace: cassava_trait
def: "Volume of a plot measured in m3, using Weibull's continuous probability distribution for deriving the scale and shape parameters. It is calculated as the sum of all z-values (the height of every point in the point cloud) multiplied by 0.01 and 0.01 (every pixel is 1cm resolution)." []
synonym: "plotvol" EXACT []
xref: CO:curator
is_a: CO_334:0001000 ! Variables
relationship: variable_of CO_334:0002030 ! Plot volume
relationship: variable_of CO_334:0010516 ! Estimation: Plot volume_method
relationship: variable_of CO_334:0100681 ! m3

[Term]
id: CO_334:0002033
name: plant height per plot in m
namespace: cassava_trait
def: "Plant height calculated from the mean of the 5% highest point in a plot point cloud (top 95 percentile)." []
synonym: "plantht" RELATED []
xref: CO:curator
is_a: CO_334:0001000 ! Variables
relationship: variable_of CO_334:0002031 ! Plant height per plot
relationship: variable_of CO_334:0010303 ! Measurement: Plant height_method
relationship: variable_of CO_334:0100679 ! m

[Term]
id: CO_334:0002034
name: Weibull scale trait
namespace: cassava_trait
def: "Parameter of weibull function fitted to the pixel height density distribution of a plot." []
xref: CO:curator
is_a: CO_334:0002029 ! Remote sensing trait

[Term]
id: CO_334:0002035
name: Weibull shape trait
namespace: cassava_trait
def: "Parameter of Weibull function fitted to the pixel height density distribution of a plot." []
xref: CO:curator
is_a: CO_334:0002029 ! Remote sensing trait

[Term]
id: CO_334:0002036
name: weibull fit scale variable
namespace: cassava_trait
def: "Parameter of Weibull function fitted to the pixel height density distribution of a plot. Weibull fit is described as : y = b/a* (x/a)^b-1 * exp(-(x/a)^b)" []
synonym: "wscale" EXACT []
xref: Co:curator
is_a: CO_334:0001000 ! Variables
relationship: variable_of CO_334:0002034 ! Weibull scale trait
relationship: variable_of CO_334:0010496 ! Calculation: Weibull function

[Term]
id: CO_334:0002037
name: weibull fit shape variable
namespace: cassava_trait
def: "Parameter of Weibull function fitted to the pixel height density distribution of a plot. Weibull fit is described as : y = b/a * (x/a)^b-1 * exp(-(x/a)^b)" []
synonym: "wshape" EXACT []
xref: CO:curator
is_a: CO_334:0001000 ! Variables
relationship: variable_of CO_334:0002035 ! Weibull shape trait
relationship: variable_of CO_334:0010496 ! Calculation: Weibull function

[Term]
id: CO_334:0002038
name: canopy width in cm
namespace: cassava_trait
def: "Width of casava leaf canopy measure in centimeter (cm) using metric ruler" []
synonym: "canwidth" EXACT []
xref: CO:curators
is_a: CO_334:0001000 ! Variables
relationship: variable_of CO_334:0002039 ! Canopy width
relationship: variable_of CO_334:0010497 ! Measurement: Canopy width_method
relationship: variable_of CO_334:0100558 ! cm

[Term]
id: CO_334:0002039
name: Canopy width
namespace: cassava_trait
def: "Width of cassava leaf canopy" []
synonym: "canwidth" EXACT []
synonym: "canwidth_cm" RELATED []
is_a: CO_334:0000002 ! Morphological trait

[Term]
id: CO_334:0002040
name: Leaf dry matter content
namespace: cassava_trait
def: "Dry matter content of leaf" []
synonym: "lfdmc" EXACT []
xref: CO:curators
is_a: CO_334:0000447 ! Dry matter content

[Term]
id: CO_334:0002041
name: Cassava rust disease severity
namespace: cassava_trait
def: "Severity of symptom caused by Uromyces manihots in leaves" []
synonym: "crds" EXACT []
xref: CO:curators
is_a: CO_334:0000029 ! fungal disease

[Term]
id: CO_334:0002042
name: Cassava rust disease incidence
namespace: cassava_trait
def: "Proportion of plants in a plot with symptom of Uromyces manihots" []
synonym: "crdi" EXACT []
xref: CO:curators
is_a: CO_334:0000029 ! fungal disease

[Term]
id: CO_334:0002043
name: cassava rust disease severity evaluation
namespace: cassava_trait
def: "Visual rating of symptoms caused by Uromyces specie in cassava leaf. Symptom rated from 1 = clean, no infection, 2 = Up to 25% leaf area symptomatic, 3 = 25-50% leaf area symptomatic, 4 = 50-75% leaf area symptomatic, 5 = 75-100% leaf area symptomatic." []
synonym: "crds" EXACT []
xref: CO:curators
is_a: CO_334:0001000 ! Variables
is_a: CO_334:0001027 ! farmer preference trait at harvest
relationship: variable_of CO_334:0002041 ! Cassava rust disease severity
relationship: variable_of CO_334:0010500 ! Visual Observation: Cassava rust disease severity_method
relationship: variable_of CO_334:0100682 ! 5 pt scale

[Term]
id: CO_334:0002044
name: cassava rust disease incidence evaluation
namespace: cassava_trait
def: "Proportion of plant in a plot with symptom of Uromyces manihot symptom. It is scored as a ratio of symptomatic plants and the total number of plants in the plot." []
synonym: "crdi" EXACT []
xref: CO:curators
is_a: CO_334:0001000 ! Variables
relationship: variable_of CO_334:0002042 ! Cassava rust disease incidence
relationship: variable_of CO_334:0010499 ! Counting: Cassava rust disease incidence_method
relationship: variable_of CO_334:0100582 ! ratio

[Term]
id: CO_334:0002045
name: Biomass dry weight
namespace: cassava_trait
def: "Total plant mass (stem, leaves and petiole) above ground." []
synonym: "biodmc" EXACT []
xref: CO:curators
is_a: CO_334:0000447 ! Dry matter content

[Term]
id: CO_334:0002046
name: dry weight of biomass in kg
def: "Measurement of the dry weight of the total plant mass above ground in kilogram (kg), by drying in oven for ten (10) days at 50 deg celsius and weighted using scale." []
synonym: "biodmc" EXACT []
xref: CO:curators
is_a: CO_334:0001000 ! Variables
relationship: variable_of CO_334:0002045 ! Biomass dry weight
relationship: variable_of CO_334:0010498 ! Measurement: Dry weight of biomass_method
relationship: variable_of CO_334:0100493 ! kg

[Term]
id: CO_334:0002047
name: Leaf edibility
namespace: cassava_trait
def: "Palatability of cassava leaves likened to be eaten as fresh vegetable" []
synonym: "leafed" RELATED []
xref: CO:curators
is_a: CO_334:0000004 ! Quality trait

[Term]
id: CO_334:0002048
name: leaf edibility sensory assessment 0&1
namespace: cassava_trait
def: "Sensory assessment of how palatable of cassava leaf is, scored on a scale of 0 and 1 where 0 = non palatable and 1 = palatable" []
xref: CO:curators
is_a: CO_334:0001000 ! Variables
relationship: variable_of CO_334:0002047 ! Leaf edibility
relationship: variable_of CO_334:0010501 ! Sensory assessment: Leaf edibility_method
relationship: variable_of CO_334:0100539 ! 2pt scale

[Term]
id: CO_334:0002049
name: Cooking quality
namespace: cassava_trait
def: "Cooking characteristics of cassava root" []
synonym: "cookqty" RELATED []
xref: CO:curators
is_a: CO_334:0000004 ! Quality trait

[Term]
id: CO_334:0002050
name: cooking quality visual rating 0-2
namespace: cassava_trait
def: "Qualitative rating of cooking characteristics of cassava. The ability of cassava root to boil in less time, with good taste and texture scored on a scale of 0 to 2; with 0 = poor, 1 = fair and 2 = good." []
synonym: "cookqty" RELATED []
xref: CO:curators
is_a: CO_334:0001000 ! Variables
is_a: CO_334:0001025 ! farmer preference trait post-harvest
relationship: variable_of CO_334:0002049 ! Cooking quality

[Term]
id: CO_334:0002051
name: Fufu smell
namespace: cassava_trait
def: "Smell of fufu after processing" []
synonym: "fufu odour" EXACT []
synonym: "fufusm" RELATED []
synonym: "FuOd" EXACT []
xref: CO:curators
is_a: CO_334:0103021 ! Aroma trait

[Term]
id: CO_334:0002052
name: Attieke smell
namespace: cassava_trait
def: "Smell of attieke after processing" []
synonym: "attksm" RELATED []
is_a: CO_334:0000004 ! Quality trait

[Term]
id: CO_334:0002053
name: fufu smell perception by rating 0&1
namespace: cassava_trait
def: "Olfactory perception of the smell of fufu after processing often rated as odourless (0) and 1(when it has some smell/odour oozing out)" []
xref: CO:curators
is_a: CO_334:0001000 ! Variables
relationship: variable_of CO_334:0002051 ! Fufu smell
relationship: variable_of CO_334:0010505 ! Olfactory Perception: Fufu smell_method
relationship: variable_of CO_334:0100539 ! 2pt scale

[Term]
id: CO_334:0002054
name: cbsv quantification with RTPCR in cycle threshold
namespace: cassava_trait
def: "Characterization of CBSVs done using the Real time PCR based one step TaqMan method with primers and probes for CBSV.The unit of measurement is cycle threshold (ct)." []
is_a: CO_334:0001000 ! Variables
relationship: variable_of CO_334:0000036 ! Cassava brown streak disease leaf severity
relationship: variable_of CO_334:0010510 ! PCR assay: Cassava Brown Streak Virus_method
relationship: variable_of CO_334:0100690 ! c/t

[Term]
id: CO_334:0002055
name: ucbsv quantification with RTPCR in cycle threshold
namespace: cassava_trait
def: "Characterization of CBSVs done using the Real time PCR based on one step TaqMan method with primers and probes for uCBSV.The unit of measurement is cycle threshold (ct)." []
is_a: CO_334:0001000 ! Variables
relationship: variable_of CO_334:0000036 ! Cassava brown streak disease leaf severity
relationship: variable_of CO_334:0010511 ! PCR assay: Ugandan Cassava Brown Streak Virus_method
relationship: variable_of CO_334:0100690 ! c/t

[Term]
id: CO_334:0002056
name: dry matter content by SciO in percentage
namespace: cassava_trait
def: "Percentage dry matter content estimated using mini handheld Near InfraRed Spectroscopy (NIRS) device called SciO. Output are spectra with wavelength range of 700 to 1100 and are converted to percentage using prediction model." []
xref: CO:curators
is_a: CO_334:0001000 ! Variables
relationship: variable_of CO_334:0000424 ! Root dry matter content
relationship: variable_of CO_334:0010508 ! Prediction: Dry matter content by SciO_method
relationship: variable_of CO_334:0100583 ! pct (%)

[Term]
id: CO_334:0002057
name: dry matter content by table-top NIRS in percentage
namespace: cassava_trait
def: "Percentage dry matter content using laboratory table-top Near InfraRed Spectroscopy (NIRS). Output are spectrum with wavelength range of 850 to 2500nm, and are converted to percentage using prediction model." []
synonym: "dmNIRS" RELATED []
xref: CO:curators
is_a: CO_334:0001000 ! Variables
relationship: variable_of CO_334:0000424 ! Root dry matter content
relationship: variable_of CO_334:0010509 ! Prediction: Dry matter content by table-top NIRS_method
relationship: variable_of CO_334:0100583 ! pct (%)

[Term]
id: CO_334:0002058
name: dry matter content by QST in percentage
namespace: cassava_trait
def: "Percentage dry matter content estimated using handheld  Near InfraRed Spectroscopy (NIRS) device called \"Quality Spec Trek\". Output are spectra with wavelength range of 350-2500nm, and are converted percentage by prediction model." []
synonym: "dmqst" RELATED []
xref: CO:curators
is_a: CO_334:0001000 ! Variables
relationship: variable_of CO_334:0000424 ! Root dry matter content
relationship: variable_of CO_334:0010507 ! Prediction: Dry matter content by QST_method
relationship: variable_of CO_334:0100583 ! pct (%)

[Term]
id: CO_334:0002059
name: attieke smell perception by rating 0&1
namespace: cassava_trait
def: "Smell of attieke after processing by olfactory perception often rated as 0 (odourless) and 1 (have some kinds of smell)" []
xref: CO:curators
is_a: CO_334:0001000 ! Variables
relationship: variable_of CO_334:0002052 ! Attieke smell
relationship: variable_of CO_334:0010506 ! Olfactory Perception: Attieke smell_method
relationship: variable_of CO_334:0100539 ! 2pt scale

[Term]
id: CO_334:0002060
name: Fibrous root weight
namespace: cassava_trait
synonym: "firtwt" RELATED []
xref: CO:curators
is_a: CO_334:0000001 ! Agronomic trait

[Term]
id: CO_334:0002061
name: L chromometer
namespace: cassava_trait
def: "L scale from chromometer indicate light vs. dark where a low number (0-50) indicates dark and a high number (51-100) indicates light" []
synonym: "lval" EXACT []
xref: CO:curators
is_a: CO_334:0000004 ! Quality trait

[Term]
id: CO_334:0002062
name: B chromometer
namespace: cassava_trait
def: "b scale indicate yellow vs. blue where a positive number indicates yellow and a negative number indicates blue." []
synonym: "bval" EXACT []
xref: CO:curators
is_a: CO_334:0000004 ! Quality trait

[Term]
id: CO_334:0002063
name: A chromometer
namespace: cassava_trait
def: "a scale indicate red vs. green where a positive number indicates red and a negative number indicates green" []
xref: CO:curators
is_a: CO_334:0000004 ! Quality trait

[Term]
id: CO_334:0002064
name: B chromometer value of fresh root
namespace: cassava_trait
def: "b scale of plant root indicating red vs. green where a positive number indicates red and a negative number indicates green" []
synonym: "b*_fresh" EXACT []
xref: CO:curators
is_a: CO_334:0001000 ! Variables
relationship: variable_of CO_334:0002062 ! B chromometer
relationship: variable_of CO_334:0010522 ! Computation: Chromometer color values

[Term]
id: CO_334:0002065
name: L chromometer of fresh root
namespace: cassava_trait
def: "L scale of plant root from chromometer indicating light vs. dark where a low number (0-50) indicates dark and a high number (51-100) indicates light" []
synonym: "L*_fresh" EXACT []
xref: CO:curators
is_a: CO_334:0001000 ! Variables
relationship: variable_of CO_334:0002061 ! L chromometer
relationship: variable_of CO_334:0010522 ! Computation: Chromometer color values
created_by: Ekanem

[Term]
id: CO_334:0002066
name: A chromometer value of fresh root
namespace: cassava_trait
def: "a scale of plant root indicating red vs. green where a positive number indicates red and a negative number indicates green" []
synonym: "a*_fresh" EXACT []
xref: CO:curators
is_a: CO_334:0001000 ! Variables
relationship: variable_of CO_334:0002063 ! A chromometer
relationship: variable_of CO_334:0010522 ! Computation: Chromometer color values

[Term]
id: CO_334:0002067
name: Change in weight after boiling
namespace: cassava_trait
def: "Change in the weight of cassava root after boiling at specific time" []
is_a: CO_334:0000004 ! Quality trait

[Term]
id: CO_334:0002068
name: Change in weight after boiling computation percentage
namespace: cassava_trait
def: "The change in weight of pieces of cassava roots in boiling water computed in percentage. Usually the weight increases as roots absorb water during boiling." []
synonym: "water absorption" RELATED []
is_a: CO_334:0001000 ! Variables
relationship: variable_of CO_334:0002067 ! Change in weight after boiling
relationship: variable_of CO_334:0010523 ! Computation: Change in weight after boiling
relationship: variable_of CO_334:0100583 ! pct (%)

[Term]
id: CO_334:0002069
name: Time of boiling
namespace: cassava_trait
def: "Time required to boil root to become soft and acceptable for consumption" []
synonym: "boiltime" EXACT []
is_a: CO_334:0000004 ! Quality trait

[Term]
id: CO_334:0002070
name: time of boiling estimation minute
namespace: cassava_trait
def: "Time of boiling required for cassava roots to become soft and acceptable for consumption, as determined by probing the pieces of roots with a fork" []
is_a: CO_334:0001000 ! Variables
relationship: variable_of CO_334:0002069 ! Time of boiling
relationship: variable_of CO_334:0010524 ! Estimation: Time of boiling
relationship: variable_of CO_334:0100696 ! minute

[Term]
id: CO_334:0002071
name: Textural characteristic
namespace: cassava_trait
def: "Textural characteristics of boiled cassava root." []
synonym: "texture" RELATED []
is_a: CO_334:0000004 ! Quality trait

[Term]
id: CO_334:0002072
name: textural characteristic gradient extrusion g/mm
namespace: cassava_trait
def: "The Gradient, or initial slope, of the texture-extrusion profile of a piece of boiled cassava root and pushed through a 5-blade grid. The shape of the piece is a half-cylinder, approx. 5.5 cm diameter and 6 cm long." []
is_a: CO_334:0001000 ! Variables
relationship: variable_of CO_334:0002071 ! Textural characteristic
relationship: variable_of CO_334:0010525 ! Measurement: Textural characteristic
relationship: variable_of CO_334:0100698 ! g/mm

[Term]
id: CO_334:0002073
name: textural characteristic max force extrusion g
namespace: cassava_trait
def: "The Maximum force of the texture-extrusion profile of a piece of boiled cassava root  and pushed through a 5-blade grid. The shape of the piece is a half-cylinder, approx. 5.5 cm diameter and 6 cm long." []
is_a: CO_334:0001000 ! Variables
relationship: variable_of CO_334:0002071 ! Textural characteristic
relationship: variable_of CO_334:0010525 ! Measurement: Textural characteristic
relationship: variable_of CO_334:0100623 ! g

[Term]
id: CO_334:0002074
name: textural characteristic distance at max force extrusion mm
namespace: cassava_trait
def: "The Distance of compression, at which Maximum force is reached on the texture-extrusion profile of a piece of boiled cassava root and pushed through a 5-blade grid. The shape of the piece is a half-cylinder, approx. 5.5 cm diameter and 6 cm long." []
is_a: CO_334:0001000 ! Variables
relationship: variable_of CO_334:0002071 ! Textural characteristic
relationship: variable_of CO_334:0010525 ! Measurement: Textural characteristic
relationship: variable_of CO_334:0100697 ! mm

[Term]
id: CO_334:0002075
name: textural characteristic end force extrusion g
namespace: cassava_trait
def: "The force at the end of the texture-extrusion test, i.e. when travel distance is 20mm, for a piece of boiled cassava root and pushed through a 5-blade grid. The shape of the piece is a half-cylinder, approx. 5.5 cm diameter and 6 cm long." []
is_a: CO_334:0001000 ! Variables
relationship: variable_of CO_334:0002071 ! Textural characteristic
relationship: variable_of CO_334:0010525 ! Measurement: Textural characteristic
relationship: variable_of CO_334:0100623 ! g

[Term]
id: CO_334:0002076
name: textural characteristic area under curve extrusion gmm
namespace: cassava_trait
def: "The Area under the curve of the texture-extrusion profile of a piece of boiled cassava root and pushed through a 5-blade grid. The shape of the piece is a half-cylinder, approx. 5.5 cm diameter and 6 cm long." []
is_a: CO_334:0001000 ! Variables
relationship: variable_of CO_334:0002071 ! Textural characteristic
relationship: variable_of CO_334:0010525 ! Measurement: Textural characteristic
relationship: variable_of CO_334:0100699 ! gmm

[Term]
id: CO_334:0002077
name: textural characteristic linear distance extrusion mm
namespace: cassava_trait
def: "The Linear distance of the texture-extrusion profile of a piece of boiled cassava root and pushed through a 5-blade grid. The shape of the piece is a half-cylinder, approx. 5.5 cm diameter and 6 cm long." []
is_a: CO_334:0001000 ! Variables
relationship: variable_of CO_334:0002071 ! Textural characteristic
relationship: variable_of CO_334:0010525 ! Measurement: Textural characteristic
relationship: variable_of CO_334:0100697 ! mm

[Term]
id: CO_334:0002078
name: cassava brown streak disease root severity computation percentage
namespace: cassava_trait
def: "Internal root discoloration or vascular streaking that renders cassava roots unfit for human or animal consumption.The percentage of tissue visible in root cross sections that appears diseased, as determined by image analysis described in https://csce.ucmss.com/cr/books/2018/LFS/CSREA2018/IPC3638.pdf" []
synonym: "CBSDpct" EXACT []
synonym: "CBSDRtSev_Cmp_pct" RELATED []
is_a: CO_334:0001000 ! Variables
relationship: variable_of CO_334:0000090 ! Cassava brown streak disease root severity
relationship: variable_of CO_334:0010526 ! Computation: Cassava brown streak disease root severity in percentage_method
relationship: variable_of CO_334:0100583 ! pct (%)
created_by: CO:curators

[Term]
id: CO_334:0002079
name: root flesh color 50% inner ring visual rating 1-8
namespace: cassava_trait
def: "Assessment of the level of yellowness in 50% of the inner ring of the storage root pulp at the time of harvest. Measured on a scale of 1 to 8, where 1 = white, 2 = light cream, 3 = cream, 4 = light yellow, 5 = yellow, 6 = deep yellow, 7 = orange, 8 = pink" []
synonym: "rtfcol50i" EXACT []
xref: CO:curators
is_a: CO_334:0001000 ! Variables
relationship: variable_of CO_334:0000490 ! Storage Root Pulp Color
relationship: variable_of CO_334:0010527 ! Visual Rating: Root flesh color ring_method
relationship: variable_of CO_334:0100700 ! 8pt scale

[Term]
id: CO_334:0002080
name: root flesh color 25% center ring visual rating 1-8
namespace: cassava_trait
def: "Assessment of the level of yellowness in 25% of the center ring of the storage root pulp at the time of harvest. Measured on a scale of 1 to 8, where 1 = white, 2 = light cream, 3 = cream, 4 = light yellow, 5 = yellow, 6 = deep yellow, 7 = orange, 8 = pink" []
synonym: "rtfcol25c" EXACT []
xref: CO:curators
is_a: CO_334:0001000 ! Variables
relationship: variable_of CO_334:0000490 ! Storage Root Pulp Color
relationship: variable_of CO_334:0010527 ! Visual Rating: Root flesh color ring_method
relationship: variable_of CO_334:0100700 ! 8pt scale

[Term]
id: CO_334:0002081
name: root flesh color 25% outer ring visual rating 1-8
namespace: cassava_trait
def: "Assessment of the level of yellowness in 25% of the outer ring of the storage root pulp at the time of harvest. Measured on a scale of 1 to 8, where 1 = white, 2 = light cream, 3 = cream, 4 = light yellow, 5 = yellow, 6 = deep yellow, 7 = orange, 8 = pink" []
synonym: "rtfcol25o" EXACT []
xref: CO:curators
is_a: CO_334:0001000 ! Variables
relationship: variable_of CO_334:0000490 ! Storage Root Pulp Color
relationship: variable_of CO_334:0010527 ! Visual Rating: Root flesh color ring_method
relationship: variable_of CO_334:0100700 ! 8pt scale

[Term]
id: CO_334:0002082
name: branching angle in degrees
namespace: cassava_trait
def: "The angle between vertical plane and first primary branching in degrees." []
synonym: "brnangdg" RELATED []
xref: CO:curators
is_a: CO_334:0001000 ! Variables
relationship: variable_of CO_334:0000294 ! Branching Angle
relationship: variable_of CO_334:0010530 ! Visual Scoring :Branching Angle_degree_method
relationship: variable_of CO_334:0100702 ! degree

[Term]
id: CO_334:0002083
name: bemisia tabaci adult : visual 1-5
namespace: cassava_trait
def: "Visual rating of number of whitefly adults present in the buds 1 (=healthy plant), 2 (=presence of few adults), 3 (=presence of adults and eggs), 4 (=presence of adults, eggs and nymphs), 5( = presence of sooty mold)" []
synonym: "btadtvs" RELATED []
xref: CO:curators
is_a: CO_334:0001000 ! Variables
relationship: variable_of CO_334:0000410 ! Number of bemisia tabaci adult
relationship: variable_of CO_334:0010528 ! Visual Observation:Whitefly severity evaluation_method
relationship: variable_of CO_334:0100701 ! 5 pt scale

[Term]
id: CO_334:0002084
name: thrips severity : visual 1-5
namespace: cassava_trait
def: "Visual rating in buds 1 (=healthy bud), 2 (=Slight yellowish marks on the apical leaves), 3 (=Bud and adjacent leaves with slight deformations and yellow marks), 4 (=Intense deformation of apical leaves or maturation of the foliar area), 5( =Bud completely deformed or dead, no adjacent leaves and symptoms of broom witch apex apical death and dead lateral buds)" []
is_a: CO_334:0001000 ! Variables
relationship: variable_of CO_334:0002085 ! Cassava Franklinella williamsi severity
relationship: variable_of CO_334:0010529 ! Visual Observation: Thrips severity evaluation_method
relationship: variable_of CO_334:0100701 ! 5 pt scale

[Term]
id: CO_334:0002085
name: Cassava Franklinella williamsi severity
namespace: cassava_trait
def: "Franklinella williamsi" []
synonym: "thrips" RELATED []
is_a: CO_334:0000030 ! insect damage

[Term]
id: CO_334:0002086
name: starch content specific gravity EMBRAPA percentage
namespace: cassava_trait
def: "Percentage (%) of starch using calculation based on specific gravity estimated from sampled roots. 158.3 * specific gravity (CO_334:0000163) - 137.35" []
synonym: "starchspg" RELATED []
xref: CO:curators
is_a: CO_334:0001000 ! Variables
relationship: variable_of CO_334:0000474 ! Starch Content
relationship: variable_of CO_334:0010531 ! Calculation: Starch content_EMBRAPA_method
relationship: variable_of CO_334:0100583 ! pct (%)

[Term]
id: CO_334:0002087
name: starch content specific gravity NRCRI percentage
namespace: cassava_trait
def: "Percentage (%) of starch using calculation based on specific gravity estimated from sampled roots. 210.8 * specific gravity (CO_334:0000163) - 213.4" []
synonym: "starchsg" RELATED []
is_a: CO_334:0001000 ! Variables
relationship: variable_of CO_334:0000474 ! Starch Content
relationship: variable_of CO_334:0010532 ! Calculation: Starch content_NRCRI_method
relationship: variable_of CO_334:0100583 ! pct (%)

[Term]
id: CO_334:0002088
name: Moisture content of cassava flour
namespace: cassava_trait
def: "Moisture content of cassava flour." []
synonym: "moisture" RELATED []
is_a: CO_334:0002109 ! Viscosity trait

[Term]
id: CO_334:0002090
name: Setback
namespace: cassava_trait
def: "Final viscosity minus trough viscosity" []
synonym: "setbck" RELATED []
is_a: CO_334:0002109 ! Viscosity trait

[Term]
id: CO_334:0002092
name: Final viscosity
namespace: cassava_trait
def: "Viscosity at the end of the Rapid Visco Analyzer test" []
synonym: "fvisc" RELATED []
xref: CO:curators
is_a: CO_334:0002109 ! Viscosity trait

[Term]
id: CO_334:0002094
name: Breakdown
namespace: cassava_trait
def: "Breakdown equals peak viscosity minus trough viscosity" []
is_a: CO_334:0002109 ! Viscosity trait

[Term]
id: CO_334:0002096
name: Trough
namespace: cassava_trait
def: "The minimum viscosity after the peak" []
synonym: "hold" RELATED []
is_a: CO_334:0002109 ! Viscosity trait

[Term]
id: CO_334:0002098
name: Peak viscosity
namespace: cassava_trait
def: "Maximum viscosity during the heating or hold phase of the RVA test. It is the maximum hot paste viscosity" []
synonym: "peakvsc" RELATED []
is_a: CO_334:0002109 ! Viscosity trait

[Term]
id: CO_334:0002100
name: Pasting temperature
namespace: cassava_trait
def: "Temperature at which the viscosity trace first raises above the baseline during the initial heating phase." []
synonym: "pstemp" RELATED []
is_a: CO_334:0002109 ! Viscosity trait

[Term]
id: CO_334:0002102
name: moisture content of flour estimation in percentage
namespace: cassava_trait
def: "Amount of moisture retained in cassava flour after milling.Determined as the loss in weight of a flour sample after oven drying expressed as a proportion of the original weight prior to oven drying in percentage." []
xref: CO:curators
is_a: CO_334:0001000 ! Variables
relationship: variable_of CO_334:0002088 ! Moisture content of cassava flour
relationship: variable_of CO_334:0010533 ! Estimation: Moisture content_method
relationship: variable_of CO_334:0100583 ! pct (%)

[Term]
id: CO_334:0002103
name: setback calculation in pascal per seconds
namespace: cassava_trait
def: "Measured on cassava flour using the Rapid Visco Analyzer (RVA). Final viscosity minus trough viscosity." []
xref: CO:curators
is_a: CO_334:0001000 ! Variables
relationship: variable_of CO_334:0002090 ! Setback
relationship: variable_of CO_334:0010534 ! Calculation: Setback_method
relationship: variable_of CO_334:0100704 ! pascal per seconds

[Term]
id: CO_334:0002104
name: final viscosity estimation in pascal per seconds
namespace: cassava_trait
def: "Viscosity at the end of the RVA test. Measured using the Rapid Visco Analyzer (RVA) in pascal per second." []
xref: CO:curators
is_a: CO_334:0001000 ! Variables
relationship: variable_of CO_334:0002092 ! Final viscosity
relationship: variable_of CO_334:0010535 ! Estimation: Final viscosity_method
relationship: variable_of CO_334:0100704 ! pascal per seconds

[Term]
id: CO_334:0002105
name: breakdown calculation in pascal per seconds
namespace: cassava_trait
def: "Breakdown equals peak viscosity minus trough viscosity. Measured with the Rapid Visco Analyzer (RVA) in pascal per seconds" []
xref: CO:curators
is_a: CO_334:0001000 ! Variables
relationship: variable_of CO_334:0002094 ! Breakdown
relationship: variable_of CO_334:0010536 ! Calculation: Breakdown_method
relationship: variable_of CO_334:0100704 ! pascal per seconds

[Term]
id: CO_334:0002106
name: trough estimation in pascal per seconds
namespace: cassava_trait
def: "The minimum viscosity after the peak.Measured with the Rapid Visco Analyzer (RVA) in pascal per seconds. it is a measure of the holding strength of the flour" []
is_a: CO_334:0001000 ! Variables
relationship: variable_of CO_334:0002096 ! Trough
relationship: variable_of CO_334:0010537 ! Estimation: Trough_method
relationship: variable_of CO_334:0100704 ! pascal per seconds

[Term]
id: CO_334:0002107
name: peak viscosity measurement in degree celsius
namespace: cassava_trait
def: "Maximum viscosity during the heating or hold phase of the RVA test measured by the Rapid Visco Analyser (RVA) in degree celsius." []
xref: CO:curators
is_a: CO_334:0001000 ! Variables
relationship: variable_of CO_334:0002098 ! Peak viscosity
relationship: variable_of CO_334:0010538 ! Measurement: Peak viscosity_method
relationship: variable_of CO_334:0100704 ! pascal per seconds

[Term]
id: CO_334:0002108
name: pasting temperature measurement in degree celsius
namespace: cassava_trait
def: "Temperature at which the viscosity trace first raises above the baseline during the initial heating phase measured by the Rapid Visco Analyser (RVA) in degree celsius." []
is_a: CO_334:0001000 ! Variables
relationship: variable_of CO_334:0002100 ! Pasting temperature
relationship: variable_of CO_334:0010539 ! Measurement: Pasting temperature_method
relationship: variable_of CO_334:0100703 ! degree celsius

[Term]
id: CO_334:0002109
name: Viscosity trait
namespace: cassava_trait
is_a: CO_334:0000004 ! Quality trait

[Term]
id: CO_334:0002110
name: Cassava white leaf spot disease severity
namespace: cassava_trait
def: "Severity of white leaf spot caused by Passalora maninhotis" []
synonym: "cwlsds" RELATED []
xref: CO:curators
is_a: CO_334:0000029 ! fungal disease

[Term]
id: CO_334:0002111
name: Cassava white leaf spot disease incidence
namespace: cassava_trait
def: "Proportion of plants showing symptoms of disease casued by Passalora maninhotis." []
synonym: "cwlsdi" RELATED []
xref: CO:curators
is_a: CO_334:0000029 ! fungal disease

[Term]
id: CO_334:0002112
name: Cassava brown leaf spot disease severity
namespace: cassava_trait
def: "Severity of brown leaf spot disease caused by Passalora henningsii." []
synonym: "cblsds" RELATED []
xref: CO:curators
is_a: CO_334:0000029 ! fungal disease

[Term]
id: CO_334:0002113
name: Cassava brown leaf spot disease incidence
namespace: cassava_trait
def: "Proportion of symptom of brown leaf spot disease caused by Passalora henningsii." []
xref: CO:curators
is_a: CO_334:0000029 ! fungal disease

[Term]
id: CO_334:0002114
name: Cassava blight leaf spot disease severity
namespace: cassava_trait
def: "Severity of blight leaf spot disease caused by Passalora vicosae." []
synonym: "cbllsds" RELATED []
xref: CO:curators
is_a: CO_334:0000029 ! fungal disease

[Term]
id: CO_334:0002115
name: Cassava blight leaf spot disease incidence
namespace: cassava_trait
def: "Proportion of symptoms caused by blight spot disease." []
synonym: "cbllsdi" RELATED []
xref: CO:curators
is_a: CO_334:0000029 ! fungal disease

[Term]
id: CO_334:0002116
name: cassava white leaf spot disease severity by visual rating 1-5
namespace: cassava_trait
def: "Visual rating of symptoms in response to the white leaf spot disease caused by Passalora maninhotis. Symptoms rated from: 0 = clean, no infection, 1 = Few leaves affected from the lower third part of the plant, 2 = > 50% of affected leaves at the lower third of the plant, 3 = Affected leaves on the middle and upper third of the plant, 4 = low incidence distributed all over the plant, 5 = Middle incidence distributed all over the plant with yellowed leaves and/or defoliation of the lower third part of the plant, 6 = Plant fully defoliated." []
synonym: "cwlsds" RELATED []
is_a: CO_334:0001000 ! Variables
relationship: variable_of CO_334:0002110 ! Cassava white leaf spot disease severity
relationship: variable_of CO_334:0010543 ! Visual Observation: Cassava white leaf spot disease severity_method
relationship: variable_of CO_334:0100705 ! 5 pt scale

[Term]
id: CO_334:0002117
name: cassava white leaf spot disease incidence in proportion
namespace: cassava_trait
def: "Proportion of plant showing symptoms of white leaf spot disease." []
is_a: CO_334:0001000 ! Variables
relationship: variable_of CO_334:0002111 ! Cassava white leaf spot disease incidence
relationship: variable_of CO_334:0010542 ! Counting: Cassava white leaf spot disease incidence_method
relationship: variable_of CO_334:0100617 ! proportion

[Term]
id: CO_334:0002118
name: cassava brown leaf spot disease severity by visual rating 1-5
namespace: cassava_trait
def: "Visual rating of symptoms in response to the brown leaf spot disease caused by Passalora henningsii. Symptoms rated from: 0 = clean, no infection, 1 = Few leaves affected from the lower third part of the plant, 2 = Low incidence at the lower third part of the plant, 3 = middle incidence distributed at the lower and middle parts of the plant with yellowed leaves and/or defoliation, 4 = high incidence distributed all over the plant with yellowed leaves and/or defoliation, 5 = Plant fully defoliated." []
synonym: "cblsds" RELATED []
is_a: CO_334:0001000 ! Variables
relationship: variable_of CO_334:0002112 ! Cassava brown leaf spot disease severity
relationship: variable_of CO_334:0010544 ! Visual Observation: Cassava brown leaf spot disease severity_method
relationship: variable_of CO_334:0100705 ! 5 pt scale

[Term]
id: CO_334:0002119
name: cassava brown leaf spot disease incidence in proportion
namespace: cassava_trait
def: "Proportion of plants showing symptoms of brown leaf spot disease." []
synonym: "cblsdi" RELATED []
is_a: CO_334:0001000 ! Variables
relationship: variable_of CO_334:0002113 ! Cassava brown leaf spot disease incidence
relationship: variable_of CO_334:0010541 ! Counting: Cassava brown leaf spot disease incidence_method
relationship: variable_of CO_334:0100617 ! proportion

[Term]
id: CO_334:0002120
name: cassava blight leaf spot disease severity by visual rating 1-5
namespace: cassava_trait
def: "Visual rating of symptoms in response to the blight leaf spot disease caused by Passalora vicosae. Symptoms rated from: 0 = clean, no infection, 1 = Few leaves affected from the lower third part of the plant, 2 = Low incidence at the lower third part of the plant, 3 = middle incidence distributed at the lower and middle parts of the plant with yellowed leaves and/or defoliation, 4 = high incidence distributed all over the plant with yellowed leaves and/or defoliation, 5 = Plant fully defoliated." []
synonym: "cbllsds" RELATED []
is_a: CO_334:0001000 ! Variables
relationship: variable_of CO_334:0002114 ! Cassava blight leaf spot disease severity
relationship: variable_of CO_334:0010545 ! Visual Observation: Cassava blight leaf spot disease severity_method
relationship: variable_of CO_334:0100705 ! 5 pt scale

[Term]
id: CO_334:0002121
name: cassava blight leaf spot disease incidence in proportion
namespace: cassava_trait
def: "Proportion of plants showing symptoms of blight leaf spot disease." []
synonym: "cbllsdi" RELATED []
is_a: CO_334:0001000 ! Variables
relationship: variable_of CO_334:0002115 ! Cassava blight leaf spot disease incidence
relationship: variable_of CO_334:0010540 ! Counting: Cassava blight leaf spot disease incidence_method
relationship: variable_of CO_334:0100617 ! proportion

[Term]
id: CO_334:0002122
name: gari yield in percentage
namespace: cassava_trait
def: "Gari yield in percentage calculated as the ratio of Gari initial weight (CO_334:0002020) and Gari fried weight (CO_334:0002026) multiplied by 100." []
xref: CO:curators
is_a: CO_334:0001000 ! Variables
relationship: variable_of CO_334:0000374 ! Gari content
relationship: variable_of CO_334:0010546 ! Calculation: Gari yield_method
relationship: variable_of CO_334:0100617 ! proportion

[Term]
id: CO_334:0002123
name: fufu yield in percentage
namespace: cassava_trait
def: "Fufu yield in percentage calculated as the ratio of fufu dewatered mash weight(CO_334:0002017) and  fufu peeled root weight (CO_334:0002013) multiplied by 100." []
xref: CO:curators
is_a: CO_334:0001000 ! Variables
relationship: variable_of CO_334:0000373 ! Fufu content
relationship: variable_of CO_334:0010549 ! Calculation: Fufu yield in percentage
relationship: variable_of CO_334:0100617 ! proportion

[Term]
id: CO_334:0002124
name: Fufu chaff weight
namespace: cassava_trait
def: "Fufu chaff weight" []
xref: CO:curators
is_a: CO_334:0000004 ! Quality trait

[Term]
id: CO_334:0002125
name: fufu chaff weight in kg
namespace: cassava_trait
def: "Weight of fufu chaff in kilogram." []
xref: CO:curators
is_a: CO_334:0001000 ! Variables
relationship: variable_of CO_334:0002124 ! Fufu chaff weight
relationship: variable_of CO_334:0010547 ! Measurement: Fufu chaff weight_method
relationship: variable_of CO_334:0100493 ! kg

[Term]
id: CO_334:0002126
name: fufu chaff loss in percentage
namespace: cassava_trait
def: "Fufu chaff loss in percentage calculated as the ratio of dewatered fufu mash weight (CO_334:0002017)- fufu chaff weight (CO_334:0002125) and dewatered fufu mash weight (CO_334:0002017)." []
xref: CO:curators
is_a: CO_334:0001000 ! Variables
relationship: variable_of CO_334:0002124 ! Fufu chaff weight
relationship: variable_of CO_334:0002127 ! Fufu  chaff loss
relationship: variable_of CO_334:0100617 ! proportion

[Term]
id: CO_334:0002127
name: Fufu  chaff loss
namespace: cassava_trait
def: "Fufu chaff loss relative to dewatered mash weight" []
xref: CO:curators
is_a: CO_334:0000004 ! Quality trait

[Term]
id: CO_334:0002128
name: root number per plant counting
namespace: cassava_trait
def: "A count of the total number of storage roots (marketable and non-marketable) harvested per plant stand that makes up a plot." []
synonym: "plntrtno" EXACT []
is_a: CO_334:0001000 ! Variables
relationship: variable_of CO_334:0000452 ! Root number
relationship: variable_of CO_334:0010285 ! Counting: Root number_method
relationship: variable_of CO_334:0100491 ! root

[Term]
id: CO_334:0002129
name: cassava brown streak viral titre absorption in ng/ml
namespace: cassava_trait
def: "Viral titre is a new trait that we are exploring in understanding the genetics of Cassava brown streak disease. ELISA assays are used to generate absorbance readings that are converted titre with the aid of a standard curve. Standard curves tend to vary with how serial dilutions are made and to some extent may depend on the reagents used. In the end, a value in ng/ml unit is generated that represents viral titre which is always in the range of the standard curve concentration" []
synonym: "cbsvt" RELATED []
xref: CO:curators
is_a: CO_334:0001000 ! Variables
relationship: variable_of CO_334:0002130 ! Cassava brown streak viral titre
relationship: variable_of CO_334:0010550 ! Absorption: Cassava brown streak viral titre_method
relationship: variable_of CO_334:0100706 ! ng/ml

[Term]
id: CO_334:0002130
name: Cassava brown streak viral titre
namespace: cassava_trait
def: "Viral titre is a new trait that we are exploring in understanding the genetics of Cassava brown streak disease." []
synonym: "cbsvt" RELATED []
xref: CO:curators
is_a: CO_334:0000028 ! viral disease

[Term]
id: CO_334:0003000
name: Boiled cassava surface yellowness scale 0-10
namespace: cassava_trait
def: "When you receive a cassava root sample, observe the surface and evaluate the intensity of the yellow colour. ; 0=Non-yellow, 10=Bright yellow" []
is_a: CO_334:0001000 ! Variables
relationship: variable_of CO_334:0003020 ! boiled root surface yellowness
relationship: variable_of CO_334:0013000 ! surface yellowness appearance method
relationship: variable_of CO_334:0103000 ! Surface yellowness scale 0-10
created_by: Paula Iragaba

[Term]
id: CO_334:0003001
name: Boiled cassava surface whitness scale 0-10
namespace: cassava_trait
def: "When you receive a cassava root sample, observe the surface and evaluate the intensity of the yellow colour. ; 0=Cream, 10=Bright white" []
is_a: CO_334:0001000 ! Variables
relationship: variable_of CO_334:0003021 ! boiled root surface whiteness
relationship: variable_of CO_334:0013047 ! surface whiteness appearance method
relationship: variable_of CO_334:0103001 ! Boiled cassava surface whitness 0-10
created_by: Paula Iragaba

[Term]
id: CO_334:0003002
name: Boiled cassava surface colour homogeneity scale 0-10
namespace: cassava_trait
def: "When you receive a cassava root sample, observe the surface and evaluate the intensity of the yellow colour. ; 0= Heterogeneous, 10=Homogeneous" []
is_a: CO_334:0001000 ! Variables
relationship: variable_of CO_334:0003022 ! boiled root surface color homogeneity
relationship: variable_of CO_334:0013018 ! color homogeneity appearance method
relationship: variable_of CO_334:0103002 ! Surface colour homogeneity 0-10
created_by: Paula Iragaba

[Term]
id: CO_334:0003003
name: Boiled cassava  surface smoothness scale 0-10
namespace: cassava_trait
def: "When you receive a cassava root sample, observe the surface and evaluate the intensity of the yellow colour. ; 0=Very rough, 10=Very smooth" []
is_a: CO_334:0001000 ! Variables
relationship: variable_of CO_334:0003023 ! boiled root surface smoothnness
relationship: variable_of CO_334:0013046 ! surface smoothness appearance method
relationship: variable_of CO_334:0103003 ! Surface smoothness scale 0-10
created_by: Paula Iragaba

[Term]
id: CO_334:0003004
name: Boiled cassava in mouth hardness scale 0-10
namespace: cassava_trait
def: "Put a part of boiled sample in the mouth, chew it and evaluate: Amount of product adhering on/in the teeth after product mastication, and force required to remove product  completely  from the palate, using the tongue, after complete compression of the sample between  tongue and palate ; 0=Soft, 5=Firm, 10=Hard" []
is_a: CO_334:0001000 ! Variables
relationship: variable_of CO_334:0003024 ! boiled root hardness  in mouth
relationship: variable_of CO_334:0013001 ! stickiness texture in the mouth method
relationship: variable_of CO_334:0103004 ! Hardness texture in the mouth scale 0-10
created_by: Paula Iragaba

[Term]
id: CO_334:0003005
name: Boiled cassava in mouth moisture scale 0-10
namespace: cassava_trait
def: "Put a part of boiled sample in the mouth, chew it and evaluate: Amount of product adhering on/in the teeth after product mastication, and force required to remove product  completely  from the palate, using the tongue, after complete compression of the sample between  tongue and palate ; 0=Dry, 10=Moist" []
is_a: CO_334:0001000 ! Variables
relationship: variable_of CO_334:0003025 ! boiled root moisture  in mouth
relationship: variable_of CO_334:0013001 ! stickiness texture in the mouth method
relationship: variable_of CO_334:0103005 ! Moisture texture in the mouth s scale 0-10
created_by: Paula Iragaba

[Term]
id: CO_334:0003006
name: Boiled cassava in mouth smoothness scale 0-10
namespace: cassava_trait
def: "Put a part of boiled sample in the mouth, chew it and evaluate: Amount of product adhering on/in the teeth after product mastication, and force required to remove product  completely  from the palate, using the tongue, after complete compression of the sample between  tongue and palate ; 0=Lumpy, 5=Grainy, 10=Smooth" []
is_a: CO_334:0001000 ! Variables
relationship: variable_of CO_334:0003026 ! boiled root smoothness in mouth
relationship: variable_of CO_334:0013001 ! stickiness texture in the mouth method
relationship: variable_of CO_334:0103006 ! Boiled root smoothness in the mouth scale 0-10
created_by: Paula Iragaba

[Term]
id: CO_334:0003007
name: Boiled cassava in mouth fibrousness scale 0-10
namespace: cassava_trait
def: "Put a part of boiled sample in the mouth, chew it and evaluate: Amount of product adhering on/in the teeth after product mastication, and force required to remove product  completely  from the palate, using the tongue, after complete compression of the sample between  tongue and palate ; 0=Non fibrous, 5=Medium intensity, 10=Very fibrous" []
is_a: CO_334:0001000 ! Variables
relationship: variable_of CO_334:0003027 ! boiled root fibrousness in mouth
relationship: variable_of CO_334:0013001 ! stickiness texture in the mouth method
relationship: variable_of CO_334:0103007 ! Boiled root fibrousness in mouth scale 0-10
created_by: Paula Iragaba

[Term]
id: CO_334:0003008
name: Boiled cassava in mouth mealiness scale 0-10
namespace: cassava_trait
def: "Put a part of boiled sample in the mouth, chew it and evaluate: Amount of product adhering on/in the teeth after product mastication, and force required to remove product  completely  from the palate, using the tongue, after complete compression of the sample between  tongue and palate ; 0=Not mealy, 5=Medium mealiness, 10=Very mealy" []
is_a: CO_334:0001000 ! Variables
relationship: variable_of CO_334:0003028 ! boiled root mealiness  in mouth
relationship: variable_of CO_334:0013001 ! stickiness texture in the mouth method
relationship: variable_of CO_334:0103008 ! Mealiness texture in the mouth scale 0-10
created_by: Paula Iragaba

[Term]
id: CO_334:0003009
name: Boiled cassava in mouth stickness scale 0-10
namespace: cassava_trait
def: "Put a part of boiled sample in the mouth, chew it and evaluate: Amount of product adhering on/in the teeth after product mastication, and force required to remove product  completely  from the palate, using the tongue, after complete compression of the sample between  tongue and palate ; 0=Non sticky, 10=Sticky" []
is_a: CO_334:0001000 ! Variables
relationship: variable_of CO_334:0003029 ! boiled root stickness in mouth
relationship: variable_of CO_334:0013001 ! stickiness texture in the mouth method
relationship: variable_of CO_334:0103009 ! Stickness in the mouth scale 0-10
created_by: Paula Iragaba

[Term]
id: CO_334:0003010
name: Boiled cassava in hand mealiness scale 0-10
namespace: cassava_trait
def: "Put a part of the boiled sample between thumb and index fingers and using tapping motions, evaluate the amount of product adhering on them ; 0=Not mealy, 5=Medium mealiness, 10=Very mealy" []
is_a: CO_334:0001000 ! Variables
relationship: variable_of CO_334:0003030 ! boiled root mealiness by hand
relationship: variable_of CO_334:0013002 ! mealiness texture in the hand method
relationship: variable_of CO_334:0103010 ! Mealiness in the hand scale 0-10
created_by: Paula Iragaba

[Term]
id: CO_334:0003011
name: Boiled cassava in hand moldability scale 0-10
namespace: cassava_trait
def: "Put a part of the boiled sample between thumb and index fingers and using tapping motions, evaluate the amount of product adhering on them ; 0=Crumbly, 10=Moldable" []
is_a: CO_334:0001000 ! Variables
relationship: variable_of CO_334:0003031 ! boiled root moldability by hand
relationship: variable_of CO_334:0013008 ! moldability texture in the hand method
relationship: variable_of CO_334:0103011 ! Boiled root moldability by hand scale 0-10
created_by: Paula Iragaba

[Term]
id: CO_334:0003012
name: Boiled cassava in hand stickness scale 0-10
namespace: cassava_trait
def: "Put a part of the boiled sample between thumb and index fingers and using tapping motions, evaluate the amount of product adhering on them ; 0=Non sticky, 10=Sticky" []
is_a: CO_334:0001000 ! Variables
relationship: variable_of CO_334:0003032 ! boiled root stickness in the hand
relationship: variable_of CO_334:0013007 ! stickiness texture in the hand method
relationship: variable_of CO_334:0103012 ! Boiled root stickness in hand  scale 0-10
created_by: Paula Iragaba

[Term]
id: CO_334:0003013
name: Boiled cassava taste sweetness scale 0-10
namespace: cassava_trait
def: "Put a part of the boiled sample in the mouth and evaluate whether bitter after swallowing ; 0=No sweetness, 3=Low intensity, 6=Medium intensity" []
is_a: CO_334:0001000 ! Variables
relationship: variable_of CO_334:0003033 ! boiled root sweetness taste
relationship: variable_of CO_334:0013003 ! sweetness taste method
relationship: variable_of CO_334:0103013 ! Boiled root sweetness taste scale 0-10
created_by: Paula Iragaba

[Term]
id: CO_334:0003014
name: Boiled cassava taste bitterness scale 0-10
namespace: cassava_trait
def: "Put a part of the boiled sample in the mouth and evaluate whether bitter after swallowing ; 0=No bitterness, 3=Low intensity, 6=Medium intensity" []
is_a: CO_334:0001000 ! Variables
relationship: variable_of CO_334:0003034 ! boiled root taste bitterness
relationship: variable_of CO_334:0013014 ! bitterness taste method
relationship: variable_of CO_334:0103014 ! Bitterness scale 0-10
created_by: Paula Iragaba

[Term]
id: CO_334:0003015
name: Boiled cassava bitterness after taste 2 pt scale
namespace: cassava_trait
def: "Put a part of the boiled sample in the mouth and evaluate whether bitter after swallowing ; YES, NO" []
is_a: CO_334:0001000 ! Variables
relationship: variable_of CO_334:0003035 ! boiled root bitterness after taste
relationship: variable_of CO_334:0013013 ! bitterness after taste method
relationship: variable_of CO_334:0103015 ! 2 pt scale
created_by: Paula Iragaba

[Term]
id: CO_334:0003016
name: Boiled cassava aroma intensity scale 0-10
namespace: cassava_trait
def: "Put a part of the boiled sample and by retro-olfaction, evaluate the presence and the intensity of sweet potato aroma ; 0=Low intensity, 5= Medium intensity, 10= High intensity" []
is_a: CO_334:0001000 ! Variables
relationship: variable_of CO_334:0003036 ! boiled root steamed cassava-like aroma
relationship: variable_of CO_334:0013004 ! steamed cassava-like_aroma  method
relationship: variable_of CO_334:0103016 ! Cassava-like aroma scale 0-10
created_by: Paula Iragaba

[Term]
id: CO_334:0003017
name: Boiled cassava roasted cassava-like aroma 2 pt scale
namespace: cassava_trait
def: "Put a part of the boiled sample and by retro-olfaction, evaluate the presence and the intensity of sweet potato aroma ; YES, NO" []
is_a: CO_334:0001000 ! Variables
relationship: variable_of CO_334:0003037 ! boiled root roasted cassava-like aroma
relationship: variable_of CO_334:0013040 ! roasted cassava-like aroma method
relationship: variable_of CO_334:0103015 ! 2 pt scale
created_by: Paula Iragaba

[Term]
id: CO_334:0003018
name: Boiled cassava yam-like aroma 2 pt scale
namespace: cassava_trait
def: "Put a part of the boiled sample and by retro-olfaction, evaluate the presence and the intensity of sweet potato aroma ; YES, NO" []
is_a: CO_334:0001000 ! Variables
relationship: variable_of CO_334:0003038 ! boiled root yam-like aroma
relationship: variable_of CO_334:0013052 ! yam-like aroma method
relationship: variable_of CO_334:0103015 ! 2 pt scale
created_by: Paula Iragaba

[Term]
id: CO_334:0003019
name: Boiled cassava sweet potato-like aroma 2 pt scale
namespace: cassava_trait
def: "Put a part of the boiled sample and by retro-olfaction, evaluate the presence and the intensity of sweet potato aroma ; YES, NO" []
is_a: CO_334:0001000 ! Variables
relationship: variable_of CO_334:0003039 ! boiled root sweet potato-like aroma
relationship: variable_of CO_334:0013048 ! sweetpotato-like aroma method
relationship: variable_of CO_334:0103015 ! 2 pt scale
created_by: Paula Iragaba

[Term]
id: CO_334:0003020
name: boiled root surface yellowness
namespace: cassava_trait
def: "Colour of cassava root surface varies from light yellow to bright yellow" []
synonym: "BoiCasSurfYell" EXACT []
is_a: CO_334:0103017 ! Appearance trait

[Term]
id: CO_334:0003021
name: boiled root surface whiteness
namespace: cassava_trait
def: "Colour of cassava root surface varies from cream to bright white" []
synonym: "BoiCasSurfWhit" EXACT []
is_a: CO_334:0103017 ! Appearance trait

[Term]
id: CO_334:0003022
name: boiled root surface color homogeneity
namespace: cassava_trait
def: "Uniformity of cassava root surface colour" []
synonym: "BoiCasSurfColHom" EXACT []
is_a: CO_334:0103017 ! Appearance trait

[Term]
id: CO_334:0003023
name: boiled root surface smoothnness
namespace: cassava_trait
def: "Absence of roughness,  lumps, holes, fibre lines, and ridges along the cassava root" []
synonym: "BoiCasSurfSmooth" EXACT []
is_a: CO_334:0103017 ! Appearance trait

[Term]
id: CO_334:0003024
name: boiled root hardness  in mouth
namespace: cassava_trait
def: "Mechanical textural attribute relating to the force required to achieve a given deformation, penetration, or breakage of a product." []
synonym: "BoiCastMthRootHard" EXACT []
is_a: CO_334:0103018 ! Texture in mouth trait

[Term]
id: CO_334:0003025
name: boiled root moisture  in mouth
namespace: cassava_trait
def: "Perception of moisture content of food by the tactile receptors in the mouth, and also in relation to the lubricating properties of the product" []
synonym: "BoiCasMthRootMoist" EXACT []
is_a: CO_334:0103018 ! Texture in mouth trait

[Term]
id: CO_334:0003026
name: boiled root smoothness in mouth
namespace: cassava_trait
def: "Geometrical textural attribute relating to lack of presence of particles in a product" []
synonym: "BoiCasMthRootSmooth" EXACT []
is_a: CO_334:0103018 ! Texture in mouth trait

[Term]
id: CO_334:0003027
name: boiled root fibrousness in mouth
namespace: cassava_trait
def: "Feeling of threads/fibres as you chew" []
synonym: "BoiCasMthFibr" EXACT []
is_a: CO_334:0103018 ! Texture in mouth trait

[Term]
id: CO_334:0003028
name: boiled root mealiness  in mouth
namespace: cassava_trait
def: "Characterised by being dry and crumbly like boiled egg yolk" []
synonym: "BoiCasMthMeal" EXACT []
is_a: CO_334:0103018 ! Texture in mouth trait

[Term]
id: CO_334:0003029
name: boiled root stickness in mouth
namespace: cassava_trait
def: "Mechanical textural attribute relating to the force required to remove material that sticks to the mouth" []
synonym: "BoiCasMthStick" EXACT []
is_a: CO_334:0103018 ! Texture in mouth trait

[Term]
id: CO_334:0003030
name: boiled root mealiness by hand
namespace: cassava_trait
def: "Characterised by being dry and crumbly like boiled egg" []
synonym: "BoiCasHdMeal" EXACT []
is_a: CO_334:0103019 ! Texture in hand trait

[Term]
id: CO_334:0003031
name: boiled root moldability by hand
namespace: cassava_trait
def: "Mechanical textural attribute relating to the degree to which a substance can be deformed before it breaks" []
synonym: "BoiCasHdMold" EXACT []
is_a: CO_334:0103019 ! Texture in hand trait

[Term]
id: CO_334:0003032
name: boiled root stickness in the hand
namespace: cassava_trait
def: "Mechanical textural attribute relating to the force required to remove material that sticks to the finger" []
synonym: "boiCasHdStick" EXACT []
is_a: CO_334:0103019 ! Texture in hand trait

[Term]
id: CO_334:0003033
name: boiled root sweetness taste
namespace: cassava_trait
def: "Basic taste produced by dilute aqueous solutions of natural or artificial substances such as sucrose" []
synonym: "BoiCasTastSweet" EXACT []
is_a: CO_334:0103020 ! Taste trait

[Term]
id: CO_334:0003034
name: boiled root taste bitterness
namespace: cassava_trait
def: "Basic taste produced by produced by dilute aqueous solutions of natural or artificial substances such as quinine" []
synonym: "BoiCasTastBit" EXACT []
is_a: CO_334:0103020 ! Taste trait

[Term]
id: CO_334:0003035
name: boiled root bitterness after taste
namespace: cassava_trait
def: "Feeling of slight bitterness after swallow" []
synonym: "BoiCasTastBit" EXACT []
is_a: CO_334:0103020 ! Taste trait

[Term]
id: CO_334:0003036
name: boiled root steamed cassava-like aroma
namespace: cassava_trait
def: "Aroma of the steamed cassava" []
synonym: "BoiCasAromInt" EXACT []
is_a: CO_334:0103021 ! Aroma trait

[Term]
id: CO_334:0003037
name: boiled root roasted cassava-like aroma
namespace: cassava_trait
def: "Aroma like that of roasted cassava" []
synonym: "boiCasAromRoas" EXACT []
is_a: CO_334:0103021 ! Aroma trait

[Term]
id: CO_334:0003038
name: boiled root yam-like aroma
namespace: cassava_trait
def: "Aroma like that of yam, Possibly like aroma of boiled, roasted or fried yam" []
synonym: "BoiCasAromYam" EXACT []
is_a: CO_334:0103021 ! Aroma trait

[Term]
id: CO_334:0003039
name: boiled root sweet potato-like aroma
namespace: cassava_trait
def: "Aroma like tha of sweet potato, Possibly like aroma of boiled, roasted or fried sweet potato" []
synonym: "BoiCasAromSweetpotat" EXACT []
is_a: CO_334:0103021 ! Aroma trait

[Term]
id: CO_334:0003040
name: Fufu colour scale 1-8
namespace: cassava_trait
def: "Measures the intensity of the different colours of the cooked fufu surface on a scale 1 to 8" []
is_a: CO_334:0001000 ! Variables
relationship: variable_of CO_334:0003047 ! fufu surface colour
relationship: variable_of CO_334:0013005 ! surface colour sppearance method
relationship: variable_of CO_334:0103022 ! Surface colour appearance scale 1-8
created_by: Ugo Chijioke

[Term]
id: CO_334:0003041
name: Fufu smoothness scale 0-10
namespace: cassava_trait
def: "Measures the absence of lumps when a sample is pressed firmly between the fingers" []
is_a: CO_334:0001000 ! Variables
relationship: variable_of CO_334:0003048 ! fufu smoothness in hand
relationship: variable_of CO_334:0013006 ! smoothness texture in the hand method
relationship: variable_of CO_334:0103023 ! Smoothness in the hand scale 0-10
created_by: Ugo Chijioke

[Term]
id: CO_334:0003042
name: Fufu stickiness scale 0-10
namespace: cassava_trait
def: "Measures the adherence of fufu onto the fingers when it is touched with fingers or during moulding into bolus for swallowing" []
is_a: CO_334:0001000 ! Variables
relationship: variable_of CO_334:0003049 ! fufu stickiness in the hand
relationship: variable_of CO_334:0013007 ! stickiness texture in the hand method
relationship: variable_of CO_334:0103024 ! Fufu stickiness in hand scale 0-10
created_by: Ugo Chijioke

[Term]
id: CO_334:0003043
name: Fufu moldability scale 0-10
namespace: cassava_trait
def: "Meassures the easiness of fufu to stick together without disintegrating easiness to mould." []
is_a: CO_334:0001000 ! Variables
relationship: variable_of CO_334:0003050 ! fufu moldability in the hand
relationship: variable_of CO_334:0013008 ! moldability texture in the hand method
relationship: variable_of CO_334:0103025 ! Fufu moldability by hand scale 0-10
created_by: Ugo Chijioke

[Term]
id: CO_334:0003044
name: Fufu hardness scale 0-10
namespace: cassava_trait
def: "Measure the easiness of pressing a sample with the index finger" []
is_a: CO_334:0001000 ! Variables
relationship: variable_of CO_334:0003051 ! fufu hardness in hand
relationship: variable_of CO_334:0013009 ! hardness texture by hand method
relationship: variable_of CO_334:0103026 ! Fufu hardness by hand scale 0-10
created_by: Ugo Chijioke

[Term]
id: CO_334:0003045
name: Fufu stretchability scale 0-10
namespace: cassava_trait
def: "Measures the ability of fufu to stretch when pulled apart with the fingers" []
is_a: CO_334:0001000 ! Variables
relationship: variable_of CO_334:0003052 ! fufu stretchability in the hand
relationship: variable_of CO_334:0013010 ! stretchability texture by the hand method
relationship: variable_of CO_334:0103027 ! Fufu stretchability in hand scale 0-10
created_by: Ugo Chijioke

[Term]
id: CO_334:0003046
name: Fufu odour scale 0-10
namespace: cassava_trait
def: "Measures the odour fufu  smelt with nose when it is just cooked" []
is_a: CO_334:0001000 ! Variables
relationship: variable_of CO_334:0003053 ! fufu odour
relationship: variable_of CO_334:0013011 ! odour method
relationship: variable_of CO_334:0103028 ! Fufu odour scale 0-10
created_by: Ugo Chijioke

[Term]
id: CO_334:0003047
name: fufu surface colour
namespace: cassava_trait
def: "Colour of cooked fufu being as white as a flip chart paper or as as off white as soy milk colour, or as grey as skin of sardine fish, or as light as cement colour, or as cream coloured as peak evaporated liquid milk, or as light yellow as cooked egg york, or as yellow as skin of ripe orange, or as brown in colour as whole wheat meal" []
synonym: "FufSurfCol" EXACT []
is_a: CO_334:0103017 ! Appearance trait

[Term]
id: CO_334:0003048
name: fufu smoothness in hand
namespace: cassava_trait
def: "Absence of lumps" []
synonym: "FufHdSmoth" EXACT []
is_a: CO_334:0103019 ! Texture in hand trait

[Term]
id: CO_334:0003049
name: fufu stickiness in the hand
namespace: cassava_trait
def: "This is when the fufu sticks or adhere to the fingers when it is touched with fingers or during moulding into bolus for swallowing" []
synonym: "FufHdStick" EXACT []
is_a: CO_334:0103019 ! Texture in hand trait

[Term]
id: CO_334:0003050
name: fufu moldability in the hand
namespace: cassava_trait
def: "Ability of the fufu to stick together easily without disintegrating or cohesive and being easy to mould." []
synonym: "FufHdMol" EXACT []
is_a: CO_334:0103019 ! Texture in hand trait

[Term]
id: CO_334:0003051
name: fufu hardness in hand
namespace: cassava_trait
def: "Softness is when it is quite easy to compress the fufu sample, while hardness is when force is used to compress the sample or takes effort to compress the sample" []
synonym: "FufHdHard" EXACT []
is_a: CO_334:0103019 ! Texture in hand trait

[Term]
id: CO_334:0003052
name: fufu stretchability in the hand
namespace: cassava_trait
def: "Ability of fufu to stretch when pulled apart with fingers" []
synonym: "FufHdStret" EXACT []
is_a: CO_334:0103019 ! Texture in hand trait

[Term]
id: CO_334:0003053
name: fufu odour
namespace: cassava_trait
def: "Odour/aroma of fufu" []
synonym: "FuOd" EXACT []
is_a: CO_334:0103021 ! Aroma trait

[Term]
id: CO_334:0003054
name: Attieke cohesiveness scale 0-10
namespace: cassava_trait
def: "Measures the cohesion between granules (ability of grains to stick together or retake initial form after force of pressure)  scale 0-10. 0=Uncooked gari	; 10=Attoukpou (Ivorian cassava dish)" []
is_a: CO_334:0001000 ! Variables
relationship: variable_of CO_334:0003102 ! attieke cohesiveness
relationship: variable_of CO_334:0013017 ! cohesiveness texture by touch method
relationship: variable_of CO_334:0103030 ! Attieke cohesiveness scale 0-10
created_by: Ebah Catherine

[Term]
id: CO_334:0003055
name: Attieke sourness scale 0-10
namespace: cassava_trait
def: "Measures the sourrness of the sample (gustatory complex sensation, generally due to presence of organic acids),   scale 0-10. 0=Absence	; 10=High intensity" []
is_a: CO_334:0001000 ! Variables
relationship: variable_of CO_334:0003103 ! attieke sourness in the mouth
relationship: variable_of CO_334:0013043 ! sourness taste method
relationship: variable_of CO_334:0103031 ! Attieke sourness in the mouth scale 0-10
created_by: Ebah Catherine

[Term]
id: CO_334:0003056
name: Attieke stickness scale 0-10
namespace: cassava_trait
def: "Measures the ability of grains to stick in the palm after the granules are pressed in the hand,   scale 0-10. 0=Non sticky	; 10=chewing gum" []
is_a: CO_334:0001000 ! Variables
relationship: variable_of CO_334:0003104 ! attieke stickness in the hand
relationship: variable_of CO_334:0013007 ! stickiness texture in the hand method
relationship: variable_of CO_334:0103032 ! Attieke Stickness in hand scale 0-10
created_by: Ebah Catherine

[Term]
id: CO_334:0003057
name: Attieke sweetness scale 0-10
namespace: cassava_trait
def: "Measures the degree or intensity of the sweet taste or after-taste (basic taste produced by dilute aqueous solutions of natural or artificial substances such as sucrose).   scale 0-10. 0=Yace cassava variety	; 10=Bonoua cassava variety" []
is_a: CO_334:0001000 ! Variables
relationship: variable_of CO_334:0003105 ! attieke sweetness taste
relationship: variable_of CO_334:0013003 ! sweetness taste method
relationship: variable_of CO_334:0103033 ! Attieke Sweetness taste scale 0-10
created_by: Ebah Catherine

[Term]
id: CO_334:0003058
name: Attieke brightness scale 0-10
namespace: cassava_trait
def: "Measures the brighter or somber  scale 0-10. 0=Dark	; 10=Clear" []
is_a: CO_334:0001000 ! Variables
relationship: variable_of CO_334:0003106 ! attieke brightness
relationship: variable_of CO_334:0013016 ! brightness appearance method
relationship: variable_of CO_334:0103039 ! Brightness appearance scale 0-10
created_by: Ebah Catherine

[Term]
id: CO_334:0003059
name: Attieke colour scale 0-10
namespace: cassava_trait
def: "Measures the color of grains from light yellow to orange,   scale 0-10. 0=White	; 5=Yellow" []
is_a: CO_334:0001000 ! Variables
relationship: variable_of CO_334:0003107 ! attieke orange colour
relationship: variable_of CO_334:0013035 ! orange colour appearance method
relationship: variable_of CO_334:0103065 ! Orange colour scale 0-10
created_by: Ebah Catherine

[Term]
id: CO_334:0003060
name: Attieke extraneous matters appearance scale 0-10
namespace: cassava_trait
def: "Measures the presence of extraneous matters (other than cassava)   scale 0-10. 0=Absence	; 10=High intensity" []
is_a: CO_334:0001000 ! Variables
relationship: variable_of CO_334:0003108 ! attieke extraneous matters
relationship: variable_of CO_334:0013021 ! extraneous matters appearance method
relationship: variable_of CO_334:0103051 ! Extraneous matters appearance scale 0-10
created_by: Ebah Catherine

[Term]
id: CO_334:0003061
name: Attieke extraneous matters texture scale 0-10
namespace: cassava_trait
def: "Measures the sensation of extraneous matters during mastication   scale 0-10. 0=Absence	; 10=High intensity" []
is_a: CO_334:0001000 ! Variables
relationship: variable_of CO_334:0003108 ! attieke extraneous matters
relationship: variable_of CO_334:0013022 ! extraneous matters texture in mouth method
relationship: variable_of CO_334:0103052 ! Extraneous matters in mouth scale 0-10
created_by: Ebah Catherine

[Term]
id: CO_334:0003062
name: Attieke fermented taste scale 0-10
namespace: cassava_trait
def: "Measures the intensity of the fermented taste   scale 0-10. 0=Gari	; 10=Mangnan (the traditional starter of attieke)" []
is_a: CO_334:0001000 ! Variables
relationship: variable_of CO_334:0003109 ! attieke fermented taste
relationship: variable_of CO_334:0013023 ! fermented taste method
relationship: variable_of CO_334:0103053 ! Fermented taste scale 0-10
created_by: Ebah Catherine

[Term]
id: CO_334:0003063
name: Attieke firmness scale 0-10
namespace: cassava_trait
def: "Measures the expression de softness or hardness of the Attieke grains.   scale 0-10. 0=Soft cheese (Laughing cow)	; 5=Pitted olives" []
is_a: CO_334:0001000 ! Variables
relationship: variable_of CO_334:0003110 ! attieke firmness
relationship: variable_of CO_334:0013026 ! firmness texture by touch method
relationship: variable_of CO_334:0103054 ! Firmness scale 0-10
created_by: Ebah Catherine

[Term]
id: CO_334:0003064
name: Attieke grain size scale 0-10
namespace: cassava_trait
def: "Measures the size or diameter of grains   scale 0-10. 0=Powdered sugar	; 10=Couscous" []
is_a: CO_334:0001000 ! Variables
relationship: variable_of CO_334:0003111 ! attieke grain size
relationship: variable_of CO_334:0013041 ! size of grains appearance method
relationship: variable_of CO_334:0103055 ! Grain size scale 0-10
created_by: Ebah Catherine

[Term]
id: CO_334:0003065
name: Attieke granularity scale 0-10
namespace: cassava_trait
def: "Measures the perception of the size, shape, and amount of grains (particles) in the sample.   scale 0-10. 0=Milk powder	; 5=medium size grain couscous" []
is_a: CO_334:0001000 ! Variables
relationship: variable_of CO_334:0003112 ! attieke granularity
relationship: variable_of CO_334:0013027 ! granularity texture in the mouth method
relationship: variable_of CO_334:0103056 ! Granularity in mouth scale 0-10
created_by: Ebah Catherine

[Term]
id: CO_334:0003066
name: Attieke homogenity of grains scale 0-10
namespace: cassava_trait
def: "Measures the degree of uniformity of the size of grains   scale 0-10. 0=Broken corn grains	; 10=Fish Eggs" []
is_a: CO_334:0001000 ! Variables
relationship: variable_of CO_334:0003113 ! attieke homogenity of grains
relationship: variable_of CO_334:0013030 ! homogenity of grains appearance method
relationship: variable_of CO_334:0103060 ! Homogenity of grains scale 0-10
created_by: Ebah Catherine

[Term]
id: CO_334:0003067
name: Attieke masticability scale 0-10
namespace: cassava_trait
def: "Measures the force required to a given deformation, penetration or to reduce to sample to a swallowable form, (being easily chewable)   scale 0-10. 0=mush (Coco baca)	; 10=uncooked gari" []
is_a: CO_334:0001000 ! Variables
relationship: variable_of CO_334:0003114 ! attieke masticability
relationship: variable_of CO_334:0013031 ! masticability texture in mouth method
relationship: variable_of CO_334:0103061 ! Masticability scale 0-10
created_by: Ebah Catherine

[Term]
id: CO_334:0003068
name: Attieke moldability scale 0-10
namespace: cassava_trait
def: "Measures the ability to form a ball  scale 0-10. 0=uncooked semolina 	; 10=Moldable paste" []
is_a: CO_334:0001000 ! Variables
relationship: variable_of CO_334:0003115 ! attieke moldability in the hand
relationship: variable_of CO_334:0013032 ! moldability texture in touch method
relationship: variable_of CO_334:0103062 ! Moldability in the hand  scale 0-10
created_by: Ebah Catherine

[Term]
id: CO_334:0003069
name: Attieke mouth filled sensations scale 0-10
namespace: cassava_trait
def: "Measures the sensation that grains fill the mouth ,   scale 0-10. 0=Compacted	; 10=Dispersed" []
is_a: CO_334:0001000 ! Variables
relationship: variable_of CO_334:0003116 ! attieke mouth filled sensations
relationship: variable_of CO_334:0013033 ! mouth filled sensations texture in mouth method
relationship: variable_of CO_334:0103063 ! Mouth filled sensations scale 0-10
created_by: Ebah Catherine

[Term]
id: CO_334:0003070
name: Attieke off-odours scale 0-10
namespace: cassava_trait
def: "Measures the undesired or atypical odor associated with transformation or deterioration of the product. (Smoke, molds, over fermented, etc),   scale 0-10. 0=Absence	; 10=High intensity" []
is_a: CO_334:0001000 ! Variables
relationship: variable_of CO_334:0003117 ! attieke off-odours
relationship: variable_of CO_334:0013034 ! off-odours aroma method
relationship: variable_of CO_334:0103064 ! Off-odours scale 0-10
created_by: Ebah Catherine

[Term]
id: CO_334:0003071
name: Attieke presence of fibers scale 0-10
namespace: cassava_trait
def: "Measures the quantity of fibers   scale 0-10. 0=Couscous	; 10=Gari" []
is_a: CO_334:0001000 ! Variables
relationship: variable_of CO_334:0003118 ! attieke presence of fibers
relationship: variable_of CO_334:0013036 ! presence of fibers appearance method
relationship: variable_of CO_334:0103066 ! Presence of fibers scale 0-10
created_by: Ebah Catherine

[Term]
id: CO_334:0003072
name: Attieke presence of lumps scale 0-10
namespace: cassava_trait
def: "Measures the presence of aggregates,   scale 0-10. 0=Absence	; 10=High intensity" []
is_a: CO_334:0001000 ! Variables
relationship: variable_of CO_334:0003119 ! attieke presence of lumps
relationship: variable_of CO_334:0013037 ! presence of lumps appearance method
relationship: variable_of CO_334:0103068 ! Presence of lumps scale 0-10
created_by: Ebah Catherine

[Term]
id: CO_334:0003073
name: Attieke red palm oil aroma scale 0-10
namespace: cassava_trait
def: "Measures the characteristic odor of red palm oil,   scale 0-10. 0=Non present	; 10=Red palm oil odor" []
is_a: CO_334:0001000 ! Variables
relationship: variable_of CO_334:0003120 ! attieke red palm oil aroma
relationship: variable_of CO_334:0013039 ! red palm oil aroma method
relationship: variable_of CO_334:0103070 ! Red palm oil aroma scale 0-10
created_by: Ebah Catherine

[Term]
id: CO_334:0003074
name: Attieke sourness aroma scale 0-10
namespace: cassava_trait
def: "Measures the odor of sourness,   scale 0-10. 0=Absence	; 10=High intensity (pure vinegar)" []
is_a: CO_334:0001000 ! Variables
relationship: variable_of CO_334:0003121 ! attieke sourness aroma
relationship: variable_of CO_334:0013042 ! sourness aroma method
relationship: variable_of CO_334:0103071 ! Sourness aroma scale 0-10
created_by: Ebah Catherine

[Term]
id: CO_334:0003075
name: Attieke taste of red palm oil scale 0-10
namespace: cassava_trait
def: "Measures the presence and Intensity of the taste of Red Palm oil ,   scale 0-10. 0=No red palm oil	; 10=Red palm oil" []
is_a: CO_334:0001000 ! Variables
relationship: variable_of CO_334:0003122 ! attieke taste of red palm oil
relationship: variable_of CO_334:0013049 ! taste of red palm oil taste method
relationship: variable_of CO_334:0103074 ! Taste of red palm oil scale 0-10
created_by: Ebah Catherine

[Term]
id: CO_334:0003076
name: Attieke undesired taste scale 0-10
namespace: cassava_trait
def: "Measures any undesired taste in the sample (smoke, over-fermented, etc.).,  scale 0-10. 0=Absence	; 10=High intensity" []
is_a: CO_334:0001000 ! Variables
relationship: variable_of CO_334:0003123 ! attieke undesired taste
relationship: variable_of CO_334:0013050 ! undesired taste taste method
relationship: variable_of CO_334:0103075 ! Undesired taste scale 0-10
created_by: Ebah Catherine

[Term]
id: CO_334:0003077
name: Boiled cassava bitter aftertaste scale 0-100
namespace: cassava_trait
def: "Measures bitter taste after swallowing, eg there is a light bitter aftertaste,  scale 0-10. 0=Absent	; 100=Present" []
is_a: CO_334:0001000 ! Variables
relationship: variable_of CO_334:0003035 ! boiled root bitterness after taste
relationship: variable_of CO_334:0013013 ! bitterness after taste method
relationship: variable_of CO_334:0103034 ! Bitter aftertaste scale 0-100
created_by: Laurent Adinsi

[Term]
id: CO_334:0003078
name: Boiled cassava bitterness scale 0-100
namespace: cassava_trait
def: "Measures bitter taste after swallowing, eg there is a light bitter aftertaste,  scale 0-10. 0=Absent; 100=Present" []
is_a: CO_334:0001000 ! Variables
relationship: variable_of CO_334:0003034 ! boiled root taste bitterness
relationship: variable_of CO_334:0013014 ! bitterness taste method
relationship: variable_of CO_334:0103035 ! Bitterness scale 0-100
created_by: Laurent Adinsi

[Term]
id: CO_334:0003079
name: Boiled cassava stickness scale 0-100
namespace: cassava_trait
def: "Measures the property related to the adhesion of the product between the fingers, scale 0-100. 0=No sticky	; 100=Sticky" []
is_a: CO_334:0001000 ! Variables
relationship: variable_of CO_334:0003032 ! boiled root stickness in the hand
relationship: variable_of CO_334:0013007 ! stickiness texture in the hand method
relationship: variable_of CO_334:0103037 ! boiled root stickness in hand scale 0-100
created_by: Laurent Adinsi

[Term]
id: CO_334:0003080
name: Boiled cassava sweetness scale 0-100
namespace: cassava_trait
def: "Measures the basic light sugary taste like a little glucose or sucrose in water solution, scale 0-100. 0=Neutral/Absent	; 100=Sweet" []
is_a: CO_334:0001000 ! Variables
relationship: variable_of CO_334:0003033 ! boiled root sweetness taste
relationship: variable_of CO_334:0013003 ! sweetness taste method
relationship: variable_of CO_334:0103038 ! Boiled root sweetness taste scale 0-100
created_by: Laurent Adinsi

[Term]
id: CO_334:0003081
name: Boiled cassava cassava odour scale 0-100
namespace: cassava_trait
def: "Measures odour of boiled cassava. Scale 0-100. 0=Low; 100=High" []
is_a: CO_334:0001000 ! Variables
relationship: variable_of CO_334:0003124 ! boiled root cassava odour
relationship: variable_of CO_334:0013015 ! boiled cassava odour method
relationship: variable_of CO_334:0103036 ! boiled root odour scale 0-100
created_by: Laurent Adinsi

[Term]
id: CO_334:0003082
name: Boiled cassava crumbness scale 0-100
namespace: cassava_trait
def: "Measures the property of the product to crumble between the fingers. Scale 0-100. 0=No crumbly	100=Crumbly" []
is_a: CO_334:0001000 ! Variables
relationship: variable_of CO_334:0003125 ! boiled root crumbness
relationship: variable_of CO_334:0013019 ! crumbly in the hand method
relationship: variable_of CO_334:0103040 ! Crumbness in the hand scale 0-100
created_by: Laurent Adinsi

[Term]
id: CO_334:0003083
name: Boiled cassava easy to chew scale 0-100
namespace: cassava_trait
def: "Measures the property related to the number of chews necessary to swallow the product.  Scale 0-100" []
is_a: CO_334:0001000 ! Variables
relationship: variable_of CO_334:0003126 ! boiled root easiness to chew
relationship: variable_of CO_334:0013020 ! easy to chew texture in the mouth method
relationship: variable_of CO_334:0103041 ! Easy to chew scale 0-100
created_by: Laurent Adinsi

[Term]
id: CO_334:0003084
name: Boiled cassava granulariness scale 0-100
namespace: cassava_trait
def: "Measures the presence of small grains during chewing.  Scale 0-100. 0=Difficult; 100=Easy" []
is_a: CO_334:0001000 ! Variables
relationship: variable_of CO_334:0003127 ! boiled root granulariness
relationship: variable_of CO_334:0013028 ! granularity texture in the mouth method
relationship: variable_of CO_334:0103057 ! Granularity in mouth scale 0-100
created_by: Laurent Adinsi

[Term]
id: CO_334:0003085
name: Boiled cassava hardness to break scale 0-100
namespace: cassava_trait
def: "Measures the force required to cut/break with hand.  Scale 0-100. 0=No granular;	100=Granular" []
is_a: CO_334:0001000 ! Variables
relationship: variable_of CO_334:0003128 ! boiled root hardness to break
relationship: variable_of CO_334:0013029 ! hardness to break/cut texture in the hand method
relationship: variable_of CO_334:0103059 ! Hardness to break in the hand scale 0-100
created_by: Laurent Adinsi

[Term]
id: CO_334:0003086
name: Boiled cassava presence of fibers scale 0-100
namespace: cassava_trait
def: "Measures the presence of fine fibers visible to the eye.  Scale 0-100. 0=Ease to cut; 	100=Difficult to cut" []
is_a: CO_334:0001000 ! Variables
relationship: variable_of CO_334:0003129 ! boiled root presence of fibers
relationship: variable_of CO_334:0013024 ! fibrouness texture appearance  method
relationship: variable_of CO_334:0103067 ! Presence of fibers texture scale 0-100
created_by: Laurent Adinsi

[Term]
id: CO_334:0003087
name: Boiled cassava presence of strips scale 0-100
namespace: cassava_trait
def: "Measures the presence of the  stripe on the surface of product.  Scale 0-100. 0=Absent; 	100=Present" []
is_a: CO_334:0001000 ! Variables
relationship: variable_of CO_334:0003130 ! boiled root presence of stripe
relationship: variable_of CO_334:0013038 ! presence of stripes appearance method
relationship: variable_of CO_334:0103069 ! Presence of strips appearance scale 0-100
created_by: Laurent Adinsi

[Term]
id: CO_334:0003088
name: Boiled cassava yellow colour scale 0-100
namespace: cassava_trait
def: "Measures yellowish to Yellow colour of product" []
is_a: CO_334:0001000 ! Variables
relationship: variable_of CO_334:0003020 ! boiled root surface yellowness
relationship: variable_of CO_334:0013000 ! surface yellowness appearance method
relationship: variable_of CO_334:0103073 ! Surface yellow ness appearance scale 0-100
created_by: Laurent Adinsi

[Term]
id: CO_334:0003089
name: Boiled cassava white colour scale 0-100
namespace: cassava_trait
def: "Measures both inner and outer colour that can range from light off-white to white (pure white).  Scale 0-100. 0=Off-white; 	100=Pure White" []
is_a: CO_334:0001000 ! Variables
relationship: variable_of CO_334:0003131 ! boiled root white colour
relationship: variable_of CO_334:0013051 ! white color appearance method
relationship: variable_of CO_334:0103076 ! White colour scale 0-100
created_by: Laurent Adinsi

[Term]
id: CO_334:0003090
name: Eba creamness scale 0-10
namespace: cassava_trait
def: "Measures the intensity of surface creamness. Scale 0to10. 0=Cream	; 5=Light cream	; 10=Dark cream" []
is_a: CO_334:0001000 ! Variables
relationship: variable_of CO_334:0003132 ! eba surface creamness
relationship: variable_of CO_334:0013044 ! surface creamness appearance method
relationship: variable_of CO_334:0103072 ! surface creamness scale 0-10
created_by: Busie Maziya-Dixon

[Term]
id: CO_334:0003091
name: Eba cohesiveness scale 0-10
namespace: cassava_trait
def: "Measures easiness to make a ball with from a sizeable piece of sample using all fingers, Scale 0to10. 0=Not mouldable	; 5=Slightly mouldable	; 10=Mouldable" []
is_a: CO_334:0001000 ! Variables
relationship: variable_of CO_334:0003133 ! eba cohessiveness/moldability
relationship: variable_of CO_334:0013017 ! cohesiveness texture by touch method
relationship: variable_of CO_334:0103042 ! Eba cohesiveness in the hand  scale 0-10
created_by: Busie Maziya-Dixon

[Term]
id: CO_334:0003092
name: Eba hardness scale 0-10
namespace: cassava_trait
def: "Measures the amount of force required to press a sample placed between fingers. Scale 0to10.  0=Soft	; 5=Slightly soft; 10=Very hard" []
is_a: CO_334:0001000 ! Variables
relationship: variable_of CO_334:0003134 ! eba hardness in hand
relationship: variable_of CO_334:0013009 ! hardness texture by hand method
relationship: variable_of CO_334:0103044 ! Eba hardness in the hand scale 0-10
created_by: Busie Maziya-Dixon

[Term]
id: CO_334:0003093
name: Eba smoothness scale 0-10
namespace: cassava_trait
def: "Measures the amount of string like particles present on sample by feeling sample between tongue and palate after chewing. Scale 0to10. 0=Fine	; 5=Moderately course	; 10=Coarse" []
is_a: CO_334:0001000 ! Variables
relationship: variable_of CO_334:0003135 ! eba smoothness in mouth
relationship: variable_of CO_334:0013053 ! smoothness texture in the mouth method
relationship: variable_of CO_334:0103045 ! Eba smoothness in the mouth scale 0-10
created_by: Busie Maziya-Dixon

[Term]
id: CO_334:0003094
name: Eba stickiness scale 0-10
namespace: cassava_trait
def: "Measures the amount of product adhering on thumb and index fingers when a sample is placed between them. Scale 0to10. 0=Not sticky	; 5=Slightly sticky	; 10=Very sticky" []
is_a: CO_334:0001000 ! Variables
relationship: variable_of CO_334:0003136 ! eba stickiness kin the hand
relationship: variable_of CO_334:0013007 ! stickiness texture in the hand method
relationship: variable_of CO_334:0103047 ! Eba stickiness in hand scale 0-10
created_by: Busie Maziya-Dixon

[Term]
id: CO_334:0003095
name: Eba streachability scale 0-10
namespace: cassava_trait
def: "Measures the ability of sample to stretch when flattened with palms. Scale 0to10. 0=Not streachable	; 5=Slightly streachable	; 10=Very streachable" []
is_a: CO_334:0001000 ! Variables
relationship: variable_of CO_334:0003137 ! eba stretchability in the hand
relationship: variable_of CO_334:0013010 ! stretchability texture by the hand method
relationship: variable_of CO_334:0103048 ! Eba streachability in hand scale 0-10
created_by: Busie Maziya-Dixon

[Term]
id: CO_334:0003096
name: Eba surface whiteness scale 0-10
namespace: cassava_trait
def: "Measures the intensity of surface white colour. Scale 0to10. 0=White	10-Off white" []
is_a: CO_334:0001000 ! Variables
relationship: variable_of CO_334:0003138 ! eba surface whiteness
relationship: variable_of CO_334:0013047 ! surface whiteness appearance method
relationship: variable_of CO_334:0103049 ! Eba surface whiteness scale 0-10
created_by: Busie Maziya-Dixon

[Term]
id: CO_334:0003097
name: Eba sourness scale 0-10
namespace: cassava_trait
def: "Measures the intensity of the sourness. Scale 0to10. 0=Slightly sour	; 5=Sour	; 10=Very sour" []
is_a: CO_334:0001000 ! Variables
relationship: variable_of CO_334:0003139 ! eba sourness in the mouth
relationship: variable_of CO_334:0013043 ! sourness taste method
relationship: variable_of CO_334:0103046 ! Eba sourness taste scale 0-10
created_by: Busie Maziya-Dixon

[Term]
id: CO_334:0003098
name: Eba sweetness scale 0-10
namespace: cassava_trait
def: "Measures the intensity of sweetness. Scale 0to10. 0=Slightly sweet	; 5=Sweet	; 10=Very sweet" []
is_a: CO_334:0001000 ! Variables
relationship: variable_of CO_334:0003140 ! eba sweetness taste
relationship: variable_of CO_334:0013003 ! sweetness taste method
relationship: variable_of CO_334:0103050 ! Eba sweetness taste scale 0-10
created_by: Busie Maziya-Dixon

[Term]
id: CO_334:0003099
name: Eba fibrousness scale 0-10
namespace: cassava_trait
def: "Measures the amount of string like particles present on sample when felt between tongue and palate. Scale 0to10. 0=Low fibre	; 5=Moderate fibre	; 10=High fibre" []
is_a: CO_334:0001000 ! Variables
relationship: variable_of CO_334:0003141 ! eba fibrousness in mouth
relationship: variable_of CO_334:0013025 ! fibrousness texture in the mouth method
relationship: variable_of CO_334:0103043 ! Eba fibrousness in mouth scale 0-10
created_by: Busie Maziya-Dixon

[Term]
id: CO_334:0003100
name: Eba greyness scale 0-10
namespace: cassava_trait
def: "Measures the intensity of surface grey colour. Scale 0to10. 0=Cream	; 5=Light cream	; 10=Dark cream" []
is_a: CO_334:0001000 ! Variables
relationship: variable_of CO_334:0003142 ! eba surface greyness
relationship: variable_of CO_334:0013045 ! surface greyness appearance method
relationship: variable_of CO_334:0103058 ! Greyness scale 0-10
created_by: Busie Maziya-Dixon

[Term]
id: CO_334:0003101
name: attieke attieke-like  aroma
namespace: cassava_trait
def: "Aroma of attieke" []
synonym: "AttArom" EXACT []
is_a: CO_334:0103021 ! Aroma trait

[Term]
id: CO_334:0003102
name: attieke cohesiveness
namespace: cassava_trait
def: "Cohesion between granules (ability of grains to stick together or retake initial form after force of pressure)" []
synonym: "AttCoh" EXACT []
is_a: CO_334:0103019 ! Texture in hand trait

[Term]
id: CO_334:0003103
name: attieke sourness in the mouth
namespace: cassava_trait
def: "Sourrness of the sample (gustatory complex sensation, generally due to presence of organic acids)" []
synonym: "AttSourn" EXACT []
is_a: CO_334:0103020 ! Taste trait

[Term]
id: CO_334:0003104
name: attieke stickness in the hand
namespace: cassava_trait
def: "Ability of grains to stick in the palm after the granules are pressed in the hand" []
synonym: "AttStickn" EXACT []
is_a: CO_334:0103019 ! Texture in hand trait

[Term]
id: CO_334:0003105
name: attieke sweetness taste
namespace: cassava_trait
def: "Basic taste produced by dilute aqueous solutions of natural or artificial substances such as sucrose" []
synonym: "AttTastSweet" EXACT []
is_a: CO_334:0103020 ! Taste trait

[Term]
id: CO_334:0003106
name: attieke brightness
namespace: cassava_trait
def: "Brighter or somber" []
synonym: "AttBrigh" EXACT []
is_a: CO_334:0103017 ! Appearance trait

[Term]
id: CO_334:0003107
name: attieke orange colour
namespace: cassava_trait
def: "Color of grains from light yellow to orange" []
synonym: "AttOrCol" EXACT []
is_a: CO_334:0103017 ! Appearance trait

[Term]
id: CO_334:0003108
name: attieke extraneous matters
namespace: cassava_trait
def: "Sensation of extraneous matters during mastication" []
synonym: "AttExtrMat" EXACT []
is_a: CO_334:0103017 ! Appearance trait
is_a: CO_334:0103018 ! Texture in mouth trait

[Term]
id: CO_334:0003109
name: attieke fermented taste
namespace: cassava_trait
def: "Intensity of the fermented taste" []
synonym: "AttFermTast" EXACT []
is_a: CO_334:0103020 ! Taste trait

[Term]
id: CO_334:0003110
name: attieke firmness
namespace: cassava_trait
def: "Expression de la douceur ou de la dureté des grains d'attiéké" []
synonym: "AttFirm" EXACT []
is_a: CO_334:0103019 ! Texture in hand trait

[Term]
id: CO_334:0003111
name: attieke grain size
namespace: cassava_trait
def: "Size or diameter of grains" []
synonym: "AttGrSiz" EXACT []
is_a: CO_334:0103017 ! Appearance trait

[Term]
id: CO_334:0003112
name: attieke granularity
namespace: cassava_trait
def: "Perception of the size, shape, and amount of grains (particles) in the sample." []
synonym: "AttGran" EXACT []
is_a: CO_334:0103018 ! Texture in mouth trait

[Term]
id: CO_334:0003113
name: attieke homogenity of grains
namespace: cassava_trait
def: "Degree of uniformity of the size of grains" []
synonym: "AttHomGr" EXACT []
is_a: CO_334:0103017 ! Appearance trait

[Term]
id: CO_334:0003114
name: attieke masticability
namespace: cassava_trait
def: "Force required to a given deformation, penetration or to reduce to sample to a swallowable form, (being easily chewable)" []
synonym: "AttMast" EXACT []
is_a: CO_334:0103018 ! Texture in mouth trait

[Term]
id: CO_334:0003115
name: attieke moldability in the hand
namespace: cassava_trait
def: "Ability to form a ball" []
synonym: "AttMold" EXACT []
is_a: CO_334:0103019 ! Texture in hand trait

[Term]
id: CO_334:0003116
name: attieke mouth filled sensations
namespace: cassava_trait
def: "Sensation that grains fill the mouth" []
synonym: "AttMouFilSens" EXACT []
is_a: CO_334:0103018 ! Texture in mouth trait

[Term]
id: CO_334:0003117
name: attieke off-odours
namespace: cassava_trait
def: "Undesired or atypical odor associated with transformation or deterioration of the product. (Smoke, molds, over fermented, etc)" []
synonym: "AttOffOdo" EXACT []
is_a: CO_334:0103021 ! Aroma trait

[Term]
id: CO_334:0003118
name: attieke presence of fibers
namespace: cassava_trait
def: "Quantity of fibers" []
synonym: "AttPrFibr" EXACT []
is_a: CO_334:0103017 ! Appearance trait

[Term]
id: CO_334:0003119
name: attieke presence of lumps
namespace: cassava_trait
def: "Presence of aggregates" []
synonym: "AttPrLum" EXACT []
is_a: CO_334:0103017 ! Appearance trait

[Term]
id: CO_334:0003120
name: attieke red palm oil aroma
namespace: cassava_trait
def: "Characteristic odor of red palm oil" []
synonym: "AttRdPlmOilArom" EXACT []
is_a: CO_334:0103021 ! Aroma trait

[Term]
id: CO_334:0003121
name: attieke sourness aroma
namespace: cassava_trait
def: "Odor of sourness" []
synonym: "AttSourArom" EXACT []
is_a: CO_334:0103021 ! Aroma trait

[Term]
id: CO_334:0003122
name: attieke taste of red palm oil
namespace: cassava_trait
def: "Presence and Intensity of the taste of Red Palm oil" []
synonym: "AttTastRdPalmOil" EXACT []
is_a: CO_334:0103020 ! Taste trait

[Term]
id: CO_334:0003123
name: attieke undesired taste
namespace: cassava_trait
def: "Any undesired taste in the sample (smoke, over-fermented, etc.)." []
synonym: "AttUndesTast" EXACT []
is_a: CO_334:0103020 ! Taste trait

[Term]
id: CO_334:0003124
name: boiled root cassava odour
namespace: cassava_trait
def: "Odour of boiled cassava" []
synonym: "BoiCasCasOd" EXACT []
is_a: CO_334:0103021 ! Aroma trait

[Term]
id: CO_334:0003125
name: boiled root crumbness
namespace: cassava_trait
def: "Property of the product to crumble between the fingers" []
synonym: "BoiCasCrum" EXACT []
is_a: CO_334:0103019 ! Texture in hand trait

[Term]
id: CO_334:0003126
name: boiled root easiness to chew
namespace: cassava_trait
def: "Property related to the number of chews necessary to swallow the product" []
synonym: "BoiCasChew" EXACT []
is_a: CO_334:0103018 ! Texture in mouth trait

[Term]
id: CO_334:0003127
name: boiled root granulariness
namespace: cassava_trait
def: "Refers to the presence of small grains during chewing" []
synonym: "BoiCasGran" EXACT []
is_a: CO_334:0103018 ! Texture in mouth trait

[Term]
id: CO_334:0003128
name: boiled root hardness to break
namespace: cassava_trait
def: "Force required to cut/break with hand" []
synonym: "BoiCasHard" EXACT []
is_a: CO_334:0103019 ! Texture in hand trait

[Term]
id: CO_334:0003129
name: boiled root presence of fibers
namespace: cassava_trait
def: "Refers to the presence of fine fibers visible to the eye" []
synonym: "boiCasFibr" EXACT []
is_a: CO_334:0103019 ! Texture in hand trait

[Term]
id: CO_334:0003130
name: boiled root presence of stripe
namespace: cassava_trait
def: "Refers to the presence of the  stripe on the surface of product" []
synonym: "BoiCasStrip" EXACT []
is_a: CO_334:0103017 ! Appearance trait

[Term]
id: CO_334:0003131
name: boiled root white colour
namespace: cassava_trait
def: "Both inner and outer colour can range from light off-white to white (pure white)" []
synonym: "BoiCasWhitCol" EXACT []
is_a: CO_334:0103017 ! Appearance trait

[Term]
id: CO_334:0003132
name: eba surface creamness
namespace: cassava_trait
def: "Colour of the surface of the sample from cream to light cream" []
synonym: "EbaSurfCream" EXACT []
is_a: CO_334:0103017 ! Appearance trait

[Term]
id: CO_334:0003133
name: eba cohessiveness/moldability
namespace: cassava_trait
def: "Textural attribute relating to degree to which a substance can be deformed before it breaks" []
synonym: "EbaHdCohe" EXACT []
is_a: CO_334:0103019 ! Texture in hand trait

[Term]
id: CO_334:0003134
name: eba hardness in hand
namespace: cassava_trait
def: "Mechanical textural attribute related to the force necessary to achieve a certain deformation" []
synonym: "EbaHdHard" EXACT []
is_a: CO_334:0103019 ! Texture in hand trait

[Term]
id: CO_334:0003135
name: eba smoothness in mouth
namespace: cassava_trait
def: "Geometrical attribute associated with the overall degree of absence of particles within sample" []
synonym: "EbaMthSmooth" EXACT []
is_a: CO_334:0103018 ! Texture in mouth trait

[Term]
id: CO_334:0003136
name: eba stickiness kin the hand
namespace: cassava_trait
def: "Mechanical textural attribute relating to the force required to remove material that sticks to the hand" []
synonym: "EbaHdStic" EXACT []
is_a: CO_334:0103019 ! Texture in hand trait

[Term]
id: CO_334:0003137
name: eba stretchability in the hand
namespace: cassava_trait
def: "The tendency of a body to return to its original shape after it has been stretched or compressed" []
synonym: "EbaHdStrea" EXACT []
is_a: CO_334:0103019 ! Texture in hand trait

[Term]
id: CO_334:0003138
name: eba surface whiteness
namespace: cassava_trait
def: "Colour of the surface of the sample from light white to off white" []
synonym: "EbaSurfWhit" EXACT []
is_a: CO_334:0103017 ! Appearance trait

[Term]
id: CO_334:0003139
name: eba sourness in the mouth
namespace: cassava_trait
def: "Gustatory complex sensation, generally due to presence of organic acids" []
synonym: "EbaSour" EXACT []
is_a: CO_334:0103020 ! Taste trait

[Term]
id: CO_334:0003140
name: eba sweetness taste
namespace: cassava_trait
def: "Basic taste produced by dilute aqueous solutions of natural or artificial substances such as sucrose" []
synonym: "EbaTastSweet" EXACT []
is_a: CO_334:0103020 ! Taste trait

[Term]
id: CO_334:0003141
name: eba fibrousness in mouth
namespace: cassava_trait
def: "Geometrical attribute of product associated with presence of long string like particles" []
synonym: "EbaFibr" EXACT []
is_a: CO_334:0103018 ! Texture in mouth trait

[Term]
id: CO_334:0003142
name: eba surface greyness
namespace: cassava_trait
def: "Colour of the surface of the sample from grey to light grey" []
synonym: "EbaSurfGrey" EXACT []
is_a: CO_334:0103017 ! Appearance trait

[Term]
id: CO_334:0003143
name: Attieke aroma scale 0-10
namespace: cassava_trait
def: "Measures the aroma of attieke scale 0-10. 0=Gari; 	10=Fresh attieke" []
is_a: CO_334:0001000 ! Variables
relationship: variable_of CO_334:0003101 ! attieke attieke-like  aroma
relationship: variable_of CO_334:0013012 ! attieke-like aroma method
relationship: variable_of CO_334:0103029 ! Attieke aroma scale 0-10
created_by: Ebah Catherine

[Term]
id: CO_334:0004001
name: fresh storage root weight per plant measured in Kg
namespace: cassava_trait
def: "Total fresh weight of storage roots harvested per plant measured in kilogram (kg)." [CO:curators]
synonym: "rtwt" EXACT []
synonym: "RtWt_Wgh_kg" EXACT []
is_a: CO_334:0001000 ! Variables
relationship: variable_of CO_334:0000302 ! Storage root weight by plot
relationship: variable_of CO_334:0010286 ! Measurement: Fresh weight of storage root_method
relationship: variable_of CO_334:0100493 ! kg

[Term]
id: CO_334:0004006
name: L chromometer of gari
namespace: cassava_trait
def: "L scale of gari from chromometer indicating light vs. dark where a low number (0-50) indicates dark and a high number (51-100) indicates light" []
synonym: "L*gari" EXACT []
xref: CO:curators
is_a: CO_334:0001000 ! Variables
relationship: variable_of CO_334:0002061 ! L chromometer
relationship: variable_of CO_334:0010522 ! Computation: Chromometer color values
created_by: Ekanem

[Term]
id: CO_334:0004007
name: L chromometer of eba
namespace: cassava_trait
def: "L scale of eba from chromometer indicating light vs. dark where a low number (0-50) indicates dark and a high number (51-100) indicates light" []
synonym: "l*eba" EXACT []
xref: CO:curators
is_a: CO_334:0001000 ! Variables
relationship: variable_of CO_334:0002061 ! L chromometer
relationship: variable_of CO_334:0010522 ! Computation: Chromometer color values
created_by: Ekanem

[Term]
id: CO_334:0004008
name: A chromometer value of gari
namespace: cassava_trait
def: "a scale of gari indicating red vs. green where a positive number indicates red and a negative number indicates green" []
synonym: "a*gari" EXACT []
xref: CO:curators
is_a: CO_334:0001000 ! Variables
relationship: variable_of CO_334:0002063 ! A chromometer
relationship: variable_of CO_334:0010522 ! Computation: Chromometer color values
created_by: Ekanem

[Term]
id: CO_334:0004009
name: A chromometer value of eba
namespace: cassava_trait
def: "a scale of eba indicating red vs. green where a positive number indicates red and a negative number indicates green" []
synonym: "a*eba" EXACT []
xref: CO:curators
is_a: CO_334:0001000 ! Variables
relationship: variable_of CO_334:0002063 ! A chromometer
relationship: variable_of CO_334:0010522 ! Computation: Chromometer color values
created_by: Ekanem

[Term]
id: CO_334:0004010
name: B chromometer value of gari
namespace: cassava_trait
def: "b scale of gari indicating red vs. green where a positive number indicates red and a negative number indicates green" []
synonym: "b*gari" EXACT []
xref: CO:curators
is_a: CO_334:0001000 ! Variables
relationship: variable_of CO_334:0002062 ! B chromometer
relationship: variable_of CO_334:0010522 ! Computation: Chromometer color values
created_by: Ekanem

[Term]
id: CO_334:0004011
name: B chromometer value of eba
namespace: cassava_trait
def: "b scale of eba indicating red vs. green where a positive number indicates red and a negative number indicates green" []
synonym: "b*eba" EXACT []
xref: CO:curators
is_a: CO_334:0001000 ! Variables
relationship: variable_of CO_334:0002062 ! B chromometer
relationship: variable_of CO_334:0010522 ! Computation: Chromometer color values
created_by: Ekanem

[Term]
id: CO_334:0004015
name: pH of gari -log (H30+)
namespace: cassava_trait
def: "The pH of gari samples is evaluated by pH meter (PH=-log(H+) and measures the acidity or alkalinity of gari solution." [CO:curators]
synonym: "PH = -log (H30+)" EXACT []
is_a: CO_334:0001000 ! Variables
relationship: variable_of CO_334:0001064 ! Gari quality
relationship: variable_of CO_334:0004016 ! Measurement: pH of gari_method
relationship: variable_of CO_334:0004017 ! -log (H30+)
created_by: Ekanem
creation_date: 9/26/2023

[Term]
id: CO_334:0004016
name: Measurement: pH of gari_method
namespace: CassavaMethod
def: "Measurement using a laboratory pH meter." [CO:curators]
is_a: CO_334:0001002 ! Methods
relationship: method_of CO_334:0001064 ! Gari quality

[Term]
id: CO_334:0004017
name: -log (H30+)
namespace: CassavaScale
def: "Negative of the logarithm of H+ activity" []
is_a: CO_334:0001001 ! Scales
relationship: scale_of CO_334:0004016 ! Measurement: pH of gari_method

[Term]
id: CO_334:0004018
name: Solubility of gari %
namespace: cassava_trait
def: "Solubility of gari is expressed in units of mass divided by volume, such as grams per liter and is the property of gari to dissolve in distilled water at 55 degree for 30 minutes." [CO:curators]
synonym: "Sol KSP =(A+)a(B-)b" EXACT []
is_a: CO_334:0001000 ! Variables
relationship: variable_of CO_334:0001064 ! Gari quality
relationship: variable_of CO_334:0004019 ! Calculation: Gari solubility_method
relationship: variable_of CO_334:0100583 ! pct (%)
created_by: Ukoabasi Ekanem
creation_date: 9/26/2023

[Term]
id: CO_334:0004019
name: Calculation: Gari solubility_method
namespace: CassavaMethod
def: "Calculation of gari solubility - mass divided by volume and expressed as the percentage of dried supernatant to the initial sample weight." [CO:curators]
is_a: CO_334:0001002 ! Methods
relationship: method_of CO_334:0001064 ! Gari quality

[Term]
id: CO_334:0004020
name: Swelling index of gari
namespace: cassava_trait
def: "Swelling index of gari is expressed as a percentage, and it indicates how much the gari swells when exposed to water." [CO:curators]
synonym: "(vd-vk)/vk)*100" EXACT []
is_a: CO_334:0001000 ! Variables
relationship: variable_of CO_334:0001064 ! Gari quality
relationship: variable_of CO_334:0004021 ! Calculation: Gari swelling index_method
relationship: variable_of CO_334:0100583 ! pct (%)
created_by: Ukoabasi Ekanem
creation_date: 9/26/2023

[Term]
id: CO_334:0004021
name: Calculation: Gari swelling index_method
namespace: CassavaMethod
def: "Calculation of gari swelling index using the volume of the gari and water mixture after soaking and the volume of the gari sample before soaking." [CO:curators]
is_a: CO_334:0001002 ! Methods
relationship: method_of CO_334:0001064 ! Gari quality

[Term]
id: CO_334:0004022
name: Swelling power of gari %
namespace: cassava_trait
def: "Swelling power of gari is expressed as a percentage, and it quantifies how much the gari expands when exposed to heat and water. A higher swelling power indicates that the gari can absorb more water and increase in volume during cooking" [CO:curators]
synonym: "Swp (%)" EXACT []
is_a: CO_334:0001000 ! Variables
relationship: variable_of CO_334:0001064 ! Gari quality
relationship: variable_of CO_334:0004023 ! Calculation: Gari swelling power_method
relationship: variable_of CO_334:0100583 ! pct (%)
created_by: Ukoabasi Ekanem
creation_date: 9/26/2023

[Term]
id: CO_334:0004023
name: Calculation: Gari swelling power_method
namespace: CassavaMethod
def: "Calculation of gari swelling power using the volume of the gari and water mixture after swelling and the initial volume of the gari sample before swelling" [CO:curators]
is_a: CO_334:0001002 ! Methods
relationship: method_of CO_334:0001064 ! Gari quality

[Term]
id: CO_334:0004030
name: Gari Rapid Visco Analyzer
namespace: cassava_trait
def: "The assessment of gari texture using rheometry and texture profile analysis" []
synonym: "RVA" EXACT []
is_a: CO_334:0000004 ! Quality trait

[Term]
id: CO_334:0004031
name: Rapid visco analyze breakdown of gari RUV
namespace: cassava_trait
def: "Rapid visco analyze breakdown of gari is regarded as the measure of the degree of disintegration of the granules or paste stability" [CO:curators]
synonym: "RVA-breakdown (RUV)" EXACT []
is_a: CO_334:0001000 ! Variables
relationship: variable_of CO_334:0004030 ! Gari Rapid Visco Analyzer
relationship: variable_of CO_334:0004032 ! Measurement: Gari rapid visco analyzer_method
relationship: variable_of CO_334:0004033 ! RUV
created_by: Ukoabasi Ekanem
creation_date: 9/27/2023

[Term]
id: CO_334:0004032
name: Measurement: Gari rapid visco analyzer_method
namespace: CassavaMethod
def: "Measurement using rapid visco analyzer." [CO:curators]
is_a: CO_334:0001002 ! Methods
relationship: method_of CO_334:0001064 ! Gari quality

[Term]
id: CO_334:0004033
name: RUV
namespace: CassavaScale
def: "Rapid Visco Units" []
is_a: CO_334:0001001 ! Scales
relationship: scale_of CO_334:0004016 ! Measurement: pH of gari_method

[Term]
id: CO_334:0004034
name: Rapid visco analyze final viscosity of gari RUV
namespace: cassava_trait
def: "The final viscosity of gari is the ability of the gari to form viscous paste after cooking and cooling" [CO:curators]
synonym: "RVA-final visc (RUV)" EXACT []
is_a: CO_334:0001000 ! Variables
relationship: variable_of CO_334:0004030 ! Gari Rapid Visco Analyzer
relationship: variable_of CO_334:0004032 ! Measurement: Gari rapid visco analyzer_method
relationship: variable_of CO_334:0004033 ! RUV
created_by: Ukoabasi Ekanem
creation_date: 9/27/2023

[Term]
id: CO_334:0004035
name: Rapid visco analyze peak viscosity of gari RUV
namespace: cassava_trait
def: "The peak viscosity of gari is achieved when the rate of granules swelling equals the breakdown granules" [CO:curators]
synonym: "RVA-peak visc (RUV)" EXACT []
is_a: CO_334:0001000 ! Variables
relationship: variable_of CO_334:0004030 ! Gari Rapid Visco Analyzer
relationship: variable_of CO_334:0004032 ! Measurement: Gari rapid visco analyzer_method
relationship: variable_of CO_334:0004033 ! RUV
created_by: Ukoabasi Ekanem
creation_date: 9/27/2023

[Term]
id: CO_334:0004036
name: Rapid visco analyze peak time of gari in minute
namespace: cassava_trait
def: "The peak viscosity of gari is achieved when the rate of granules swelling equals the breakdown granules" [CO:curators]
synonym: "RVA-peak time (m)" EXACT []
is_a: CO_334:0001000 ! Variables
relationship: variable_of CO_334:0004030 ! Gari Rapid Visco Analyzer
relationship: variable_of CO_334:0004032 ! Measurement: Gari rapid visco analyzer_method
relationship: variable_of CO_334:0100696 ! minute
created_by: Ukoabasi Ekanem
creation_date: 9/27/2023

[Term]
id: CO_334:0004037
name: Rapid visco analyze setback viscosity of gari RUV
namespace: cassava_trait
def: "The setback viscosity of gari is determined by the difference between the peak viscosity and the final viscosity" [CO:curators]
synonym: "RVA-setback visc (RUV)" EXACT []
is_a: CO_334:0001000 ! Variables
relationship: variable_of CO_334:0004030 ! Gari Rapid Visco Analyzer
relationship: variable_of CO_334:0004032 ! Measurement: Gari rapid visco analyzer_method
relationship: variable_of CO_334:0004033 ! RUV
created_by: Ukoabasi Ekanem
creation_date: 9/27/2023

[Term]
id: CO_334:0004038
name: Rapid visco analyze trough viscosity of gari RUV
namespace: cassava_trait
def: "Trough viscosity of gari is the disruption of granules resulting in a decrease in paste viscosity" [CO:curators]
synonym: "RVA-trough (RUV)" EXACT []
is_a: CO_334:0001000 ! Variables
relationship: variable_of CO_334:0004030 ! Gari Rapid Visco Analyzer
relationship: variable_of CO_334:0004032 ! Measurement: Gari rapid visco analyzer_method
relationship: variable_of CO_334:0004033 ! RUV
created_by: Ukoabasi Ekanem
creation_date: 9/27/2023

[Term]
id: CO_334:0004039
name: Rapid visco analyze pasting temperature of gari in °C
namespace: cassava_trait
def: "The rapid visco analyze pasting temperature of gari is the temperature at which the starch in gari begins to gelatinize and thicken as it is heated and stirred" [CO:curators]
synonym: "RVA-pasting temp (°C))" EXACT []
is_a: CO_334:0001000 ! Variables
relationship: variable_of CO_334:0004030 ! Gari Rapid Visco Analyzer
relationship: variable_of CO_334:0004032 ! Measurement: Gari rapid visco analyzer_method
relationship: variable_of CO_334:0100703 ! degree celsius
created_by: Ukoabasi Ekanem
creation_date: 9/27/2023

[Term]
id: CO_334:0010000
name: Measurement: Plant height with leaf_method
namespace: CassavaMethod
is_a: CO_334:0001002 ! Methods
relationship: method_of CO_334:0000478 ! Stem height
created_by: naama
creation_date: 2015-09-23T16:16:50Z

[Term]
id: CO_334:0010001
name: Estimation: Post-harvest physiological deterioration method
namespace: CassavaMethod
def: "Estimation of post-harvest physiological deterioration by slicing the roots." [CO:curators]
is_a: CO_334:0001002 ! Methods
relationship: method_of CO_334:0000266 ! Post-harvest physiological deterioration
created_by: naama
creation_date: 2015-09-25T11:48:31Z

[Term]
id: CO_334:0010002
name: Visual Rating: Staygreen_method
namespace: CassavaMethod
def: "Visual rating of leaf retention or longevity" [CO:curators]
is_a: CO_334:0001002 ! Methods
relationship: method_of CO_334:0000396 ! Leaf retention
created_by: AAfolabi
creation_date: 2015-09-29T12:31:09Z

[Term]
id: CO_334:0010003
name: Visual Rating: Size of shoot apices_method
namespace: CassavaMethod
is_a: CO_334:0001002 ! Methods
relationship: method_of CO_334:0000268 ! Shoot apices
created_by: AAfolabi
creation_date: 2015-09-29T13:44:26Z

[Term]
id: CO_334:0010004
name: Visual Rating: Compactness of shoot apices_method
namespace: CassavaMethod
is_a: CO_334:0001002 ! Methods
relationship: method_of CO_334:0000268 ! Shoot apices
created_by: AAfolabi
creation_date: 2015-09-29T13:56:16Z

[Term]
id: CO_334:0010005
name: Measurement: Stem diameter_method
namespace: CassavaMethod
is_a: CO_334:0001002 ! Methods
relationship: method_of CO_334:0000480 ! Stem weight
created_by: AAfolabi
creation_date: 2015-09-29T14:06:39Z

[Term]
id: CO_334:0010006
name: Counting: Female flower number all levels_method
namespace: CassavaMethod
def: "Count of the number of female flowers after the buds appear,mature, and grow in size to become distinctive at all branching levels." []
is_a: CO_334:0001002 ! Methods
relationship: method_of CO_334:0000364 ! Female flower number
created_by: aafolabi
creation_date: 2016-05-12T12:51:09Z

[Term]
id: CO_334:0010007
name: Counting: Male flower number on all levels_method
namespace: CassavaMethod
def: "Count of the number of male flowers after the buds appear,mature, and grow in size to become distinctive at all branching levels." []
is_a: CO_334:0001002 ! Methods
relationship: method_of CO_334:0000403 ! Male flower number
created_by: aafolabi
creation_date: 2016-05-12T14:54:46Z

[Term]
id: CO_334:0010008
name: Visual Observation: Days to first male flower opens
namespace: CassavaMethod
def: "Observation of the actual date from the date of planting, when the first male flowers opens." []
is_a: CO_334:0001002 ! Methods
relationship: method_of CO_334:0000286 ! Days to first male flower opens
created_by: aafolabi
creation_date: 2016-05-12T17:29:12Z

[Term]
id: CO_334:0010009
name: Estimation: Dry matter content of leaf percentage
namespace: CassavaMethod
def: "Leaf dry matter content estimated as the ratio of measured leaf dry weight and leaf fresh weight multiplied by 100." [CO:curator]
is_a: CO_334:0001002 ! Methods
relationship: method_of CO_334:0000447 ! Dry matter content
created_by: AAfolabi
creation_date: 2017-07-18T15:13:10Z

[Term]
id: CO_334:0010010
name: Estimation: Dry matter content of lower stem percentage
namespace: CassavaMethod
def: "Dry matter content of lower stem estimated as the ratio of measured lower stem dry weight and lower stem fresh weight multiplied by 100." [CO:curator]
is_a: CO_334:0001002 ! Methods
relationship: method_of CO_334:0000447 ! Dry matter content
created_by: AAfolabi
creation_date: 2017-07-18T15:19:20Z

[Term]
id: CO_334:0010011
name: Estimation: Dry matter content of fibrous root percentage
namespace: CassavaMethod
def: "Estimation of fibrous root dry matter content as the ratio of measured fibrous root dry weight and fibrous root fresh weight multiplied by 100." [CO:curator]
is_a: CO_334:0001002 ! Methods
relationship: method_of CO_334:0000447 ! Dry matter content
created_by: AAfolabi
creation_date: 2017-07-18T15:24:49Z

[Term]
id: CO_334:0010012
name: Estimation: Total leaf area_method
namespace: CassavaMethod
def: "Estimation of leaf area using handheld device." [CO:curator]
is_a: CO_334:0001002 ! Methods
relationship: method_of CO_334:0000425 ! Total leaf area
created_by: AAfolabi
creation_date: 2017-07-18T15:34:16Z

[Term]
id: CO_334:0010013
name: Visual Observation: Days to branching event
namespace: CassavaMethod
def: "Visual observation of branching event in a plot" []
is_a: CO_334:0001002 ! Methods
relationship: method_of CO_334:0000449 ! Days to branching event
created_by: AAfolabi
creation_date: 2017-07-25T10:18:21Z

[Term]
id: CO_334:0010014
name: Visual Observation: Days to abortion by branching level
namespace: CassavaMethod
def: "Visual observation (actual date in the format of dd/mm/yyyy from the date of planting) of the death of immatured flower." [CO:curator]
is_a: CO_334:0001002 ! Methods
relationship: method_of CO_334:0000471 ! Days to abortion by branching levels
created_by: AAfolabi
creation_date: 2017-07-25T11:28:02Z

[Term]
id: CO_334:0010015
name: Visual Observation: Days to first female flower opens by branch levels
namespace: CassavaMethod
def: "Visual observation (actual date in the format of dd/mm/yyyy from the date of planting) of the opening of the first female flower" [CO:curator]
is_a: CO_334:0001002 ! Methods
relationship: method_of CO_334:0000512 ! Days to first female flower opens by branch levels
created_by: AAfolabi
creation_date: 2017-07-25T12:00:48Z

[Term]
id: CO_334:0010016
name: Visual Observation: Days to senescence by branch level
namespace: CassavaMethod
def: "Visual observation (actual date in the format of dd/mm/yyyy from the date of planting) of the death of matured flowers." [CO:curator]
is_a: CO_334:0001002 ! Methods
relationship: method_of CO_334:0000517 ! Days to senescence by branch level
created_by: AAfolabi
creation_date: 2017-07-25T12:27:33Z

[Term]
id: CO_334:0010017
name: Counting: Number of forks by branch level
namespace: CassavaMethod
def: "A count of the number of branches (2 forks/branches (dichotomous), 3 forks/branches (trichotomous), or 4 forks/branches (tetrachotomous)) at specific branching level." [CO:curator]
is_a: CO_334:0001002 ! Methods
relationship: method_of CO_334:0000521 ! Number of forks by branch level
created_by: AAfolabi
creation_date: 2017-07-25T15:06:07Z

[Term]
id: CO_334:0010018
name: Counting: Number of inflorescence by branch level
namespace: CassavaMethod
def: "Count of the number of inflorescence by branch levels." [CO:curator]
is_a: CO_334:0001002 ! Methods
relationship: method_of CO_334:0000525 ! Number of inflorescence by branch level
created_by: AAfolabi
creation_date: 2017-07-25T16:04:51Z

[Term]
id: CO_334:0010019
name: Counting: Number of buds by branch level
namespace: CassavaMethod
def: "Count of the number of buds" []
is_a: CO_334:0001002 ! Methods
relationship: method_of CO_334:0000530 ! Number of buds by branch level
created_by: AAfolabi
creation_date: 2017-07-25T16:23:40Z

[Term]
id: CO_334:0010020
name: Counting: Male flower number by branch level
namespace: CassavaMethod
def: "Count of the number male flowers after the buds appears, matures, and grows in size to become distinctive." [CO:curator]
is_a: CO_334:0001002 ! Methods
relationship: method_of CO_334:0000534 ! male flower number counting by branch level
created_by: AAfolabi
creation_date: 2017-07-25T16:36:30Z

[Term]
id: CO_334:0010021
name: Visual Observation: Days to fruitset by branch level
namespace: CassavaMethod
def: "Visual observation (actual date in the format of dd/mm/yyyy from the date of planting) of the date when fruit is first seen." [CO:curator]
is_a: CO_334:0001002 ! Methods
relationship: method_of CO_334:0000538 ! Days to fruitset by branch level
created_by: AAfolabi
creation_date: 2017-07-25T16:54:49Z

[Term]
id: CO_334:0010022
name: Counting: Number of fruitset by branch level
namespace: CassavaMethod
def: "A count of the number of fruits formed from the seeds after pollination." [CO:curator]
is_a: CO_334:0001002 ! Methods
relationship: method_of CO_334:0000542 ! number of fruitset by branch level
created_by: AAfolabi
creation_date: 2017-07-25T17:05:17Z

[Term]
id: CO_334:0010220
name: Counting: Sprouting_method
namespace: CassavaMethod
def: "The number of germinated stakes divided by the total number of planted stakes scored one month after planting" [CO:curators]
is_a: CO_334:0001002 ! Methods
relationship: method_of CO_334:0000472 ! Sprouting

[Term]
id: CO_334:0010221
name: Counting: Number of planted stakes_method
namespace: CassavaMethod
def: "Count of the number of stakes planted per plot" [CO:curators]
is_a: CO_334:0001002 ! Methods
relationship: method_of CO_334:0000416 ! Number of planted stakes

[Term]
id: CO_334:0010222
name: Counting: Sprout count _method
namespace: CassavaMethod
def: "A count of the number of germinated stakes" [CO:curators]
is_a: CO_334:0001002 ! Methods
relationship: method_of CO_334:0000466 ! Sprout count

[Term]
id: CO_334:0010223
name: Counting: Sprout count at one-month_method
namespace: CassavaMethod
def: "Count of the number of stakes germinated, one month after planting" [CO:curators]
is_a: CO_334:0001002 ! Methods
relationship: method_of CO_334:0000466 ! Sprout count

[Term]
id: CO_334:0010224
name: Counting: Sprout count at three-month_method
namespace: CassavaMethod
def: "Count of the number of stakes germinated, three months after planting" [CO:curators]
is_a: CO_334:0001002 ! Methods
relationship: method_of CO_334:0000466 ! Sprout count

[Term]
id: CO_334:0010225
name: Counting: Sprout count at six-month_method
namespace: CassavaMethod
def: "Count of the number of stakes germinated, six months after planting" [CO:curators]
is_a: CO_334:0001002 ! Methods
relationship: method_of CO_334:0000466 ! Sprout count

[Term]
id: CO_334:0010226
name: Counting: Sprout count at nine-month_method
namespace: CassavaMethod
def: "Count of the number of stakes germinated, nine months after planting" [CO:curators]
is_a: CO_334:0001002 ! Methods
relationship: method_of CO_334:0000466 ! Sprout count

[Term]
id: CO_334:0010227
name: Counting: Sprout count at twelve-month_method
namespace: CassavaMethod
def: "Count of the number of stakes germinated, twelve months after planting" [CO:curators]
is_a: CO_334:0001002 ! Methods
relationship: method_of CO_334:0000466 ! Sprout count

[Term]
id: CO_334:0010228
name: Visual Rating: Initial vigor_method
namespace: CassavaMethod
def: "Trait monitored by observing plant vigor one month after planting" [CO:curators]
is_a: CO_334:0001002 ! Methods
relationship: method_of CO_334:0000386 ! Initial vigor

[Term]
id: CO_334:0010230
name: Visual Observation: Cassava mosaic disease severity 1-month evaluation_method
namespace: CassavaMethod
def: "Symptoms of infection by cassava mosaic virus is scored between one to six weeks after planting. Symptoms rated from 1=(clean,no infection) to 5=(extremely severe, severely diseased)" [CO:curators]
is_a: CO_334:0001002 ! Methods
relationship: method_of CO_334:0000035 ! Cassava mosaic disease severity

[Term]
id: CO_334:0010231
name: Visual Observation: Cassava mosaic disease severity 3-month evaluation_method
namespace: CassavaMethod
def: "Symptoms of infection by cassava mosaic virus is scored between two and three months  after planting. Symptoms rated from 1=(clean,no infection) to 5=(extremely severe, severely diseased)" [CO:curators]
is_a: CO_334:0001002 ! Methods
relationship: method_of CO_334:0000035 ! Cassava mosaic disease severity

[Term]
id: CO_334:0010232
name: Visual Observation: Cassava mosaic disease severity 6-month evaluation_method
namespace: CassavaMethod
def: "Symptoms of infection by cassava mosaic virus is scored between four and six months  after planting. Symptoms rated from 1=(clean,no infection) to 5=(extremely severe, severely diseased)" [CO:curators]
is_a: CO_334:0001002 ! Methods
relationship: method_of CO_334:0000035 ! Cassava mosaic disease severity

[Term]
id: CO_334:0010233
name: Visual Observation: Cassava mosaic disease severity 9-month evaluation_method
namespace: CassavaMethod
def: "Symptoms of infection by cassava mosaic virus is scored between seven and nine months  after planting. Symptoms rated from 1=(clean,no infection) to 5=(extremely severe, severely diseased)" [CO:curators]
is_a: CO_334:0001002 ! Methods
relationship: method_of CO_334:0000035 ! Cassava mosaic disease severity

[Term]
id: CO_334:0010234
name: Visual Observation: Cassava mosaic disease severity 12-month evaluation_method
namespace: CassavaMethod
def: "Symptoms of infection by cassava mosaic virus is scored between ten and twelve months  after planting. Symptoms rated from 1=(clean,no infection) to 5=(extremely severe, severely diseased)" [CO:curators]
is_a: CO_334:0001002 ! Methods
relationship: method_of CO_334:0000035 ! Cassava mosaic disease severity

[Term]
id: CO_334:0010236
name: Counting: Cassava mosaic disease incidence 1-month evaluation_method
namespace: CassavaMethod
def: "The ratio of plants showing symptoms of cassava mosaic disease as a proportion of the total plant stands scored at one to six weeks after planting" [CO:curators]
is_a: CO_334:0001002 ! Methods
relationship: method_of CO_334:0000039 ! Cassava mosaic disease incidence

[Term]
id: CO_334:0010237
name: Counting: Cassava mosaic disease incidence 3-month evaluation_method
namespace: CassavaMethod
def: "The ratio of plants showing symptoms of cassava mosaic disease as a proportion of the total plant stands scored at two to three months after planting" [CO:curators]
is_a: CO_334:0001002 ! Methods
relationship: method_of CO_334:0000039 ! Cassava mosaic disease incidence

[Term]
id: CO_334:0010238
name: Counting: Cassava mosaic disease incidence 6-month evaluation_method
namespace: CassavaMethod
def: "The ratio of plants showing symptoms of cassava mosaic disease as a proportion of the total plant stands scored at four to six months after planting" [CO:curators]
is_a: CO_334:0001002 ! Methods
relationship: method_of CO_334:0000039 ! Cassava mosaic disease incidence

[Term]
id: CO_334:0010239
name: Counting: Cassava mosaic disease incidence 9-month evaluation_method
namespace: CassavaMethod
def: "The ratio of plants showing symptoms of cassava mosaic disease as a proportion of the total plant stands scored at seven to nine months after planting" [CO:curators]
is_a: CO_334:0001002 ! Methods
relationship: method_of CO_334:0000039 ! Cassava mosaic disease incidence

[Term]
id: CO_334:0010240
name: Counting: Cassava mosaic disease incidence 12-month evaluation_method
namespace: CassavaMethod
def: "The ratio of plants showing symptoms of cassava mosaic disease as a proportion of the total plant stands scored at ten to twelve months after planting" [CO:curators]
is_a: CO_334:0001002 ! Methods
relationship: method_of CO_334:0000039 ! Cassava mosaic disease incidence

[Term]
id: CO_334:0010242
name: Visual Observation: Cassava bacterial blight severity 3-month evalution_method
namespace: CassavaMethod
def: "The trait is scored at two to three months after planting as severity of cassava bacterial blight symptoms caused by Xanthomonas axonopodis pv. Manihotis and rated on a scale from 1 (= no symptom) to 5 (= extremely severe)" [CO:curators]
is_a: CO_334:0001002 ! Methods
relationship: method_of CO_334:0000031 ! Cassava bacterial blight severity

[Term]
id: CO_334:0010243
name: Visual Observation: Cassava bacterial blight severity 6-month evalution_method
namespace: CassavaMethod
def: "The trait is scored at four to six months after planting as severity of cassava bacterial blight symptoms caused by Xanthomonas axonopodis pv. Manihotis and rated on a scale from 1 (= no symptom) to 5 (= extremely severe)" [CO:curators]
is_a: CO_334:0001002 ! Methods
relationship: method_of CO_334:0000031 ! Cassava bacterial blight severity

[Term]
id: CO_334:0010244
name: Visual Observation: Cassava bacterial blight severity 9-month evalution_method
namespace: CassavaMethod
def: "The trait is scored at seven to nine months after planting as severity of cassava bacterial blight symptoms caused by Xanthomonas axonopodis pv. Manihotis and rated on a scale from 1 (= no symptom) to 5 (= extremely severe)" [CO:curators]
is_a: CO_334:0001002 ! Methods
relationship: method_of CO_334:0000031 ! Cassava bacterial blight severity

[Term]
id: CO_334:0010245
name: Visual Observation: Cassava bacterial blight severity 12-month evaluation_method
namespace: CassavaMethod
def: "The trait is scored at ten to twelve months after planting as severity of cassava bacterial blight symptoms caused by Xanthomonas axonopodis pv. Manihotis and rated on a scale from 1 (= no symptom) to 5 (= extremely severe)" [CO:curators]
is_a: CO_334:0001002 ! Methods
relationship: method_of CO_334:0000031 ! Cassava bacterial blight severity

[Term]
id: CO_334:0010247
name: Counting: Cassava bacterial blight incidence 3-month evalution_method
namespace: CassavaMethod
def: "A ratio of infected plants with cassava bacterial blight to total plant stands scored at two to three months after planting" [CO:curators]
is_a: CO_334:0001002 ! Methods
relationship: method_of CO_334:0000037 ! Cassava bacterial blight incidence

[Term]
id: CO_334:0010248
name: Counting: Cassava bacterial blight incidence 6-month evalution_method
namespace: CassavaMethod
def: "A ratio of infected plants with cassava bacterial blight to total plant stands scored at four to six months after planting" [CO:curators]
is_a: CO_334:0001002 ! Methods
relationship: method_of CO_334:0000037 ! Cassava bacterial blight incidence

[Term]
id: CO_334:0010249
name: Counting: Cassava bacterial blight incidence 9-month evalution_method
namespace: CassavaMethod
def: "A ratio of infected plants with cassava bacterial blight to total plant stands scored at seven to nine months after planting" [CO:curators]
is_a: CO_334:0001002 ! Methods
relationship: method_of CO_334:0000037 ! Cassava bacterial blight incidence

[Term]
id: CO_334:0010250
name: Counting: Cassava bacterial blight incidence 12-month evaluation_method
namespace: CassavaMethod
def: "A ratio of infected plants with cassava bacterial blight to total plant stands scored at ten to twelve months after planting" [CO:curators]
is_a: CO_334:0001002 ! Methods
relationship: method_of CO_334:0000037 ! Cassava bacterial blight incidence

[Term]
id: CO_334:0010252
name: Visual Observation: Cassava anthractnose disease severity in 3-months_method
namespace: CassavaMethod
def: "Cassava anthracnose stem lesion severity is scored at different times after planting to coincide with typically high symptom expression.  Symptoms are rated on a scale from 1 (= no symptoms) to 5 (= extremely severe stem lesions and dieback of stem)" [CO:curators]
is_a: CO_334:0001002 ! Methods
relationship: method_of CO_334:0000032 ! Cassava anthracnose disease severity

[Term]
id: CO_334:0010253
name: Visual Observation: Cassava anthractnose disease severity in 6-months_method
namespace: CassavaMethod
def: "Cassava anthracnose stem lesion severity is scored at different times after planting to coincide with typically high symptom expression.  Symptoms are rated on a scale from 1 (= no symptoms) to 5 (= extremely severe stem lesions and dieback of stem)" [CO:curators]
is_a: CO_334:0001002 ! Methods
relationship: method_of CO_334:0000032 ! Cassava anthracnose disease severity

[Term]
id: CO_334:0010254
name: Visual Observation: Cassava anthractnose disease severity in 9-months_method
namespace: CassavaMethod
def: "Cassava anthracnose stem lesion severity is scored at different times after planting to coincide with typically high symptom expression.  Symptoms are rated on a scale from 1 (= no symptoms) to 5 (= extremely severe stem lesions and dieback of stem)" [CO:curators]
is_a: CO_334:0001002 ! Methods
relationship: method_of CO_334:0000032 ! Cassava anthracnose disease severity

[Term]
id: CO_334:0010255
name: Visual Observation: Cassava anthractnose disease severity in 12-months_method
namespace: CassavaMethod
def: "Cassava anthracnose stem lesion severity is scored at different times after planting to coincide with typically high symptom expression.  Symptoms are rated on a scale from 1 (= no symptoms) to 5 (= extremely severe stem lesions and dieback of stem)" [CO:curators]
is_a: CO_334:0001002 ! Methods
relationship: method_of CO_334:0000032 ! Cassava anthracnose disease severity

[Term]
id: CO_334:0010257
name: Counting: Cassava anthractnose disease incidence in 3-months_method
namespace: CassavaMethod
def: "A ratio of the number of plants showing sysmptoms of cassava anthracnose disease to total plant stands at four to six months after planting" [CO:curators]
is_a: CO_334:0001002 ! Methods
relationship: method_of CO_334:0000038 ! Cassava anthracnose disease incidence

[Term]
id: CO_334:0010258
name: Counting: Cassava anthractnose disease incidence in 6-months_method
namespace: CassavaMethod
def: "A ratio of the number of plants showing sysmptoms of cassava anthracnose disease to total plant stands at four to six months after planting" [CO:curators]
is_a: CO_334:0001002 ! Methods
relationship: method_of CO_334:0000038 ! Cassava anthracnose disease incidence

[Term]
id: CO_334:0010259
name: Counting: Cassava anthractnose disease incidence in 9-months_method
namespace: CassavaMethod
def: "A ratio of the number of plants showing sysmptoms of cassava anthracnose disease to total plant stands at seven to nine months after planting" [CO:curators]
is_a: CO_334:0001002 ! Methods
relationship: method_of CO_334:0000038 ! Cassava anthracnose disease incidence

[Term]
id: CO_334:0010260
name: Counting: Cassava anthractnose disease incidence in 12-months_method
namespace: CassavaMethod
def: "A ratio of the number of plants showing sysmptoms of cassava anthracnose disease to total plant stands at ten to twelve months after planting" [CO:curators]
is_a: CO_334:0001002 ! Methods
relationship: method_of CO_334:0000038 ! Cassava anthracnose disease incidence

[Term]
id: CO_334:0010262
name: Counting: Cassava green mite incidence first evaluation_method
namespace: CassavaMethod
def: "A ratio of the number of plants showing cassava green might symtoms to total plant stands at the peak of the dry season" [CO:curators]
is_a: CO_334:0001002 ! Methods
relationship: method_of CO_334:0000122 ! Cassava green mite incidence

[Term]
id: CO_334:0010263
name: Counting: Cassava green mite incidence second evaluation_method
namespace: CassavaMethod
def: "A ratio of the number of plants showing cassava green might symtoms to total plant stands at the peak of the dry season" [CO:curators]
is_a: CO_334:0001002 ! Methods
relationship: method_of CO_334:0000122 ! Cassava green mite incidence

[Term]
id: CO_334:0010265
name: Visual Observation: Cassava green mite severity first evaluation_method
namespace: CassavaMethod
def: "Visual rating of damage caused by cassava green mite,Mononychellus tanajoa. Symptoms rated from 1=(clean,no infection) to 5=(extremely severe, severely diseased), evaluated at the early period of the peak of dry season" [CO:curators]
is_a: CO_334:0001002 ! Methods
relationship: method_of CO_334:0000033 ! Cassava green mite severity

[Term]
id: CO_334:0010266
name: Visual Observation: Cassava green mite severity second evaluation_method
namespace: CassavaMethod
def: "Visual rating of damage caused by cassava green mite,Mononychellus tanajoa. Symptoms rated from 1=(clean,no infection) to 5=(extremely severe, severely diseased), evaluated at the early period of the peak of dry season" [CO:curators]
is_a: CO_334:0001002 ! Methods
relationship: method_of CO_334:0000033 ! Cassava green mite severity

[Term]
id: CO_334:0010267
name: Visual Observation: Cassava mealy bug severity_method
namespace: CassavaMethod
def: "Severity of cassava mealy bug symptoms caused by mealybug, Phenacoccus Manihoti" [CO:curators]
is_a: CO_334:0001002 ! Methods
relationship: method_of CO_334:0000340 ! Cassava mealy bug severity

[Term]
id: CO_334:0010268
name: Counting: Cassava mealy bug incidence_method
namespace: CassavaMethod
def: "A ratio of plants showing symptoms of cassava mealy bug damage divided by the total number of plant stands" [CO:curators]
is_a: CO_334:0001002 ! Methods
relationship: method_of CO_334:0000339 ! Cassava mealy bug incidence

[Term]
id: CO_334:0010270
name: Visual Observation: Cassava brown streak disease leaf severity 1-month evaluation_method
namespace: CassavaMethod
def: "Severity on leaf symptoms caused by cassava brown streak virus,  in the family Potyviridae and genus Ipomovirus and rated on a scale from 1 (= no symptom) to 5 (= extremely severe) " [CO:curators]
is_a: CO_334:0001002 ! Methods
relationship: method_of CO_334:0000036 ! Cassava brown streak disease leaf severity

[Term]
id: CO_334:0010271
name: Visual Observation: Cassava brown streak disease leaf severity 3-month evaluation_method
namespace: CassavaMethod
def: "Severity on leaf symptoms caused by cassava brown streak virus,  in the family Potyviridae and genus Ipomovirus and rated on a scale from 1 (= no symptom) to 5 (= extremely severe) " [CO:curators]
is_a: CO_334:0001002 ! Methods
relationship: method_of CO_334:0000036 ! Cassava brown streak disease leaf severity

[Term]
id: CO_334:0010272
name: Visual Observation: Cassava brown streak disease leaf severity 6-month evaluation_method
namespace: CassavaMethod
def: "Severity on leaf symptoms caused by cassava brown streak virus,  in the family Potyviridae and genus Ipomovirus and rated on a scale from 1 (= no symptom) to 5 (= extremely severe) " [CO:curators]
is_a: CO_334:0001002 ! Methods
relationship: method_of CO_334:0000036 ! Cassava brown streak disease leaf severity

[Term]
id: CO_334:0010273
name: Visual Observation: Cassava brown streak disease leaf severity 9-month evaluation_method
namespace: CassavaMethod
def: "Severity on leaf symptoms caused by cassava brown streak virus,  in the family Potyviridae and genus Ipomovirus and rated on a scale from 1 (= no symptom) to 5 (= extremely severe) " [CO:curators]
is_a: CO_334:0001002 ! Methods
relationship: method_of CO_334:0000036 ! Cassava brown streak disease leaf severity

[Term]
id: CO_334:0010275
name: Counting: Cassava brown streak disease leaf incidence 1-month evaluation_method
namespace: CassavaMethod
def: "Ratio of the number of plants showing leaf symptoms from cassava brown streak disease out of the total plant stands" [CO:curators]
is_a: CO_334:0001002 ! Methods
relationship: method_of CO_334:0000040 ! Cassava brown streak disease leaf incidence

[Term]
id: CO_334:0010276
name: Counting: Cassava brown streak disease leaf incidence 3-month evaluation_method
namespace: CassavaMethod
def: "Ratio of the number of plants showing leaf symptoms from cassava brown streak disease out of the total plant stands" [CO:curators]
is_a: CO_334:0001002 ! Methods
relationship: method_of CO_334:0000040 ! Cassava brown streak disease leaf incidence

[Term]
id: CO_334:0010277
name: Counting: Cassava brown streak disease leaf incidence 6-month evaluation_method
namespace: CassavaMethod
def: "Ratio of the number of plants showing leaf symptoms from cassava brown streak disease out of the total plant stands" [CO:curators]
is_a: CO_334:0001002 ! Methods
relationship: method_of CO_334:0000040 ! Cassava brown streak disease leaf incidence

[Term]
id: CO_334:0010278
name: Counting: Cassava brown streak disease leaf incidence 9-month evaluation_method
namespace: CassavaMethod
def: "Ratio of the number of plants showing leaf symptoms from cassava brown streak disease out of the total plant stands" [CO:curators]
is_a: CO_334:0001002 ! Methods
relationship: method_of CO_334:0000040 ! Cassava brown streak disease leaf incidence

[Term]
id: CO_334:0010280
name: Visual Observation: Cassava brown streak disease root severity 12-month evaluation_method
namespace: CassavaMethod
def: "Visual rating of root symptoms caused by cassava brown streak virus at twelve months after planting, in the family of Potyviridae and genus Ipomovirus. Symptoms rated from 1=(clean,no infection) to 5=(extremely severe, severely diseased)" [CO:curators]
is_a: CO_334:0001002 ! Methods
relationship: method_of CO_334:0000090 ! Cassava brown streak disease root severity

[Term]
id: CO_334:0010282
name: Counting: Cassava brown streak disease root incidence 12-month evaluation_method
namespace: CassavaMethod
def: "A ratio of the number of plants showing root symptoms from cassava brown streak disease as a proportion of  total plant stands" [CO:curators]
is_a: CO_334:0001002 ! Methods
relationship: method_of CO_334:0000089 ! Cassava brown streak disease root incidence

[Term]
id: CO_334:0010283
name: Visual Observation: Frog skin disease_method
namespace: CassavaMethod
def: "Visual scoring of the severity of frog skin disease symptoms caused by unknown causal agent" [CO:curators]
is_a: CO_334:0001002 ! Methods
relationship: method_of CO_334:0000370 ! Frog skin disease

[Term]
id: CO_334:0010284
name: Counting: Plant stands harvested_method
namespace: CassavaMethod
def: "Count the number of plant stands that are harvested in a plot" [CO:curators]
is_a: CO_334:0001002 ! Methods
relationship: method_of CO_334:0000434 ! Plant stands harvested

[Term]
id: CO_334:0010285
name: Counting: Root number_method
namespace: CassavaMethod
def: "Count the number of storage root." [CO:curators]
is_a: CO_334:0001002 ! Methods
relationship: method_of CO_334:0000452 ! Root number

[Term]
id: CO_334:0010286
name: Measurement: Fresh weight of storage root_method
namespace: CassavaMethod
def: "Weigh harvested storage roots per plot at harvest" [CO:curators]
is_a: CO_334:0001002 ! Methods
relationship: method_of CO_334:0000302 ! Storage root weight by plot

[Term]
id: CO_334:0010287
name: Measurement: Fresh shoot weight_method
namespace: CassavaMethod
def: "Weigh foliage and stems per plot at harvest" [CO:curators]
is_a: CO_334:0001002 ! Methods
relationship: method_of CO_334:0000305 ! Fresh shoot weight by plot

[Term]
id: CO_334:0010288
name: Visual Rating: Storage root size_method
namespace: CassavaMethod
def: "Visual scoring of root length" [CO:curators]
is_a: CO_334:0001002 ! Methods
relationship: method_of CO_334:0000492 ! Storage Root Size

[Term]
id: CO_334:0010289
name: Visual Rating: Storage root shape_method
namespace: CassavaMethod
def: "Visual rating of root shape" [CO:curators]
is_a: CO_334:0001002 ! Methods
relationship: method_of CO_334:0000491 ! Storage Root Shape

[Term]
id: CO_334:0010290
name: Visual Rating: Storage root cortex color_method
namespace: CassavaMethod
def: "Visual rating of root cortex colour" [CO:curators]
is_a: CO_334:0001002 ! Methods
relationship: method_of CO_334:0000486 ! Storage Root Cortex Color

[Term]
id: CO_334:0010291
name: Visual Rating: Storage root periderm color_method
namespace: CassavaMethod
def: "Visual rating of root periderm colour" [CO:curators]
is_a: CO_334:0001002 ! Methods
relationship: method_of CO_334:0000489 ! Storage Root Periderm Color

[Term]
id: CO_334:0010292
name: Visual Rating: Storage root pulp color _method
namespace: CassavaMethod
def: "Visual rating of root pulp colour immediately after roots are cut" [CO:curators]
is_a: CO_334:0001002 ! Methods
relationship: method_of CO_334:0000490 ! Storage Root Pulp Color

[Term]
id: CO_334:0010293
name: Visual Rating: Root neck length_method
namespace: CassavaMethod
def: "Visual  rating of the root neck length" [CO:curators]
is_a: CO_334:0001002 ! Methods
relationship: method_of CO_334:0000451 ! Storage root neck length

[Term]
id: CO_334:0010294
name: Visual Scoring: Ease of peeling root cortex_method
namespace: CassavaMethod
def: "Qualitative rating of the ease of  peeling root cortex" [CO:curators]
is_a: CO_334:0001002 ! Methods
relationship: method_of CO_334:0000362 ! Ease of peeling storage root cortex

[Term]
id: CO_334:0010295
name: Counting: Rotted storage roots _method
namespace: CassavaMethod
def: "Count the number of rotted storage roots per plot at the time of harvest." [CO:curators]
is_a: CO_334:0001002 ! Methods
relationship: method_of CO_334:0000457 ! Rotted storage roots

[Term]
id: CO_334:0010296
name: Sensory Assesment: Poundability_method
namespace: CassavaMethod
def: "Mealiness of boiled cassava storage roots determined qualitatively by applying pressure to boiled roots" [CO:curators]
is_a: CO_334:0001002 ! Methods
relationship: method_of CO_334:0000437 ! Poundability

[Term]
id: CO_334:0010297
name: Gustation: Taste of boiled roots_method
namespace: CassavaMethod
def: "Rating of the taste of boiled root" [CO:curators]
is_a: CO_334:0001002 ! Methods
relationship: method_of CO_334:0000498 ! Taste of boiled roots

[Term]
id: CO_334:0010298
name: Visual Rating: Color of boiled storage roots_method
namespace: CassavaMethod
def: "Visual  rating of boiled roots" [CO:curators]
is_a: CO_334:0001002 ! Methods
relationship: method_of CO_334:0000355 ! Color of boiled storage roots

[Term]
id: CO_334:0010299
name: Estimation: Hydrogen cyanide potential picrate method
namespace: CassavaMethod
def: "Visual scoring of the root cyanide content estimated using the sodium picrate test. This test consist is applying sodium picrate on the storage root and observing the reacting colour " [CO:curators]
is_a: CO_334:0001002 ! Methods
relationship: method_of CO_334:0000502 ! Storage root cyanide content

[Term]
id: CO_334:0010300
name: Estimation: Root dry matter content_method
namespace: CassavaMethod
def: "Estimated root dry matter estimated by multiplying 100 times the ratio of dry root weight after oven drying to constant weight divided by the weight of an approximately 100 gram sample of fresh roots" [CO:curators]
is_a: CO_334:0001002 ! Methods
relationship: method_of CO_334:0000447 ! Dry matter content

[Term]
id: CO_334:0010301
name: Visual Scoring: Stem color_method
namespace: CassavaMethod
def: "Visual rating of stem color  nine months after planting" [CO:curators]
is_a: CO_334:0001002 ! Methods
relationship: method_of CO_334:0000475 ! Stem Color

[Term]
id: CO_334:0010302
name: Visual Scoring: Branching angle_method
namespace: CassavaMethod
def: "Visual rating of the angle between a vertical plane and first primary branch. 0 = no branching, 3 = 15-30 degree, 5 = 45-60 degree, 7 = 75-90 degree" [CO:curators]
is_a: CO_334:0001002 ! Methods
relationship: method_of CO_334:0000294 ! Branching Angle

[Term]
id: CO_334:0010303
name: Measurement: Plant height_method
namespace: CassavaMethod
def: "Measured as height from ground level to the top of canopy at harvest" [CO:curators]
is_a: CO_334:0001002 ! Methods
relationship: method_of CO_334:0000432 ! Plant height

[Term]
id: CO_334:0010304
name: Counting: Proportion of lodged plants_method
namespace: CassavaMethod
def: "Proportion of plants lodged at greater than 45 degrees in a plot" [CO:curators]
is_a: CO_334:0001002 ! Methods
relationship: method_of CO_334:0000440 ! Lodged plants

[Term]
id: CO_334:0010305
name: Visual Rating: Leaf retention_method
namespace: CassavaMethod
def: "Visual scoring of leaf retention or longevity" [CO:curators]
is_a: CO_334:0001002 ! Methods
relationship: method_of CO_334:0000396 ! Leaf retention

[Term]
id: CO_334:0010306
name: Visual Rating: Plant architecture_method
namespace: CassavaMethod
def: "Visual scoring of the plant architecture" [CO:curators]
is_a: CO_334:0001002 ! Methods
relationship: method_of CO_334:0000431 ! Plant architecture

[Term]
id: CO_334:0010308
name: Visual Rating: Fruit set _method
namespace: CassavaMethod
def: "Visual rating of presence of fruit set" [CO:curators]
is_a: CO_334:0001002 ! Methods
relationship: method_of CO_334:0000372 ! Fruit set presence

[Term]
id: CO_334:0010309
name: Visual Rating: Storage root peduncle_method
namespace: CassavaMethod
def: "Visual rating of root peduncle length of the plant" [CO:curators]
is_a: CO_334:0001002 ! Methods
relationship: method_of CO_334:0000488 ! Storage Root Peduncle

[Term]
id: CO_334:0010310
name: Visual Rating: Storage root constrictions_method
namespace: CassavaMethod
def: "Visual rating of mature root constrictions" [CO:curators]
is_a: CO_334:0001002 ! Methods
relationship: method_of CO_334:0000485 ! Storage Root Constrictions

[Term]
id: CO_334:0010311
name: Visual Rating: Root surface color_method
namespace: CassavaMethod
def: "Visual rating of root surface color" [CO:curators]
is_a: CO_334:0001002 ! Methods
relationship: method_of CO_334:0000454 ! Storage root surface color

[Term]
id: CO_334:0010312
name: Visual Rating: Root surface texture_method
namespace: CassavaMethod
def: "Visual rating of root surface texture" [CO:curators]
is_a: CO_334:0001002 ! Methods
relationship: method_of CO_334:0000455 ! Storage root surface texture

[Term]
id: CO_334:0010313
name: Estimation: Starch content _method
namespace: CassavaMethod
def: "Estimated percentage of complex carbohydrates or start after extraction from cassava storage root" [CO:curators]
is_a: CO_334:0001002 ! Methods
relationship: method_of CO_334:0000474 ! Starch Content

[Term]
id: CO_334:0010314
name: Estimation: Moisture content_method
namespace: CassavaMethod
def: "Measured percentage of water contained in cassava storage roots at harvest usually estimated as one minus the dry matter content" [CO:curators]
is_a: CO_334:0001002 ! Methods
relationship: method_of CO_334:0000407 ! Moisture content of fresh root

[Term]
id: CO_334:0010315
name: Measurement: Gari content_method
namespace: CassavaMethod
def: "Measured gari content of fresh root tubers" [CO:curators]
is_a: CO_334:0001002 ! Methods
relationship: method_of CO_334:0000374 ! Gari content

[Term]
id: CO_334:0010316
name: Measurement: Stock weight_method
namespace: CassavaMethod
def: "Measurement of the fresh weight of the planted part anchoring the storage root(kg)" [CO:curators]
is_a: CO_334:0001002 ! Methods
relationship: method_of CO_334:0000484 ! Stock weight

[Term]
id: CO_334:0010317
name: Counting: Stem yield_method
namespace: CassavaMethod
def: "Measurement of the fresh weight of harvested plant biomass excluding leaves " [CO:curators]
is_a: CO_334:0001002 ! Methods
relationship: method_of CO_334:0000480 ! Stem weight

[Term]
id: CO_334:0010318
name: Estimation: Dry matter content by specific gravity method
namespace: CassavaMethod
def: "Estimated dry  matter content from the specific gravity value weighted cassava (4-5kg)" [CO:curators]
is_a: CO_334:0001002 ! Methods
relationship: method_of CO_334:0000447 ! Dry matter content

[Term]
id: CO_334:0010319
name: Visual Rating: Total carotenoid by chart_method
namespace: CassavaMethod
def: "Assessment of the level of yellowness in cassava storage root pulp using the tc chart" [CO:curators]
is_a: CO_334:0001002 ! Methods
relationship: method_of CO_334:0000297 ! Carotenoid content

[Term]
id: CO_334:0010320
name: Counting: Non marketable root number_method
namespace: CassavaMethod
def: "Count of the number of small or less than 1kg root size" [CO:curators]
is_a: CO_334:0001002 ! Methods
relationship: method_of CO_334:0000408 ! Non marketable root number

[Term]
id: CO_334:0010321
name: Counting: Marketable root number_method
namespace: CassavaMethod
def: "Count of the number of big or more than 1kg root size" [CO:curators]
is_a: CO_334:0001002 ! Methods
relationship: method_of CO_334:0000405 ! Marketable root number

[Term]
id: CO_334:0010322
name: Visual Rating: Branching_method
namespace: CassavaMethod
def: "Visual scoring of the height of the branches" [CO:curators]
is_a: CO_334:0001002 ! Methods
relationship: method_of CO_334:0000293 ! Branch height

[Term]
id: CO_334:0010323
name: Visual Observation: Red spider mite severity_method
namespace: CassavaMethod
def: "The trait is scored for severity of red spider mite symptoms caused by Oligonychus gossypii and Tetranychus spp." [CO:curators]
is_a: CO_334:0001002 ! Methods
relationship: method_of CO_334:0000444 ! Red spider mite severity

[Term]
id: CO_334:0010324
name: Counting: Red spider mite incidence_method
namespace: CassavaMethod
def: "A ratio of infected plants with red spider mite to total plant stands." [CO:curators]
is_a: CO_334:0001002 ! Methods
relationship: method_of CO_334:0000443 ! Red spider mite incidence

[Term]
id: CO_334:0010325
name: Visual Observation: Spiraling whitefly severity_method
namespace: CassavaMethod
def: "The trait is scored for severity of cassava spiraling whitefly symptoms caused by Aleurodicus dispersus" [CO:curators]
is_a: CO_334:0001002 ! Methods
relationship: method_of CO_334:0000465 ! Spiraling whitefly severity

[Term]
id: CO_334:0010326
name: Counting: Spiraling whitefly incidence_method
namespace: CassavaMethod
def: "A ratio of infected plants with spiraling whitefly to total plant stands." [CO:curators]
is_a: CO_334:0001002 ! Methods
relationship: method_of CO_334:0000464 ! Spiraling whitefly incidence

[Term]
id: CO_334:0010327
name: Counting: Bemisia tabaci adult_method
namespace: CassavaMethod
def: "Counting of the number of Bemisia tabaci adult white flies on the top five leaves." [CO:curators]
is_a: CO_334:0001002 ! Methods
relationship: method_of CO_334:0000410 ! Number of bemisia tabaci adult

[Term]
id: CO_334:0010328
name: Counting: Bemisia tabaci nymphs_method
namespace: CassavaMethod
def: "Counting of the number of Bemisia tabaci nymphs white flies on the 14th leaf." [CO:curators]
is_a: CO_334:0001002 ! Methods
relationship: method_of CO_334:0000411 ! Number of bemisia tabaci nymphs

[Term]
id: CO_334:0010329
name: Calculation: Fresh root yield_method
namespace: CassavaMethod
def: "Calculated as weight of fresh storage roots expressed in tons per hectares per plant at harvest" [CO:curators]
is_a: CO_334:0001002 ! Methods
relationship: method_of CO_334:0000456 ! Root yield

[Term]
id: CO_334:0010330
name: Calculation: Dry yield_method
namespace: CassavaMethod
def: "Dry weight of harvested roots derived by multiplying fresh storage root yield by dry matter content expressed in tons per hectares." [CO:curators]
is_a: CO_334:0001002 ! Methods
relationship: method_of CO_334:0000456 ! Root yield

[Term]
id: CO_334:0010332
name: Calculation: Top yield_method
namespace: CassavaMethod
def: "Calculated as weight of foliage and stems expressed in tons per hectares per plot at harvest" [CO:curators]
is_a: CO_334:0001002 ! Methods
relationship: method_of CO_334:0000456 ! Root yield

[Term]
id: CO_334:0010333
name: Visual Rating: Suitability for intercropping_method
namespace: CassavaMethod
def: "Qualitative rating of compatibility for use in intercroping" [CO:curators]
is_a: CO_334:0001002 ! Methods
relationship: method_of CO_334:0000496 ! Suitability for intercropping

[Term]
id: CO_334:0010334
name: Estimation: Hydrogen cyanide potential enzymatic method
namespace: CassavaMethod
def: "Visual scoring of the root cyanide content evaluated using the enzymatic method" [CO:curators]
is_a: CO_334:0001002 ! Methods
relationship: method_of CO_334:0000502 ! Storage root cyanide content

[Term]
id: CO_334:0010335
name: Visual Rating: Unexpanded apical leaves colors_method
namespace: CassavaMethod
def: "Visual rating of unexpanded apical leaf color." [CO:curators]
is_a: CO_334:0001002 ! Methods
relationship: method_of CO_334:0000389 ! Leaf color

[Term]
id: CO_334:0010336
name: Visual Rating: First fully expanded leaf color_method
namespace: CassavaMethod
def: "Trait monitored by observing the color of first fully expanded leaves" [CO:curators]
is_a: CO_334:0001002 ! Methods
relationship: method_of CO_334:0000389 ! Leaf color

[Term]
id: CO_334:0010337
name: Visual Rating: Leaf vein color_method
namespace: CassavaMethod
def: "Trait monitored by observing the color of  leaf vein" [CO:curators]
is_a: CO_334:0001002 ! Methods
relationship: method_of CO_334:0000401 ! Leaf Vein Color

[Term]
id: CO_334:0010338
name: Visual Rating: Apical pubescence_method
namespace: CassavaMethod
def: "Visual rating of the young leaves pubescence" [CO:curators]
is_a: CO_334:0001002 ! Methods
relationship: method_of CO_334:0000283 ! Apical pubescence

[Term]
id: CO_334:0010339
name: Visual Rating: Stipules length_method
namespace: CassavaMethod
def: "A qualitative scoring of the length of the leaflike appendage at the base of the leaf " [CO:curators]
is_a: CO_334:0001002 ! Methods
relationship: method_of CO_334:0000483 ! Stipules length

[Term]
id: CO_334:0010340
name: Visual Rating: Leaf lobes number_method
namespace: CassavaMethod
def: "Most common number of leaf lobes assessed on five leaves from the middle of the plant at six months after planting." [CO:curators]
is_a: CO_334:0001002 ! Methods
relationship: method_of CO_334:0000395 ! Leaf Lobes Number

[Term]
id: CO_334:0010341
name: Visual Rating: Leaf lobe position_method
namespace: CassavaMethod
def: "Trait monitored by observing the position in which leaf lobes are held" [CO:curators]
is_a: CO_334:0001002 ! Methods
relationship: method_of CO_334:0000393 ! Leaf Lobe Position

[Term]
id: CO_334:0010342
name: Visual Rating: Central leaf shape_method
namespace: CassavaMethod
def: "Trait monitored by observing the leaf shape from a middle-height position." [CO:curators]
is_a: CO_334:0001002 ! Methods
relationship: method_of CO_334:0000353 ! Central Leaf Shape

[Term]
id: CO_334:0010343
name: Visual Rating: Petiole Insertion Angle_method
namespace: CassavaMethod
def: "Trait monitored by observing the angle between branch and petiole" [CO:curators]
is_a: CO_334:0001002 ! Methods
relationship: method_of CO_334:0000428 ! Petiole Insertion Angle

[Term]
id: CO_334:0010344
name: Visual Rating: Petiole Length_method
namespace: CassavaMethod
def: "Visual  rating of the petiole length" [CO:curators]
is_a: CO_334:0001002 ! Methods
relationship: method_of CO_334:0000429 ! Petiole length

[Term]
id: CO_334:0010345
name: Visual Rating: Petiole color_method
namespace: CassavaMethod
def: "Visual rating of petiole color" [CO:curators]
is_a: CO_334:0001002 ! Methods
relationship: method_of CO_334:0000427 ! Petiole Color

[Term]
id: CO_334:0010346
name: Visual Rating: Anthocyanin pigmentation_method
namespace: CassavaMethod
def: "Visual rating of distribution of anthocyanin pigmentation" [CO:curators]
is_a: CO_334:0001002 ! Methods
relationship: method_of CO_334:0000281 ! Anthocyanin pigmentation

[Term]
id: CO_334:0010347
name: Visual Rating: Young stem growth habit_method
namespace: CassavaMethod
def: "Visual rating of growth habit of young stem" [CO:curators]
is_a: CO_334:0001002 ! Methods
relationship: method_of CO_334:0000505 ! Young Stem Growth Habit

[Term]
id: CO_334:0010348
name: Visual Rating: Young stem pubescence_method
namespace: CassavaMethod
def: "Visual rating of young stem pubescence " [CO:curators]
is_a: CO_334:0001002 ! Methods
relationship: method_of CO_334:0000506 ! Young Stem Pubescence

[Term]
id: CO_334:0010349
name: Visual Rating: Leaf scar prominence_method
namespace: CassavaMethod
def: "Visual rating of prominence leaf scars" [CO:curators]
is_a: CO_334:0001002 ! Methods
relationship: method_of CO_334:0000400 ! Leaf Scar Prominence

[Term]
id: CO_334:0010350
name: Visual Rating: Apical branching_method
namespace: CassavaMethod
def: "Count the number of weeks from planting to first apical branching associated with the formation of inflorescence." [CO:curators]
is_a: CO_334:0001002 ! Methods
relationship: method_of CO_334:0000282 ! Apical branching

[Term]
id: CO_334:0010351
name: Counting: Branching levels_method
namespace: CassavaMethod
def: "Count of the actual number of levels of branching at or before harvest." [CO:curators]
is_a: CO_334:0001002 ! Methods
relationship: method_of CO_334:0000296 ! Branching Levels

[Term]
id: CO_334:0010352
name: Measurement: First apical branch height_method
namespace: CassavaMethod
def: "Measured as height from ground level to point of first apical branch" [CO:curators]
is_a: CO_334:0001002 ! Methods
relationship: method_of CO_334:0000293 ! Branch height

[Term]
id: CO_334:0010353
name: Visual Rating: Sepal color_method
namespace: CassavaMethod
def: "Visual rating of sepal color" [CO:curators]
is_a: CO_334:0001002 ! Methods
relationship: method_of CO_334:0000462 ! Sepal Color

[Term]
id: CO_334:0010354
name: Visual Rating: Disc color_method
namespace: CassavaMethod
def: "Visual rating of floral disc color" [CO:curators]
is_a: CO_334:0001002 ! Methods
relationship: method_of CO_334:0000360 ! Disc color

[Term]
id: CO_334:0010355
name: Visual Rating: Stigma color_method
namespace: CassavaMethod
def: "Visual rating of sigma color" [CO:curators]
is_a: CO_334:0001002 ! Methods
relationship: method_of CO_334:0000481 ! Stigma Color

[Term]
id: CO_334:0010356
name: Visual Rating: Ovary color_method
namespace: CassavaMethod
def: "Visual rating of ovary color" [CO:curators]
is_a: CO_334:0001002 ! Methods
relationship: method_of CO_334:0000421 ! Ovary Color

[Term]
id: CO_334:0010357
name: Visual Rating: Anther color_method
namespace: CassavaMethod
def: "Visual rating of anthers color" [CO:curators]
is_a: CO_334:0001002 ! Methods
relationship: method_of CO_334:0000280 ! Anther Color

[Term]
id: CO_334:0010358
name: Visual Rating: Female stamenoids_method
namespace: CassavaMethod
def: "Visual rating of female flowers without rudimentory stamen" [CO:curators]
is_a: CO_334:0001002 ! Methods
relationship: method_of CO_334:0000365 ! Female stamenoids

[Term]
id: CO_334:0010359
name: Visual Rating: Male sterile_method
namespace: CassavaMethod
def: "Visual rating of presence of male pollen" [CO:curators]
is_a: CO_334:0001002 ! Methods
relationship: method_of CO_334:0000404 ! Male sterile

[Term]
id: CO_334:0010360
name: Visual Rating: Fruit exocarp Texture_method
namespace: CassavaMethod
def: "Visual rating of texture of the outer most layer of the cassava fruit" [CO:curators]
is_a: CO_334:0001002 ! Methods
relationship: method_of CO_334:0000371 ! Fruit exocarp texture

[Term]
id: CO_334:0010361
name: Visual Rating: Ploidy_method
namespace: CassavaMethod
def: "Visual rating of the ploidy level" [CO:curators]
is_a: CO_334:0001002 ! Methods
relationship: method_of CO_334:0000436 ! Ploidy

[Term]
id: CO_334:0010362
name: Visual Rating: Seed color_method
namespace: CassavaMethod
def: "Trait monitored by observing the color of  the seed" [CO:curators]
is_a: CO_334:0001002 ! Methods
relationship: method_of CO_334:0000459 ! Seed color

[Term]
id: CO_334:0010363
name: Visual Rating: Caruncle color_method
namespace: CassavaMethod
def: "Visual rating of the caruncle color" [CO:curators]
is_a: CO_334:0001002 ! Methods
relationship: method_of CO_334:0000298 ! Caruncle Color

[Term]
id: CO_334:0010364
name: Visual Rating: Root position_method
namespace: CassavaMethod
def: "Visual rating of root position in the soil" [CO:curators]
is_a: CO_334:0001002 ! Methods
relationship: method_of CO_334:0000453 ! Root Position

[Term]
id: CO_334:0010365
name: Visual Rating: Storage root diameter_method
namespace: CassavaMethod
def: "Visual rating of root diameter" [CO:curators]
is_a: CO_334:0001002 ! Methods
relationship: method_of CO_334:0000487 ! Storage Root Diameter

[Term]
id: CO_334:0010366
name: Estimation: Abscisic acid content_method
namespace: CassavaMethod
def: "Abscisic acid content of leaf sample." [CO:curators]
is_a: CO_334:0001002 ! Methods
relationship: method_of CO_334:0000276 ! Abscisic acid content

[Term]
id: CO_334:0010367
name: Calculation: Leaf life _method
namespace: CassavaMethod
def: "Measures leaf life span estimated as days." [CO:curators]
is_a: CO_334:0001002 ! Methods
relationship: method_of CO_334:0000390 ! Leaf life span

[Term]
id: CO_334:0010368
name: Estimation: Total carotenoid content_method
namespace: CassavaMethod
def: "Total extracted carotenoids in cassava storage root as estimated by spectrophotometer" [CO:curators]
is_a: CO_334:0001002 ! Methods
relationship: method_of CO_334:0000297 ! Carotenoid content

[Term]
id: CO_334:0010369
name: Estimation: Beta carotene_method
namespace: CassavaMethod
def: "Concentration of beta carotene extracted from root samples and estimated by HPLC expressed in ug per gram fresh weight.\n\nFresh cassava roots are ground into a mash and carotenoids are extracted with acetone and petroleum ether. The extracts are analyzed by HPLC with mobile phases (methanol + ammonium acetate) followed by methy-ter-butyl-ether. The resulting peaks are identified and quantified using calibration standards and calibration curve. Concentrations are expressed in ug/g wet basis." [CO:curators]
is_a: CO_334:0001002 ! Methods
relationship: method_of CO_334:0000291 ! Beta carotene

[Term]
id: CO_334:0010370
name: Estimation: Iron content_method
namespace: CassavaMethod
def: "Measured total iron content in cassava storage roots." [CO:curators]
is_a: CO_334:0001002 ! Methods
relationship: method_of CO_334:0000387 ! Iron content

[Term]
id: CO_334:0010371
name: Estimation: Zinc content_method
namespace: CassavaMethod
def: "Measured total zinc content in cassava storage roots." [CO:curators]
is_a: CO_334:0001002 ! Methods
relationship: method_of CO_334:0000507 ! Zinc content

[Term]
id: CO_334:0010372
name: Estimation: Protein content_method
namespace: CassavaMethod
def: "Measured Percentage of protein content in cassava storage roots." [CO:curators]
is_a: CO_334:0001002 ! Methods
relationship: method_of CO_334:0000442 ! Protein content

[Term]
id: CO_334:0010373
name: Estimation: Fibre content_method
namespace: CassavaMethod
def: "Measured part of tuber root that cannot be digested by humans." [CO:curators]
is_a: CO_334:0001002 ! Methods
relationship: method_of CO_334:0000366 ! Fibre content

[Term]
id: CO_334:0010374
name: Estimation: Amylose  content_method
namespace: CassavaMethod
def: "Measured amylose content of cassava roots." [CO:curators]
is_a: CO_334:0001002 ! Methods
relationship: method_of CO_334:0000279 ! Amylose content

[Term]
id: CO_334:0010375
name: Estimation: Amylopectin content_method
namespace: CassavaMethod
def: "Measured amylopectin content of cassava roots." [CO:curators]
is_a: CO_334:0001002 ! Methods
relationship: method_of CO_334:0000277 ! Amylopectin content

[Term]
id: CO_334:0010376
name: Calculation: Amylose amylopectin ratio_method
namespace: CassavaMethod
def: "The amylose content of a cassava root sample divided by the amylopectin content of the same sample" [CO:curators]
is_a: CO_334:0001002 ! Methods
relationship: method_of CO_334:0000278 ! Amylose amylopectin ratio

[Term]
id: CO_334:0010377
name: Estimation: Ascorbic acid_method
namespace: CassavaMethod
def: "Antioxidant and water soluble vitamin of cassava storage root." [CO:curators]
is_a: CO_334:0001002 ! Methods
relationship: method_of CO_334:0000284 ! Ascorbic acid

[Term]
id: CO_334:0010378
name: Estimation: Ash content_method
namespace: CassavaMethod
def: "Residue left behind after all organic matter has been burnt off, a measure of total mineral salts in a food" [CO:curators]
is_a: CO_334:0001002 ! Methods
relationship: method_of CO_334:0000285 ! Ash content

[Term]
id: CO_334:0010379
name: Estimation: Sugar content_method
namespace: CassavaMethod
def: "Sugar content in cassava storage root." [CO:curators]
is_a: CO_334:0001002 ! Methods
relationship: method_of CO_334:0000495 ! Sugar content

[Term]
id: CO_334:0010380
name: Estimation: Fufu content_method
namespace: CassavaMethod
def: "Measured percentage fufu processed from fresh storage roots." [CO:curators]
is_a: CO_334:0001002 ! Methods
relationship: method_of CO_334:0000373 ! Fufu content

[Term]
id: CO_334:0010381
name: Estimation: Lafun content_method
namespace: CassavaMethod
def: "Measured percentage Lafun processed from fresh storage roots." [CO:curators]
is_a: CO_334:0001002 ! Methods
relationship: method_of CO_334:0000388 ! Lafun content

[Term]
id: CO_334:0010382
name: Estimation: Beta carotenoid retention_method
namespace: CassavaMethod
def: "Measured percentage of beta carotene content in a prepared food product compared to the nutrient content in the raw food." [CO:curators]
is_a: CO_334:0001002 ! Methods
relationship: method_of CO_334:0000292 ! Beta carotenoid retention

[Term]
id: CO_334:0010383
name: Estimation: Total carotenoid retention_method
namespace: CassavaMethod
def: "Measured percentage of total carotene content in a prepared food product compared to the nutrient content in the raw food." [CO:curators]
is_a: CO_334:0001002 ! Methods
relationship: method_of CO_334:0000500 ! Total carotenoid retention

[Term]
id: CO_334:0010384
name: Measurement: Plant height without leaf_method
namespace: CassavaMethod
def: "Measured stem portion without leaf in centimeter" [CO:curators]
is_a: CO_334:0001002 ! Methods
relationship: method_of CO_334:0000478 ! Stem height

[Term]
id: CO_334:0010385
name: Measurement: Plantable stem_method
namespace: CassavaMethod
def: "Measured stem portion above the stump comprising the hardwood,semi hardwood upper shoot portion but excluding the immature greenish shoot portion" [CO:curators]
is_a: CO_334:0001002 ! Methods
relationship: method_of CO_334:0000435 ! Plantable stem length

[Term]
id: CO_334:0010386
name: Measurement: Stem weight_method
namespace: CassavaMethod
def: "Measured stem weight excluding leaves and stump." [CO:curators]
is_a: CO_334:0001002 ! Methods
relationship: method_of CO_334:0000480 ! Stem weight

[Term]
id: CO_334:0010387
name: Measurement: Average stem length_method
namespace: CassavaMethod
def: "Measured total stem length per plot or per number of plant stands" [CO:curators]
is_a: CO_334:0001002 ! Methods
relationship: method_of CO_334:0000478 ! Stem height

[Term]
id: CO_334:0010388
name: Counting: Stem number_method
namespace: CassavaMethod
def: "Count of the number of stems per plot" [CO:curators]
is_a: CO_334:0001002 ! Methods
relationship: method_of CO_334:0000479 ! Stem number

[Term]
id: CO_334:0010389
name: Measurement: Tip shoot weight_method
namespace: CassavaMethod
def: "Measured weight of tip shoot portion of the stem" [CO:curators]
is_a: CO_334:0001002 ! Methods
relationship: method_of CO_334:0000499 ! Tip shoot weight

[Term]
id: CO_334:0010390
name: Measurement: Marketable root weight_method
namespace: CassavaMethod
def: "Measured weight of harvested cassava roots usually classified as large size and medium size excluding small sized roots" [CO:curators]
is_a: CO_334:0001002 ! Methods
relationship: method_of CO_334:0000406 ! Marketable root weight

[Term]
id: CO_334:0010391
name: Measurement: Non marketable root weight_method
namespace: CassavaMethod
def: "Measured weight of harvested cassava roots (small sized roots)" [CO:curators]
is_a: CO_334:0001002 ! Methods
relationship: method_of CO_334:0000409 ! Non marketable root weight

[Term]
id: CO_334:0010392
name: Counting: Stem rot_method
namespace: CassavaMethod
def: "Count of the rotted stems per plot at the time of harvest" [CO:curators]
is_a: CO_334:0001002 ! Methods
relationship: method_of CO_334:0000417 ! Number of rotten stem

[Term]
id: CO_334:0010393
name: Measurement: Leaf weight_method
namespace: CassavaMethod
def: "Measure weight of fresh foliage leaf with above ground biomass excuding the stem" [CO:curators]
is_a: CO_334:0001002 ! Methods
relationship: method_of CO_334:0000402 ! Leaf weight

[Term]
id: CO_334:0010394
name: Measurement: Stump weight_method
namespace: CassavaMethod
def: "Measured fresh weight of plant parts at soil level from the neck of the root to the beginning of the plantable stem" [CO:curators]
is_a: CO_334:0001002 ! Methods
relationship: method_of CO_334:0000494 ! Stump weight

[Term]
id: CO_334:0010395
name: Counting: Leaf scar number_method
namespace: CassavaMethod
def: "Count of the leaf scars on the main stem" [CO:curators]
is_a: CO_334:0001002 ! Methods
relationship: method_of CO_334:0000399 ! Leaf scar number

[Term]
id: CO_334:0010396
name: Measurement: Leaf scar level_method
namespace: CassavaMethod
def: "Measured height from ground level to the lowest retained leaf on the main stem" [CO:curators]
is_a: CO_334:0001002 ! Methods
relationship: method_of CO_334:0000398 ! Leaf scar height

[Term]
id: CO_334:0010397
name: Visual Rating: Branching habit_method
namespace: CassavaMethod
def: "Rating of the branching habit of the lowest branching " [CO:curators]
is_a: CO_334:0001002 ! Methods
relationship: method_of CO_334:0000295 ! Branching habit

[Term]
id: CO_334:0010398
name: Visual Observation: Days to 50% branching_method
namespace: CassavaMethod
def: "Visual observation at 50% of the plant stand per plot branches(dd/mm/yyyy)" [CO:curators]
is_a: CO_334:0001002 ! Methods
relationship: method_of CO_334:0000357 ! Days to 50% branching

[Term]
id: CO_334:0010399
name: Visual Observation: Days to first inflorescence_method
namespace: CassavaMethod
def: "Observation of the appearance of developing inflorescence on a plant or plot" [CO:curators]
is_a: CO_334:0001002 ! Methods
relationship: method_of CO_334:0000359 ! Days to first inflorescence

[Term]
id: CO_334:0010400
name: Counting: Female flower number_method
namespace: CassavaMethod
def: "Count of the number of female flowers after the buds appear,mature, and grow in size to become distinctive at first,second and third branch levels" [CO:curators]
is_a: CO_334:0001002 ! Methods
relationship: method_of CO_334:0000364 ! Female flower number

[Term]
id: CO_334:0010401
name: Counting: Male flower number_method
namespace: CassavaMethod
def: "Count of the number of male flowers after the buds appear,mature, and grow in size to become distinctive at first,second and third branch levels" [CO:curators]
is_a: CO_334:0001002 ! Methods
relationship: method_of CO_334:0000403 ! Male flower number

[Term]
id: CO_334:0010402
name: Counting: Number of flowering stalks per branch level _method
namespace: CassavaMethod
def: "Count of the number of stalks carrying the buds at every point of branching where inflorescence starts" [CO:curators]
is_a: CO_334:0001002 ! Methods
relationship: method_of CO_334:0000412 ! Number of flowering stalks

[Term]
id: CO_334:0010403
name: Counting: Number of forks_method
namespace: CassavaMethod
def: "A count of the number of branches (2 forks/branches (dichotomous), 3 forks/branches (trichotomous), or 4 forks/branches (tetrachotomous)) at every branching level." [CO:curators]
is_a: CO_334:0001002 ! Methods
relationship: method_of CO_334:0000413 ! Number of  forks

[Term]
id: CO_334:0010404
name: Visual Observation: Days to first anthesis_method
namespace: CassavaMethod
def: "Duration from planting to first anthesis derived as the date of observation of the first female flower to expose pistil is visually observed minus the date of planting" [CO:curators]
is_a: CO_334:0001002 ! Methods
relationship: method_of CO_334:0000358 ! Days to first anthesis

[Term]
id: CO_334:0010405
name: Visual Observation: Days to 50% anthesis_method
namespace: CassavaMethod
def: "Duration from planting to first anthesis derived as the date of observation of 50% of the female flowers exposing pistil minus the date of planting" [CO:curators]
is_a: CO_334:0001002 ! Methods
relationship: method_of CO_334:0000356 ! Days to 50% anthesis

[Term]
id: CO_334:0010406
name: Counting: Number of fruitset_method
namespace: CassavaMethod
def: "Count of number of fruits formed from the seeds after pollination" [CO:curators]
is_a: CO_334:0001002 ! Methods
relationship: method_of CO_334:0000415 ! Number of fruitset

[Term]
id: CO_334:0010407
name: Counting: Bemisia tabaci nymphs yellow_method
namespace: CassavaMethod
def: "Count of the number of number of yellow bemisia tabaci nymphs on 14th leaf on the same tallest shoot" [CO:curators]
is_a: CO_334:0001002 ! Methods
relationship: method_of CO_334:0000290 ! Bemisia tabaci nymphs yellow

[Term]
id: CO_334:0010408
name: Counting: Bemisia tabaci nymphs black_method
namespace: CassavaMethod
def: "Count of the number of number of black bemisia tabaci nymphs on 14th leaf on the same tallest shoot" [CO:curators]
is_a: CO_334:0001002 ! Methods
relationship: method_of CO_334:0000288 ! Bemisia tabaci nymphs black

[Term]
id: CO_334:0010409
name: Visual Observation: Bemisia tabaci nymphs severity_method
namespace: CassavaMethod
def: "Visual rating of chlorotic blotches infestation on leaves caused by white fly" [CO:curators]
is_a: CO_334:0001002 ! Methods
relationship: method_of CO_334:0000289 ! Bemisia tabaci nymphs severity

[Term]
id: CO_334:0010410
name: Visual Observation: Typhlodromalus aripo_method
namespace: CassavaMethod
def: "Visual observation of the presence of t.aripo" [CO:curators]
is_a: CO_334:0001002 ! Methods
relationship: method_of CO_334:0000503 ! Typhlodromalus aripo

[Term]
id: CO_334:0010411
name: Counting: Plant number with inflorescence_method
namespace: CassavaMethod
def: "Proportion of plant per plot with inflorescence at varying growth stages including pollinated and unpollinated flowers" [CO:curators]
is_a: CO_334:0001002 ! Methods
relationship: method_of CO_334:0000441 ! Proportion of plant with inflorescence

[Term]
id: CO_334:0010412
name: Counting: Number of terminal branches with inflorescence_method
namespace: CassavaMethod
def: "The maximum number of terminal branches with inflorescence observed at all levels of branching in a plot" [CO:curators]
is_a: CO_334:0001002 ! Methods
relationship: method_of CO_334:0000420 ! Number of terminal branches with inflorescence

[Term]
id: CO_334:0010413
name: Counting: Number of fruits _method
namespace: CassavaMethod
def: "Count of the number of fruits observed at all levels of branching per plot" [CO:curators]
is_a: CO_334:0001002 ! Methods
relationship: method_of CO_334:0000414 ! Number of fruits

[Term]
id: CO_334:0010414
name: Estimation: Total carotenoid by icheck method
namespace: CassavaMethod
def: "Measurement of total carotenoid content in a giving cassava storage root sample using icheck kits or device" [CO:curators]
is_a: CO_334:0001002 ! Methods
relationship: method_of CO_334:0000297 ! Carotenoid content

[Term]
id: CO_334:0010415
name: Measurement: Root weight in air_method
namespace: CassavaMethod
def: "Measured weight of cassava root samples (kg) between 4 - 5kg of each of the harvested plot to determine the dry matter by specific gravity" [CO:curators]
is_a: CO_334:0001002 ! Methods
relationship: method_of CO_334:0000493 ! Storage root weight

[Term]
id: CO_334:0010416
name: Measurement: Root weight in water_method
namespace: CassavaMethod
def: "As part of the dry matter determination method by specific gravimetry, suspend in water the root sample initially weighed in air and then weigh." [CO:curators]
is_a: CO_334:0001002 ! Methods
relationship: method_of CO_334:0000493 ! Storage root weight

[Term]
id: CO_334:0010417
name: Measurement: Specific gravity_method
namespace: CassavaMethod
def: "Estimated value obtained by weighing 4-5kg of cassava in air and in water" [CO:curators]
is_a: CO_334:0001002 ! Methods
relationship: method_of CO_334:0000447 ! Dry matter content

[Term]
id: CO_334:0010418
name: Measurement: Leaf lobe length_method
namespace: CassavaMethod
def: "Measured length of the middle finger or lobe of matured leaf" [CO:curators]
is_a: CO_334:0001002 ! Methods
relationship: method_of CO_334:0000391 ! Leaf lobe length

[Term]
id: CO_334:0010419
name: Measurement: Leaf lobe width_method
namespace: CassavaMethod
def: "Measured width of the middle finger or lobe of matured leaf" [CO:curators]
is_a: CO_334:0001002 ! Methods
relationship: method_of CO_334:0000394 ! Leaf lobe width

[Term]
id: CO_334:0010420
name: Counting: Germination count_method
namespace: CassavaMethod
def: "Count of the number of emerging seedlings from each family in the pre-nursery done on a daily bases until its ready for transplanting" [CO:curators]
is_a: CO_334:0001002 ! Methods
relationship: method_of CO_334:0000460 ! Seedling number

[Term]
id: CO_334:0010421
name: Counting: Number of seeds sown_method
namespace: CassavaMethod
def: "Count of the number of seeds sown per family in the pre-nursery or directly in the nursery bed" [CO:curators]
is_a: CO_334:0001002 ! Methods
relationship: method_of CO_334:0000418 ! Number of seeds sown

[Term]
id: CO_334:0010422
name: Estimation: Trans 9_method
namespace: CassavaMethod
def: "Estimation of beta carotenoid components with 100% proVitamin A activity" [CO:curators]
is_a: CO_334:0001002 ! Methods
relationship: method_of CO_334:0000501 ! Trans-9 activity

[Term]
id: CO_334:0010423
name: Estimation: Cis 9_method
namespace: CassavaMethod
def: "Estimation of isomer activity with 50%  proVitamin A" [CO:curators]
is_a: CO_334:0001002 ! Methods
relationship: method_of CO_334:0000354 ! Cis 9 activity

[Term]
id: CO_334:0010424
name: Estimation: B crypto_method
namespace: CassavaMethod
def: "Estimation of  b-cryptoxanthin (carotenoid that has hydroxyl group with 50% activity " [CO:curators]
is_a: CO_334:0001002 ! Methods
relationship: method_of CO_334:0000287 ! B crypto activity

[Term]
id: CO_334:0010425
name: Sensory Assesment: Ease of harvest_method
namespace: CassavaMethod
def: "Rating of the difficulty in pulling the plants from the ground during harvesting" [CO:curators]
is_a: CO_334:0001002 ! Methods
relationship: method_of CO_334:0000361 ! Ease of harvest

[Term]
id: CO_334:0010426
name: Visual Rating: Root length evaluation_method
namespace: CassavaMethod
def: "Visual assessment of the root length" [CO:curators]
is_a: CO_334:0001002 ! Methods
relationship: method_of CO_334:0000450 ! Root length

[Term]
id: CO_334:0010427
name: Visual Rating: Stalk average length evaluation_method
namespace: CassavaMethod
def: "Visual assessment of the average length of the stalks" [CO:curators]
is_a: CO_334:0001002 ! Methods
relationship: method_of CO_334:0000473 ! Stalk length

[Term]
id: CO_334:0010428
name: Visual rating: Root constriction_method
namespace: CassavaMethod
def: "Visual rating of root constrictions, as evaluated by CIAT" [CO:curators]
is_a: CO_334:0001002 ! Methods
relationship: method_of CO_334:0000446 ! Root constrictions number

[Term]
id: CO_334:0010429
name: Visual Rating: Root evaluation_method
namespace: CassavaMethod
def: "An evaluation of the integration of root shape, size, diameter, constriction, neck length on a scale. Before scoring the roots, the field technician walks the harvested plot to get an idea of the average root type of the trial which will then be used as the middle level of the scale. Genotypes better than average will be scored with scale levels lower than the middle level. Similiar genotype that are certainly worse compared to the average score are rated with levels higher than the middle level. Trait description is provided by Hernan Ceballos of CIAT" [CO:curators]
is_a: CO_334:0001002 ! Methods
relationship: method_of CO_334:0000448 ! Root evaluation

[Term]
id: CO_334:0010430
name: Calculation: Percent of rotten roots_method
namespace: CassavaMethod
def: "Number of rotten storage root relative to the storage root harvested in a plot estimated in percentage (%)" [CO:curators]
is_a: CO_334:0001002 ! Methods
relationship: method_of CO_334:0000458 ! Rotten root proportion

[Term]
id: CO_334:0010431
name: Estimation: Plant yield_method
namespace: CassavaMethod
def: "Average yield per plant in a plot. It is estimated by dividing the total weight of roots by the number of plants harvested." [CO:curators]
is_a: CO_334:0001002 ! Methods
relationship: method_of CO_334:0000456 ! Root yield

[Term]
id: CO_334:0010432
name: Estimation: Yield per year_method
namespace: CassavaMethod
def: "Annual root yield using yield per hectare as a function of the crop duration." [CO:curators]
is_a: CO_334:0001002 ! Methods
relationship: method_of CO_334:0000456 ! Root yield

[Term]
id: CO_334:0010433
name: Selection: Selected variety_method
namespace: CassavaMethod
def: "Report whether the variety has been selected or not" [CO:curators]
is_a: CO_334:0001002 ! Methods
relationship: method_of CO_334:0000461 ! Selected variety

[Term]
id: CO_334:0010434
name: Visual Observation: Flowering_method
namespace: CassavaMethod
def: "Rate the abundance of flowers on a plant" [CO:curators]
is_a: CO_334:0001002 ! Methods
relationship: method_of CO_334:0000367 ! Flowering

[Term]
id: CO_334:0010435
name: Visual Rating: Initial plant vigor_method
namespace: CassavaMethod
def: "Visual assessment of plant vigor during establishment as evaluated by CIAT" [CO:curators]
is_a: CO_334:0001002 ! Methods
relationship: method_of CO_334:0000386 ! Initial vigor

[Term]
id: CO_334:0010436
name: Visual Rating: Root color_method
namespace: CassavaMethod
def: "Visual rating of storage root surface color as evaluated by CIAT" [CO:curators]
is_a: CO_334:0001002 ! Methods
relationship: method_of CO_334:0000454 ! Storage root surface color

[Term]
id: CO_334:0010437
name: Visual Rating: Root flesh color_method
namespace: CassavaMethod
def: "Visual rating of root pulp color as evaluated by CIAT" [CO:curators]
is_a: CO_334:0001002 ! Methods
relationship: method_of CO_334:0000490 ! Storage Root Pulp Color

[Term]
id: CO_334:0010438
name: Visual Rating: Root neck length_method
namespace: CassavaMethod
def: "Visual rating of root neck length as evaluated by CIAT" [CO:curators]
is_a: CO_334:0001002 ! Methods
relationship: method_of CO_334:0000451 ! Storage root neck length

[Term]
id: CO_334:0010439
name: Visual Rating: Female flower evaluation_method
namespace: CassavaMethod
def: "Visual rating of the abundance of female flowers present at all branching levels on a plant stand on per plot basis" [CO:curators]
is_a: CO_334:0001002 ! Methods
relationship: method_of CO_334:0000364 ! Female flower number

[Term]
id: CO_334:0010440
name: Visual Rating: Staygreen_method
namespace: CassavaMethod
def: "Visual rating of leaf retention or longevity" [CO:curators]
is_a: CO_334:0001002 ! Methods
relationship: method_of CO_334:0000396 ! Leaf retention

[Term]
id: CO_334:0010441
name: Counting: Flowering incidence_method
namespace: CassavaMethod
def: "Proportion of the number of female flowers in a plot to the number of plant stand in the plot" [CO:curators]
is_a: CO_334:0001002 ! Methods
relationship: method_of CO_334:0000439 ! Proportion of female flower

[Term]
id: CO_334:0010442
name: Visual Observation: Hairiness_method
namespace: CassavaMethod
def: "Rating of the level of pubescence on the growing part. It is a proportion of tissue covered by hair on the tip leaves." [CO:curators]
is_a: CO_334:0001002 ! Methods
relationship: method_of CO_334:0000382 ! Hairiness

[Term]
id: CO_334:0010443
name: Visual Observation: Sooty mould_method
namespace: CassavaMethod
def: "Rating of the proportion of black mould on the lower leaves" [CO:curators]
is_a: CO_334:0001002 ! Methods
relationship: method_of CO_334:0000463 ! Sooty mould

[Term]
id: CO_334:0010444
name: Measurement: Root weight after washing_method
namespace: CassavaMethod
def: "Fresh cassava roots are washed in water and weighed on a pan suspended to a weighing scale" [CO:curators]
is_a: CO_334:0001002 ! Methods
relationship: method_of CO_334:0000493 ! Storage root weight

[Term]
id: CO_334:0010445
name: Measurement: Root weight after peel_method
namespace: CassavaMethod
def: "This is the weight of peeled cassava roots using a pan suspended to a weighing scale" [CO:curators]
is_a: CO_334:0001002 ! Methods
relationship: method_of CO_334:0000493 ! Storage root weight

[Term]
id: CO_334:0010446
name: Measurement: Peel weight_method
namespace: CassavaMethod
def: "The weight of the peels (outer and inner skin) removed from the fresh root cassava using salter scale." [CO:curators]
is_a: CO_334:0001002 ! Methods
relationship: method_of CO_334:0000422 ! Peel weight

[Term]
id: CO_334:0010447
name: Measurement: Gari weight after grinding_method
namespace: CassavaMethod
def: "Weighing of the grated cassava before fermentation in jute bags" [CO:curators]
is_a: CO_334:0001002 ! Methods
relationship: method_of CO_334:0000377 ! Gari weight after grinding

[Term]
id: CO_334:0010448
name: Measurement: Weight of mashed cassava cake_method
namespace: CassavaMethod
def: "Weigh the cassava cake after pressing and dehydrating using hydraulic press" [CO:curators]
is_a: CO_334:0001002 ! Methods
relationship: method_of CO_334:0000504 ! Weight of mashed cassava cake

[Term]
id: CO_334:0010449
name: Measurement: Gari shaft weight_method
namespace: CassavaMethod
def: "Weighing of the residues after sieving the roasted gari" [CO:curators]
is_a: CO_334:0001002 ! Methods
relationship: method_of CO_334:0000375 ! Gari chaff weight

[Term]
id: CO_334:0010450
name: Measurement: Gari sampled weight_method
namespace: CassavaMethod
def: "Sample of gari weighed before and after frying usually for experimental purposes" [CO:curators]
is_a: CO_334:0001002 ! Methods
relationship: method_of CO_334:0000379 ! Gari sampled weight

[Term]
id: CO_334:0010451
name: Measurement: Gari weight after drying_method
namespace: CassavaMethod
def: "Weight of cassava after drying using the frying pan" [CO:curators]
is_a: CO_334:0001002 ! Methods
relationship: method_of CO_334:0000376 ! Gari weight after drying

[Term]
id: CO_334:0010452
name: Estimation: Gari starch_method
namespace: CassavaMethod
def: "Percentage of starch compostion of gari. This is done locally by using hydraulic jerk to press the gari while it is fresh after grating." [CO:curators]
is_a: CO_334:0001002 ! Methods
relationship: method_of CO_334:0000380 ! Gari starch

[Term]
id: CO_334:0010453
name: Sensory Assesment: Gari fibre_method
namespace: CassavaMethod
def: "Sensory assessment of the fibre content after the fried gary is locally sieved and milled and then prepared as eba (a popular dish in Nigeria)." [CO:curators]
is_a: CO_334:0001002 ! Methods
relationship: method_of CO_334:0000378 ! Gari fibre

[Term]
id: CO_334:0010454
name: Gustation: Gari taste_method
namespace: CassavaMethod
def: "Culinary assessment of the taste of gari" [CO:curators]
is_a: CO_334:0001002 ! Methods
relationship: method_of CO_334:0000381 ! Gari taste

[Term]
id: CO_334:0010455
name: Visual Rating: Swelling capacity_method
namespace: CassavaMethod
def: "Visual assessment of the increment in quantity when water is added to the gari" [CO:curators]
is_a: CO_334:0001002 ! Methods
relationship: method_of CO_334:0000497 ! Gari swelling capacity

[Term]
id: CO_334:0010456
name: Counting: Number of stakes_method
namespace: CassavaMethod
def: "An estimated number of plantable stakes (about 20cm long, with approximately six nodes) that can be made out of the total number of stems in a plot" [CO:curators]
is_a: CO_334:0001002 ! Methods
relationship: method_of CO_334:0000419 ! Number of stakes

[Term]
id: CO_334:0010457
name: Estimation: Percentage leaf retention_method
namespace: CassavaMethod
def: "An estimation of the percentage stem length with retained leaf measured in percentage (%) using a representative plant stand in a plot" [CO:curators]
is_a: CO_334:0001002 ! Methods
relationship: method_of CO_334:0000396 ! Leaf retention

[Term]
id: CO_334:0010458
name: Estimation: Percentage leaf retention at 5 months after planting_method
namespace: CassavaMethod
def: "An estimation of the percentage stem length with retained leaf measured in percentage (%) using a representative plant stand in a plot, between 5 to 6 months after planting" [CO:curators]
is_a: CO_334:0001002 ! Methods
relationship: method_of CO_334:0000396 ! Leaf retention

[Term]
id: CO_334:0010459
name: Estimation: Percentage leaf retention at 6 months after planting_method
namespace: CassavaMethod
def: "An estimation of the percentage stem length with retained leaf measured in percentage (%) using a representative plant stand in a plot, between 6 to 7 months after planting" [CO:curators]
is_a: CO_334:0001002 ! Methods
relationship: method_of CO_334:0000396 ! Leaf retention

[Term]
id: CO_334:0010460
name: Estimation: Percentage leaf retention at 7 months after planting_method
namespace: CassavaMethod
def: "An estimation of the percentage stem length with retained leaf measured in percentage (%) using a representative plant stand in a plot, between 7 to 8 months after planting" [CO:curators]
is_a: CO_334:0001002 ! Methods
relationship: method_of CO_334:0000396 ! Leaf retention

[Term]
id: CO_334:0010461
name: Estimation: Leaf retention at harvest_method
namespace: CassavaMethod
def: "An estimation of the percentage stem length with retained leaf measured in percentage (%) using a representative plant stand in a plot, at harvest" [CO:curators]
is_a: CO_334:0001002 ! Methods
relationship: method_of CO_334:0000396 ! Leaf retention

[Term]
id: CO_334:0010462
name: Visual Observation: Assessment of presence of leaf pubescence_method
namespace: CassavaMethod
def: "Assessment of the young leaf pubescence . Record whether apical leaves most frequently have or do not have hairs." [CO:curators]
is_a: CO_334:0001002 ! Methods
relationship: method_of CO_334:0000283 ! Apical pubescence

[Term]
id: CO_334:0010463
name: Visual Observation: Leaf lobe margin_method
namespace: CassavaMethod
def: "Observe from the middle third of the plant. Record the most frequently observed leaf margin shape" [CO:curators]
is_a: CO_334:0001002 ! Methods
relationship: method_of CO_334:0000392 ! Leaf lobe margin

[Term]
id: CO_334:0010464
name: Measurement: Petiole length_method
namespace: CassavaMethod
def: "Observe from the middle third of the plant. Measure two leaves per plant. Expressed in centimeter (cm)" [CO:curators]
is_a: CO_334:0001002 ! Methods
relationship: method_of CO_334:0000429 ! Petiole length

[Term]
id: CO_334:0010465
name: Visual Observation: Petiole orientation_method
namespace: CassavaMethod
def: "Visual observation of petiole orientation. Observe from the middle of the plant, take a general picture across the row. No intermediates allowed." [CO:curators]
is_a: CO_334:0001002 ! Methods
relationship: method_of CO_334:0000430 ! Petiole orientation

[Term]
id: CO_334:0010466
name: Visual Observation: Presence of pollen_method
namespace: CassavaMethod
def: "Visual rating of the presence of pollen at the same time of flowering" [CO:curators]
is_a: CO_334:0001002 ! Methods
relationship: method_of CO_334:0000438 ! Presence of pollen

[Term]
id: CO_334:0010467
name: Visual Scoring: Stem cortex color_method
namespace: CassavaMethod
def: "Visual scoring of stem color. Observe from the middle third of the plant. Make a small shallow cut and peel back the epidermis" [CO:curators]
is_a: CO_334:0001002 ! Methods
relationship: method_of CO_334:0000476 ! Stem cortex color

[Term]
id: CO_334:0010468
name: Visual Scoring: Stem epidermis color_method
namespace: CassavaMethod
def: "Visual scoring of stem color. Peel epidermis back and look at underside of epidermis(skin)." [CO:curators]
is_a: CO_334:0001002 ! Methods
relationship: method_of CO_334:0000477 ! Stem epidermis color

[Term]
id: CO_334:0010469
name: Visual Rating: Leaf scar distance_method
namespace: CassavaMethod
def: "Scoring of the distance between leaf scars. Measured from the middle of stem on the middle third of the plant, where the scars are not flat. Make a measurement along the stem then divide the distance by the number of nodes in the measured part. Avoid taking measurement on mealy bug infected plants." [CO:curators]
is_a: CO_334:0001002 ! Methods
relationship: method_of CO_334:0000397 ! Leaf scar distance

[Term]
id: CO_334:0010470
name: Visual Observation: Plant shape_method
namespace: CassavaMethod
def: "Visual assessment of the shape of plant. Record the most observed shape on the plot." [CO:curators]
is_a: CO_334:0001002 ! Methods
relationship: method_of CO_334:0000433 ! Plant shape

[Term]
id: CO_334:0010471
name: Visual Observation: Stipule margin_method
namespace: CassavaMethod
def: "Observe the shape of the stipule margin shapes from the upper third of the plants and record the most frequent occurence. No intermediates is allowed." [CO:curators]
is_a: CO_334:0001002 ! Methods
relationship: method_of CO_334:0000482 ! Stipule margin

[Term]
id: CO_334:0010472
name: Measurement: Peel thickness_method
namespace: CassavaMethod
def: "Measurement of peel thickness using vernier caliper" []
is_a: CO_334:0001002 ! Methods

[Term]
id: CO_334:0010473
name: Visual Rating: In-ground storability_method
namespace: CassavaMethod
def: "Visual rating of the duration of underground storage of cassava roots without sig of deterioration or rot" []
is_a: CO_334:0001002 ! Methods

[Term]
id: CO_334:0010474
name: Visual Rating: Early bulking_method
namespace: CassavaMethod
def: "Visual rating of the assessment of time taken for storage root to begin to accumulate and store starch" []
is_a: CO_334:0001002 ! Methods

[Term]
id: CO_334:0010475
name: Visual Rating: Weed tolerance_method
namespace: CassavaMethod
def: "Visual rating of the ability of palnt to withstand weed infestation without or with minimal effect." []
is_a: CO_334:0001002 ! Methods

[Term]
id: CO_334:0010476
name: Visual Rating: Yield rating_method
namespace: CassavaMethod
def: "Visual rating of the yield of freshly harvested cassava root." []
xref: CO:curators
is_a: CO_334:0001002 ! Methods
relationship: method_of CO_334:0000456 ! Root yield

[Term]
id: CO_334:0010477
name: Visual Rating: Dry matter rating_method
namespace: CassavaMethod
def: "Visual rating of the dry matter content of fresh cassava root." []
xref: CO:curators
is_a: CO_334:0001002 ! Methods
relationship: method_of CO_334:0000424 ! Root dry matter content

[Term]
id: CO_334:0010478
name: Measurement: Fufu initial weight_method
namespace: CassavaMethod
def: "Weigh root sample before processing into fufu" []
xref: CO:curators
is_a: CO_334:0001002 ! Methods
relationship: method_of CO_334:0000373 ! Fufu content

[Term]
id: CO_334:0010479
name: Measurement: Fufu peel weight_method
namespace: CassavaMethod
def: "Weigh cassava root peels before processing into fufu." []
xref: CO:curators
is_a: CO_334:0001002 ! Methods
relationship: method_of CO_334:0000373 ! Fufu content

[Term]
id: CO_334:0010480
name: Measurement: Fufu peeled root weight_method
namespace: CassavaMethod
def: "Weigh cassava roots after peeling for proocessing fufu." []
xref: CO:curators
is_a: CO_334:0001002 ! Methods
relationship: method_of CO_334:0000373 ! Fufu content

[Term]
id: CO_334:0010481
name: Measurement: Fufu fibre weight_method
namespace: CassavaMethod
def: "Weigh oven dired fibre after washing soaked root for fufu." []
xref: CO:curators
is_a: CO_334:0001002 ! Methods
relationship: method_of CO_334:0000373 ! Fufu content

[Term]
id: CO_334:0010482
name: Measurement: Fufu mash weight_method
namespace: CassavaMethod
def: "Weigh cassava roots after grinding for processing fufu." []
xref: CO:curators
is_a: CO_334:0001002 ! Methods
relationship: method_of CO_334:0000373 ! Fufu content

[Term]
id: CO_334:0010483
name: Measurement: Fufu pressed weight_method
namespace: CassavaMethod
def: "Weigh pressed cassava mash." []
xref: CO:curators
is_a: CO_334:0001002 ! Methods
relationship: method_of CO_334:0000373 ! Fufu content

[Term]
id: CO_334:0010484
name: Measurement: Fufu dry weight_method
namespace: CassavaMethod
def: "Weigh oven dried fufu" []
xref: CO:curators
is_a: CO_334:0001002 ! Methods
relationship: method_of CO_334:0000373 ! Fufu content

[Term]
id: CO_334:0010485
name: Measurement: Gari initial weight_method
namespace: CassavaMethod
def: "Weigh sample roots before processing into gari" []
xref: CO:curators
is_a: CO_334:0001002 ! Methods
relationship: method_of CO_334:0000374 ! Gari content

[Term]
id: CO_334:0010486
name: Measurement: Gari peel weight_method
namespace: CassavaMethod
def: "Weigh cassva root peels before processing into gari." []
xref: CO:curators
is_a: CO_334:0001002 ! Methods
relationship: method_of CO_334:0000374 ! Gari content

[Term]
id: CO_334:0010487
name: Measurement: Gari peeled root weight_method
namespace: CassavaMethod
def: "Weigh peeled cassava roots before processing into gari." []
xref: CO:curators
is_a: CO_334:0001002 ! Methods
relationship: method_of CO_334:0000374 ! Gari content

[Term]
id: CO_334:0010488
name: Measurement: Gari mash weight_method
namespace: CassavaMethod
def: "Weigh grinded roots (mash) to be processed into gari." []
xref: CO:curators
is_a: CO_334:0001002 ! Methods
relationship: method_of CO_334:0000374 ! Gari content

[Term]
id: CO_334:0010489
name: Measurement: Gari pressed weight_method
namespace: CassavaMethod
def: "Weigh pressed mash (grinded root)." []
xref: CO:curators
is_a: CO_334:0001002 ! Methods
relationship: method_of CO_334:0000374 ! Gari content

[Term]
id: CO_334:0010490
name: Measurement: Gari pulverised weight_method
namespace: CassavaMethod
def: "Weigh mashed (grinded) pulverised cassava root." []
xref: CO:curators
is_a: CO_334:0001002 ! Methods
relationship: method_of CO_334:0000374 ! Gari content

[Term]
id: CO_334:0010491
name: Measurement: Gari fried weight_method
namespace: CassavaMethod
def: "Weigh gari after frying and sieving." []
xref: CO:curators
is_a: CO_334:0001002 ! Methods
relationship: method_of CO_334:0000374 ! Gari content

[Term]
id: CO_334:0010492
name: Measurement: Gari shaft weight coarse_method
namespace: CassavaMethod
def: "Weigh gari shaft using coarse sieve." []
xref: CO:curators
is_a: CO_334:0001002 ! Methods
relationship: method_of CO_334:0000375 ! Gari chaff weight

[Term]
id: CO_334:0010493
name: Measurement: Gari shaft weight medium_method
namespace: CassavaMethod
def: "Weigh gari shaft using medium sieve." []
xref: CO:curators
is_a: CO_334:0001002 ! Methods
relationship: method_of CO_334:0000375 ! Gari chaff weight

[Term]
id: CO_334:0010494
name: Calculation: Plot volume_method
namespace: CassavaMethod
def: "Plot volume calculated using the sum of all z-values (the height of every point in the point cloud) multiplied by 0.01 X 0.01. Estimates are derived from Weibull's distribution." []
xref: CO:curator
is_a: CO_334:0001002 ! Methods
relationship: method_of CO_334:0002030 ! Plot volume

[Term]
id: CO_334:0010495
name: Calculation: Plant height per plot_method
namespace: CassavaMethod
def: "Height of plant calculated from the mean of the 5% highest points in a plot point cloud." []
xref: CO:curator
is_a: CO_334:0001002 ! Methods
relationship: method_of CO_334:0002031 ! Plant height per plot

[Term]
id: CO_334:0010496
name: Calculation: Weibull function
namespace: CassavaMethod
def: "Weibull continous probability distribution" []
xref: CO:curator
is_a: CO_334:0001002 ! Methods
relationship: method_of CO_334:0002034 ! Weibull scale trait
relationship: method_of CO_334:0002035 ! Weibull shape trait

[Term]
id: CO_334:0010497
name: Measurement: Canopy width_method
namespace: CassavaMethod
is_a: CO_334:0001002 ! Methods
relationship: method_of CO_334:0002039 ! Canopy width

[Term]
id: CO_334:0010498
name: Measurement: Dry weight of biomass_method
namespace: CassavaMethod
def: "Measurement of total plant biomass by drying in oven for ten days at fifty degrees celsius." []
is_a: CO_334:0001002 ! Methods
relationship: method_of CO_334:0002045 ! Biomass dry weight

[Term]
id: CO_334:0010499
name: Counting: Cassava rust disease incidence_method
namespace: CassavaMethod
def: "Proportion of plants in a plot showing symptom of rust (Uromyces manihot)." []
is_a: CO_334:0001002 ! Methods
relationship: method_of CO_334:0002042 ! Cassava rust disease incidence

[Term]
id: CO_334:0010500
name: Visual Observation: Cassava rust disease severity_method
namespace: CassavaMethod
def: "Visual rating of cassava rust disease by observing symptomatic plants in a plot." []
is_a: CO_334:0001002 ! Methods
relationship: method_of CO_334:0002041 ! Cassava rust disease severity

[Term]
id: CO_334:0010501
name: Sensory assessment: Leaf edibility_method
namespace: CassavaMethod
def: "Assessment of how delicious and palatable cooked cassava leaf is by eating" []
xref: CO:curators
is_a: CO_334:0001002 ! Methods
relationship: method_of CO_334:0002047 ! Leaf edibility

[Term]
id: CO_334:0010502
name: Visual Rating: Cooking quality_method
namespace: CassavaMethod
def: "Qualittaive rating of cassava root after boiling taking into consideration the cooking time, texture and color" []
is_a: CO_334:0001002 ! Methods

[Term]
id: CO_334:0010504
name: Visual Rating: Apical pubescence_method
is_a: CO_334:0001002 ! Methods
relationship: method_of CO_334:0000283 ! Apical pubescence

[Term]
id: CO_334:0010505
name: Olfactory Perception: Fufu smell_method
namespace: CassavaMethod
def: "Percieve the fufu product and check to see if it has some smell." []
xref: CO:curators
is_a: CO_334:0001002 ! Methods
relationship: method_of CO_334:0002051 ! Fufu smell

[Term]
id: CO_334:0010506
name: Olfactory Perception: Attieke smell_method
namespace: CassavaMethod
def: "Percieve the fufu product and check to see if it has some smell." []
xref: CO:curators
is_a: CO_334:0001002 ! Methods
relationship: method_of CO_334:0002052 ! Attieke smell
relationship: variable_of CO_334:0002052 ! Attieke smell

[Term]
id: CO_334:0010507
name: Prediction: Dry matter content by QST_method
namespace: CassavaMethod
def: "Prediction of dry matter content using spectrum generated by hand-held NIRS device ( wavelength range of 350-2500) done by placing the device consistently on three different parts of dissected root sections ( proximal, axial and distal)." []
xref: CO:curators
is_a: CO_334:0001002 ! Methods
relationship: method_of CO_334:0000424 ! Root dry matter content

[Term]
id: CO_334:0010508
name: Prediction: Dry matter content by SciO_method
namespace: CassavaMethod
def: "Prediction of dry matter content using spectrum generated by mini hand-held NIRS device (700-1100) done by placing the device consistently on three different parts of dissected root sections ( proximal, axial and distal)." []
xref: CO:curators
is_a: CO_334:0001002 ! Methods
relationship: method_of CO_334:0000424 ! Root dry matter content

[Term]
id: CO_334:0010509
name: Prediction: Dry matter content by table-top NIRS_method
namespace: CassavaMethod
def: "Prediction of dry matter content based on spectrum generated using table-top NIRS (wavelength of 850-2500) done by placing chopped and mashed cassava sample into the machine; the sample is rotated at four different degrees (0, 90, 180 and 270)" []
xref: CO:curators
is_a: CO_334:0001002 ! Methods
relationship: method_of CO_334:0000424 ! Root dry matter content

[Term]
id: CO_334:0010510
name: PCR assay: Cassava Brown Streak Virus_method
namespace: CassavaMethod
def: "One step TaqMan method used with primers and probes for CBSV" []
xref: CO:curators
is_a: CO_334:0001002 ! Methods
relationship: method_of CO_334:0000090 ! Cassava brown streak disease root severity

[Term]
id: CO_334:0010511
name: PCR assay: Ugandan Cassava Brown Streak Virus_method
namespace: CassavaMethod
def: "One step TaqMan method used with primers and probes for UCBSV amplification" []
xref: CO:curators
is_a: CO_334:0001002 ! Methods
relationship: method_of CO_334:0000090 ! Cassava brown streak disease root severity

[Term]
id: CO_334:0010512
name: Calculation: Harvest index_method
namespace: CassavaMethod
def: "Plot biomass estimated as the ratio of root weight and the sum of root and shoot weight" []
is_a: CO_334:0001002 ! Methods
relationship: method_of CO_334:0000267 ! Harvest index

[Term]
id: CO_334:0010513
name: Visual Rating: Apical pubescence_method
namespace: CassavaMethod
def: "Rating of the presence of pubescence on the leaf apices" []
is_a: CO_334:0001002 ! Methods
relationship: method_of CO_334:0000283 ! Apical pubescence

[Term]
id: CO_334:0010514
name: Measurement: Storage root weight per plant_method
namespace: CassavaMethod
def: "Weight of root using scales from individual plant stands" []
is_a: CO_334:0001002 ! Methods
relationship: method_of CO_334:0000303 ! Storage root weight by plant

[Term]
id: CO_334:0010515
name: Measurement: Fresh shoot weight per plant_method
namespace: CassavaMethod
def: "Weight of shoot (stem and foliar) using scales" []
is_a: CO_334:0001002 ! Methods
relationship: method_of CO_334:0000306 ! Fresh shoot weight by plant

[Term]
id: CO_334:0010516
name: Estimation: Plot volume_method
namespace: CassavaMethod
def: "Estimation based on Weibull's continuous probability distribution for deriving the scale and shape parameters. It is calculated as the sum of all z-values (the height of every point in the point cloud) multiplied by 0.01 and 0.01 (every pixel is 1cm resolution)." []
is_a: CO_334:0001002 ! Methods
relationship: method_of CO_334:0002030 ! Plot volume

[Term]
id: CO_334:0010517
name: Calculation: Softness of boiled root_method
namespace: CassavaMethod
def: "Assessment of the softness of boiled root through calculation of the force it takes using a penetrometer to penetrate the root." []
is_a: CO_334:0001002 ! Methods
relationship: method_of CO_334:0001012 ! Softness of boiled cassava roots

[Term]
id: CO_334:0010518
name: Visual Rating: Ease of peel_method
namespace: CassavaMethod
def: "Visual rating of ease of peeling root cortex." []
is_a: CO_334:0001002 ! Methods
relationship: method_of CO_334:0000362 ! Ease of peeling storage root cortex

[Term]
id: CO_334:0010519
name: Measurement: Starch granule_method
namespace: CassavaMethod
def: "Measurement of starch granule" []
is_a: CO_334:0001002 ! Methods
relationship: method_of CO_334:0000318 ! Starch granule morphology
relationship: method_of CO_334:0000320 ! Starch granule size

[Term]
id: CO_334:0010520
name: Counting: Number of node_method
namespace: CassavaMethod
def: "Count of the number of nodes on a stem" []
is_a: CO_334:0001002 ! Methods
relationship: method_of CO_334:0000342 ! Node number
relationship: method_of CO_334:0000351 ! Node number per branch

[Term]
id: CO_334:0010521
name: Measurement: Fresh fibrous root_method
namespace: CassavaMethod
def: "Weigh fibrous root" []
is_a: CO_334:0001002 ! Methods
relationship: method_of CO_334:0002060 ! Fibrous root weight

[Term]
id: CO_334:0010522
name: Computation: Chromometer color values
namespace: CassavaMethod
def: "Color scales based on the Opponent-Color Theory" []
is_a: CO_334:0001002 ! Methods
relationship: method_of CO_334:0002061 ! L chromometer
relationship: method_of CO_334:0002062 ! B chromometer
relationship: method_of CO_334:0002063 ! A chromometer

[Term]
id: CO_334:0010523
name: Computation: Change in weight after boiling
namespace: CassavaMethod
def: "The weight of 8 pieces of cassava roots pooled together is measured before boiling. Change in weight is calculated as the weight difference before and after boiling divided by the initial weight before boiling, and expressed as percentage. The experiment is recommended in triplicate (8 pieces x 3)" []
is_a: CO_334:0001002 ! Methods
relationship: method_of CO_334:0002067 ! Change in weight after boiling

[Term]
id: CO_334:0010524
name: Estimation: Time of boiling
namespace: CassavaMethod
def: "Eight pieces of cassava roots are monitored during boiling by carefully probing their surface with a fork and visually assessing their appearance, until becoming soft. The time at which six out of the eight pieces become soft, is recorded as Optimum Cooking Time (OCT) (after subtracting if necessary the cumulated time the strainer was outside the boiling water for Change in weight measurements). Three replications are recommended. If the roots need more than 60 minutes to boil, the experiment is interrupted and OCT of 60 min is reported." []
is_a: CO_334:0001002 ! Methods
relationship: method_of CO_334:0002069 ! Time of boiling

[Term]
id: CO_334:0010525
name: Measurement: Textural characteristic
namespace: CassavaMethod
def: "A piece of boiled cassava root (half-cylinder 5.5 cm diameter, 6 cm long) was placed flat-face down in an Ottawa cell and pushed through a 5-blade grid over a distance of 20 mm at 1 mm/s. The force to carry out this extrusion was recorded, together with the distance traveled and the time. The texture profile was represented on a diagram as Force vs Distance traveled. The measurement was repeated 18 times with 18 different pieces of roots, and the average was reported." []
is_a: CO_334:0001002 ! Methods
relationship: method_of CO_334:0002071 ! Textural characteristic

[Term]
id: CO_334:0010526
name: Computation: Cassava brown streak disease root severity in percentage_method
namespace: CassavaMethod
def: "Computation of visible tissues in the root cross sections that appear to be diseased using image analysis as described in https://csce.ucmss.com/cr/books/2018/LFS/CSREA2018/IPC3638.pdf" []
is_a: CO_334:0001002 ! Methods
relationship: method_of CO_334:0000090 ! Cassava brown streak disease root severity

[Term]
id: CO_334:0010527
name: Visual Rating: Root flesh color ring_method
namespace: CassavaMethod
def: "An assesment of the ring formed around the pulp. Rating is done by cutting the root and ring pattern is then checked from the center of the pulp." []
xref: CO:curators
is_a: CO_334:0001002 ! Methods
relationship: method_of CO_334:0000490 ! Storage Root Pulp Color

[Term]
id: CO_334:0010528
name: Visual Observation:Whitefly severity evaluation_method
namespace: CassavaMethod
def: "The number of whitefly adults present in the buds" []
is_a: CO_334:0001002 ! Methods
relationship: method_of CO_334:0000410 ! Number of bemisia tabaci adult

[Term]
id: CO_334:0010529
name: Visual Observation: Thrips severity evaluation_method
namespace: CassavaMethod
def: "Assessment of the buds and apical leaf for discoloration and deformation" []
is_a: CO_334:0001002 ! Methods
relationship: method_of CO_334:0002085 ! Cassava Franklinella williamsi severity

[Term]
id: CO_334:0010530
name: Visual Scoring :Branching Angle_degree_method
namespace: CassavaMethod
def: "Visual rating of the angle between a vertical plane and first primary branch." []
is_a: CO_334:0001002 ! Methods
relationship: method_of CO_334:0000294 ! Branching Angle

[Term]
id: CO_334:0010531
name: Calculation: Starch content_EMBRAPA_method
namespace: CassavaMethod
def: "Starch content calculation based specific gravity (spg)estimation of sampled cassava (weighing 4-5 kilogram of cassava root in air, and in water.It is calculated as root weight in air divided by the sum of root weight in air and root weight in water as described Kawano et al. (1987)). Starch value is derived using the equation: 158.3 * spg - 137.35 .It is applied in the Brazilian starch industry" []
xref: CO:curator
is_a: CO_334:0001002 ! Methods
relationship: method_of CO_334:0000474 ! Starch Content

[Term]
id: CO_334:0010532
name: Calculation: Starch content_NRCRI_method
namespace: CassavaMethod
def: "Starch content calculation based specific gravity (spg)estimation of sampled cassava (weighing 4-5 kilogram of cassava root in air, and in water.It is calculated as root weight in air divided by the sum of root weight in air and root weight in water as described Kawano et al. (1987)). Starch value is derived using the equation: 210.8 * spg - 213.4" []
is_a: CO_334:0001002 ! Methods

[Term]
id: CO_334:0010533
name: Estimation: Moisture content_method
namespace: CassavaMethod
def: "Determined as the loss in weight of a flour sample after oven drying expressed as a proportion of the original weight prior to oven drying" []
is_a: CO_334:0001002 ! Methods
relationship: method_of CO_334:0002088 ! Moisture content of cassava flour

[Term]
id: CO_334:0010534
name: Calculation: Setback_method
namespace: CassavaMethod
def: "Measured on cassava flour using the Rapid Visco Analyzer (RVA)" []
is_a: CO_334:0001002 ! Methods
relationship: method_of CO_334:0002090 ! Setback

[Term]
id: CO_334:0010535
name: Estimation: Final viscosity_method
namespace: CassavaMethod
def: "Viscosity at the end of the RVA test" []
is_a: CO_334:0001002 ! Methods
relationship: method_of CO_334:0002092 ! Final viscosity

[Term]
id: CO_334:0010536
name: Calculation: Breakdown_method
namespace: CassavaMethod
def: "Breakdown equals peak viscosity minus trough viscosity" []
is_a: CO_334:0001002 ! Methods
relationship: method_of CO_334:0002094 ! Breakdown

[Term]
id: CO_334:0010537
name: Estimation: Trough_method
namespace: CassavaMethod
def: "The minimum viscosity after the peak" []
is_a: CO_334:0001002 ! Methods
relationship: method_of CO_334:0002096 ! Trough

[Term]
id: CO_334:0010538
name: Measurement: Peak viscosity_method
namespace: CassavaMethod
def: "Maximum viscosity during the heating or hold phase of the RVA test" []
is_a: CO_334:0001002 ! Methods
relationship: method_of CO_334:0002098 ! Peak viscosity

[Term]
id: CO_334:0010539
name: Measurement: Pasting temperature_method
namespace: CassavaMethod
def: "Temperature at which the viscosity trace first raises above the baseline during the initial heating phase." []
is_a: CO_334:0001002 ! Methods
relationship: method_of CO_334:0002100 ! Pasting temperature

[Term]
id: CO_334:0010540
name: Counting: Cassava blight leaf spot disease incidence_method
namespace: CassavaMethod
def: "Count of the number of plants showing symptoms of blight leaf spot relative to the total nu,ber of plants in a plot." []
is_a: CO_334:0001002 ! Methods
relationship: method_of CO_334:0002115 ! Cassava blight leaf spot disease incidence

[Term]
id: CO_334:0010541
name: Counting: Cassava brown leaf spot disease incidence_method
namespace: CassavaMethod
def: "Count of the number plants showing symptoms of brown leaf spot relative to the total number of plants in a plot." []
is_a: CO_334:0001002 ! Methods
relationship: method_of CO_334:0002113 ! Cassava brown leaf spot disease incidence

[Term]
id: CO_334:0010542
name: Counting: Cassava white leaf spot disease incidence_method
namespace: CassavaMethod
def: "Count of the number of plants showing symptoms of white leaf spot relative to the total number of plants in a plot." []
is_a: CO_334:0001002 ! Methods
relationship: method_of CO_334:0002111 ! Cassava white leaf spot disease incidence

[Term]
id: CO_334:0010543
name: Visual Observation: Cassava white leaf spot disease severity_method
namespace: CassavaMethod
def: "Visual rating of symptoms in response to the white leaf spot disease caused by Passalora maninhotis. Symptoms rated from: 0 = clean, no infection, 1 = Few leaves affected from the lower third part of the plant, 2 = > 50% of affected leaves at the lower third of the plant, 3 = Affected leaves on the middle and upper third of the plant, 4 = low incidence distributed all over the plant, 5 = Middle incidence distributed all over the plant with yellowed leaves and/or defoliation of the lower third part of the plant, 6 = Plant fully defoliated." []
is_a: CO_334:0001002 ! Methods
relationship: method_of CO_334:0002110 ! Cassava white leaf spot disease severity

[Term]
id: CO_334:0010544
name: Visual Observation: Cassava brown leaf spot disease severity_method
namespace: CassavaMethod
def: "Visual rating of symptoms in response to the brown leaf spot disease caused by Passalora henningsii. Symptoms rated from: 0 = clean, no infection, 1 = Few leaves affected from the lower third part of the plant, 2 = Low incidence at the lower third part of the plant, 3 = middle incidence distributed at the lower and middle parts of the plant with yellowed leaves and/or defoliation, 4 = high incidence distributed all over the plant with yellowed leaves and/or defoliation, 5 = Plant fully defoliated." []
is_a: CO_334:0001002 ! Methods
relationship: method_of CO_334:0002112 ! Cassava brown leaf spot disease severity

[Term]
id: CO_334:0010545
name: Visual Observation: Cassava blight leaf spot disease severity_method
namespace: CassavaMethod
def: "Visual rating of symptoms in response to the blight leaf spot disease caused by Passalora vicosae. Symptoms rated from: 0 = clean, no infection, 1 = Few leaves affected from the lower third part of the plant, 2 = Low incidence at the lower third part of the plant, 3 = middle incidence distributed at the lower and middle parts of the plant with yellowed leaves and/or defoliation, 4 = high incidence distributed all over the plant with yellowed leaves and/or defoliation, 5 = Plant fully defoliated." []
is_a: CO_334:0001002 ! Methods
relationship: method_of CO_334:0002114 ! Cassava blight leaf spot disease severity

[Term]
id: CO_334:0010546
name: Calculation: Gari yield_method
namespace: CassavaMethod
def: "Gari yield calculated as the ratio of Gari initial weight (CO_334:0002020) and Gari fried weight (CO_334:0002026) multiplied by 100." []
xref: CO:curators
is_a: CO_334:0001002 ! Methods
relationship: method_of CO_334:0000374 ! Gari content

[Term]
id: CO_334:0010547
name: Measurement: Fufu chaff weight_method
namespace: CassavaMethod
def: "Measurement of fufu chaff weight using laboratory scale." []
xref: CO:curators
is_a: CO_334:0001002 ! Methods
relationship: method_of CO_334:0002124 ! Fufu chaff weight

[Term]
id: CO_334:0010548
name: Calculation: Fufu chaff loss in percentage
namespace: CassavaMethod
def: "Fufu chaff loss calculated as the ratio of dewatered fufu mash weight (CO_334:0002017)- fufu chaff weight (CO_334:0002125) and dewatered fufu mash weight (CO_334:0002017)." []
is_a: CO_334:0001002 ! Methods
relationship: method_of CO_334:0002127 ! Fufu  chaff loss

[Term]
id: CO_334:0010549
name: Calculation: Fufu yield in percentage
namespace: CassavaMethod
def: "Fufu yield calculated as the ratio of fufu dewatered mash weight(CO_334:0002017) and  fufu peeled root weight (CO_334:0002013) multiplied by 100." []
is_a: CO_334:0001002 ! Methods
relationship: method_of CO_334:0000373 ! Fufu content

[Term]
id: CO_334:0010550
name: Absorption: Cassava brown streak viral titre_method
namespace: CassavaMethod
def: "ELISA assays are used to generate absorbance readings that are converted titre with the aid of a standard curve. Standard curves tend to vary with how serial dilutions are made and to some extent may depend on the reagents used" []
is_a: CO_334:0001002 ! Methods
relationship: method_of CO_334:0002130 ! Cassava brown streak viral titre

[Term]
id: CO_334:0012000
name: Observation: Farmer trait preference_method
namespace: CassavaMethod
def: "Farmers were given three(3) varieties each and they give their opinion on each, rank and as well score on an ordinal scale of 1-5." []
is_a: CO_334:0001002 ! Methods
relationship: method_of CO_334:0001025 ! farmer preference trait post-harvest
relationship: method_of CO_334:0001027 ! farmer preference trait at harvest

[Term]
id: CO_334:0012001
name: Measurement: total root length_method
namespace: CassavaMethod
def: "Measurement of the total root length" [CO:curators]
is_a: CO_334:0001002 ! Methods
relationship: method_of CO_334:0001034 ! root length measurement in cm

[Term]
id: CO_334:0012002
name: Measurement: total root diameter_method
namespace: CassavaMethod
def: "Measurement of the total root diameter" [CO:curators]
is_a: CO_334:0001002 ! Methods
relationship: method_of CO_334:0001035 ! storage root diameter in cm

[Term]
id: CO_334:0013000
name: surface yellowness appearance method
namespace: CassavaMethod
def: "When you receive a cassava root sample, observe the surface and evaluate the intensity of the yellow colour." []
is_a: CO_334:0001002 ! Methods
relationship: method_of CO_334:0003020 ! boiled root surface yellowness

[Term]
id: CO_334:0013001
name: stickiness texture in the mouth method
namespace: CassavaMethod
def: "Put a part of boiled sample in the mouth, chew it and evaluate: Amount of product adhering on/in the teeth after product mastication, and force required to remove product  completely  from the palate, using the tongue, after complete compression of the sample between  tongue and palate" []
is_a: CO_334:0001002 ! Methods
relationship: method_of CO_334:0003029 ! boiled root stickness in mouth

[Term]
id: CO_334:0013002
name: mealiness texture in the hand method
namespace: CassavaMethod
def: "Put a part of the boiled sample between thumb and index fingers and using tapping motions, evaluate the amount of product adhering on them" []
is_a: CO_334:0001002 ! Methods
relationship: method_of CO_334:0003030 ! boiled root mealiness by hand

[Term]
id: CO_334:0013003
name: sweetness taste method
namespace: CassavaMethod
def: "Put a part of the sample in the mouth and on the tongue; then evaluate the intensity of sugary taste" []
is_a: CO_334:0001002 ! Methods
relationship: method_of CO_334:0003140 ! eba sweetness taste

[Term]
id: CO_334:0013004
name: steamed cassava-like_aroma  method
namespace: CassavaMethod
def: "Put a part of the boiled sample and by retro-olfaction, evaluate the presence and the intensity of sweet potato aroma" []
is_a: CO_334:0001002 ! Methods
relationship: method_of CO_334:0003036 ! boiled root steamed cassava-like aroma

[Term]
id: CO_334:0013005
name: surface colour sppearance method
namespace: CassavaMethod
def: "Visually inspect sample surface" []
is_a: CO_334:0001002 ! Methods
relationship: method_of CO_334:0003047 ! fufu surface colour

[Term]
id: CO_334:0013006
name: smoothness texture in the hand method
namespace: CassavaMethod
def: "Sample is pressed firmly between the fingers" []
is_a: CO_334:0001002 ! Methods
relationship: method_of CO_334:0003048 ! fufu smoothness in hand

[Term]
id: CO_334:0013007
name: stickiness texture in the hand method
namespace: CassavaMethod
def: "Put a part of the boiled sample between thumb and index fingers and using tapping motions, evaluate the amount of product adhering on them" []
is_a: CO_334:0001002 ! Methods
relationship: method_of CO_334:0003136 ! eba stickiness kin the hand

[Term]
id: CO_334:0013008
name: moldability texture in the hand method
namespace: CassavaMethod
def: "Sample is put in the hands and moulded" []
is_a: CO_334:0001002 ! Methods
relationship: method_of CO_334:0003050 ! fufu moldability in the hand

[Term]
id: CO_334:0013009
name: hardness texture by hand method
namespace: CassavaMethod
def: "Place sample between fingers and feel to access the amount of force required to press it" []
is_a: CO_334:0001002 ! Methods
relationship: method_of CO_334:0003134 ! eba hardness in hand

[Term]
id: CO_334:0013010
name: stretchability texture by the hand method
namespace: CassavaMethod
def: "Take a sizeable piece of sample, flatten it with palms and stretch" []
is_a: CO_334:0001002 ! Methods
relationship: method_of CO_334:0003137 ! eba stretchability in the hand

[Term]
id: CO_334:0013011
name: odour method
namespace: CassavaMethod
def: "Take a whiff and evaluate the intensity of fufu odour" []
is_a: CO_334:0001002 ! Methods
relationship: method_of CO_334:0003053 ! fufu odour

[Term]
id: CO_334:0013012
name: attieke-like aroma method
namespace: CassavaMethod
def: "Smell the sample and asses the intensity of attieke aroma" []
is_a: CO_334:0001002 ! Methods
relationship: method_of CO_334:0003101 ! attieke attieke-like  aroma

[Term]
id: CO_334:0013013
name: bitterness after taste method
namespace: CassavaMethod
def: "Put a part of the boiled sample in the mouth and evaluate whether bitter after swallowing" []
is_a: CO_334:0001002 ! Methods
relationship: method_of CO_334:0003035 ! boiled root bitterness after taste

[Term]
id: CO_334:0013014
name: bitterness taste method
namespace: CassavaMethod
def: "Put a part of the boiled sample in the mouth and evaluate whether bitter after swallowing" []
is_a: CO_334:0001002 ! Methods
relationship: method_of CO_334:0003034 ! boiled root taste bitterness

[Term]
id: CO_334:0013015
name: boiled cassava odour method
namespace: CassavaMethod
def: "Take a whiff and evaluate the intensity of cassava odour" []
is_a: CO_334:0001002 ! Methods
relationship: method_of CO_334:0003124 ! boiled root cassava odour

[Term]
id: CO_334:0013016
name: brightness appearance method
namespace: CassavaMethod
def: "Observe the sample and evaluate the degree of brightness" []
is_a: CO_334:0001002 ! Methods
relationship: method_of CO_334:0003106 ! attieke brightness

[Term]
id: CO_334:0013017
name: cohesiveness texture by touch method
namespace: CassavaMethod
def: "Put the sample between fingers and press to evaluate how grains adhere to each other." []
is_a: CO_334:0001002 ! Methods
relationship: method_of CO_334:0003133 ! eba cohessiveness/moldability

[Term]
id: CO_334:0013018
name: color homogeneity appearance method
namespace: CassavaMethod
def: "When you receive a cassava root sample, observe the surface and evaluate the intensity of the yellow colour." []
is_a: CO_334:0001002 ! Methods
relationship: method_of CO_334:0003022 ! boiled root surface color homogeneity

[Term]
id: CO_334:0013019
name: crumbly in the hand method
namespace: CassavaMethod
def: "Crush the product between two fingers and assess the ease of  crumbliness" []
is_a: CO_334:0001002 ! Methods
relationship: method_of CO_334:0003125 ! boiled root crumbness

[Term]
id: CO_334:0013020
name: easy to chew texture in the mouth method
namespace: CassavaMethod
def: "Put the product between the molars and mash it to assess the number of chews before swallowing" []
is_a: CO_334:0001002 ! Methods
relationship: method_of CO_334:0003126 ! boiled root easiness to chew

[Term]
id: CO_334:0013021
name: extraneous matters appearance method
namespace: CassavaMethod
def: "Observe the sample and evaluate the presence of absence of extraneous matter" []
is_a: CO_334:0001002 ! Methods
relationship: method_of CO_334:0003108 ! attieke extraneous matters

[Term]
id: CO_334:0013022
name: extraneous matters texture in mouth method
namespace: CassavaMethod
def: "Put a part of the sample in mouth, chew it and after 5 chews, evaluate the presence or absence of extraneous matter" []
is_a: CO_334:0001002 ! Methods
relationship: method_of CO_334:0003108 ! attieke extraneous matters

[Term]
id: CO_334:0013023
name: fermented taste method
namespace: CassavaMethod
def: "Put a part of the sample in the mouth and evaluate the intensity of fermented taste" []
is_a: CO_334:0001002 ! Methods
relationship: method_of CO_334:0003109 ! attieke fermented taste

[Term]
id: CO_334:0013024
name: fibrouness texture appearance  method
namespace: CassavaMethod
def: "After breaking / cutting, breaking / crumbling, evaluate the presence/intensity of fine fibers visible to the eye" []
is_a: CO_334:0001002 ! Methods
relationship: method_of CO_334:0003129 ! boiled root presence of fibers

[Term]
id: CO_334:0013025
name: fibrousness texture in the mouth method
namespace: CassavaMethod
def: "After chewing feel sample between tongue and palate to assess the amount of string like particles present on sample" []
is_a: CO_334:0001002 ! Methods
relationship: method_of CO_334:0003141 ! eba fibrousness in mouth

[Term]
id: CO_334:0013026
name: firmness texture by touch method
namespace: CassavaMethod
def: "Put the sample between fingers and press to evaluate how hard the grains are." []
is_a: CO_334:0001002 ! Methods
relationship: method_of CO_334:0003110 ! attieke firmness

[Term]
id: CO_334:0013027
name: granularity texture in the mouth method
namespace: CassavaMethod
def: "Put a part of the sample in mouth, chew it and after 5 chews, evaluate the granurality" []
is_a: CO_334:0001002 ! Methods
relationship: method_of CO_334:0003112 ! attieke granularity

[Term]
id: CO_334:0013028
name: granularity texture in the mouth method
namespace: CassavaMethod
def: "Put the product in mouth and mash/crush it between the molars to assess the presence of small grains on the tongue" []
is_a: CO_334:0001002 ! Methods
relationship: method_of CO_334:0003127 ! boiled root granulariness

[Term]
id: CO_334:0013029
name: hardness to break/cut texture in the hand method
namespace: CassavaMethod
def: "Crush the product between fingers and assess the ease of breaking" []
is_a: CO_334:0001002 ! Methods
relationship: method_of CO_334:0003128 ! boiled root hardness to break

[Term]
id: CO_334:0013030
name: homogenity of grains appearance method
namespace: CassavaMethod
def: "Observe the sample and evaluate the uniformity of grains" []
is_a: CO_334:0001002 ! Methods
relationship: method_of CO_334:0003113 ! attieke homogenity of grains

[Term]
id: CO_334:0013031
name: masticability texture in mouth method
namespace: CassavaMethod
def: "Put a part of the sample in mouth, chew it and after 5 chews, evaluate the masticability" []
is_a: CO_334:0001002 ! Methods
relationship: method_of CO_334:0003114 ! attieke masticability

[Term]
id: CO_334:0013032
name: moldability texture in touch method
namespace: CassavaMethod
def: "Try to make a ball of the sample and evaluate how easy it is to deform or break the sample" []
is_a: CO_334:0001002 ! Methods
relationship: method_of CO_334:0003115 ! attieke moldability in the hand

[Term]
id: CO_334:0013033
name: mouth filled sensations texture in mouth method
namespace: CassavaMethod
def: "Put a part of the sample in mouth, chew it and after 5 chews, evaluate the mouth filled sensetions" []
is_a: CO_334:0001002 ! Methods
relationship: method_of CO_334:0003116 ! attieke mouth filled sensations

[Term]
id: CO_334:0013034
name: off-odours aroma method
namespace: CassavaMethod
def: "Smell the sample and asses the presence or absence of off-odours" []
is_a: CO_334:0001002 ! Methods
relationship: method_of CO_334:0003117 ! attieke off-odours

[Term]
id: CO_334:0013035
name: orange colour appearance method
namespace: CassavaMethod
def: "Observe the sample and evaluate the intensity of the orange colour" []
is_a: CO_334:0001002 ! Methods
relationship: method_of CO_334:0003107 ! attieke orange colour

[Term]
id: CO_334:0013036
name: presence of fibers appearance method
namespace: CassavaMethod
def: "Observe the sample and evaluate the presence of absence of fibers" []
is_a: CO_334:0001002 ! Methods
relationship: method_of CO_334:0003118 ! attieke presence of fibers

[Term]
id: CO_334:0013037
name: presence of lumps appearance method
namespace: CassavaMethod
def: "Observe the sample and evaluate the presence of absence of lumps" []
is_a: CO_334:0001002 ! Methods
relationship: method_of CO_334:0003119 ! attieke presence of lumps

[Term]
id: CO_334:0013038
name: presence of stripes appearance method
namespace: CassavaMethod
def: "Observe the surface of product and evaluate the size and the number of stripe" []
is_a: CO_334:0001002 ! Methods
relationship: method_of CO_334:0003130 ! boiled root presence of stripe

[Term]
id: CO_334:0013039
name: red palm oil aroma method
namespace: CassavaMethod
def: "Smell the sample and asses the presence or absence of red palm oil aroma" []
is_a: CO_334:0001002 ! Methods
relationship: method_of CO_334:0003120 ! attieke red palm oil aroma

[Term]
id: CO_334:0013040
name: roasted cassava-like aroma method
namespace: CassavaMethod
def: "Put a part of the boiled sample and by retro-olfaction, evaluate the presence and the intensity of sweet potato aroma" []
is_a: CO_334:0001002 ! Methods
relationship: method_of CO_334:0003037 ! boiled root roasted cassava-like aroma

[Term]
id: CO_334:0013041
name: size of grains appearance method
namespace: CassavaMethod
def: "Observe the sample and evaluate the size of grains" []
is_a: CO_334:0001002 ! Methods
relationship: method_of CO_334:0003111 ! attieke grain size

[Term]
id: CO_334:0013042
name: sourness aroma method
namespace: CassavaMethod
def: "Smell the sample and asses the presence or absence of odour of sourness" []
is_a: CO_334:0001002 ! Methods
relationship: method_of CO_334:0003121 ! attieke sourness aroma

[Term]
id: CO_334:0013043
name: sourness taste method
namespace: CassavaMethod
def: "Put a part of the sample in the mouth and evaluate the intensity of the sourness" []
is_a: CO_334:0001002 ! Methods
relationship: method_of CO_334:0003139 ! eba sourness in the mouth

[Term]
id: CO_334:0013044
name: surface creamness appearance method
namespace: CassavaMethod
def: "When you receive the sample, immediately open it  and examine the cream colour" []
is_a: CO_334:0001002 ! Methods
relationship: method_of CO_334:0003132 ! eba surface creamness

[Term]
id: CO_334:0013045
name: surface greyness appearance method
namespace: CassavaMethod
def: "When you receive the sample, immediately open it  and examine the grey colour" []
is_a: CO_334:0001002 ! Methods
relationship: method_of CO_334:0003142 ! eba surface greyness

[Term]
id: CO_334:0013046
name: surface smoothness appearance method
namespace: CassavaMethod
def: "When you receive a cassava root sample, observe the surface and evaluate the intensity of the yellow colour." []
is_a: CO_334:0001002 ! Methods
relationship: method_of CO_334:0003023 ! boiled root surface smoothnness

[Term]
id: CO_334:0013047
name: surface whiteness appearance method
namespace: CassavaMethod
def: "When you receive the sample, observe the surface and evaluate the intensity of the white colour." []
is_a: CO_334:0001002 ! Methods
relationship: method_of CO_334:0003138 ! eba surface whiteness

[Term]
id: CO_334:0013048
name: sweetpotato-like aroma method
namespace: CassavaMethod
def: "Put a part of the boiled sample and by retro-olfaction, evaluate the presence and the intensity of sweet potato aroma" []
is_a: CO_334:0001002 ! Methods
relationship: method_of CO_334:0003039 ! boiled root sweet potato-like aroma

[Term]
id: CO_334:0013049
name: taste of red palm oil taste method
namespace: CassavaMethod
def: "Put a part of the sample in the mouth and evaluate the intensity of taste of red palm oil" []
is_a: CO_334:0001002 ! Methods
relationship: method_of CO_334:0003122 ! attieke taste of red palm oil

[Term]
id: CO_334:0013050
name: undesired taste taste method
namespace: CassavaMethod
def: "Put a part of the sample in the mouth and evaluate the intensity of undesired taste" []
is_a: CO_334:0001002 ! Methods
relationship: method_of CO_334:0003123 ! attieke undesired taste

[Term]
id: CO_334:0013051
name: white color appearance method
namespace: CassavaMethod
def: "Observe the surface of product and evaluate the intensity of each type of the colour and its homogeneity" []
is_a: CO_334:0001002 ! Methods
relationship: method_of CO_334:0003131 ! boiled root white colour

[Term]
id: CO_334:0013052
name: yam-like aroma method
namespace: CassavaMethod
def: "Put a part of the boiled sample and by retro-olfaction, evaluate the presence and the intensity of sweet potato aroma" []
is_a: CO_334:0001002 ! Methods
relationship: method_of CO_334:0003038 ! boiled root yam-like aroma

[Term]
id: CO_334:0013053
name: smoothness texture in the mouth method
namespace: CassavaMethod
def: "After chewing feel sample between tongue and palate to assess the amount of string like particles present on sample" []
is_a: CO_334:0001002 ! Methods
relationship: method_of CO_334:0003135 ! eba smoothness in mouth

[Term]
id: CO_334:0100000
name: 3pt scale
namespace: CassavaScale
is_a: CO_334:0100684 ! 3 point scales
relationship: scale_of CO_334:0010002 ! Visual Rating: Staygreen_method
created_by: AAfolabi
creation_date: 2015-09-29T12:35:31Z

[Term]
id: CO_334:0100001
name: 3pt scale
namespace: CassavaScale
is_a: CO_334:0100684 ! 3 point scales
relationship: scale_of CO_334:0010003 ! Visual Rating: Size of shoot apices_method
created_by: AAfolabi
creation_date: 2015-09-29T13:50:02Z

[Term]
id: CO_334:0100002
name: 3pt scale
namespace: CassavaScale
is_a: CO_334:0100684 ! 3 point scales
relationship: scale_of CO_334:0010004 ! Visual Rating: Compactness of shoot apices_method
created_by: AAfolabi
creation_date: 2015-09-29T13:58:16Z

[Term]
id: CO_334:0100007
name: cm square
namespace: CassavaScale
is_a: CO_334:0001001 ! Scales
relationship: scale_of CO_334:0010012 ! Estimation: Total leaf area_method
created_by: AAfolabi
creation_date: 2017-07-18T15:37:40Z

[Term]
id: CO_334:0100012
name: branches
namespace: CassavaScale
is_a: CO_334:0001001 ! Scales
relationship: scale_of CO_334:0010412 ! Counting: Number of terminal branches with inflorescence_method
created_by: AAfolabi
creation_date: 2017-07-25T15:09:59Z

[Term]
id: CO_334:0100013
name: buds
namespace: CassavaScale
def: "Number of flower buds." [CO:curator]
is_a: CO_334:0001001 ! Scales
relationship: scale_of CO_334:0010019 ! Counting: Number of buds by branch level
created_by: AAfolabi
creation_date: 2017-07-25T16:24:36Z

[Term]
id: CO_334:0100014
name: inflorescence
namespace: CassavaScale
def: "Number of inflorescence." [CO:curator]
is_a: CO_334:0001001 ! Scales
relationship: scale_of CO_334:0010018 ! Counting: Number of inflorescence by branch level
created_by: AAfolabi
creation_date: 2017-07-25T16:06:30Z

[Term]
id: CO_334:0100017
name: fruitset
namespace: CassavaScale
is_a: CO_334:0001001 ! Scales
relationship: scale_of CO_334:0010022 ! Counting: Number of fruitset by branch level
created_by: AAfolabi
creation_date: 2017-07-25T17:06:23Z

[Term]
id: CO_334:0100434
name: 7pt scale
namespace: CassavaScale
is_a: CO_334:0100687 ! 7 point scales
relationship: scale_of CO_334:0010228 ! Visual Rating: Initial vigor_method

[Term]
id: CO_334:0100436
name: 5 point scales
namespace: CassavaScale
is_a: CO_334:0001001 ! Scales
relationship: scale_of CO_334:0010230 ! Visual Observation: Cassava mosaic disease severity 1-month evaluation_method

[Term]
id: CO_334:0100437
name: 5pt scale
namespace: CassavaScale
is_a: CO_334:0100436 ! 5 point scales
relationship: scale_of CO_334:0010231 ! Visual Observation: Cassava mosaic disease severity 3-month evaluation_method

[Term]
id: CO_334:0100438
name: 5 pt scale
namespace: CassavaScale
is_a: CO_334:0100436 ! 5 point scales
relationship: scale_of CO_334:0010232 ! Visual Observation: Cassava mosaic disease severity 6-month evaluation_method

[Term]
id: CO_334:0100439
name: 5 pt scale
namespace: CassavaScale
is_a: CO_334:0100436 ! 5 point scales
relationship: scale_of CO_334:0010233 ! Visual Observation: Cassava mosaic disease severity 9-month evaluation_method

[Term]
id: CO_334:0100440
name: 5 pt scale
namespace: CassavaScale
is_a: CO_334:0100436 ! 5 point scales
relationship: scale_of CO_334:0010234 ! Visual Observation: Cassava mosaic disease severity 12-month evaluation_method

[Term]
id: CO_334:0100448
name: 5 pt scale
namespace: CassavaScale
is_a: CO_334:0100436 ! 5 point scales
relationship: scale_of CO_334:0010242 ! Visual Observation: Cassava bacterial blight severity 3-month evalution_method

[Term]
id: CO_334:0100449
name: 5 pt scale
namespace: CassavaScale
is_a: CO_334:0100436 ! 5 point scales
relationship: scale_of CO_334:0010243 ! Visual Observation: Cassava bacterial blight severity 6-month evalution_method

[Term]
id: CO_334:0100450
name: 5 pt scale
namespace: CassavaScale
is_a: CO_334:0100436 ! 5 point scales
relationship: scale_of CO_334:0010244 ! Visual Observation: Cassava bacterial blight severity 9-month evalution_method

[Term]
id: CO_334:0100451
name: 5 pt scale
namespace: CassavaScale
is_a: CO_334:0100436 ! 5 point scales
relationship: scale_of CO_334:0010245 ! Visual Observation: Cassava bacterial blight severity 12-month evaluation_method

[Term]
id: CO_334:0100458
name: 5 pt scale
namespace: CassavaScale
is_a: CO_334:0100436 ! 5 point scales
relationship: scale_of CO_334:0010252 ! Visual Observation: Cassava anthractnose disease severity in 3-months_method

[Term]
id: CO_334:0100459
name: 5 pt scale
namespace: CassavaScale
is_a: CO_334:0100436 ! 5 point scales
relationship: scale_of CO_334:0010253 ! Visual Observation: Cassava anthractnose disease severity in 6-months_method

[Term]
id: CO_334:0100460
name: 5 pt scale
namespace: CassavaScale
is_a: CO_334:0100436 ! 5 point scales
relationship: scale_of CO_334:0010254 ! Visual Observation: Cassava anthractnose disease severity in 9-months_method

[Term]
id: CO_334:0100461
name: 5 pt scale
namespace: CassavaScale
is_a: CO_334:0100436 ! 5 point scales
relationship: scale_of CO_334:0010255 ! Visual Observation: Cassava anthractnose disease severity in 12-months_method

[Term]
id: CO_334:0100471
name: 5 pt scale
namespace: CassavaScale
is_a: CO_334:0100436 ! 5 point scales
relationship: scale_of CO_334:0010265 ! Visual Observation: Cassava green mite severity first evaluation_method

[Term]
id: CO_334:0100472
name: 5 pt scale
namespace: CassavaScale
is_a: CO_334:0100436 ! 5 point scales
relationship: scale_of CO_334:0010266 ! Visual Observation: Cassava green mite severity second evaluation_method

[Term]
id: CO_334:0100473
name: 5 pt scale
namespace: CassavaScale
is_a: CO_334:0100436 ! 5 point scales
relationship: scale_of CO_334:0010267 ! Visual Observation: Cassava mealy bug severity_method

[Term]
id: CO_334:0100476
name: 5 pt scale
namespace: CassavaScale
is_a: CO_334:0100436 ! 5 point scales
relationship: scale_of CO_334:0010270 ! Visual Observation: Cassava brown streak disease leaf severity 1-month evaluation_method

[Term]
id: CO_334:0100477
name: 5 pt scale
namespace: CassavaScale
is_a: CO_334:0100436 ! 5 point scales
relationship: scale_of CO_334:0010271 ! Visual Observation: Cassava brown streak disease leaf severity 3-month evaluation_method

[Term]
id: CO_334:0100478
name: 5 pt scale
namespace: CassavaScale
is_a: CO_334:0100436 ! 5 point scales
relationship: scale_of CO_334:0010272 ! Visual Observation: Cassava brown streak disease leaf severity 6-month evaluation_method

[Term]
id: CO_334:0100479
name: 5 pt scale
namespace: CassavaScale
is_a: CO_334:0100436 ! 5 point scales
relationship: scale_of CO_334:0010273 ! Visual Observation: Cassava brown streak disease leaf severity 9-month evaluation_method

[Term]
id: CO_334:0100486
name: 5 pt scale
namespace: CassavaScale
is_a: CO_334:0100436 ! 5 point scales
relationship: scale_of CO_334:0010280 ! Visual Observation: Cassava brown streak disease root severity 12-month evaluation_method

[Term]
id: CO_334:0100489
name: 5 pt scale
namespace: CassavaScale
is_a: CO_334:0100436 ! 5 point scales
relationship: scale_of CO_334:0010283 ! Visual Observation: Frog skin disease_method

[Term]
id: CO_334:0100490
name: plant
namespace: CassavaScale
is_a: CO_334:0001001 ! Scales
relationship: scale_of CO_334:0010284 ! Counting: Plant stands harvested_method

[Term]
id: CO_334:0100491
name: root
namespace: CassavaScale
is_a: CO_334:0001001 ! Scales
relationship: scale_of CO_334:0010285 ! Counting: Root number_method
relationship: scale_of CO_334:0010295 ! Counting: Rotted storage roots _method

[Term]
id: CO_334:0100493
name: kg
namespace: CassavaScale
is_a: CO_334:0001001 ! Scales
relationship: scale_of CO_334:0010286 ! Measurement: Fresh weight of storage root_method
relationship: scale_of CO_334:0010287 ! Measurement: Fresh shoot weight_method
relationship: scale_of CO_334:0010316 ! Measurement: Stock weight_method
relationship: scale_of CO_334:0010317 ! Counting: Stem yield_method
relationship: scale_of CO_334:0010318 ! Estimation: Dry matter content by specific gravity method
relationship: scale_of CO_334:0010386 ! Measurement: Stem weight_method
relationship: scale_of CO_334:0010389 ! Measurement: Tip shoot weight_method
relationship: scale_of CO_334:0010390 ! Measurement: Marketable root weight_method
relationship: scale_of CO_334:0010391 ! Measurement: Non marketable root weight_method
relationship: scale_of CO_334:0010393 ! Measurement: Leaf weight_method
relationship: scale_of CO_334:0010394 ! Measurement: Stump weight_method
relationship: scale_of CO_334:0010415 ! Measurement: Root weight in air_method
relationship: scale_of CO_334:0010416 ! Measurement: Root weight in water_method
relationship: scale_of CO_334:0010444 ! Measurement: Root weight after washing_method
relationship: scale_of CO_334:0010445 ! Measurement: Root weight after peel_method
relationship: scale_of CO_334:0010446 ! Measurement: Peel weight_method
relationship: scale_of CO_334:0010447 ! Measurement: Gari weight after grinding_method
relationship: scale_of CO_334:0010448 ! Measurement: Weight of mashed cassava cake_method
relationship: scale_of CO_334:0010449 ! Measurement: Gari shaft weight_method
relationship: scale_of CO_334:0010498 ! Measurement: Dry weight of biomass_method

[Term]
id: CO_334:0100494
name: 7pt scale
namespace: CassavaScale
is_a: CO_334:0100687 ! 7 point scales
relationship: scale_of CO_334:0010288 ! Visual Rating: Storage root size_method

[Term]
id: CO_334:0100495
name: 6pt scale
namespace: CassavaScale
is_a: CO_334:0001001 ! Scales
relationship: scale_of CO_334:0010289 ! Visual Rating: Storage root shape_method

[Term]
id: CO_334:0100496
name: 4pt scale
namespace: CassavaScale
is_a: CO_334:0100686 ! 4 point scales
relationship: scale_of CO_334:0010290 ! Visual Rating: Storage root cortex color_method

[Term]
id: CO_334:0100497
name: 4pt scale
namespace: CassavaScale
is_a: CO_334:0100686 ! 4 point scales
relationship: scale_of CO_334:0010291 ! Visual Rating: Storage root periderm color_method

[Term]
id: CO_334:0100498
name: 3pt scale
namespace: CassavaScale
is_a: CO_334:0100684 ! 3 point scales
relationship: scale_of CO_334:0010292 ! Visual Rating: Storage root pulp color _method

[Term]
id: CO_334:0100499
name: 8pt scale
namespace: CassavaScale
is_a: CO_334:0100688 ! 8 point scales
relationship: scale_of CO_334:0010293 ! Visual Rating: Root neck length_method

[Term]
id: CO_334:0100500
name: 7pt scale
namespace: CassavaScale
is_a: CO_334:0100687 ! 7 point scales
relationship: scale_of CO_334:0010294 ! Visual Scoring: Ease of peeling root cortex_method

[Term]
id: CO_334:0100502
name: 4pt scale
namespace: CassavaScale
is_a: CO_334:0100686 ! 4 point scales
relationship: scale_of CO_334:0010296 ! Sensory Assesment: Poundability_method
relationship: scale_of CO_334:0010473 ! Visual Rating: In-ground storability_method
relationship: scale_of CO_334:0010474 ! Visual Rating: Early bulking_method
relationship: scale_of CO_334:0010475 ! Visual Rating: Weed tolerance_method

[Term]
id: CO_334:0100503
name: 3pt scale
namespace: CassavaScale
is_a: CO_334:0100684 ! 3 point scales
relationship: scale_of CO_334:0010297 ! Gustation: Taste of boiled roots_method

[Term]
id: CO_334:0100504
name: 3pt scale
namespace: CassavaScale
is_a: CO_334:0100684 ! 3 point scales
relationship: scale_of CO_334:0010298 ! Visual Rating: Color of boiled storage roots_method

[Term]
id: CO_334:0100505
name: 9pt scale
namespace: CassavaScale
is_a: CO_334:0100689 ! 9 point scales
relationship: scale_of CO_334:0010299 ! Estimation: Hydrogen cyanide potential picrate method

[Term]
id: CO_334:0100507
name: 4pt scale
namespace: CassavaScale
is_a: CO_334:0100686 ! 4 point scales
relationship: scale_of CO_334:0010301 ! Visual Scoring: Stem color_method

[Term]
id: CO_334:0100508
name: 8pt scale
namespace: CassavaScale
is_a: CO_334:0100688 ! 8 point scales
relationship: scale_of CO_334:0010302 ! Visual Scoring: Branching angle_method

[Term]
id: CO_334:0100511
name: 5pt scale
namespace: CassavaScale
is_a: CO_334:0100436 ! 5 point scales
relationship: scale_of CO_334:0010305 ! Visual Rating: Leaf retention_method

[Term]
id: CO_334:0100512
name: 5pt scale
namespace: CassavaScale
is_a: CO_334:0100436 ! 5 point scales
relationship: scale_of CO_334:0010306 ! Visual Rating: Plant architecture_method

[Term]
id: CO_334:0100513
name: 2pt scale
namespace: CassavaScale
is_a: CO_334:0100685 ! 2 point scales
relationship: scale_of CO_334:0010434 ! Visual Observation: Flowering_method

[Term]
id: CO_334:0100514
name: 2pt scale
namespace: CassavaScale
is_a: CO_334:0100685 ! 2 point scales
relationship: scale_of CO_334:0010308 ! Visual Rating: Fruit set _method

[Term]
id: CO_334:0100515
name: 8pt scale
namespace: CassavaScale
is_a: CO_334:0100688 ! 8 point scales
relationship: scale_of CO_334:0010309 ! Visual Rating: Storage root peduncle_method

[Term]
id: CO_334:0100516
name: 2pt scale
namespace: CassavaScale
is_a: CO_334:0100685 ! 2 point scales
relationship: scale_of CO_334:0010310 ! Visual Rating: Storage root constrictions_method

[Term]
id: CO_334:0100517
name: 3pt scale
namespace: CassavaScale
is_a: CO_334:0100684 ! 3 point scales
relationship: scale_of CO_334:0010311 ! Visual Rating: Root surface color_method

[Term]
id: CO_334:0100518
name: 3pt scale
namespace: CassavaScale
is_a: CO_334:0100684 ! 3 point scales
relationship: scale_of CO_334:0010312 ! Visual Rating: Root surface texture_method
relationship: scale_of CO_334:0010518 ! Visual Rating: Ease of peel_method
relationship: scale_of CO_334:0010519 ! Measurement: Starch granule_method

[Term]
id: CO_334:0100525
name: 8pt scale
namespace: CassavaScale
is_a: CO_334:0100688 ! 8 point scales
relationship: scale_of CO_334:0010319 ! Visual Rating: Total carotenoid by chart_method

[Term]
id: CO_334:0100528
name: 4pt scale
namespace: CassavaScale
is_a: CO_334:0100686 ! 4 point scales
relationship: scale_of CO_334:0010322 ! Visual Rating: Branching_method

[Term]
id: CO_334:0100529
name: 5 pt scale
namespace: CassavaScale
is_a: CO_334:0100436 ! 5 point scales
relationship: scale_of CO_334:0010323 ! Visual Observation: Red spider mite severity_method

[Term]
id: CO_334:0100531
name: 5 pt scale
namespace: CassavaScale
is_a: CO_334:0100436 ! 5 point scales
relationship: scale_of CO_334:0010325 ! Visual Observation: Spiraling whitefly severity_method

[Term]
id: CO_334:0100535
name: t/ha
namespace: CassavaScale
is_a: CO_334:0001001 ! Scales
relationship: scale_of CO_334:0010329 ! Calculation: Fresh root yield_method
relationship: scale_of CO_334:0010330 ! Calculation: Dry yield_method
relationship: scale_of CO_334:0010332 ! Calculation: Top yield_method

[Term]
id: CO_334:0100539
name: 2pt scale
namespace: CassavaScale
is_a: CO_334:0100685 ! 2 point scales
relationship: scale_of CO_334:0000256 ! assessment of apical pubescence boolean 0&1
relationship: scale_of CO_334:0010333 ! Visual Rating: Suitability for intercropping_method
relationship: scale_of CO_334:0010501 ! Sensory assessment: Leaf edibility_method
relationship: scale_of CO_334:0010505 ! Olfactory Perception: Fufu smell_method
relationship: scale_of CO_334:0010506 ! Olfactory Perception: Attieke smell_method

[Term]
id: CO_334:0100540
name: 3pt scale
namespace: CassavaScale
is_a: CO_334:0100684 ! 3 point scales
relationship: scale_of CO_334:0010334 ! Estimation: Hydrogen cyanide potential enzymatic method

[Term]
id: CO_334:0100541
name: 9pt scale
namespace: CassavaScale
is_a: CO_334:0100689 ! 9 point scales
relationship: scale_of CO_334:0010335 ! Visual Rating: Unexpanded apical leaves colors_method

[Term]
id: CO_334:0100542
name: 9pt scale
namespace: CassavaScale
is_a: CO_334:0100689 ! 9 point scales
relationship: scale_of CO_334:0010336 ! Visual Rating: First fully expanded leaf color_method

[Term]
id: CO_334:0100543
name: 9pt scale
namespace: CassavaScale
is_a: CO_334:0100689 ! 9 point scales
relationship: scale_of CO_334:0010337 ! Visual Rating: Leaf vein color_method

[Term]
id: CO_334:0100544
name: 8pt scale
namespace: CassavaScale
is_a: CO_334:0100688 ! 8 point scales
relationship: scale_of CO_334:0010338 ! Visual Rating: Apical pubescence_method

[Term]
id: CO_334:0100545
name: 7pt scale
namespace: CassavaScale
is_a: CO_334:0100687 ! 7 point scales
relationship: scale_of CO_334:0010339 ! Visual Rating: Stipules length_method

[Term]
id: CO_334:0100546
name: number
namespace: CassavaScale
is_a: CO_334:0001001 ! Scales
relationship: scale_of CO_334:0010221 ! Counting: Number of planted stakes_method
relationship: scale_of CO_334:0010222 ! Counting: Sprout count _method
relationship: scale_of CO_334:0010223 ! Counting: Sprout count at one-month_method
relationship: scale_of CO_334:0010224 ! Counting: Sprout count at three-month_method
relationship: scale_of CO_334:0010225 ! Counting: Sprout count at six-month_method
relationship: scale_of CO_334:0010226 ! Counting: Sprout count at nine-month_method
relationship: scale_of CO_334:0010227 ! Counting: Sprout count at twelve-month_method
relationship: scale_of CO_334:0010320 ! Counting: Non marketable root number_method
relationship: scale_of CO_334:0010321 ! Counting: Marketable root number_method
relationship: scale_of CO_334:0010327 ! Counting: Bemisia tabaci adult_method
relationship: scale_of CO_334:0010328 ! Counting: Bemisia tabaci nymphs_method
relationship: scale_of CO_334:0010340 ! Visual Rating: Leaf lobes number_method
relationship: scale_of CO_334:0010392 ! Counting: Stem rot_method
relationship: scale_of CO_334:0010413 ! Counting: Number of fruits _method

[Term]
id: CO_334:0100547
name: 4pt scale
namespace: CassavaScale
is_a: CO_334:0100686 ! 4 point scales
relationship: scale_of CO_334:0010341 ! Visual Rating: Leaf lobe position_method

[Term]
id: CO_334:0100548
name: 10pt scale
namespace: CassavaScale
is_a: CO_334:0001001 ! Scales
relationship: scale_of CO_334:0010342 ! Visual Rating: Central leaf shape_method

[Term]
id: CO_334:0100549
name: 7pt scale
namespace: CassavaScale
is_a: CO_334:0100687 ! 7 point scales
relationship: scale_of CO_334:0010343 ! Visual Rating: Petiole Insertion Angle_method

[Term]
id: CO_334:0100550
name: 4pt scale
namespace: CassavaScale
is_a: CO_334:0100686 ! 4 point scales
relationship: scale_of CO_334:0010344 ! Visual Rating: Petiole Length_method

[Term]
id: CO_334:0100551
name: 7pt scale
namespace: CassavaScale
is_a: CO_334:0100687 ! 7 point scales
relationship: scale_of CO_334:0010345 ! Visual Rating: Petiole color_method

[Term]
id: CO_334:0100552
name: 4pt scale
namespace: CassavaScale
is_a: CO_334:0100686 ! 4 point scales
relationship: scale_of CO_334:0010346 ! Visual Rating: Anthocyanin pigmentation_method

[Term]
id: CO_334:0100553
name: 2pt scale
namespace: CassavaScale
is_a: CO_334:0100685 ! 2 point scales
relationship: scale_of CO_334:0010347 ! Visual Rating: Young stem growth habit_method

[Term]
id: CO_334:0100554
name: 8pt scale
namespace: CassavaScale
is_a: CO_334:0100688 ! 8 point scales
relationship: scale_of CO_334:0010348 ! Visual Rating: Young stem pubescence_method

[Term]
id: CO_334:0100555
name: 7pt scale
namespace: CassavaScale
is_a: CO_334:0100687 ! 7 point scales
relationship: scale_of CO_334:0010349 ! Visual Rating: Leaf scar prominence_method

[Term]
id: CO_334:0100556
name: weeks
namespace: CassavaScale
is_a: CO_334:0001001 ! Scales
relationship: scale_of CO_334:0010350 ! Visual Rating: Apical branching_method

[Term]
id: CO_334:0100557
name: number of levels
namespace: CassavaScale
is_a: CO_334:0001001 ! Scales
relationship: scale_of CO_334:0010351 ! Counting: Branching levels_method

[Term]
id: CO_334:0100558
name: cm
namespace: CassavaScale
is_a: CO_334:0001001 ! Scales
relationship: scale_of CO_334:0010000 ! Measurement: Plant height with leaf_method
relationship: scale_of CO_334:0010005 ! Measurement: Stem diameter_method
relationship: scale_of CO_334:0010303 ! Measurement: Plant height_method
relationship: scale_of CO_334:0010352 ! Measurement: First apical branch height_method
relationship: scale_of CO_334:0010384 ! Measurement: Plant height without leaf_method
relationship: scale_of CO_334:0010385 ! Measurement: Plantable stem_method
relationship: scale_of CO_334:0010387 ! Measurement: Average stem length_method
relationship: scale_of CO_334:0010396 ! Measurement: Leaf scar level_method
relationship: scale_of CO_334:0010418 ! Measurement: Leaf lobe length_method
relationship: scale_of CO_334:0010419 ! Measurement: Leaf lobe width_method
relationship: scale_of CO_334:0010464 ! Measurement: Petiole length_method
relationship: scale_of CO_334:0010472 ! Measurement: Peel thickness_method
relationship: scale_of CO_334:0010497 ! Measurement: Canopy width_method

[Term]
id: CO_334:0100559
name: 5pt scale
namespace: CassavaScale
is_a: CO_334:0100436 ! 5 point scales
relationship: scale_of CO_334:0010353 ! Visual Rating: Sepal color_method

[Term]
id: CO_334:0100560
name: 5pt scale
namespace: CassavaScale
is_a: CO_334:0100436 ! 5 point scales
relationship: scale_of CO_334:0010354 ! Visual Rating: Disc color_method

[Term]
id: CO_334:0100561
name: 5pt scale
namespace: CassavaScale
is_a: CO_334:0100436 ! 5 point scales
relationship: scale_of CO_334:0010355 ! Visual Rating: Stigma color_method

[Term]
id: CO_334:0100562
name: 5pt scale
namespace: CassavaScale
is_a: CO_334:0100436 ! 5 point scales
relationship: scale_of CO_334:0010356 ! Visual Rating: Ovary color_method

[Term]
id: CO_334:0100563
name: 3pt scale
namespace: CassavaScale
is_a: CO_334:0100684 ! 3 point scales
relationship: scale_of CO_334:0010357 ! Visual Rating: Anther color_method

[Term]
id: CO_334:0100564
name: 2pt scale
namespace: CassavaScale
is_a: CO_334:0100685 ! 2 point scales
relationship: scale_of CO_334:0010358 ! Visual Rating: Female stamenoids_method

[Term]
id: CO_334:0100565
name: 2pt scale
namespace: CassavaScale
is_a: CO_334:0100685 ! 2 point scales
relationship: scale_of CO_334:0010359 ! Visual Rating: Male sterile_method

[Term]
id: CO_334:0100566
name: 7pt scale
namespace: CassavaScale
is_a: CO_334:0100687 ! 7 point scales
relationship: scale_of CO_334:0010360 ! Visual Rating: Fruit exocarp Texture_method

[Term]
id: CO_334:0100567
name: 4pt scale
namespace: CassavaScale
is_a: CO_334:0100686 ! 4 point scales
relationship: scale_of CO_334:0010361 ! Visual Rating: Ploidy_method

[Term]
id: CO_334:0100568
name: 5pt scale
namespace: CassavaScale
is_a: CO_334:0100436 ! 5 point scales
relationship: scale_of CO_334:0010362 ! Visual Rating: Seed color_method

[Term]
id: CO_334:0100569
name: 4pt scale
namespace: CassavaScale
is_a: CO_334:0100686 ! 4 point scales
relationship: scale_of CO_334:0010363 ! Visual Rating: Caruncle color_method

[Term]
id: CO_334:0100570
name: 3pt scale
namespace: CassavaScale
is_a: CO_334:0100684 ! 3 point scales
relationship: scale_of CO_334:0010364 ! Visual Rating: Root position_method

[Term]
id: CO_334:0100571
name: 7pt scale
namespace: CassavaScale
is_a: CO_334:0100687 ! 7 point scales
relationship: scale_of CO_334:0010365 ! Visual Rating: Storage root diameter_method

[Term]
id: CO_334:0100572
name: ug/g
namespace: CassavaScale
is_a: CO_334:0001001 ! Scales
relationship: scale_of CO_334:0010366 ! Estimation: Abscisic acid content_method
relationship: scale_of CO_334:0010369 ! Estimation: Beta carotene_method
relationship: scale_of CO_334:0010370 ! Estimation: Iron content_method
relationship: scale_of CO_334:0010371 ! Estimation: Zinc content_method
relationship: scale_of CO_334:0010374 ! Estimation: Amylose  content_method
relationship: scale_of CO_334:0010375 ! Estimation: Amylopectin content_method
relationship: scale_of CO_334:0010414 ! Estimation: Total carotenoid by icheck method

[Term]
id: CO_334:0100574
name: ug beta caroten / g fresh weight
namespace: CassavaScale
is_a: CO_334:0001001 ! Scales
relationship: scale_of CO_334:0010368 ! Estimation: Total carotenoid content_method

[Term]
id: CO_334:0100582
name: ratio
namespace: CassavaScale
is_a: CO_334:0001001 ! Scales
relationship: scale_of CO_334:0010009 ! Estimation: Dry matter content of leaf percentage
relationship: scale_of CO_334:0010010 ! Estimation: Dry matter content of lower stem percentage
relationship: scale_of CO_334:0010011 ! Estimation: Dry matter content of fibrous root percentage
relationship: scale_of CO_334:0010220 ! Counting: Sprouting_method
relationship: scale_of CO_334:0010236 ! Counting: Cassava mosaic disease incidence 1-month evaluation_method
relationship: scale_of CO_334:0010237 ! Counting: Cassava mosaic disease incidence 3-month evaluation_method
relationship: scale_of CO_334:0010238 ! Counting: Cassava mosaic disease incidence 6-month evaluation_method
relationship: scale_of CO_334:0010239 ! Counting: Cassava mosaic disease incidence 9-month evaluation_method
relationship: scale_of CO_334:0010240 ! Counting: Cassava mosaic disease incidence 12-month evaluation_method
relationship: scale_of CO_334:0010247 ! Counting: Cassava bacterial blight incidence 3-month evalution_method
relationship: scale_of CO_334:0010248 ! Counting: Cassava bacterial blight incidence 6-month evalution_method
relationship: scale_of CO_334:0010249 ! Counting: Cassava bacterial blight incidence 9-month evalution_method
relationship: scale_of CO_334:0010250 ! Counting: Cassava bacterial blight incidence 12-month evaluation_method
relationship: scale_of CO_334:0010257 ! Counting: Cassava anthractnose disease incidence in 3-months_method
relationship: scale_of CO_334:0010258 ! Counting: Cassava anthractnose disease incidence in 6-months_method
relationship: scale_of CO_334:0010259 ! Counting: Cassava anthractnose disease incidence in 9-months_method
relationship: scale_of CO_334:0010260 ! Counting: Cassava anthractnose disease incidence in 12-months_method
relationship: scale_of CO_334:0010262 ! Counting: Cassava green mite incidence first evaluation_method
relationship: scale_of CO_334:0010263 ! Counting: Cassava green mite incidence second evaluation_method
relationship: scale_of CO_334:0010268 ! Counting: Cassava mealy bug incidence_method
relationship: scale_of CO_334:0010275 ! Counting: Cassava brown streak disease leaf incidence 1-month evaluation_method
relationship: scale_of CO_334:0010276 ! Counting: Cassava brown streak disease leaf incidence 3-month evaluation_method
relationship: scale_of CO_334:0010277 ! Counting: Cassava brown streak disease leaf incidence 6-month evaluation_method
relationship: scale_of CO_334:0010278 ! Counting: Cassava brown streak disease leaf incidence 9-month evaluation_method
relationship: scale_of CO_334:0010282 ! Counting: Cassava brown streak disease root incidence 12-month evaluation_method
relationship: scale_of CO_334:0010300 ! Estimation: Root dry matter content_method
relationship: scale_of CO_334:0010304 ! Counting: Proportion of lodged plants_method
relationship: scale_of CO_334:0010324 ! Counting: Red spider mite incidence_method
relationship: scale_of CO_334:0010326 ! Counting: Spiraling whitefly incidence_method
relationship: scale_of CO_334:0010376 ! Calculation: Amylose amylopectin ratio_method
relationship: scale_of CO_334:0010441 ! Counting: Flowering incidence_method
relationship: scale_of CO_334:0010499 ! Counting: Cassava rust disease incidence_method
relationship: scale_of CO_334:0010512 ! Calculation: Harvest index_method

[Term]
id: CO_334:0100583
name: pct (%)
namespace: CassavaScale
is_a: CO_334:0001001 ! Scales
relationship: scale_of CO_334:0010313 ! Estimation: Starch content _method
relationship: scale_of CO_334:0010314 ! Estimation: Moisture content_method
relationship: scale_of CO_334:0010372 ! Estimation: Protein content_method
relationship: scale_of CO_334:0010373 ! Estimation: Fibre content_method
relationship: scale_of CO_334:0010377 ! Estimation: Ascorbic acid_method
relationship: scale_of CO_334:0010378 ! Estimation: Ash content_method
relationship: scale_of CO_334:0010379 ! Estimation: Sugar content_method
relationship: scale_of CO_334:0010382 ! Estimation: Beta carotenoid retention_method
relationship: scale_of CO_334:0010383 ! Estimation: Total carotenoid retention_method
relationship: scale_of CO_334:0010422 ! Estimation: Trans 9_method
relationship: scale_of CO_334:0010423 ! Estimation: Cis 9_method
relationship: scale_of CO_334:0010424 ! Estimation: B crypto_method
relationship: scale_of CO_334:0010430 ! Calculation: Percent of rotten roots_method
relationship: scale_of CO_334:0010452 ! Estimation: Gari starch_method
relationship: scale_of CO_334:0010457 ! Estimation: Percentage leaf retention_method
relationship: scale_of CO_334:0010458 ! Estimation: Percentage leaf retention at 5 months after planting_method
relationship: scale_of CO_334:0010459 ! Estimation: Percentage leaf retention at 6 months after planting_method
relationship: scale_of CO_334:0010460 ! Estimation: Percentage leaf retention at 7 months after planting_method
relationship: scale_of CO_334:0010461 ! Estimation: Leaf retention at harvest_method
relationship: scale_of CO_334:0010507 ! Prediction: Dry matter content by QST_method
relationship: scale_of CO_334:0010508 ! Prediction: Dry matter content by SciO_method
relationship: scale_of CO_334:0010509 ! Prediction: Dry matter content by table-top NIRS_method
relationship: scale_of CO_334:0010523 ! Computation: Change in weight after boiling
relationship: scale_of CO_334:0010526 ! Computation: Cassava brown streak disease root severity in percentage_method
relationship: scale_of CO_334:0010533 ! Estimation: Moisture content_method

[Term]
id: CO_334:0100586
name: g/kg
namespace: CassavaScale
is_a: CO_334:0001001 ! Scales
relationship: scale_of CO_334:0010315 ! Measurement: Gari content_method
relationship: scale_of CO_334:0010380 ! Estimation: Fufu content_method
relationship: scale_of CO_334:0010381 ! Estimation: Lafun content_method

[Term]
id: CO_334:0100594
name: stem
namespace: CassavaScale
is_a: CO_334:0001001 ! Scales
relationship: scale_of CO_334:0010388 ! Counting: Stem number_method

[Term]
id: CO_334:0100601
name: scars
namespace: CassavaScale
is_a: CO_334:0001001 ! Scales
relationship: scale_of CO_334:0010395 ! Counting: Leaf scar number_method

[Term]
id: CO_334:0100603
name: 4pt scale
namespace: CassavaScale
is_a: CO_334:0100686 ! 4 point scales
relationship: scale_of CO_334:0010397 ! Visual Rating: Branching habit_method

[Term]
id: CO_334:0100606
name: flowers
namespace: CassavaScale
is_a: CO_334:0001001 ! Scales
relationship: scale_of CO_334:0010006 ! Counting: Female flower number all levels_method
relationship: scale_of CO_334:0010007 ! Counting: Male flower number on all levels_method
relationship: scale_of CO_334:0010020 ! Counting: Male flower number by branch level
relationship: scale_of CO_334:0010400 ! Counting: Female flower number_method
relationship: scale_of CO_334:0010401 ! Counting: Male flower number_method

[Term]
id: CO_334:0100608
name: stalks
namespace: CassavaScale
is_a: CO_334:0001001 ! Scales
relationship: scale_of CO_334:0010402 ! Counting: Number of flowering stalks per branch level _method

[Term]
id: CO_334:0100609
name: forks
namespace: CassavaScale
is_a: CO_334:0001001 ! Scales
relationship: scale_of CO_334:0010017 ! Counting: Number of forks by branch level
relationship: scale_of CO_334:0010403 ! Counting: Number of forks_method

[Term]
id: CO_334:0100611
name: days
namespace: CassavaScale
is_a: CO_334:0001001 ! Scales
relationship: scale_of CO_334:0010008 ! Visual Observation: Days to first male flower opens
relationship: scale_of CO_334:0010013 ! Visual Observation: Days to branching event
relationship: scale_of CO_334:0010014 ! Visual Observation: Days to abortion by branching level
relationship: scale_of CO_334:0010015 ! Visual Observation: Days to first female flower opens by branch levels
relationship: scale_of CO_334:0010016 ! Visual Observation: Days to senescence by branch level
relationship: scale_of CO_334:0010021 ! Visual Observation: Days to fruitset by branch level
relationship: scale_of CO_334:0010367 ! Calculation: Leaf life _method
relationship: scale_of CO_334:0010398 ! Visual Observation: Days to 50% branching_method
relationship: scale_of CO_334:0010399 ! Visual Observation: Days to first inflorescence_method
relationship: scale_of CO_334:0010404 ! Visual Observation: Days to first anthesis_method
relationship: scale_of CO_334:0010405 ! Visual Observation: Days to 50% anthesis_method

[Term]
id: CO_334:0100612
name: fruits
namespace: CassavaScale
is_a: CO_334:0001001 ! Scales
relationship: scale_of CO_334:0010406 ! Counting: Number of fruitset_method

[Term]
id: CO_334:0100614
name: nymphs
namespace: CassavaScale
is_a: CO_334:0001001 ! Scales
relationship: scale_of CO_334:0010407 ! Counting: Bemisia tabaci nymphs yellow_method
relationship: scale_of CO_334:0010408 ! Counting: Bemisia tabaci nymphs black_method

[Term]
id: CO_334:0100615
name: 5pt scale
namespace: CassavaScale
is_a: CO_334:0100436 ! 5 point scales
relationship: scale_of CO_334:0010409 ! Visual Observation: Bemisia tabaci nymphs severity_method

[Term]
id: CO_334:0100616
name: 2pt scale
namespace: CassavaScale
is_a: CO_334:0100685 ! 2 point scales
relationship: scale_of CO_334:0010410 ! Visual Observation: Typhlodromalus aripo_method

[Term]
id: CO_334:0100617
name: proportion
namespace: CassavaScale
is_a: CO_334:0001001 ! Scales
relationship: scale_of CO_334:0010411 ! Counting: Plant number with inflorescence_method
relationship: scale_of CO_334:0010540 ! Counting: Cassava blight leaf spot disease incidence_method
relationship: scale_of CO_334:0010541 ! Counting: Cassava brown leaf spot disease incidence_method
relationship: scale_of CO_334:0010542 ! Counting: Cassava white leaf spot disease incidence_method

[Term]
id: CO_334:0100623
name: g
namespace: CassavaScale
is_a: CO_334:0001001 ! Scales
relationship: scale_of CO_334:0010417 ! Measurement: Specific gravity_method

[Term]
id: CO_334:0100626
name: seedling
namespace: CassavaScale
is_a: CO_334:0001001 ! Scales
relationship: scale_of CO_334:0010420 ! Counting: Germination count_method

[Term]
id: CO_334:0100627
name: seed
namespace: CassavaScale
is_a: CO_334:0001001 ! Scales
relationship: scale_of CO_334:0010421 ! Counting: Number of seeds sown_method

[Term]
id: CO_334:0100631
name: 3pt scale
namespace: CassavaScale
is_a: CO_334:0100684 ! 3 point scales
relationship: scale_of CO_334:0010425 ! Sensory Assesment: Ease of harvest_method

[Term]
id: CO_334:0100632
name: 3pt scale
namespace: CassavaScale
is_a: CO_334:0100684 ! 3 point scales
relationship: scale_of CO_334:0010426 ! Visual Rating: Root length evaluation_method

[Term]
id: CO_334:0100633
name: 3pt scale
namespace: CassavaScale
is_a: CO_334:0100684 ! 3 point scales
relationship: scale_of CO_334:0010427 ! Visual Rating: Stalk average length evaluation_method

[Term]
id: CO_334:0100634
name: 3pt scale
namespace: CassavaScale
is_a: CO_334:0100684 ! 3 point scales
relationship: scale_of CO_334:0010428 ! Visual rating: Root constriction_method

[Term]
id: CO_334:0100635
name: 5pt scale
namespace: CassavaScale
is_a: CO_334:0100436 ! 5 point scales
relationship: scale_of CO_334:0010429 ! Visual Rating: Root evaluation_method

[Term]
id: CO_334:0100637
name: kg/plant
namespace: CassavaScale
is_a: CO_334:0001001 ! Scales
relationship: scale_of CO_334:0010431 ! Estimation: Plant yield_method

[Term]
id: CO_334:0100638
name: t/ha/year
namespace: CassavaScale
is_a: CO_334:0001001 ! Scales
relationship: scale_of CO_334:0010432 ! Estimation: Yield per year_method

[Term]
id: CO_334:0100639
name: yes/no scale
namespace: CassavaScale
is_a: CO_334:0001001 ! Scales
relationship: scale_of CO_334:0010433 ! Selection: Selected variety_method

[Term]
id: CO_334:0100640
name: 4pt scale
namespace: CassavaScale
is_a: CO_334:0100686 ! 4 point scales
relationship: scale_of CO_334:0010434 ! Visual Observation: Flowering_method

[Term]
id: CO_334:0100641
name: 2pt scale
namespace: CassavaScale
is_a: CO_334:0100685 ! 2 point scales
relationship: scale_of CO_334:0010435 ! Visual Rating: Initial plant vigor_method

[Term]
id: CO_334:0100642
name: 3pt scale
namespace: CassavaScale
is_a: CO_334:0100684 ! 3 point scales
relationship: scale_of CO_334:0010436 ! Visual Rating: Root color_method

[Term]
id: CO_334:0100643
name: 3pt scale
namespace: CassavaScale
is_a: CO_334:0100684 ! 3 point scales
relationship: scale_of CO_334:0010437 ! Visual Rating: Root flesh color_method

[Term]
id: CO_334:0100644
name: 3pt scale
namespace: CassavaScale
is_a: CO_334:0100684 ! 3 point scales
relationship: scale_of CO_334:0010438 ! Visual Rating: Root neck length_method

[Term]
id: CO_334:0100645
name: 4pt scale
namespace: CassavaScale
is_a: CO_334:0100686 ! 4 point scales
relationship: scale_of CO_334:0010439 ! Visual Rating: Female flower evaluation_method

[Term]
id: CO_334:0100646
name: 9pt scale
namespace: CassavaScale
is_a: CO_334:0100689 ! 9 point scales
relationship: scale_of CO_334:0010440 ! Visual Rating: Staygreen_method

[Term]
id: CO_334:0100648
name: 5pt scale
namespace: CassavaScale
is_a: CO_334:0100436 ! 5 point scales
relationship: scale_of CO_334:0010442 ! Visual Observation: Hairiness_method

[Term]
id: CO_334:0100649
name: 5pt scale
namespace: CassavaScale
is_a: CO_334:0100436 ! 5 point scales
relationship: scale_of CO_334:0010443 ! Visual Observation: Sooty mould_method

[Term]
id: CO_334:0100657
name: kg/g
namespace: CassavaScale
is_a: CO_334:0001001 ! Scales
relationship: scale_of CO_334:0010450 ! Measurement: Gari sampled weight_method
relationship: scale_of CO_334:0010451 ! Measurement: Gari weight after drying_method

[Term]
id: CO_334:0100659
name: 4pt scale
namespace: CassavaScale
is_a: CO_334:0100686 ! 4 point scales
relationship: scale_of CO_334:0010453 ! Sensory Assesment: Gari fibre_method

[Term]
id: CO_334:0100660
name: 3pt scale
namespace: CassavaScale
is_a: CO_334:0100684 ! 3 point scales
relationship: scale_of CO_334:0010454 ! Gustation: Gari taste_method

[Term]
id: CO_334:0100661
name: 3pt scale
namespace: CassavaScale
is_a: CO_334:0100684 ! 3 point scales
relationship: scale_of CO_334:0010455 ! Visual Rating: Swelling capacity_method

[Term]
id: CO_334:0100662
name: stakes
namespace: CassavaScale
is_a: CO_334:0001001 ! Scales
relationship: scale_of CO_334:0010456 ! Counting: Number of stakes_method

[Term]
id: CO_334:0100668
name: 2pt scale
namespace: CassavaScale
is_a: CO_334:0100685 ! 2 point scales
relationship: scale_of CO_334:0010462 ! Visual Observation: Assessment of presence of leaf pubescence_method

[Term]
id: CO_334:0100669
name: 7pt scale
namespace: CassavaScale
is_a: CO_334:0100687 ! 7 point scales
relationship: scale_of CO_334:0010463 ! Visual Observation: Leaf lobe margin_method

[Term]
id: CO_334:0100671
name: 4pt scale
namespace: CassavaScale
is_a: CO_334:0100686 ! 4 point scales
relationship: scale_of CO_334:0010465 ! Visual Observation: Petiole orientation_method

[Term]
id: CO_334:0100672
name: 2pt scale
namespace: CassavaScale
is_a: CO_334:0100685 ! 2 point scales
relationship: scale_of CO_334:0010466 ! Visual Observation: Presence of pollen_method

[Term]
id: CO_334:0100673
name: 3pt scale
namespace: CassavaScale
is_a: CO_334:0100684 ! 3 point scales
relationship: scale_of CO_334:0010467 ! Visual Scoring: Stem cortex color_method

[Term]
id: CO_334:0100674
name: 4pt scale
namespace: CassavaScale
is_a: CO_334:0100686 ! 4 point scales
relationship: scale_of CO_334:0010468 ! Visual Scoring: Stem epidermis color_method

[Term]
id: CO_334:0100675
name: 7pt scale
namespace: CassavaScale
is_a: CO_334:0100687 ! 7 point scales
relationship: scale_of CO_334:0010469 ! Visual Rating: Leaf scar distance_method

[Term]
id: CO_334:0100676
name: 4pt scale
namespace: CassavaScale
is_a: CO_334:0100686 ! 4 point scales
relationship: scale_of CO_334:0010470 ! Visual Observation: Plant shape_method

[Term]
id: CO_334:0100677
name: 2pt scale
namespace: CassavaScale
is_a: CO_334:0100685 ! 2 point scales
relationship: scale_of CO_334:0010471 ! Visual Observation: Stipule margin_method

[Term]
id: CO_334:0100678
name: cubic meter
namespace: CassavaScale
is_a: CO_334:0001001 ! Scales

[Term]
id: CO_334:0100679
name: m
namespace: CassavaScale
is_a: CO_334:0001001 ! Scales

[Term]
id: CO_334:0100680
name: 11pt scale
namespace: CassavaScale
is_a: CO_334:0001001 ! Scales
relationship: scale_of CO_334:0010001 ! Estimation: Post-harvest physiological deterioration method

[Term]
id: CO_334:0100681
name: m3
namespace: CassavaScale
is_a: CO_334:0001001 ! Scales
relationship: scale_of CO_334:0010494 ! Calculation: Plot volume_method

[Term]
id: CO_334:0100682
name: 5 pt scale
namespace: CassavaScale
is_a: CO_334:0100436 ! 5 point scales
relationship: scale_of CO_334:0010500 ! Visual Observation: Cassava rust disease severity_method

[Term]
id: CO_334:0100683
name: 3pt scale
namespace: CassavaScale
is_a: CO_334:0100684 ! 3 point scales
relationship: scale_of CO_334:0010502 ! Visual Rating: Cooking quality_method
relationship: scale_of CO_334:0010504 ! Visual Rating: Apical pubescence_method

[Term]
id: CO_334:0100684
name: 3 point scales
namespace: CassavaScale
is_a: CO_334:0001001 ! Scales

[Term]
id: CO_334:0100685
name: 2 point scales
namespace: CassavaScale
is_a: CO_334:0001001 ! Scales

[Term]
id: CO_334:0100686
name: 4 point scales
namespace: CassavaScale
is_a: CO_334:0001001 ! Scales

[Term]
id: CO_334:0100687
name: 7 point scales
namespace: CassavaScale
is_a: CO_334:0001001 ! Scales

[Term]
id: CO_334:0100688
name: 8 point scales
namespace: CassavaScale
is_a: CO_334:0001001 ! Scales

[Term]
id: CO_334:0100689
name: 9 point scales
namespace: CassavaScale
is_a: CO_334:0001001 ! Scales

[Term]
id: CO_334:0100690
name: c/t
namespace: CassavaScale
def: "CO_334:0100690" []
is_a: CO_334:0001001 ! Scales
relationship: scale_of CO_334:0010510 ! PCR assay: Cassava Brown Streak Virus_method
relationship: scale_of CO_334:0010511 ! PCR assay: Ugandan Cassava Brown Streak Virus_method

[Term]
id: CO_334:0100691
name: nodes
namespace: CassavaScale
def: "Number of nodes." []
is_a: CO_334:0001001 ! Scales

[Term]
id: CO_334:0100692
name: um
namespace: CassavaScale
is_a: CO_334:0001001 ! Scales

[Term]
id: CO_334:0100693
name: dp
namespace: CassavaScale
is_a: CO_334:0001001 ! Scales

[Term]
id: CO_334:0100695
name: newton
namespace: CassavaScale
is_a: CO_334:0001001 ! Scales

[Term]
id: CO_334:0100696
name: minute
namespace: CassavaScale
synonym: "min" EXACT []
is_a: CO_334:0001001 ! Scales
relationship: scale_of CO_334:0010524 ! Estimation: Time of boiling

[Term]
id: CO_334:0100697
name: mm
namespace: CassavaScale
is_a: CO_334:0001001 ! Scales
relationship: scale_of CO_334:0010525 ! Measurement: Textural characteristic

[Term]
id: CO_334:0100698
name: g/mm
namespace: CassavaScale
is_a: CO_334:0001001 ! Scales
relationship: scale_of CO_334:0010525 ! Measurement: Textural characteristic

[Term]
id: CO_334:0100699
name: gmm
namespace: CassavaScale
is_a: CO_334:0001001 ! Scales
relationship: scale_of CO_334:0010525 ! Measurement: Textural characteristic

[Term]
id: CO_334:0100700
name: 8pt scale
namespace: CassavaScale
is_a: CO_334:0100688 ! 8 point scales
relationship: scale_of CO_334:0010527 ! Visual Rating: Root flesh color ring_method

[Term]
id: CO_334:0100701
name: 5 pt scale
namespace: CassavaScale
is_a: CO_334:0100436 ! 5 point scales
relationship: scale_of CO_334:0010528 ! Visual Observation:Whitefly severity evaluation_method
relationship: scale_of CO_334:0010529 ! Visual Observation: Thrips severity evaluation_method

[Term]
id: CO_334:0100702
name: degree
namespace: CassavaScale
is_a: CO_334:0001001 ! Scales
relationship: scale_of CO_334:0010530 ! Visual Scoring :Branching Angle_degree_method

[Term]
id: CO_334:0100703
name: degree celsius
namespace: CassavaScale
is_a: CO_334:0001001 ! Scales
relationship: scale_of CO_334:0010538 ! Measurement: Peak viscosity_method
relationship: scale_of CO_334:0010539 ! Measurement: Pasting temperature_method

[Term]
id: CO_334:0100704
name: pascal per seconds
namespace: CassavaScale
is_a: CO_334:0001001 ! Scales
relationship: scale_of CO_334:0010534 ! Calculation: Setback_method
relationship: scale_of CO_334:0010535 ! Estimation: Final viscosity_method
relationship: scale_of CO_334:0010536 ! Calculation: Breakdown_method
relationship: scale_of CO_334:0010537 ! Estimation: Trough_method

[Term]
id: CO_334:0100705
name: 5 pt scale
namespace: CassavaScale
is_a: CO_334:0100436 ! 5 point scales
relationship: scale_of CO_334:0010543 ! Visual Observation: Cassava white leaf spot disease severity_method
relationship: scale_of CO_334:0010544 ! Visual Observation: Cassava brown leaf spot disease severity_method
relationship: scale_of CO_334:0010545 ! Visual Observation: Cassava blight leaf spot disease severity_method

[Term]
id: CO_334:0100706
name: ng/ml
namespace: CassavaScale
def: "Nanograms per milliliter, abbreviated ng/ml" []
is_a: CO_334:0001001 ! Scales
relationship: scale_of CO_334:0010550 ! Absorption: Cassava brown streak viral titre_method

[Term]
id: CO_334:0103000
name: Surface yellowness scale 0-10
namespace: CassavaScale
is_a: CO_334:0001001 ! Scales
relationship: scale_of CO_334:0013000 ! surface yellowness appearance method

[Term]
id: CO_334:0103001
name: Boiled cassava surface whitness 0-10
namespace: CassavaScale
is_a: CO_334:0001001 ! Scales
relationship: scale_of CO_334:0013047 ! surface whiteness appearance method

[Term]
id: CO_334:0103002
name: Surface colour homogeneity 0-10
namespace: CassavaScale
is_a: CO_334:0001001 ! Scales
relationship: scale_of CO_334:0013018 ! color homogeneity appearance method

[Term]
id: CO_334:0103003
name: Surface smoothness scale 0-10
namespace: CassavaScale
is_a: CO_334:0001001 ! Scales
relationship: scale_of CO_334:0013046 ! surface smoothness appearance method

[Term]
id: CO_334:0103004
name: Hardness texture in the mouth scale 0-10
namespace: CassavaScale
is_a: CO_334:0001001 ! Scales
relationship: scale_of CO_334:0013001 ! stickiness texture in the mouth method

[Term]
id: CO_334:0103005
name: Moisture texture in the mouth s scale 0-10
namespace: CassavaScale
is_a: CO_334:0001001 ! Scales
relationship: scale_of CO_334:0013001 ! stickiness texture in the mouth method

[Term]
id: CO_334:0103006
name: Boiled root smoothness in the mouth scale 0-10
namespace: CassavaScale
is_a: CO_334:0001001 ! Scales
relationship: scale_of CO_334:0013001 ! stickiness texture in the mouth method

[Term]
id: CO_334:0103007
name: Boiled root fibrousness in mouth scale 0-10
namespace: CassavaScale
is_a: CO_334:0001001 ! Scales
relationship: scale_of CO_334:0013001 ! stickiness texture in the mouth method

[Term]
id: CO_334:0103008
name: Mealiness texture in the mouth scale 0-10
namespace: CassavaScale
is_a: CO_334:0001001 ! Scales
relationship: scale_of CO_334:0013001 ! stickiness texture in the mouth method

[Term]
id: CO_334:0103009
name: Stickness in the mouth scale 0-10
namespace: CassavaScale
is_a: CO_334:0001001 ! Scales
relationship: scale_of CO_334:0013001 ! stickiness texture in the mouth method

[Term]
id: CO_334:0103010
name: Mealiness in the hand scale 0-10
namespace: CassavaScale
is_a: CO_334:0001001 ! Scales
relationship: scale_of CO_334:0013002 ! mealiness texture in the hand method

[Term]
id: CO_334:0103011
name: Boiled root moldability by hand scale 0-10
namespace: CassavaScale
is_a: CO_334:0001001 ! Scales
relationship: scale_of CO_334:0013008 ! moldability texture in the hand method

[Term]
id: CO_334:0103012
name: Boiled root stickness in hand  scale 0-10
namespace: CassavaScale
is_a: CO_334:0001001 ! Scales
relationship: scale_of CO_334:0013007 ! stickiness texture in the hand method

[Term]
id: CO_334:0103013
name: Boiled root sweetness taste scale 0-10
namespace: CassavaScale
is_a: CO_334:0001001 ! Scales
relationship: scale_of CO_334:0013003 ! sweetness taste method

[Term]
id: CO_334:0103014
name: Bitterness scale 0-10
namespace: CassavaScale
is_a: CO_334:0001001 ! Scales
relationship: scale_of CO_334:0013014 ! bitterness taste method

[Term]
id: CO_334:0103015
name: 2 pt scale
namespace: CassavaScale
is_a: CO_334:0001001 ! Scales
relationship: scale_of CO_334:0013048 ! sweetpotato-like aroma method

[Term]
id: CO_334:0103016
name: Cassava-like aroma scale 0-10
namespace: CassavaScale
is_a: CO_334:0001001 ! Scales
relationship: scale_of CO_334:0013004 ! steamed cassava-like_aroma  method

[Term]
id: CO_334:0103017
name: Appearance trait
namespace: cassava_trait
is_a: CO_334:0000004 ! Quality trait

[Term]
id: CO_334:0103018
name: Texture in mouth trait
namespace: cassava_trait
is_a: CO_334:0000004 ! Quality trait

[Term]
id: CO_334:0103019
name: Texture in hand trait
namespace: cassava_trait
is_a: CO_334:0000004 ! Quality trait

[Term]
id: CO_334:0103020
name: Taste trait
namespace: cassava_trait
is_a: CO_334:0000004 ! Quality trait

[Term]
id: CO_334:0103021
name: Aroma trait
namespace: cassava_trait
is_a: CO_334:0000004 ! Quality trait

[Term]
id: CO_334:0103022
name: Surface colour appearance scale 1-8
namespace: CassavaScale
is_a: CO_334:0001001 ! Scales
relationship: scale_of CO_334:0013005 ! surface colour sppearance method

[Term]
id: CO_334:0103023
name: Smoothness in the hand scale 0-10
namespace: CassavaScale
is_a: CO_334:0001001 ! Scales
relationship: scale_of CO_334:0013006 ! smoothness texture in the hand method

[Term]
id: CO_334:0103024
name: Fufu stickiness in hand scale 0-10
namespace: CassavaScale
is_a: CO_334:0001001 ! Scales
relationship: scale_of CO_334:0013007 ! stickiness texture in the hand method

[Term]
id: CO_334:0103025
name: Fufu moldability by hand scale 0-10
namespace: CassavaScale
is_a: CO_334:0001001 ! Scales
relationship: scale_of CO_334:0013008 ! moldability texture in the hand method

[Term]
id: CO_334:0103026
name: Fufu hardness by hand scale 0-10
namespace: CassavaScale
is_a: CO_334:0001001 ! Scales
relationship: scale_of CO_334:0013009 ! hardness texture by hand method

[Term]
id: CO_334:0103027
name: Fufu stretchability in hand scale 0-10
namespace: CassavaScale
is_a: CO_334:0001001 ! Scales
relationship: scale_of CO_334:0013010 ! stretchability texture by the hand method

[Term]
id: CO_334:0103028
name: Fufu odour scale 0-10
namespace: CassavaScale
is_a: CO_334:0001001 ! Scales
relationship: scale_of CO_334:0013011 ! odour method

[Term]
id: CO_334:0103029
name: Attieke aroma scale 0-10
namespace: CassavaScale
is_a: CO_334:0001001 ! Scales
relationship: scale_of CO_334:0013012 ! attieke-like aroma method

[Term]
id: CO_334:0103030
name: Attieke cohesiveness scale 0-10
namespace: CassavaScale
is_a: CO_334:0001001 ! Scales
relationship: scale_of CO_334:0013017 ! cohesiveness texture by touch method

[Term]
id: CO_334:0103031
name: Attieke sourness in the mouth scale 0-10
namespace: CassavaScale
is_a: CO_334:0001001 ! Scales
relationship: scale_of CO_334:0013043 ! sourness taste method

[Term]
id: CO_334:0103032
name: Attieke Stickness in hand scale 0-10
namespace: CassavaScale
is_a: CO_334:0001001 ! Scales
relationship: scale_of CO_334:0013007 ! stickiness texture in the hand method

[Term]
id: CO_334:0103033
name: Attieke Sweetness taste scale 0-10
namespace: CassavaScale
is_a: CO_334:0001001 ! Scales
relationship: scale_of CO_334:0013003 ! sweetness taste method

[Term]
id: CO_334:0103034
name: Bitter aftertaste scale 0-100
namespace: CassavaScale
is_a: CO_334:0001001 ! Scales
relationship: scale_of CO_334:0013013 ! bitterness after taste method

[Term]
id: CO_334:0103035
name: Bitterness scale 0-100
namespace: CassavaScale
is_a: CO_334:0001001 ! Scales
relationship: scale_of CO_334:0013014 ! bitterness taste method

[Term]
id: CO_334:0103036
name: boiled root odour scale 0-100
namespace: CassavaScale
is_a: CO_334:0001001 ! Scales
relationship: scale_of CO_334:0013015 ! boiled cassava odour method

[Term]
id: CO_334:0103037
name: boiled root stickness in hand scale 0-100
namespace: CassavaScale
is_a: CO_334:0001001 ! Scales
relationship: scale_of CO_334:0013007 ! stickiness texture in the hand method

[Term]
id: CO_334:0103038
name: Boiled root sweetness taste scale 0-100
namespace: CassavaScale
is_a: CO_334:0001001 ! Scales
relationship: scale_of CO_334:0013003 ! sweetness taste method

[Term]
id: CO_334:0103039
name: Brightness appearance scale 0-10
namespace: CassavaScale
is_a: CO_334:0001001 ! Scales
relationship: scale_of CO_334:0013016 ! brightness appearance method

[Term]
id: CO_334:0103040
name: Crumbness in the hand scale 0-100
namespace: CassavaScale
is_a: CO_334:0001001 ! Scales
relationship: scale_of CO_334:0013019 ! crumbly in the hand method

[Term]
id: CO_334:0103041
name: Easy to chew scale 0-100
namespace: CassavaScale
is_a: CO_334:0001001 ! Scales
relationship: scale_of CO_334:0013020 ! easy to chew texture in the mouth method

[Term]
id: CO_334:0103042
name: Eba cohesiveness in the hand  scale 0-10
namespace: CassavaScale
is_a: CO_334:0001001 ! Scales
relationship: scale_of CO_334:0013017 ! cohesiveness texture by touch method

[Term]
id: CO_334:0103043
name: Eba fibrousness in mouth scale 0-10
namespace: CassavaScale
is_a: CO_334:0001001 ! Scales
relationship: scale_of CO_334:0013025 ! fibrousness texture in the mouth method

[Term]
id: CO_334:0103044
name: Eba hardness in the hand scale 0-10
namespace: CassavaScale
is_a: CO_334:0001001 ! Scales
relationship: scale_of CO_334:0013009 ! hardness texture by hand method

[Term]
id: CO_334:0103045
name: Eba smoothness in the mouth scale 0-10
namespace: CassavaScale
is_a: CO_334:0001001 ! Scales
relationship: scale_of CO_334:0013053 ! smoothness texture in the mouth method

[Term]
id: CO_334:0103046
name: Eba sourness taste scale 0-10
namespace: CassavaScale
is_a: CO_334:0001001 ! Scales
relationship: scale_of CO_334:0013043 ! sourness taste method

[Term]
id: CO_334:0103047
name: Eba stickiness in hand scale 0-10
namespace: CassavaScale
is_a: CO_334:0001001 ! Scales
relationship: scale_of CO_334:0013007 ! stickiness texture in the hand method

[Term]
id: CO_334:0103048
name: Eba streachability in hand scale 0-10
namespace: CassavaScale
is_a: CO_334:0001001 ! Scales
relationship: scale_of CO_334:0013010 ! stretchability texture by the hand method

[Term]
id: CO_334:0103049
name: Eba surface whiteness scale 0-10
namespace: CassavaScale
is_a: CO_334:0001001 ! Scales
relationship: scale_of CO_334:0013047 ! surface whiteness appearance method

[Term]
id: CO_334:0103050
name: Eba sweetness taste scale 0-10
namespace: CassavaScale
is_a: CO_334:0001001 ! Scales
relationship: scale_of CO_334:0013003 ! sweetness taste method

[Term]
id: CO_334:0103051
name: Extraneous matters appearance scale 0-10
namespace: CassavaScale
is_a: CO_334:0001001 ! Scales
relationship: scale_of CO_334:0013021 ! extraneous matters appearance method

[Term]
id: CO_334:0103052
name: Extraneous matters in mouth scale 0-10
namespace: CassavaScale
is_a: CO_334:0001001 ! Scales
relationship: scale_of CO_334:0013022 ! extraneous matters texture in mouth method

[Term]
id: CO_334:0103053
name: Fermented taste scale 0-10
namespace: CassavaScale
is_a: CO_334:0001001 ! Scales
relationship: scale_of CO_334:0013023 ! fermented taste method

[Term]
id: CO_334:0103054
name: Firmness scale 0-10
namespace: CassavaScale
is_a: CO_334:0001001 ! Scales
relationship: scale_of CO_334:0013026 ! firmness texture by touch method

[Term]
id: CO_334:0103055
name: Grain size scale 0-10
namespace: CassavaScale
is_a: CO_334:0001001 ! Scales
relationship: scale_of CO_334:0013041 ! size of grains appearance method

[Term]
id: CO_334:0103056
name: Granularity in mouth scale 0-10
namespace: CassavaScale
is_a: CO_334:0001001 ! Scales
relationship: scale_of CO_334:0013027 ! granularity texture in the mouth method

[Term]
id: CO_334:0103057
name: Granularity in mouth scale 0-100
namespace: CassavaScale
is_a: CO_334:0001001 ! Scales
relationship: scale_of CO_334:0013028 ! granularity texture in the mouth method

[Term]
id: CO_334:0103058
name: Greyness scale 0-10
namespace: CassavaScale
is_a: CO_334:0001001 ! Scales
relationship: scale_of CO_334:0013045 ! surface greyness appearance method

[Term]
id: CO_334:0103059
name: Hardness to break in the hand scale 0-100
namespace: CassavaScale
is_a: CO_334:0001001 ! Scales
relationship: scale_of CO_334:0013029 ! hardness to break/cut texture in the hand method

[Term]
id: CO_334:0103060
name: Homogenity of grains scale 0-10
namespace: CassavaScale
is_a: CO_334:0001001 ! Scales
relationship: scale_of CO_334:0013030 ! homogenity of grains appearance method

[Term]
id: CO_334:0103061
name: Masticability scale 0-10
namespace: CassavaScale
is_a: CO_334:0001001 ! Scales
relationship: scale_of CO_334:0013031 ! masticability texture in mouth method

[Term]
id: CO_334:0103062
name: Moldability in the hand  scale 0-10
namespace: CassavaScale
is_a: CO_334:0001001 ! Scales
relationship: scale_of CO_334:0013032 ! moldability texture in touch method

[Term]
id: CO_334:0103063
name: Mouth filled sensations scale 0-10
namespace: CassavaScale
is_a: CO_334:0001001 ! Scales
relationship: scale_of CO_334:0013033 ! mouth filled sensations texture in mouth method

[Term]
id: CO_334:0103064
name: Off-odours scale 0-10
namespace: CassavaScale
is_a: CO_334:0001001 ! Scales
relationship: scale_of CO_334:0013034 ! off-odours aroma method

[Term]
id: CO_334:0103065
name: Orange colour scale 0-10
namespace: CassavaScale
is_a: CO_334:0001001 ! Scales
relationship: scale_of CO_334:0013035 ! orange colour appearance method

[Term]
id: CO_334:0103066
name: Presence of fibers scale 0-10
namespace: CassavaScale
is_a: CO_334:0001001 ! Scales
relationship: scale_of CO_334:0013036 ! presence of fibers appearance method

[Term]
id: CO_334:0103067
name: Presence of fibers texture scale 0-100
namespace: CassavaScale
is_a: CO_334:0001001 ! Scales
relationship: scale_of CO_334:0013024 ! fibrouness texture appearance  method

[Term]
id: CO_334:0103068
name: Presence of lumps scale 0-10
namespace: CassavaScale
is_a: CO_334:0001001 ! Scales
relationship: scale_of CO_334:0013037 ! presence of lumps appearance method

[Term]
id: CO_334:0103069
name: Presence of strips appearance scale 0-100
namespace: CassavaScale
is_a: CO_334:0001001 ! Scales
relationship: scale_of CO_334:0013038 ! presence of stripes appearance method

[Term]
id: CO_334:0103070
name: Red palm oil aroma scale 0-10
namespace: CassavaScale
is_a: CO_334:0001001 ! Scales
relationship: scale_of CO_334:0013039 ! red palm oil aroma method

[Term]
id: CO_334:0103071
name: Sourness aroma scale 0-10
namespace: CassavaScale
is_a: CO_334:0001001 ! Scales
relationship: scale_of CO_334:0013042 ! sourness aroma method

[Term]
id: CO_334:0103072
name: surface creamness scale 0-10
namespace: CassavaScale
is_a: CO_334:0001001 ! Scales
relationship: scale_of CO_334:0013044 ! surface creamness appearance method

[Term]
id: CO_334:0103073
name: Surface yellow ness appearance scale 0-100
namespace: CassavaScale
is_a: CO_334:0001001 ! Scales
relationship: scale_of CO_334:0013000 ! surface yellowness appearance method

[Term]
id: CO_334:0103074
name: Taste of red palm oil scale 0-10
namespace: CassavaScale
is_a: CO_334:0001001 ! Scales
relationship: scale_of CO_334:0013049 ! taste of red palm oil taste method

[Term]
id: CO_334:0103075
name: Undesired taste scale 0-10
namespace: CassavaScale
is_a: CO_334:0001001 ! Scales
relationship: scale_of CO_334:0013050 ! undesired taste taste method

[Term]
id: CO_334:0103076
name: White colour scale 0-100
namespace: CassavaScale
is_a: CO_334:0001001 ! Scales
relationship: scale_of CO_334:0013051 ! white color appearance method

[Typedef]
id: derives_from
name: derives_from

[Typedef]
id: method_of
name: method_of

[Typedef]
id: scale_of
name: scale_of

[Typedef]
id: variable_of
name: variable_of

